<?xml version="1.0" encoding="UTF-8"?>
<rdf:RDF
   xmlns:dcterms="http://purl.org/dc/terms/"
   xmlns:doap="http://usefulinc.com/ns/doap#"
   xmlns:owl="http://www.w3.org/2002/07/owl#"
   xmlns:prov="http://www.w3.org/ns/prov#"
   xmlns:rdf="http://www.w3.org/1999/02/22-rdf-syntax-ns#"
   xmlns:rdfs="http://www.w3.org/2000/01/rdf-schema#"
   xmlns:schema-https="https://schema.org/"
   xmlns:skos="http://www.w3.org/2004/02/skos/core#"
>
  <rdf:Description rdf:nodeID="ub1bL981C19">
    <owl:onProperty rdf:resource="https://w3id.org/tern/ontologies/tern/isSamplingPointOf"/>
    <owl:onClass rdf:resource="https://w3id.org/tern/ontologies/tern/Transect"/>
    <owl:maxQualifiedCardinality rdf:datatype="http://www.w3.org/2001/XMLSchema#nonNegativeInteger">1</owl:maxQualifiedCardinality>
    <rdf:type rdf:resource="http://www.w3.org/2002/07/owl#Restriction"/>
  </rdf:Description>
  <rdf:Description rdf:about="https://w3id.org/tern/ontologies/tern/Method">
    <skos:definition>A Method describes in detailed steps how a workflow, protocol, plan or algorithm is carried out to make an [Observation](#Observation) or a [Sample](#Sample). It explains the steps to be carried out to arrive at reproducible [Result](#Result).</skos:definition>
    <rdfs:subClassOf rdf:nodeID="ub1bL492C19"/>
    <rdfs:subClassOf rdf:nodeID="ub1bL510C19"/>
    <rdfs:subClassOf rdf:resource="http://www.w3.org/2004/02/skos/core#Concept"/>
    <rdfs:subClassOf rdf:nodeID="ub1bL486C19"/>
    <rdfs:subClassOf rdf:nodeID="ub1bL469C19"/>
    <rdfs:subClassOf rdf:nodeID="ub1bL504C19"/>
    <rdf:type rdf:resource="http://www.w3.org/2002/07/owl#Class"/>
    <rdfs:seeAlso rdf:resource="https://the9000store.com/iso-9001-2015-requirements/iso-9001-2015-context-of-the-organization/processes-procedures-work-instructions/"/>
    <rdfs:label>Method</rdfs:label>
    <rdfs:subClassOf rdf:nodeID="ub1bL480C19"/>
    <rdfs:subClassOf rdf:nodeID="ub1bL498C19"/>
    <skos:example>Borehole logging is a field method in which 
in situ physical measurements (e.g., temperature) are made down the 
length of a borehole by lowering measurement instruments down the borehole via cable. (Credit: PaST Thesaurus)</skos:example>
    <rdfs:scopeNote>We recommend representing the method information following [ISO 9001 Processes, Procedures and Work Instructions](https://3yn1j14c4twk1bmdg82226en-wpengine.netdna-ssl.com/wp-content/uploads/2016/08/iso-9001-procedure.pdf)</rdfs:scopeNote>
    <rdfs:seeAlso rdf:resource="https://apps.usgs.gov/thesaurus/term-simple.php?thcode=2&amp;code=376"/>
  </rdf:Description>
  <rdf:Description rdf:about="https://w3id.org/tern/ontologies/tern/SoilHorizon">
    <rdfs:label>Soil Horizon</rdfs:label>
    <rdfs:subClassOf rdf:resource="https://w3id.org/tern/ontologies/tern/Sample"/>
    <rdfs:subClassOf rdf:nodeID="ub1bL1332C19"/>
    <skos:example>C Horizon consists of weathering rock.</skos:example>
    <skos:definition>A soil horizon is a layer of soil, approximately parallel to the land surface, with morphological properties different from layers below and/or above it. Tongues of material from one horizon may penetrate into adjacent horizons (Credit: Australian Soil and Land Survey Field Handbook).</skos:definition>
    <rdfs:subClassOf rdf:nodeID="ub1bL1322C19"/>
    <rdfs:subClassOf rdf:nodeID="ub1bL1327C19"/>
    <rdf:type rdf:resource="http://www.w3.org/2002/07/owl#Class"/>
  </rdf:Description>
  <rdf:Description rdf:about="https://w3id.org/tern/ontologies/tern/dimension">
    <rdf:type rdf:resource="http://www.w3.org/1999/02/22-rdf-syntax-ns#Property"/>
    <skos:definition>A property that links, e.g., a [Site](#EcologicalSite) to its [Dimension](#Dimension).</skos:definition>
    <rdfs:label>dimension</rdfs:label>
  </rdf:Description>
  <rdf:Description rdf:nodeID="ub1bL969C19">
    <rdf:type rdf:resource="http://www.w3.org/2002/07/owl#Restriction"/>
    <owl:onClass rdf:resource="http://linked.data.gov.au/def/datatype/QuantitativeMeasure"/>
    <owl:maxQualifiedCardinality rdf:datatype="http://www.w3.org/2001/XMLSchema#nonNegativeInteger">1</owl:maxQualifiedCardinality>
    <owl:onProperty rdf:resource="https://w3id.org/tern/ontologies/loc/elevation"/>
  </rdf:Description>
  <rdf:Description rdf:about="https://w3id.org/tern/ontologies/tern/PhysicalSpecimen">
    <skos:definition>A [Physical Specimen](#PhysicalSpecimen) is a physical [specimen](#Sample) collected from the field. </skos:definition>
    <rdfs:subClassOf rdf:resource="https://w3id.org/tern/ontologies/tern/Sample"/>
    <rdfs:subClassOf rdf:nodeID="ub1bL701C19"/>
    <rdfs:subClassOf rdf:nodeID="ub1bL696C19"/>
    <rdfs:label>Physical Specimen</rdfs:label>
    <rdfs:subClassOf rdf:resource="http://rs.tdwg.org/dwc/terms/MaterialSample"/>
    <skos:example>A soil specimen or a plant specimen are examples of physical specimens.</skos:example>
    <rdf:type rdf:resource="http://www.w3.org/2002/07/owl#Class"/>
  </rdf:Description>
  <rdf:Description rdf:nodeID="f5a816f5a0f7a4e439059a4ae4caf6ab4b14">
    <rdf:rest rdf:nodeID="f5a816f5a0f7a4e439059a4ae4caf6ab4b15"/>
    <rdf:first rdf:resource="https://w3id.org/tern/ontologies/tern/Observation"/>
  </rdf:Description>
  <rdf:Description rdf:nodeID="ub1bL1113C19">
    <owl:onProperty rdf:resource="https://w3id.org/tern/ontologies/tern/cardinalDirection"/>
    <owl:maxQualifiedCardinality rdf:datatype="http://www.w3.org/2001/XMLSchema#nonNegativeInteger">1</owl:maxQualifiedCardinality>
    <owl:onClass rdf:resource="http://www.w3.org/2001/XMLSchema#string"/>
    <rdf:type rdf:resource="http://www.w3.org/2002/07/owl#Restriction"/>
  </rdf:Description>
  <rdf:Description rdf:nodeID="ub1bL480C19">
    <owl:onProperty rdf:resource="http://www.w3.org/2004/02/skos/core#definition"/>
    <owl:maxQualifiedCardinality rdf:datatype="http://www.w3.org/2001/XMLSchema#nonNegativeInteger">1</owl:maxQualifiedCardinality>
    <owl:onClass rdf:resource="http://www.w3.org/2001/XMLSchema#string"/>
    <rdf:type rdf:resource="http://www.w3.org/2002/07/owl#Restriction"/>
  </rdf:Description>
  <rdf:Description rdf:about="https://w3id.org/tern/ontologies/tern/DigitalCamera">
    <rdfs:subClassOf rdf:nodeID="ub1bL257C19"/>
    <skos:definition>The model as defined by the manufacturer.</skos:definition>
    <rdfs:subClassOf rdf:resource="http://www.w3.org/2004/02/skos/core#Concept"/>
    <rdfs:subClassOf rdf:nodeID="ub1bL247C19"/>
    <rdf:type rdf:resource="http://www.w3.org/2002/07/owl#Class"/>
    <skos:example>E.g. EOS 350D</skos:example>
    <rdfs:subClassOf rdf:nodeID="ub1bL237C19"/>
    <rdfs:subClassOf rdf:nodeID="ub1bL263C19"/>
    <rdfs:subClassOf rdf:nodeID="ub1bL242C19"/>
    <rdfs:subClassOf rdf:nodeID="ub1bL252C19"/>
    <rdfs:label>Digital Camera</rdfs:label>
    <rdfs:subClassOf rdf:resource="https://w3id.org/tern/ontologies/tern/Sampler"/>
  </rdf:Description>
  <rdf:Description rdf:nodeID="ub1bL887C19">
    <owl:onProperty rdf:resource="http://www.w3.org/ns/sosa/madeSampling"/>
    <owl:allValuesFrom rdf:resource="https://w3id.org/tern/ontologies/tern/Sampling"/>
    <rdf:type rdf:resource="http://www.w3.org/2002/07/owl#Restriction"/>
  </rdf:Description>
  <rdf:Description rdf:about="https://w3id.org/tern/ontologies/tern/Sampler">
    <skos:example>Soil probe is an example of device used to collect a soil core.</skos:example>
    <rdf:type rdf:resource="http://www.w3.org/2002/07/owl#Class"/>
    <rdfs:subClassOf rdf:resource="https://w3id.org/tern/ontologies/tern/Instrument"/>
    <rdfs:subClassOf rdf:nodeID="ub1bL887C19"/>
    <rdfs:label>Sampler</rdfs:label>
    <rdfs:subClassOf rdf:resource="http://www.w3.org/ns/sosa/Sampler"/>
    <skos:definition>A device that is used by, or implements, a (Sampling) [Procedure](#Procedure) to create or transform one or more samples.</skos:definition>
    <rdfs:subClassOf rdf:nodeID="ub1bL892C19"/>
  </rdf:Description>
  <rdf:Description rdf:nodeID="ub1bL50C19">
    <owl:cardinality rdf:datatype="http://www.w3.org/2001/XMLSchema#nonNegativeInteger">1</owl:cardinality>
    <owl:onProperty rdf:resource="https://w3id.org/tern/ontologies/tern/globalVocabulary"/>
    <rdf:type rdf:resource="http://www.w3.org/2002/07/owl#Restriction"/>
  </rdf:Description>
  <rdf:Description rdf:about="https://w3id.org/tern/ontologies/tern/Sample">
    <rdfs:subClassOf rdf:nodeID="ub1bL862C19"/>
    <rdfs:label>Sample</rdfs:label>
    <rdfs:subClassOf rdf:nodeID="ub1bL852C19"/>
    <skos:definition>*A feature which is intended to be representative of a [FeatureOfInterest](http://w3.org/ns/sosa/FeatureOfInterest) on which [Observations](#Observation) may be made. Physical samples are sometimes known as physical specimens.</skos:definition>
    <rdfs:subClassOf rdf:nodeID="ub1bL872C19"/>
    <skos:example>Plant, animal, soil and water are all 
examples of samples of some feature of interest.</skos:example>
    <rdfs:subClassOf rdf:nodeID="ub1bL847C19"/>
    <rdfs:subClassOf rdf:nodeID="ub1bL867C19"/>
    <rdf:type rdf:resource="http://www.w3.org/2002/07/owl#Class"/>
    <rdfs:subClassOf rdf:nodeID="ub1bL857C19"/>
    <rdfs:subClassOf rdf:resource="https://w3id.org/tern/ontologies/tern/FeatureOfInterest"/>
    <rdfs:subClassOf rdf:nodeID="ub1bL842C19"/>
  </rdf:Description>
  <rdf:Description rdf:nodeID="ub1bL769C19">
    <owl:onProperty rdf:resource="http://www.w3.org/ns/sosa/hasResult"/>
    <owl:qualifiedCardinality rdf:datatype="http://www.w3.org/2001/XMLSchema#nonNegativeInteger">1</owl:qualifiedCardinality>
    <owl:onClass rdf:resource="https://w3id.org/tern/ontologies/tern/Result"/>
    <rdf:type rdf:resource="http://www.w3.org/2002/07/owl#Restriction"/>
  </rdf:Description>
  <rdf:Description rdf:nodeID="ub1bL1119C19">
    <owl:onProperty rdf:resource="https://w3id.org/tern/ontologies/tern/locationDescription"/>
    <owl:maxQualifiedCardinality rdf:datatype="http://www.w3.org/2001/XMLSchema#nonNegativeInteger">1</owl:maxQualifiedCardinality>
    <rdf:type rdf:resource="http://www.w3.org/2002/07/owl#Restriction"/>
    <owl:onClass rdf:resource="http://www.w3.org/2001/XMLSchema#string"/>
  </rdf:Description>
  <rdf:Description rdf:about="https://w3id.org/tern/ontologies/tern/hasSubActivity">
    <rdfs:label>has sub activity</rdfs:label>
    <skos:definition>Link to an [Observation](#Observation) or [Sampling](#Sampling).</skos:definition>
    <rdf:type rdf:resource="http://www.w3.org/1999/02/22-rdf-syntax-ns#Property"/>
  </rdf:Description>
  <rdf:Description rdf:about="https://w3id.org/tern/ontologies/tern/Dimension">
    <rdfs:subClassOf rdf:nodeID="ub1bL286C19"/>
    <rdf:type rdf:resource="http://www.w3.org/2002/07/owl#Class"/>
    <skos:definition>The dimension of a 2D square or rectangular feature. Example, the dimension of a rectangular plot [Site](#EcologicalSite). This class should perhaps have specialised classes to express not just square or rectangular features but also others such as circular features.</skos:definition>
    <rdfs:subClassOf rdf:nodeID="ub1bL275C19"/>
    <rdfs:subClassOf rdf:nodeID="ub1bL307C19"/>
    <rdfs:subClassOf rdf:nodeID="ub1bL297C19"/>
    <rdfs:label>Dimension</rdfs:label>
    <rdfs:subClassOf rdf:nodeID="ub1bL302C19"/>
  </rdf:Description>
  <rdf:Description rdf:about="https://w3id.org/tern/ontologies/tern/sampleStorageLocation">
    <rdf:type rdf:resource="http://www.w3.org/1999/02/22-rdf-syntax-ns#Property"/>
    <rdfs:label>sample storage location</rdfs:label>
    <rdfs:subPropertyOf rdf:resource="http://www.opengis.net/ont/geosparql#hasGeometry"/>
    <skos:definition>A property that links a [PhysicalSpecimen](#PhysicalSpecimen) to the location [Point](https://w3id.org/tern/ontologies/loc/Point) of where it is stored.</skos:definition>
  </rdf:Description>
  <rdf:Description rdf:nodeID="ub1bL1101C19">
    <owl:maxQualifiedCardinality rdf:datatype="http://www.w3.org/2001/XMLSchema#nonNegativeInteger">1</owl:maxQualifiedCardinality>
    <rdf:type rdf:resource="http://www.w3.org/2002/07/owl#Restriction"/>
    <owl:onProperty rdf:resource="https://w3id.org/tern/ontologies/tern/area"/>
    <owl:onClass rdf:resource="http://linked.data.gov.au/def/datatype/QuantitativeMeasure"/>
  </rdf:Description>
  <rdf:Description rdf:nodeID="ub1bL993C19">
    <owl:onClass rdf:resource="http://linked.data.gov.au/def/datatype/QuantitativeMeasure"/>
    <owl:qualifiedCardinality rdf:datatype="http://www.w3.org/2001/XMLSchema#nonNegativeInteger">1</owl:qualifiedCardinality>
    <rdf:type rdf:resource="http://www.w3.org/2002/07/owl#Restriction"/>
    <owl:onProperty rdf:resource="https://w3id.org/tern/ontologies/loc/longitude"/>
  </rdf:Description>
  <rdf:Description rdf:nodeID="f5a816f5a0f7a4e439059a4ae4caf6ab4b19">
    <rdf:rest rdf:resource="http://www.w3.org/1999/02/22-rdf-syntax-ns#nil"/>
    <rdf:first rdf:resource="https://w3id.org/tern/ontologies/tern/Sampling"/>
  </rdf:Description>
  <rdf:Description rdf:about="https://w3id.org/tern/ontologies/tern/hasCategoricalCollection">
    <rdfs:label>has categorical collection</rdfs:label>
    <skos:definition>A property that links a concept to a collection containing its categorical values.</skos:definition>
    <rdf:type rdf:resource="http://www.w3.org/1999/02/22-rdf-syntax-ns#Property"/>
  </rdf:Description>
  <rdf:Description rdf:about="https://w3id.org/tern/ontologies/tern/">
    <dcterms:publisher rdf:resource="https://w3id.org/tern/resources/a083902d-d821-41be-b663-1d7cb33eea66"/>
    <rdfs:seeAlso rdf:resource="https://www.w3.org/TR/vocab-ssn-ext/"/>
    <owl:imports rdf:resource="http://www.w3.org/2006/time#"/>
    <dcterms:license rdf:resource="http://creativecommons.org/publicdomain/zero/1.0/"/>
    <dcterms:contributor rdf:nodeID="ub1bL104C23"/>
    <owl:versionIRI rdf:resource="http://linked.data.gov.au/def/plot/0.2.1"/>
    <owl:imports rdf:resource="http://www.w3.org/2004/02/skos/core#"/>
    <prov:wasGeneratedBy rdf:nodeID="ub1bL172C23"/>
    <rdfs:label>TERN Ontology</rdfs:label>
    <rdfs:seeAlso rdf:resource="https://www.w3.org/ns/ssn/"/>
    <owl:imports rdf:resource="https://w3id.org/tern/ontologies/sd/"/>
    <owl:imports rdf:resource="http://qudt.org/schema/qudt/"/>
    <dcterms:creator rdf:nodeID="ub1bL129C19"/>
    <dcterms:contributor rdf:nodeID="ub1bL98C23"/>
    <dcterms:creator rdf:nodeID="ub1bL136C19"/>
    <rdfs:comment>The TERN Ontology comprises a set of vocabularies for representing plot-based ecological data. It was developed primarily based on the SOSA (Sensor, Observation, Sample, and Actuator) ontology. The TERN Ontology's classes and properties have been tailored to describe terrestrial ecology survey data including flora, vegetation and soil, following the methodologies outlined in the Australian Soil and Land Survey Field Handbook.
  
  
  </rdfs:comment>
    <dcterms:contributor rdf:nodeID="ub1bL92C23"/>
    <owl:imports rdf:resource="https://raw.githubusercontent.com/AGLDWG/datatype-ont/master/rdf/datatype.rdf"/>
    <owl:imports rdf:resource="http://datashapes.org/dash"/>
    <owl:imports rdf:resource="http://www.w3.org/ns/prov#"/>
    <owl:imports rdf:resource="https://w3id.org/tern/ontologies/org/"/>
    <dcterms:contributor rdf:nodeID="ub1bL110C23"/>
    <owl:imports rdf:resource="http://www.w3.org/ns/sosa/"/>
    <owl:imports rdf:resource="http://www.w3.org/ns/dcat#"/>
    <rdf:type rdf:resource="http://www.w3.org/2002/07/owl#Ontology"/>
    <rdfs:seeAlso rdf:resource="https://www.publish.csiro.au/book/5230/"/>
    <dcterms:modified rdf:datatype="http://www.w3.org/2001/XMLSchema#date">2020-03-18</dcterms:modified>
    <owl:versionInfo>0.2.1</owl:versionInfo>
    <dcterms:contributor rdf:nodeID="ub1bL116C23"/>
    <owl:imports rdf:resource="http://www.w3.org/ns/ssn/"/>
    <dcterms:creator rdf:nodeID="ub1bL122C19"/>
    <owl:imports rdf:resource="https://w3id.org/tern/ontologies/loc/"/>
  </rdf:Description>
  <rdf:Description rdf:nodeID="ub1bL1260C19">
    <owl:onProperty rdf:resource="http://www.w3.org/2000/01/rdf-schema#comment"/>
    <owl:allValuesFrom rdf:resource="http://www.w3.org/2001/XMLSchema#string"/>
    <rdf:type rdf:resource="http://www.w3.org/2002/07/owl#Restriction"/>
  </rdf:Description>
  <rdf:Description rdf:nodeID="ub1bL724C19">
    <rdf:type rdf:resource="http://www.w3.org/2002/07/owl#Restriction"/>
    <owl:onProperty rdf:resource="https://w3id.org/tern/ontologies/tern/methodType"/>
    <owl:allValuesFrom rdf:resource="http://www.w3.org/2004/02/skos/core#Concept"/>
  </rdf:Description>
  <rdf:Description rdf:about="https://w3id.org/tern/ontologies/tern/purpose">
    <rdf:type rdf:resource="http://www.w3.org/2002/07/owl#DatatypeProperty"/>
    <rdfs:label>purpose</rdfs:label>
    <rdfs:range rdf:resource="http://www.w3.org/2001/XMLSchema#string"/>
    <skos:definition>Describe the purpose of something.</skos:definition>
  </rdf:Description>
  <rdf:Description rdf:nodeID="ub1bL358C19">
    <owl:allValuesFrom rdf:resource="http://www.w3.org/2001/XMLSchema#string"/>
    <owl:onProperty rdf:resource="http://purl.org/dc/terms/description"/>
    <rdf:type rdf:resource="http://www.w3.org/2002/07/owl#Restriction"/>
  </rdf:Description>
  <rdf:Description rdf:about="https://w3id.org/tern/ontologies/tern/Result">
    <skos:example>The value 20 as the height of a certain 
tree together with the unit, e.g., Meter.</skos:example>
    <rdfs:subClassOf rdf:nodeID="ub1bL805C19"/>
    <rdfs:subClassOf rdf:resource="http://www.w3.org/ns/sosa/Result"/>
    <skos:definition>The result of an [Observation](#Observation), [Actuation](http://w3.org/ns/sosa/Actuation), or act of [Sampling](#Sampling). To store an observation's simple result value one can use the [hasSimpleResult](http://w3.org/ns/sosa/hasSimpleResult) property.</skos:definition>
    <rdf:type rdf:resource="http://www.w3.org/2002/07/owl#Class"/>
    <rdfs:label>Result</rdfs:label>
    <rdfs:subClassOf rdf:nodeID="ub1bL810C19"/>
    <rdfs:subClassOf rdf:nodeID="ub1bL821C19"/>
  </rdf:Description>
  <rdf:Description rdf:nodeID="ub1bL1065C19">
    <rdf:type rdf:resource="http://www.w3.org/2002/07/owl#Restriction"/>
    <owl:onProperty rdf:resource="http://purl.org/dc/terms/hasPart"/>
    <owl:allValuesFrom rdf:resource="https://w3id.org/tern/ontologies/tern/Site"/>
  </rdf:Description>
  <rdf:Description rdf:nodeID="ub1bL1080C19">
    <rdf:type rdf:resource="http://www.w3.org/2002/07/owl#Restriction"/>
    <owl:allValuesFrom rdf:nodeID="ub1bL1082C25"/>
    <owl:onProperty rdf:resource="http://www.opengis.net/ont/geosparql#hasGeometry"/>
  </rdf:Description>
  <rdf:Description rdf:about="https://w3id.org/tern/ontologies/tern/swPoint">
    <rdfs:range rdf:resource="https://w3id.org/tern/ontologies/loc/Point"/>
    <rdfs:subPropertyOf rdf:resource="http://www.opengis.net/ont/geosparql#hasGeometry"/>
    <rdfs:label>sw point</rdfs:label>
    <rdf:type rdf:resource="http://www.w3.org/1999/02/22-rdf-syntax-ns#Property"/>
    <skos:definition>The south-west point of the subject.</skos:definition>
  </rdf:Description>
  <rdf:Description rdf:nodeID="ub1bL1091C19">
    <owl:maxCardinality rdf:datatype="http://www.w3.org/2001/XMLSchema#nonNegativeInteger">1</owl:maxCardinality>
    <rdf:type rdf:resource="http://www.w3.org/2002/07/owl#Restriction"/>
    <owl:onProperty rdf:resource="http://www.w3.org/ns/prov#generatedAtTime"/>
  </rdf:Description>
  <rdf:Description rdf:nodeID="ub1bL922C19">
    <owl:qualifiedCardinality rdf:datatype="http://www.w3.org/2001/XMLSchema#nonNegativeInteger">1</owl:qualifiedCardinality>
    <owl:onProperty rdf:resource="http://www.w3.org/2000/01/rdf-schema#label"/>
    <owl:onClass rdf:resource="http://www.w3.org/2001/XMLSchema#string"/>
    <rdf:type rdf:resource="http://www.w3.org/2002/07/owl#Restriction"/>
  </rdf:Description>
  <rdf:Description rdf:nodeID="ub1bL1292C19">
    <owl:maxQualifiedCardinality rdf:datatype="http://www.w3.org/2001/XMLSchema#nonNegativeInteger">1</owl:maxQualifiedCardinality>
    <rdf:type rdf:resource="http://www.w3.org/2002/07/owl#Restriction"/>
    <owl:onClass rdf:resource="http://www.w3.org/2001/XMLSchema#string"/>
    <owl:onProperty rdf:resource="https://w3id.org/tern/ontologies/tern/siteDescription"/>
  </rdf:Description>
  <rdf:Description rdf:about="https://w3id.org/tern/ontologies/tern/stratum">
    <rdf:type rdf:resource="http://www.w3.org/1999/02/22-rdf-syntax-ns#Property"/>
    <skos:definition>A stratum is a distinct, easily seen, layer of foliage and branches of a measurable height.</skos:definition>
    <rdfs:subPropertyOf rdf:resource="http://purl.org/dc/terms/type"/>
    <rdfs:label>stratum</rdfs:label>
    <skos:scopeNote>Value should be from a controlled vocabulary identified by a URI.</skos:scopeNote>
  </rdf:Description>
  <rdf:Description rdf:about="https://w3id.org/tern/ontologies/tern/Instrument">
    <rdfs:subClassOf rdf:resource="http://www.w3.org/ns/ssn/System"/>
    <skos:definition>A device or instrument that is used for making measurements or observations.</skos:definition>
    <rdf:type rdf:resource="http://www.w3.org/2002/07/owl#Class"/>
    <rdfs:subClassOf rdf:nodeID="ub1bL455C19"/>
    <rdfs:subClassOf rdf:nodeID="ub1bL442C19"/>
    <rdfs:label>Instrument</rdfs:label>
  </rdf:Description>
  <rdf:Description rdf:about="https://w3id.org/tern/ontologies/tern/Platform">
    <rdfs:label>Platform</rdfs:label>
    <skos:definition>An entity that hosts other entities, particularly [Sensors](#Sensor), [Samplers](#Sampler), and other [Platforms](#Platform).</skos:definition>
    <skos:example>Ocean buoy is an example of platform that is equipped with 
an array of sensors such as GPS, current meters, atmospheric sensors and water 
quality monitors. Sensors measuring weather variables are attached to 
a weather station (a platform)</skos:example>
    <rdf:type rdf:resource="http://www.w3.org/2002/07/owl#Class"/>
    <rdfs:subClassOf rdf:resource="http://www.w3.org/ns/sosa/Platform"/>
  </rdf:Description>
  <rdf:Description rdf:about="https://w3id.org/tern/ontologies/tern/OEHSite">
    <rdf:type rdf:resource="http://www.w3.org/2002/07/owl#Class"/>
    <skos:definition>A plot survey site managed by the NSW Office of Environment and Heritage (OEH).</skos:definition>
    <rdfs:subClassOf rdf:resource="https://w3id.org/tern/ontologies/tern/Site"/>
    <rdfs:label>OEH Site</rdfs:label>
    <rdfs:seeAlso rdf:resource="https://www.environment.nsw.gov.au/surveys/AnimalAndPlantSurveys.htm"/>
  </rdf:Description>
  <rdf:Description rdf:nodeID="ub1bL1149C19">
    <owl:maxQualifiedCardinality rdf:datatype="http://www.w3.org/2001/XMLSchema#nonNegativeInteger">1</owl:maxQualifiedCardinality>
    <owl:onClass rdf:resource="https://w3id.org/tern/ontologies/loc/Polygon"/>
    <owl:onProperty rdf:resource="https://w3id.org/tern/ontologies/tern/polygon"/>
    <rdf:type rdf:resource="http://www.w3.org/2002/07/owl#Restriction"/>
  </rdf:Description>
  <rdf:Description rdf:about="http://linked.data.gov.au/def/datatype/Concept">
    <rdfs:subClassOf rdf:nodeID="ub1bL50C19"/>
    <rdfs:subClassOf rdf:resource="https://w3id.org/tern/ontologies/tern/Result"/>
    <rdf:type rdf:resource="http://www.w3.org/2002/07/owl#Class"/>
    <rdfs:subClassOf rdf:nodeID="ub1bL45C19"/>
  </rdf:Description>
  <rdf:Description rdf:nodeID="ub1bL1027C19">
    <owl:onProperty rdf:resource="http://schema.org/serialNumber"/>
    <rdf:type rdf:resource="http://www.w3.org/2002/07/owl#Restriction"/>
    <owl:onDataRange rdf:resource="http://www.w3.org/2001/XMLSchema#string"/>
    <owl:maxQualifiedCardinality rdf:datatype="http://www.w3.org/2001/XMLSchema#nonNegativeInteger">1</owl:maxQualifiedCardinality>
  </rdf:Description>
  <rdf:Description rdf:about="https://w3id.org/tern/ontologies/tern/SiteStratum">
    <rdfs:subClassOf rdf:resource="https://w3id.org/tern/ontologies/tern/Sample"/>
    <rdfs:label>Site Stratum</rdfs:label>
    <rdfs:subClassOf rdf:nodeID="ub1bL1204C19"/>
    <rdfs:subClassOf rdf:nodeID="ub1bL1198C19"/>
    <skos:definition>Structural element covering a recognisable height range in vegetation ecosystem occurring at an observation [Site](#EcologicalSite).</skos:definition>
    <rdf:type rdf:resource="http://www.w3.org/2002/07/owl#Class"/>
  </rdf:Description>
  <rdf:Description rdf:nodeID="ub1bL550C19">
    <rdf:type rdf:resource="http://www.w3.org/2002/07/owl#Restriction"/>
    <owl:onProperty rdf:resource="http://linked.data.gov.au/def/datatype/vocabulary"/>
    <owl:cardinality rdf:datatype="http://www.w3.org/2001/XMLSchema#nonNegativeInteger">1</owl:cardinality>
  </rdf:Description>
  <rdf:Description rdf:nodeID="ub1bL1275C19">
    <rdf:type rdf:resource="http://www.w3.org/2002/07/owl#Restriction"/>
    <owl:allValuesFrom rdf:nodeID="ub1bL1277C25"/>
    <owl:onProperty rdf:resource="https://w3id.org/tern/ontologies/tern/hasSubActivity"/>
  </rdf:Description>
  <rdf:Description rdf:about="https://w3id.org/tern/ontologies/tern/PropertyValue">
    <rdfs:subClassOf rdf:nodeID="ub1bL769C19"/>
    <skos:definition>A property-value pair. Use the [schema:name](http://schema.org/name) property for the name of the property. If there is an additional human-readable version of the value, put that into the [schema:description](http://schema.org/description) property.</skos:definition>
    <rdf:type rdf:resource="http://www.w3.org/2002/07/owl#Class"/>
    <skos:example>@prefix tern: &lt;https://w3id.org/tern/ontologies/tern/&gt; .
@prefix schema: &lt;http://schema.org/&gt; .
@prefix data: &lt;http://linked.data.gov.au/def/datatype/&gt; .
@prefix sosa: &lt;http://w3.org/ns/sosa/&gt; .

&lt;example&gt; a tern:PropertyValue ;
	schema:name "AUSPLOTS_RANGELANDS.SITE.PROPERTY" ;
	schema:description "The property name" ;
	sosa:hasResult [
		a data:Text ;
		data:value "Great Victoria Desert Nature Reserve" ;
	] .</skos:example>
    <rdfs:label>Property Value</rdfs:label>
    <rdfs:subClassOf rdf:nodeID="ub1bL758C19"/>
    <rdfs:subClassOf rdf:nodeID="ub1bL763C19"/>
    <rdfs:subClassOf rdf:resource="http://schema.org/PropertyValue"/>
  </rdf:Description>
  <rdf:Description rdf:nodeID="ub1bL1155C19">
    <owl:onClass rdf:resource="https://w3id.org/tern/ontologies/tern/Dimension"/>
    <rdf:type rdf:resource="http://www.w3.org/2002/07/owl#Restriction"/>
    <owl:onProperty rdf:resource="https://w3id.org/tern/ontologies/tern/dimension"/>
    <owl:maxQualifiedCardinality rdf:datatype="http://www.w3.org/2001/XMLSchema#nonNegativeInteger">1</owl:maxQualifiedCardinality>
  </rdf:Description>
  <rdf:Description rdf:about="https://w3id.org/tern/ontologies/tern/Observation">
    <rdfs:subClassOf rdf:nodeID="ub1bL628C19"/>
    <rdfs:subClassOf rdf:nodeID="ub1bL598C19"/>
    <rdfs:subClassOf rdf:nodeID="ub1bL640C19"/>
    <rdfs:subClassOf rdf:nodeID="ub1bL616C19"/>
    <rdfs:subClassOf rdf:nodeID="ub1bL592C19"/>
    <rdfs:subClassOf rdf:nodeID="ub1bL582C19"/>
    <rdfs:subClassOf rdf:nodeID="ub1bL587C19"/>
    <skos:definition>Act of carrying out an (Observation) [Procedure](#Procedure) to estimate or calculate a value of a property of a [FeatureOfInterest](http://w3.org/ns/sosa/FeatureOfInterest). Links to a [Sensor](http://w3.org/ns/sosa/Sensor) to describe what made the [Observation](#Observation) and how; links to an [ObservableProperty](#ObservableProperty) to describe what the result is an estimate of, and to a [FeatureOfInterest](http://w3.org/ns/sosa/FeatureOfInterest) to detail what that property was associated with.</skos:definition>
    <skos:example>The activity of measuring properties such as wind speed and direction by 
an anemometer sensor. The results of the observation are the measurement values 
of the properties estimated by the sensor.</skos:example>
    <rdfs:subClassOf rdf:nodeID="ub1bL634C19"/>
    <rdfs:subClassOf rdf:resource="http://www.w3.org/ns/prov#Activity"/>
    <rdfs:subClassOf rdf:resource="http://www.w3.org/ns/sosa/Observation"/>
    <rdfs:label>Observation</rdfs:label>
    <rdf:type rdf:resource="http://www.w3.org/2002/07/owl#Class"/>
    <rdfs:subClassOf rdf:nodeID="ub1bL610C19"/>
    <rdfs:subClassOf rdf:nodeID="ub1bL604C19"/>
    <rdfs:subClassOf rdf:nodeID="ub1bL622C19"/>
  </rdf:Description>
  <rdf:Description rdf:about="https://w3id.org/tern/ontologies/tern/FluxTower">
    <rdfs:subClassOf rdf:nodeID="ub1bL358C19"/>
    <rdfs:subClassOf rdf:nodeID="ub1bL398C19"/>
    <rdfs:subClassOf rdf:nodeID="ub1bL386C19"/>
    <skos:example>Alice Springs Mulga flux tower</skos:example>
    <rdfs:subClassOf rdf:resource="https://w3id.org/tern/ontologies/tern/FixedPlatform"/>
    <rdfs:subClassOf rdf:nodeID="ub1bL392C19"/>
    <rdfs:label>Flux Tower</rdfs:label>
    <rdfs:subClassOf rdf:nodeID="ub1bL380C19"/>
    <skos:definition>Across the globe, towers stand among the landscape, with sensors monitoring these eddies for carbon dioxide, water vapor and other gasses.  These so-called flux towers collect data on carbon dioxide exchange rates between the earth and atmosphere.</skos:definition>
    <rdfs:subClassOf rdf:nodeID="ub1bL368C19"/>
    <rdfs:subClassOf rdf:nodeID="ub1bL374C19"/>
    <rdfs:subClassOf rdf:nodeID="ub1bL363C19"/>
    <rdfs:subClassOf rdf:nodeID="ub1bL404C19"/>
    <rdf:type rdf:resource="http://www.w3.org/2002/07/owl#Class"/>
    <skos:example rdf:resource="https://w3id.org/tern/resources/fd2809a2-e705-4961-b09c-7e9ae1ffa87e"/>
  </rdf:Description>
  <rdf:Description rdf:nodeID="ub1bL1070C19">
    <owl:onProperty rdf:resource="http://purl.org/dc/terms/isPartOf"/>
    <owl:allValuesFrom rdf:resource="https://w3id.org/tern/ontologies/tern/Site"/>
    <rdf:type rdf:resource="http://www.w3.org/2002/07/owl#Restriction"/>
  </rdf:Description>
  <rdf:Description rdf:about="https://w3id.org/tern/ontologies/tern/fluxnetID">
    <rdf:type rdf:resource="http://www.w3.org/1999/02/22-rdf-syntax-ns#Property"/>
    <rdfs:seeAlso rdf:resource="https://fluxnet.org/"/>
    <skos:definition>The unique identifier for flux towers registered with FLUXNET.</skos:definition>
    <rdfs:label>fluxnet ID</rdfs:label>
    <skos:example>AU-ASM</skos:example>
  </rdf:Description>
  <rdf:Description rdf:nodeID="ub1bL428C19">
    <rdf:type rdf:resource="http://www.w3.org/2002/07/owl#Restriction"/>
    <owl:onClass rdf:resource="http://www.w3.org/2001/XMLSchema#string"/>
    <owl:qualifiedCardinality rdf:datatype="http://www.w3.org/2001/XMLSchema#nonNegativeInteger">1</owl:qualifiedCardinality>
    <owl:onProperty rdf:resource="http://www.w3.org/2000/01/rdf-schema#label"/>
  </rdf:Description>
  <rdf:Description rdf:nodeID="ub1bL380C19">
    <rdf:type rdf:resource="http://www.w3.org/2002/07/owl#Restriction"/>
    <owl:onClass rdf:resource="https://w3id.org/tern/ontologies/tern/Site"/>
    <owl:maxQualifiedCardinality rdf:datatype="http://www.w3.org/2001/XMLSchema#nonNegativeInteger">1</owl:maxQualifiedCardinality>
    <owl:onProperty rdf:resource="http://www.w3.org/ns/sosa/isHostedBy"/>
  </rdf:Description>
  <rdf:Description rdf:nodeID="ub1bL1322C19">
    <owl:onProperty rdf:resource="https://w3id.org/tern/ontologies/loc/depth"/>
    <rdf:type rdf:resource="http://www.w3.org/2002/07/owl#Restriction"/>
    <owl:allValuesFrom rdf:resource="http://linked.data.gov.au/def/datatype/QuantitativeRange"/>
  </rdf:Description>
  <rdf:Description rdf:about="http://rs.tdwg.org/dwc/terms/materialSampleID">
    <rdfs:label>material sample ID</rdfs:label>
    <skos:example>IGSN:ASR000001 (Resulting URI: http://igsn.org/ASR000001) 
is a globally unique and persistent identifier of a soil sample.</skos:example>
    <rdfs:isDefinedBy rdf:resource="http://rs.tdwg.org/dwc/terms/"/>
    <rdfs:comment>An identifier for the MaterialSample (as opposed to a particular digital record of the material sample). In the absence of a persistent global unique identifier, construct one from a combination of identifiers in the record that will most closely make the materialSampleID globally unique.</rdfs:comment>
    <rdf:type rdf:resource="http://www.w3.org/1999/02/22-rdf-syntax-ns#Property"/>
  </rdf:Description>
  <rdf:Description rdf:nodeID="ub1bL275C19">
    <rdf:type rdf:resource="http://www.w3.org/2002/07/owl#Restriction"/>
    <owl:allValuesFrom rdf:nodeID="ub1bL277C25"/>
    <owl:onProperty rdf:resource="https://w3id.org/tern/ontologies/tern/length"/>
  </rdf:Description>
  <rdf:Description rdf:nodeID="ub1bL1382C19">
    <owl:allValuesFrom rdf:resource="https://w3id.org/tern/ontologies/tern/SamplingPoint"/>
    <owl:onProperty rdf:resource="https://w3id.org/tern/ontologies/tern/hasSamplingPoint"/>
    <rdf:type rdf:resource="http://www.w3.org/2002/07/owl#Restriction"/>
  </rdf:Description>
  <rdf:Description rdf:nodeID="ub1bL504C19">
    <owl:maxQualifiedCardinality rdf:datatype="http://www.w3.org/2001/XMLSchema#nonNegativeInteger">1</owl:maxQualifiedCardinality>
    <owl:onDataRange rdf:resource="http://www.w3.org/2001/XMLSchema#string"/>
    <rdf:type rdf:resource="http://www.w3.org/2002/07/owl#Restriction"/>
    <owl:onProperty rdf:resource="https://w3id.org/tern/ontologies/tern/scope"/>
  </rdf:Description>
  <rdf:Description rdf:nodeID="ub1bL1178C19">
    <owl:onClass rdf:resource="http://www.w3.org/2001/XMLSchema#string"/>
    <rdf:type rdf:resource="http://www.w3.org/2002/07/owl#Restriction"/>
    <owl:qualifiedCardinality rdf:datatype="http://www.w3.org/2001/XMLSchema#nonNegativeInteger">1</owl:qualifiedCardinality>
    <owl:onProperty rdf:resource="http://www.w3.org/2000/01/rdf-schema#label"/>
  </rdf:Description>
  <rdf:Description rdf:nodeID="ub1bL1255C19">
    <rdf:type rdf:resource="http://www.w3.org/2002/07/owl#Restriction"/>
    <owl:onProperty rdf:resource="http://www.w3.org/ns/prov#startedAtTime"/>
    <owl:allValuesFrom rdf:resource="http://www.w3.org/2001/XMLSchema#dateTime"/>
  </rdf:Description>
  <rdf:Description rdf:nodeID="ub1bL812C25">
    <owl:unionOf rdf:nodeID="f5a816f5a0f7a4e439059a4ae4caf6ab4b14"/>
    <rdf:type rdf:resource="http://www.w3.org/2002/07/owl#Class"/>
  </rdf:Description>
  <rdf:Description rdf:about="https://w3id.org/tern/ontologies/tern/FeatureOfInterest">
    <skos:example xml:lang="en">When measuring the height of a tree, the height is the observed ObservableProperty, 20m may be the Result of the Observation, and the tree is the FeatureOfInterest. A window is a FeatureOfInterest for an automatic window control Actuator.</skos:example>
    <rdf:type rdf:resource="http://www.w3.org/2002/07/owl#Class"/>
    <rdfs:subClassOf rdf:resource="http://www.w3.org/ns/sosa/FeatureOfInterest"/>
    <skos:definition xml:lang="en">The thing whose property is being estimated or calculated in the course of an Observation to arrive at a Result or whose property is being manipulated by an Actuator, or which is being sampled or transformed in an act of Sampling.</skos:definition>
    <rdf:type rdf:resource="http://www.w3.org/2000/01/rdf-schema#Class"/>
    <rdfs:label>Feature of Interest</rdfs:label>
  </rdf:Description>
  <rdf:Description rdf:about="https://w3id.org/tern/ontologies/tern/Site">
    <rdfs:subClassOf rdf:resource="https://w3id.org/tern/ontologies/tern/Platform"/>
    <rdfs:subClassOf rdf:nodeID="ub1bL1055C19"/>
    <rdfs:subClassOf rdf:resource="https://w3id.org/tern/ontologies/tern/Sample"/>
    <skos:scopeNote>Use [dcterms:hasPart](http://purl.org/dc/terms/hasPart) and [dcterms:isPartOf](http://purl.org/dc/terms/isPartOf) to model [Site](#EcologicalSite) and [Subsite](#EcologicalSite) relationships. E.g. In TERN, there are SuperSites that contain multiple core 1 ha subsites.</skos:scopeNote>
    <rdfs:subClassOf rdf:nodeID="ub1bL1065C19"/>
    <rdfs:subClassOf rdf:nodeID="ub1bL1131C19"/>
    <rdfs:subClassOf rdf:nodeID="ub1bL1178C19"/>
    <skos:example>Ausplots Rangelands Site 59858 (Site Name: WAACOO0011)</skos:example>
    <rdfs:subClassOf rdf:nodeID="ub1bL1075C19"/>
    <rdfs:subClassOf rdf:nodeID="ub1bL1143C19"/>
    <rdf:type rdf:resource="http://www.w3.org/2002/07/owl#Class"/>
    <rdfs:subClassOf rdf:nodeID="ub1bL1045C19"/>
    <rdfs:subClassOf rdf:nodeID="ub1bL1101C19"/>
    <rdfs:subClassOf rdf:nodeID="ub1bL1080C19"/>
    <rdfs:subClassOf rdf:nodeID="ub1bL1113C19"/>
    <rdfs:subClassOf rdf:nodeID="ub1bL1172C19"/>
    <rdfs:subClassOf rdf:nodeID="ub1bL1096C19"/>
    <rdfs:subClassOf rdf:nodeID="ub1bL1050C19"/>
    <rdfs:subClassOf rdf:nodeID="ub1bL1137C19"/>
    <rdfs:subClassOf rdf:nodeID="ub1bL1107C19"/>
    <rdfs:label>Ecological Site</rdfs:label>
    <rdfs:subClassOf rdf:nodeID="ub1bL1149C19"/>
    <rdfs:subClassOf rdf:nodeID="ub1bL1155C19"/>
    <rdfs:subClassOf rdf:nodeID="ub1bL1040C19"/>
    <rdfs:subClassOf rdf:nodeID="ub1bL1125C19"/>
    <rdfs:subClassOf rdf:nodeID="ub1bL1184C19"/>
    <rdfs:subClassOf rdf:nodeID="ub1bL1161C19"/>
    <skos:definition>Location where observations may be made. This is a subclass of [Sample](#Sample) because a site should be designed to be representative of an environmental system (which may be an ecosystem or bioregion) or zone (which may be a zone such as a parcel or tract).</skos:definition>
    <rdfs:subClassOf rdf:nodeID="ub1bL1070C19"/>
    <rdfs:subClassOf rdf:nodeID="ub1bL1091C19"/>
    <rdfs:subClassOf rdf:nodeID="ub1bL1119C19"/>
    <rdfs:subClassOf rdf:nodeID="ub1bL1060C19"/>
    <rdfs:subClassOf rdf:nodeID="ub1bL1166C19"/>
  </rdf:Description>
  <rdf:Description rdf:nodeID="ub1bL987C19">
    <owl:onProperty rdf:resource="https://w3id.org/tern/ontologies/loc/latitude"/>
    <owl:onClass rdf:resource="http://linked.data.gov.au/def/datatype/QuantitativeMeasure"/>
    <owl:qualifiedCardinality rdf:datatype="http://www.w3.org/2001/XMLSchema#nonNegativeInteger">1</owl:qualifiedCardinality>
    <rdf:type rdf:resource="http://www.w3.org/2002/07/owl#Restriction"/>
  </rdf:Description>
  <rdf:Description rdf:nodeID="ub1bL672C19">
    <owl:allValuesFrom rdf:resource="http://www.w3.org/2001/XMLSchema#string"/>
    <owl:onProperty rdf:resource="http://schema.org/serialNumber"/>
    <rdf:type rdf:resource="http://www.w3.org/2002/07/owl#Restriction"/>
  </rdf:Description>
  <rdf:Description rdf:about="https://w3id.org/tern/ontologies/tern/CategoricalValue">
    <rdfs:label>Categorical Value</rdfs:label>
    <rdfs:subClassOf rdf:resource="http://www.w3.org/2004/02/skos/core#Concept"/>
    <rdf:type rdf:resource="http://www.w3.org/2002/07/owl#Class"/>
  </rdf:Description>
  <rdf:Description rdf:nodeID="ub1bL469C19">
    <owl:onProperty rdf:resource="http://purl.org/dc/terms/source"/>
    <owl:allValuesFrom rdf:nodeID="ub1bL471C25"/>
    <rdf:type rdf:resource="http://www.w3.org/2002/07/owl#Restriction"/>
  </rdf:Description>
  <rdf:Description rdf:about="https://w3id.org/tern/ontologies/tern/siteVisit">
    <rdfs:label>site visit</rdfs:label>
    <skos:definition>A property that links, e.g., a [Site](#EcologicalSite) to a [Site Visit](#EcologicalSiteVisit).</skos:definition>
    <rdf:type rdf:resource="http://www.w3.org/1999/02/22-rdf-syntax-ns#Property"/>
    <rdfs:range rdf:resource="https://w3id.org/tern/ontologies/tern/SiteVisit"/>
  </rdf:Description>
  <rdf:Description rdf:nodeID="ub1bL263C19">
    <owl:onProperty rdf:resource="http://schema.org/manufacturer"/>
    <rdf:type rdf:resource="http://www.w3.org/2002/07/owl#Restriction"/>
    <owl:onClass rdf:resource="http://www.w3.org/2001/XMLSchema#string"/>
    <owl:minQualifiedCardinality rdf:datatype="http://www.w3.org/2001/XMLSchema#nonNegativeInteger">1</owl:minQualifiedCardinality>
  </rdf:Description>
  <rdf:Description rdf:nodeID="ub1bL1270C19">
    <rdf:type rdf:resource="http://www.w3.org/2002/07/owl#Restriction"/>
    <owl:allValuesFrom rdf:resource="https://w3id.org/tern/ontologies/tern/PropertyValue"/>
    <owl:onProperty rdf:resource="http://schema.org/additionalProperty"/>
  </rdf:Description>
  <rdf:Description rdf:about="https://w3id.org/tern/ontologies/tern/hasEnvironmentalCharacteristic">
    <rdfs:label>has environmental characteristic</rdfs:label>
    <skos:definition>The subject has some environmental characteristic. Points to a set of [Observations](#Observation) within an [EnvironmentalCharacteristic](#EnvironmentalCharacteristic).</skos:definition>
    <rdf:type rdf:resource="http://www.w3.org/2002/07/owl#ObjectProperty"/>
    <rdfs:range rdf:resource="https://w3id.org/tern/ontologies/tern/EnvironmentalCharacteristic"/>
  </rdf:Description>
  <rdf:Description rdf:nodeID="ub1bL810C19">
    <rdf:type rdf:resource="http://www.w3.org/2002/07/owl#Restriction"/>
    <owl:onProperty rdf:resource="http://www.w3.org/ns/sosa/isResultOf"/>
    <owl:allValuesFrom rdf:nodeID="ub1bL812C25"/>
  </rdf:Description>
  <rdf:Description rdf:about="https://w3id.org/tern/ontologies/tern/FixedPlatform">
    <rdfs:label>Fixed Platform</rdfs:label>
    <rdfs:subClassOf rdf:resource="https://w3id.org/tern/ontologies/tern/Platform"/>
    <rdf:type rdf:resource="http://www.w3.org/2002/07/owl#Class"/>
    <skos:definition>A fixed platform based on land.</skos:definition>
  </rdf:Description>
  <rdf:Description rdf:about="https://w3id.org/tern/ontologies/tern/equipment">
    <rdf:type rdf:resource="http://www.w3.org/2002/07/owl#DatatypeProperty"/>
    <rdfs:range rdf:resource="http://www.w3.org/2001/XMLSchema#string"/>
    <rdfs:label>equipment</rdfs:label>
    <skos:definition>Describe the equipment used as text.</skos:definition>
  </rdf:Description>
  <rdf:Description rdf:about="https://w3id.org/tern/ontologies/tern/siteShape">
    <skos:definition>The shape of the site. The value is expected to be from a controlled vocabulary with a persistent URI identifier.</skos:definition>
    <rdf:type rdf:resource="http://www.w3.org/1999/02/22-rdf-syntax-ns#Property"/>
    <rdfs:domain rdf:resource="https://w3id.org/tern/ontologies/tern/Site"/>
    <rdfs:label>site shape</rdfs:label>
  </rdf:Description>
  <rdf:Description rdf:nodeID="ub1bL1286C19">
    <owl:onProperty rdf:resource="https://w3id.org/tern/ontologies/tern/locationDescription"/>
    <rdf:type rdf:resource="http://www.w3.org/2002/07/owl#Restriction"/>
    <owl:onClass rdf:resource="http://www.w3.org/2001/XMLSchema#string"/>
    <owl:maxQualifiedCardinality rdf:datatype="http://www.w3.org/2001/XMLSchema#nonNegativeInteger">1</owl:maxQualifiedCardinality>
  </rdf:Description>
  <rdf:Description rdf:nodeID="f5a816f5a0f7a4e439059a4ae4caf6ab4b2">
    <rdf:first rdf:resource="http://www.w3.org/2001/XMLSchema#integer"/>
    <rdf:rest rdf:resource="http://www.w3.org/1999/02/22-rdf-syntax-ns#nil"/>
  </rdf:Description>
  <rdf:Description rdf:nodeID="ub1bL1398C19">
    <rdf:type rdf:resource="http://www.w3.org/2002/07/owl#Restriction"/>
    <owl:qualifiedCardinality rdf:datatype="http://www.w3.org/2001/XMLSchema#nonNegativeInteger">1</owl:qualifiedCardinality>
    <owl:onClass rdf:resource="https://w3id.org/tern/ontologies/loc/Point"/>
    <owl:onProperty rdf:resource="https://w3id.org/tern/ontologies/tern/transectEndPoint"/>
  </rdf:Description>
  <rdf:Description rdf:about="https://w3id.org/tern/ontologies/tern/hasParameter">
    <rdfs:subPropertyOf rdf:resource="http://www.w3.org/2004/02/skos/core#relatedMatch"/>
    <rdf:type rdf:resource="http://www.w3.org/1999/02/22-rdf-syntax-ns#Property"/>
    <skos:definition>A property that links a concept to a parameter.</skos:definition>
    <rdfs:label>has parameter</rdfs:label>
  </rdf:Description>
  <rdf:Description rdf:nodeID="ub1bL616C19">
    <owl:onClass rdf:resource="http://www.w3.org/2006/time#Instant"/>
    <owl:qualifiedCardinality rdf:datatype="http://www.w3.org/2001/XMLSchema#nonNegativeInteger">1</owl:qualifiedCardinality>
    <rdf:type rdf:resource="http://www.w3.org/2002/07/owl#Restriction"/>
    <owl:onProperty rdf:resource="http://www.w3.org/ns/sosa/phenomenonTime"/>
  </rdf:Description>
  <rdf:Description rdf:about="https://w3id.org/tern/ontologies/tern/globalValue">
    <rdf:type rdf:resource="http://www.w3.org/1999/02/22-rdf-syntax-ns#Property"/>
    <skos:example>The concept dry soil colour is defined in two vocabularies, 
[CORVEG](http://linked.data.gov.au/def/corveg-cv/1842b772-72a4-430f-a264-dcfd6c2c23b4) and 
[Ausplots](http://linked.data.gov.au/def/ausplots-cv/aa11e5f7-aec2-4e92-95b8-6332911f0c4e). 
The property global value is used to map the concept from the two vocabularies to the relevant 
[concept](http://linked.data.gov.au/def/tern-cv/beceaa5a-a296-4385-a55a-3b8c8d5b2369) 
specified in the main vocabulary, i.e., TERN Vocabularies.</skos:example>
    <skos:definition>A property that links a concept from a vocabulary to another concept in an authoritative/endorsed vocabulary.</skos:definition>
    <rdfs:label>global value</rdfs:label>
  </rdf:Description>
  <rdf:Description rdf:about="https://w3id.org/tern/ontologies/tern/Input">
    <skos:definition>*Input* - Any information that is provided to a [Procedure](#Procedure) for its use.</skos:definition>
    <skos:example>A **wedge prism** or **relascope** can be used to estimate the Basal Area per hectare. 
The number of counted trees and the Basal Area Factor are inputs to estimate the Basal Area.</skos:example>
    <rdf:type rdf:resource="http://www.w3.org/2002/07/owl#Class"/>
    <rdfs:subClassOf rdf:nodeID="ub1bL428C19"/>
    <rdfs:subClassOf rdf:nodeID="ub1bL418C19"/>
    <rdfs:label>Input</rdfs:label>
    <rdfs:subClassOf rdf:nodeID="ub1bL423C19"/>
    <rdfs:subClassOf rdf:resource="http://www.w3.org/ns/ssn/Input"/>
  </rdf:Description>
  <rdf:Description rdf:nodeID="ub1bL442C19">
    <owl:allValuesFrom rdf:nodeID="ub1bL444C25"/>
    <owl:onProperty rdf:resource="http://purl.org/dc/terms/type"/>
    <rdf:type rdf:resource="http://www.w3.org/2002/07/owl#Restriction"/>
  </rdf:Description>
  <rdf:Description rdf:about="https://w3id.org/tern/ontologies/tern/dateDecommissioned">
    <rdf:type rdf:resource="http://www.w3.org/1999/02/22-rdf-syntax-ns#Property"/>
    <skos:scopeNote>Use ISO 8601 international standard for representing dates and times. Missing end date may be set to the end of the month.</skos:scopeNote>
    <skos:definition>The date when, e.g., a [Site](#EcologicalSite) is decommissioned or stopped operating.</skos:definition>
    <rdfs:label>date decommissioned</rdfs:label>
    <skos:example>30 Nov 2019 is the date decommisioned of the 
[Collie flux station](http://ozflux.org.au/monitoringsites/collie/index.html)</skos:example>
  </rdf:Description>
  <rdf:Description rdf:nodeID="ub1bL1172C19">
    <owl:qualifiedCardinality rdf:datatype="http://www.w3.org/2001/XMLSchema#nonNegativeInteger">1</owl:qualifiedCardinality>
    <owl:onClass rdf:resource="http://www.w3.org/2001/XMLSchema#string"/>
    <owl:onProperty rdf:resource="http://purl.org/dc/terms/identifier"/>
    <rdf:type rdf:resource="http://www.w3.org/2002/07/owl#Restriction"/>
  </rdf:Description>
  <rdf:Description rdf:nodeID="ub1bL1143C19">
    <owl:maxQualifiedCardinality rdf:datatype="http://www.w3.org/2001/XMLSchema#nonNegativeInteger">1</owl:maxQualifiedCardinality>
    <owl:onClass rdf:resource="https://w3id.org/tern/ontologies/loc/Point"/>
    <rdf:type rdf:resource="http://www.w3.org/2002/07/owl#Restriction"/>
    <owl:onProperty rdf:resource="https://w3id.org/tern/ontologies/tern/swPoint"/>
  </rdf:Description>
  <rdf:Description rdf:nodeID="ub1bL1204C19">
    <owl:onProperty rdf:resource="http://www.w3.org/ns/sosa/isSampleOf"/>
    <rdf:type rdf:resource="http://www.w3.org/2002/07/owl#Restriction"/>
    <owl:onClass rdf:resource="https://w3id.org/tern/ontologies/tern/Site"/>
    <owl:qualifiedCardinality rdf:datatype="http://www.w3.org/2001/XMLSchema#nonNegativeInteger">1</owl:qualifiedCardinality>
  </rdf:Description>
  <rdf:Description rdf:about="https://w3id.org/tern/ontologies/tern/isSamplingPointOf">
    <rdf:type rdf:resource="http://www.w3.org/1999/02/22-rdf-syntax-ns#Property"/>
    <rdfs:label>is sampling point of</rdfs:label>
    <owl:inverseOf rdf:resource="https://w3id.org/tern/ontologies/tern/hasSamplingPoint"/>
    <skos:definition>The inverse property [hasSamplingPoint](#hasSamplingPoint).</skos:definition>
  </rdf:Description>
  <rdf:Description rdf:about="https://w3id.org/tern/ontologies/tern/hasObservationTheme">
    <rdf:type rdf:resource="http://www.w3.org/1999/02/22-rdf-syntax-ns#Property"/>
    <skos:definition>Link a concept to an observation theme.</skos:definition>
    <rdfs:label>has observation theme</rdfs:label>
    <rdfs:subPropertyOf rdf:resource="http://www.w3.org/2004/02/skos/core#relatedMatch"/>
  </rdf:Description>
  <rdf:Description rdf:nodeID="ub1bL696C19">
    <owl:cardinality rdf:datatype="http://www.w3.org/2001/XMLSchema#nonNegativeInteger">1</owl:cardinality>
    <owl:onProperty rdf:resource="http://rs.tdwg.org/dwc/terms/materialSampleID"/>
    <rdf:type rdf:resource="http://www.w3.org/2002/07/owl#Restriction"/>
  </rdf:Description>
  <rdf:Description rdf:about="https://w3id.org/tern/ontologies/tern/TERNDerivedObservation">
    <rdf:type rdf:resource="http://www.w3.org/2002/07/owl#Class"/>
    <skos:definition>A derived observation created by TERN.</skos:definition>
    <rdfs:subClassOf rdf:resource="https://w3id.org/tern/ontologies/tern/DerivedObservation"/>
    <rdfs:label>TERN Derived Observation</rdfs:label>
  </rdf:Description>
  <rdf:Description rdf:about="https://w3id.org/tern/ontologies/tern/Transect">
    <rdfs:subClassOf rdf:nodeID="ub1bL1392C19"/>
    <rdfs:subClassOf rdf:nodeID="ub1bL1404C19"/>
    <rdf:type rdf:resource="http://www.w3.org/2002/07/owl#Class"/>
    <rdfs:label>Transect</rdfs:label>
    <rdfs:subClassOf rdf:nodeID="ub1bL1398C19"/>
    <skos:definition>A straight line or narrow section through an object or natural feature or across the earth's surface, along which observations are made or measurements taken.</skos:definition>
    <rdfs:subClassOf rdf:nodeID="ub1bL1382C19"/>
    <rdfs:subClassOf rdf:resource="https://w3id.org/tern/ontologies/tern/Sample"/>
    <rdfs:subClassOf rdf:nodeID="ub1bL1387C19"/>
  </rdf:Description>
  <rdf:Description rdf:about="https://w3id.org/tern/ontologies/tern/EarthObservationSatellite">
    <rdf:type rdf:resource="http://www.w3.org/2002/07/owl#Class"/>
    <rdfs:subClassOf rdf:resource="https://w3id.org/tern/ontologies/tern/MobilePlatform"/>
    <skos:definition>Earth observation satellites are satellites specifically designed to observe Earth from orbit, similar to spy satellites but intended for non-military uses such as environmental monitoring, meteorology, map making etc. Source: Wikipedia, http://en.wikipedia.org/wiki/Earth_observation_satellite Group: Platform_Details Entry_ID: Earth Observation Satellites Group: Platform_Identification Platform_Category: Earth Observation Satellites Short_Name: Earth Observation Satellites End_Group End_Group</skos:definition>
    <rdfs:seeAlso rdf:resource="https://gcmd.earthdata.nasa.gov/kms/concept/3466eed1-2fbb-49bf-ab0b-dc08731d502b"/>
    <rdfs:label>Earth Observation Satellite</rdfs:label>
  </rdf:Description>
  <rdf:Description rdf:nodeID="ub1bL110C23">
    <rdf:type rdf:resource="https://schema.org/Person"/>
    <schema-https:affiliation rdf:resource="https://w3id.org/tern/resources/a083902d-d821-41be-b663-1d7cb33eea66"/>
    <schema-https:email>mosheh.eliyahu@adelaide.edu.au</schema-https:email>
    <schema-https:name>Mosheh Eliyahu</schema-https:name>
  </rdf:Description>
  <rdf:Description rdf:nodeID="ub1bL701C19">
    <owl:onClass rdf:resource="https://w3id.org/tern/ontologies/loc/Point"/>
    <owl:maxQualifiedCardinality rdf:datatype="http://www.w3.org/2001/XMLSchema#nonNegativeInteger">1</owl:maxQualifiedCardinality>
    <owl:onProperty rdf:resource="https://w3id.org/tern/ontologies/tern/sampleStorageLocation"/>
    <rdf:type rdf:resource="http://www.w3.org/2002/07/owl#Restriction"/>
  </rdf:Description>
  <rdf:Description rdf:nodeID="ub1bL1349C19">
    <owl:minQualifiedCardinality rdf:datatype="http://www.w3.org/2001/XMLSchema#nonNegativeInteger">1</owl:minQualifiedCardinality>
    <owl:onClass rdf:resource="https://w3id.org/tern/ontologies/tern/SoilHorizon"/>
    <owl:onProperty rdf:resource="http://www.w3.org/ns/sosa/hasSample"/>
    <rdf:type rdf:resource="http://www.w3.org/2002/07/owl#Restriction"/>
  </rdf:Description>
  <rdf:Description rdf:nodeID="ub1bL842C19">
    <owl:onProperty rdf:resource="http://www.w3.org/2000/01/rdf-schema#comment"/>
    <rdf:type rdf:resource="http://www.w3.org/2002/07/owl#Restriction"/>
    <owl:allValuesFrom rdf:resource="http://www.w3.org/2001/XMLSchema#string"/>
  </rdf:Description>
  <rdf:Description rdf:about="https://w3id.org/tern/ontologies/tern/polygon">
    <rdfs:subPropertyOf rdf:resource="http://www.opengis.net/ont/geosparql#hasGeometry"/>
    <rdf:type rdf:resource="http://www.w3.org/1999/02/22-rdf-syntax-ns#Property"/>
    <skos:definition>The polygon of the subject.</skos:definition>
    <rdfs:range rdf:resource="https://w3id.org/tern/ontologies/loc/Polygon"/>
    <rdfs:label>polygon</rdfs:label>
  </rdf:Description>
  <rdf:Description rdf:nodeID="ub1bL758C19">
    <owl:allValuesFrom rdf:resource="http://www.w3.org/2001/XMLSchema#string"/>
    <owl:onProperty rdf:resource="http://schema.org/description"/>
    <rdf:type rdf:resource="http://www.w3.org/2002/07/owl#Restriction"/>
  </rdf:Description>
  <rdf:Description rdf:nodeID="f5a816f5a0f7a4e439059a4ae4caf6ab4b18">
    <rdf:rest rdf:nodeID="f5a816f5a0f7a4e439059a4ae4caf6ab4b19"/>
    <rdf:first rdf:resource="https://w3id.org/tern/ontologies/tern/Observation"/>
  </rdf:Description>
  <rdf:Description rdf:about="https://w3id.org/tern/ontologies/tern/SoilProfile">
    <rdfs:subClassOf rdf:nodeID="ub1bL1344C19"/>
    <rdf:type rdf:resource="http://www.w3.org/2002/07/owl#Class"/>
    <skos:example rdf:resource="https://www.qld.gov.au/environment/land/management/soil/soil-explained/forms"/>
    <rdfs:subClassOf rdf:nodeID="ub1bL1349C19"/>
    <rdfs:label>Soil Profile</rdfs:label>
    <rdfs:subClassOf rdf:resource="https://w3id.org/tern/ontologies/tern/Sample"/>
    <skos:definition>A soil profile is a vertical section of a soil from the soil surface through all its horizons to parent material, other consolidated substrate material or selected depth in unconsolidated material (Credit: Australian Soil and Land Survey Field Handbook).</skos:definition>
  </rdf:Description>
  <rdf:Description rdf:nodeID="ub1bL729C19">
    <owl:onProperty rdf:resource="http://linked.data.gov.au/def/datatype/vocabulary"/>
    <owl:cardinality rdf:datatype="http://www.w3.org/2001/XMLSchema#nonNegativeInteger">1</owl:cardinality>
    <rdf:type rdf:resource="http://www.w3.org/2002/07/owl#Restriction"/>
  </rdf:Description>
  <rdf:Description rdf:nodeID="ub1bL906C19">
    <owl:onProperty rdf:resource="http://www.w3.org/2000/01/rdf-schema#comment"/>
    <owl:allValuesFrom rdf:resource="http://www.w3.org/2001/XMLSchema#string"/>
    <rdf:type rdf:resource="http://www.w3.org/2002/07/owl#Restriction"/>
  </rdf:Description>
  <rdf:Description rdf:nodeID="ub1bL423C19">
    <owl:onProperty rdf:resource="http://linked.data.gov.au/def/datatype/value"/>
    <rdf:type rdf:resource="http://www.w3.org/2002/07/owl#Restriction"/>
    <owl:cardinality rdf:datatype="http://www.w3.org/2001/XMLSchema#nonNegativeInteger">1</owl:cardinality>
  </rdf:Description>
  <rdf:Description rdf:nodeID="ub1bL592C19">
    <rdf:type rdf:resource="http://www.w3.org/2002/07/owl#Restriction"/>
    <owl:onClass rdf:resource="https://w3id.org/tern/ontologies/tern/Site"/>
    <owl:maxQualifiedCardinality rdf:datatype="http://www.w3.org/2001/XMLSchema#nonNegativeInteger">1</owl:maxQualifiedCardinality>
    <owl:onProperty rdf:resource="https://w3id.org/tern/ontologies/tern/site"/>
  </rdf:Description>
  <rdf:Description rdf:nodeID="ub1bL418C19">
    <owl:onProperty rdf:resource="http://purl.org/dc/terms/description"/>
    <rdf:type rdf:resource="http://www.w3.org/2002/07/owl#Restriction"/>
    <owl:allValuesFrom rdf:resource="http://www.w3.org/2001/XMLSchema#string"/>
  </rdf:Description>
  <rdf:Description rdf:about="https://w3id.org/tern/ontologies/tern/Procedure">
    <rdfs:subClassOf rdf:nodeID="ub1bL724C19"/>
    <rdf:type rdf:resource="http://www.w3.org/2002/07/owl#Class"/>
    <skos:scopeNote>[Input](#Input) can be used to capture any input values for a procedure, such as the input value of the basal wedge to estimate the basal area per hectare.</skos:scopeNote>
    <skos:definition>A workflow, protocol, plan, algorithm, or computational method specifying how to make an [Observation](#Observation), create a [Sample](#Sample), or make a change to the state of the world (via an [Actuator](http://w3.org/ns/sosa/Actuator). A [Procedure](#Procedure) is re-usable, and might be involved in many [Observations](#Observation), [Samplings](#Sampling), or [Actuations](http://w3.org/ns/sosa/Actuation). it explains the steps to be carried out to arrive at reproducible [Results](#Result).</skos:definition>
    <rdfs:subClassOf rdf:nodeID="ub1bL734C19"/>
    <rdfs:subClassOf rdf:nodeID="ub1bL729C19"/>
    <rdfs:label>Procedure</rdfs:label>
    <skos:example>The procedure for collecting photopoints are specified in the 
[AusPlots Rangelands Survey Protocols Manual](http://dx.doi.org/10.13140/2.1.4287.3607).
The DEC Nature Conservation Service Biodiversity have defined 
[standard procedures](https://www.dpaw.wa.gov.au/images/documents/plants-animals/monitoring/sop/sop_establishingvegetationquadrats_20090818_v1.0.pdf)
for establishing quadrats for vegetation sampling.</skos:example>
    <rdfs:subClassOf rdf:nodeID="ub1bL740C19"/>
    <rdfs:subClassOf rdf:resource="http://www.w3.org/ns/sosa/Procedure"/>
  </rdf:Description>
  <rdf:Description rdf:about="https://w3id.org/tern/ontologies/tern/Sampling">
    <rdf:type rdf:resource="http://www.w3.org/2002/07/owl#Class"/>
    <rdfs:subClassOf rdf:nodeID="ub1bL911C19"/>
    <rdfs:subClassOf rdf:nodeID="ub1bL934C19"/>
    <rdfs:subClassOf rdf:nodeID="ub1bL906C19"/>
    <skos:definition>An activity of [Sampling](#Sampling) carries out a (Sampling) [Procedure](#Procedure) to create or transform one or more [Samples](#Sample).</skos:definition>
    <rdfs:subClassOf rdf:resource="http://www.w3.org/ns/sosa/Sampling"/>
    <skos:example>Crushing a rock sample in a ball mill to create sub-samples of the rock.
Digging a pit through a soil sequence.
Dividing a field site into quadrants.
Drawing blood from a patient.
Drilling an observation well.
Establishing a station for environmental monitoring.
Registering an image of the landscape.
Sieving a powder to separate the subset finer than 100-mesh.
Selecting a subset of a population.
Splitting a piece of drill-core to create two new samples.
Taking a diamond-drill core from a rock outcrop.</skos:example>
    <rdfs:subClassOf rdf:resource="http://www.w3.org/ns/prov#Activity"/>
    <rdfs:subClassOf rdf:nodeID="ub1bL922C19"/>
    <rdfs:subClassOf rdf:nodeID="ub1bL916C19"/>
    <rdfs:subClassOf rdf:nodeID="ub1bL928C19"/>
    <rdfs:label>Sampling</rdfs:label>
  </rdf:Description>
  <rdf:Description rdf:about="https://w3id.org/tern/ontologies/tern/ObservationTheme">
    <rdf:type rdf:resource="http://www.w3.org/2002/07/owl#Class"/>
    <rdfs:label>Observation Theme</rdfs:label>
    <skos:example>Field observations can be categorized into themes 
such as vegetation communities, landscape features, 
soil features and fauna populations.</skos:example>
    <skos:definition>An [Observation Theme](#ObservationTheme) categorises [Parameters](#Parameter) (i.e., properties observed) based on a topic of interest.</skos:definition>
    <skos:scopeNote>This concept is more commonly used at the application level and is usually mappable to a [FeatureOfInterest](http://w3.org/ns/sosa/FeatureOfInterest).</skos:scopeNote>
    <rdfs:subClassOf rdf:resource="http://www.w3.org/2004/02/skos/core#Concept"/>
  </rdf:Description>
  <rdf:Description rdf:nodeID="ub1bL934C19">
    <owl:onProperty rdf:resource="http://www.w3.org/ns/sosa/hasResult"/>
    <owl:onClass rdf:resource="https://w3id.org/tern/ontologies/tern/Sample"/>
    <owl:qualifiedCardinality rdf:datatype="http://www.w3.org/2001/XMLSchema#nonNegativeInteger">1</owl:qualifiedCardinality>
    <rdf:type rdf:resource="http://www.w3.org/2002/07/owl#Restriction"/>
  </rdf:Description>
  <rdf:Description rdf:nodeID="ub1bL975C19">
    <owl:onProperty rdf:resource="http://purl.org/dc/terms/identifier"/>
    <owl:maxQualifiedCardinality rdf:datatype="http://www.w3.org/2001/XMLSchema#nonNegativeInteger">1</owl:maxQualifiedCardinality>
    <owl:onClass rdf:resource="http://www.w3.org/2001/XMLSchema#string"/>
    <rdf:type rdf:resource="http://www.w3.org/2002/07/owl#Restriction"/>
  </rdf:Description>
  <rdf:Description rdf:nodeID="ub1bL857C19">
    <owl:onProperty rdf:resource="http://www.w3.org/ns/sosa/hasSample"/>
    <rdf:type rdf:resource="http://www.w3.org/2002/07/owl#Restriction"/>
    <owl:allValuesFrom rdf:resource="https://w3id.org/tern/ontologies/tern/Sample"/>
  </rdf:Description>
  <rdf:Description rdf:nodeID="ub1bL763C19">
    <rdf:type rdf:resource="http://www.w3.org/2002/07/owl#Restriction"/>
    <owl:onProperty rdf:resource="http://schema.org/name"/>
    <owl:onClass rdf:resource="http://www.w3.org/2001/XMLSchema#string"/>
    <owl:qualifiedCardinality rdf:datatype="http://www.w3.org/2001/XMLSchema#nonNegativeInteger">1</owl:qualifiedCardinality>
  </rdf:Description>
  <rdf:Description rdf:nodeID="ub1bL122C19">
    <schema-https:affiliation rdf:resource="https://w3id.org/tern/resources/a083902d-d821-41be-b663-1d7cb33eea66"/>
    <schema-https:identifier rdf:resource="https://orcid.org/0000-0002-6047-9864"/>
    <rdf:type rdf:resource="https://schema.org/Person"/>
    <schema-https:email>e.chuc@uq.edu.au</schema-https:email>
    <schema-https:name>Edmond Chuc</schema-https:name>
  </rdf:Description>
  <rdf:Description rdf:nodeID="ub1bL486C19">
    <owl:onProperty rdf:resource="https://w3id.org/tern/ontologies/tern/equipment"/>
    <owl:maxQualifiedCardinality rdf:datatype="http://www.w3.org/2001/XMLSchema#nonNegativeInteger">1</owl:maxQualifiedCardinality>
    <owl:onDataRange rdf:resource="http://www.w3.org/2001/XMLSchema#string"/>
    <rdf:type rdf:resource="http://www.w3.org/2002/07/owl#Restriction"/>
  </rdf:Description>
  <rdf:Description rdf:about="https://w3id.org/tern/ontologies/tern/PhenologyCamera">
    <rdf:type rdf:resource="http://www.w3.org/2002/07/owl#Class"/>
    <rdfs:subClassOf rdf:nodeID="ub1bL682C19"/>
    <skos:altLabel>Phenocamera</skos:altLabel>
    <rdfs:subClassOf rdf:nodeID="ub1bL672C19"/>
    <rdfs:seeAlso rdf:resource="https://www.neonscience.org/data-collection/phenocams"/>
    <rdfs:subClassOf rdf:resource="https://w3id.org/tern/ontologies/tern/Sampler"/>
    <skos:definition>A "phenocam" is a digital camera capturing time-lapse images of foliage which can be used to generate quantitative measures of plant phenology. Over time, these data provide a near-continuous visual record of canopy change and environmental conditions.</skos:definition>
    <skos:altLabel>Phenocam</skos:altLabel>
    <rdfs:label>Phenology Camera</rdfs:label>
    <rdfs:subClassOf rdf:nodeID="ub1bL677C19"/>
  </rdf:Description>
  <rdf:Description rdf:nodeID="ub1bL1332C19">
    <rdf:type rdf:resource="http://www.w3.org/2002/07/owl#Restriction"/>
    <owl:allValuesFrom rdf:resource="https://w3id.org/tern/ontologies/tern/SoilProfile"/>
    <owl:onProperty rdf:resource="http://www.w3.org/ns/sosa/isSampleOf"/>
  </rdf:Description>
  <rdf:Description rdf:about="https://w3id.org/tern/ontologies/tern/SiteVisit">
    <skos:definition>A discrete time-bounded visit to a site, during which sampling or observation activities are undertaken.</skos:definition>
    <rdfs:subClassOf rdf:nodeID="ub1bL1310C19"/>
    <rdfs:subClassOf rdf:nodeID="ub1bL1292C19"/>
    <rdf:type rdf:resource="http://www.w3.org/2002/07/owl#Class"/>
    <rdfs:subClassOf rdf:resource="http://www.w3.org/ns/prov#Activity"/>
    <rdfs:subClassOf rdf:nodeID="ub1bL1286C19"/>
    <rdfs:label>Site Visit</rdfs:label>
    <rdfs:subClassOf rdf:nodeID="ub1bL1265C19"/>
    <rdfs:subClassOf rdf:nodeID="ub1bL1275C19"/>
    <rdfs:subClassOf rdf:nodeID="ub1bL1260C19"/>
    <rdfs:subClassOf rdf:nodeID="ub1bL1304C19"/>
    <rdfs:subClassOf rdf:nodeID="ub1bL1255C19"/>
    <rdfs:subClassOf rdf:nodeID="ub1bL1298C19"/>
    <rdfs:subClassOf rdf:nodeID="ub1bL1250C19"/>
    <rdfs:subClassOf rdf:nodeID="ub1bL1270C19"/>
  </rdf:Description>
  <rdf:Description rdf:nodeID="ub1bL622C19">
    <owl:onClass rdf:resource="http://www.w3.org/ns/sosa/FeatureOfInterest"/>
    <owl:qualifiedCardinality rdf:datatype="http://www.w3.org/2001/XMLSchema#nonNegativeInteger">1</owl:qualifiedCardinality>
    <rdf:type rdf:resource="http://www.w3.org/2002/07/owl#Restriction"/>
    <owl:onProperty rdf:resource="http://www.w3.org/ns/sosa/hasFeatureOfInterest"/>
  </rdf:Description>
  <rdf:Description rdf:nodeID="ub1bL911C19">
    <owl:allValuesFrom rdf:resource="https://w3id.org/tern/ontologies/org/Person"/>
    <owl:onProperty rdf:resource="http://www.w3.org/ns/prov#wasAttributedTo"/>
    <rdf:type rdf:resource="http://www.w3.org/2002/07/owl#Restriction"/>
  </rdf:Description>
  <rdf:Description rdf:about="https://w3id.org/tern/ontologies/tern/isGlobalMatchOf">
    <rdf:type rdf:resource="http://www.w3.org/1999/02/22-rdf-syntax-ns#Property"/>
    <rdfs:subPropertyOf rdf:resource="http://www.w3.org/2004/02/skos/core#exactMatch"/>
    <skos:definition>An inverse property of [globalMatch](#globalMatch); Links an upper concept to a concept (in the closed system).</skos:definition>
    <skos:scopeNote>Use in between controlled vocabularies.</skos:scopeNote>
    <owl:inverseOf rdf:resource="https://w3id.org/tern/ontologies/tern/globalMatch"/>
    <rdfs:label>is global match of</rdfs:label>
  </rdf:Description>
  <rdf:Description rdf:nodeID="ub1bL852C19">
    <owl:allValuesFrom rdf:resource="https://w3id.org/tern/ontologies/tern/Observation"/>
    <owl:onProperty rdf:resource="http://www.w3.org/ns/sosa/isFeatureOfInterestOf"/>
    <rdf:type rdf:resource="http://www.w3.org/2002/07/owl#Restriction"/>
  </rdf:Description>
  <rdf:Description rdf:nodeID="ub1bL740C19">
    <owl:qualifiedCardinality rdf:datatype="http://www.w3.org/2001/XMLSchema#nonNegativeInteger">1</owl:qualifiedCardinality>
    <rdf:type rdf:resource="http://www.w3.org/2002/07/owl#Restriction"/>
    <owl:onProperty rdf:resource="http://www.w3.org/1999/02/22-rdf-syntax-ns#value"/>
    <owl:onClass rdf:resource="https://w3id.org/tern/ontologies/tern/Method"/>
  </rdf:Description>
  <rdf:Description rdf:nodeID="ub1bL555C19">
    <owl:maxCardinality rdf:datatype="http://www.w3.org/2001/XMLSchema#nonNegativeInteger">1</owl:maxCardinality>
    <rdf:type rdf:resource="http://www.w3.org/2002/07/owl#Restriction"/>
    <owl:onProperty rdf:resource="https://w3id.org/tern/ontologies/tern/globalVocabulary"/>
  </rdf:Description>
  <rdf:Description rdf:nodeID="ub1bL867C19">
    <owl:onProperty rdf:resource="http://www.w3.org/2000/01/rdf-schema#label"/>
    <rdf:type rdf:resource="http://www.w3.org/2002/07/owl#Restriction"/>
    <owl:cardinality rdf:datatype="http://www.w3.org/2001/XMLSchema#nonNegativeInteger">1</owl:cardinality>
  </rdf:Description>
  <rdf:Description rdf:about="https://w3id.org/tern/ontologies/tern/centroidPoint">
    <rdf:type rdf:resource="http://www.w3.org/1999/02/22-rdf-syntax-ns#Property"/>
    <rdfs:subPropertyOf rdf:resource="http://www.opengis.net/ont/geosparql#hasGeometry"/>
    <skos:example>The geometric center of 1-ha vegetation plot expressed 
as [tern-loc:Point](https://w3id.org/tern/ontologies/loc/Point).</skos:example>
    <rdfs:range rdf:resource="https://w3id.org/tern/ontologies/loc/Point"/>
    <rdfs:label>centroid point</rdfs:label>
    <skos:definition>The centroid point of an object-of-interest.</skos:definition>
    <rdfs:seeAlso rdf:resource="https://en.wikipedia.org/wiki/List_of_centroids"/>
  </rdf:Description>
  <rdf:Description rdf:nodeID="ub1bL1107C19">
    <owl:maxQualifiedCardinality rdf:datatype="http://www.w3.org/2001/XMLSchema#nonNegativeInteger">1</owl:maxQualifiedCardinality>
    <owl:onClass rdf:resource="http://www.w3.org/2001/XMLSchema#date"/>
    <rdf:type rdf:resource="http://www.w3.org/2002/07/owl#Restriction"/>
    <owl:onProperty rdf:resource="https://w3id.org/tern/ontologies/tern/dateDecommissioned"/>
  </rdf:Description>
  <rdf:Description rdf:nodeID="ub1bL237C19">
    <owl:allValuesFrom rdf:resource="http://www.w3.org/2001/XMLSchema#string"/>
    <rdf:type rdf:resource="http://www.w3.org/2002/07/owl#Restriction"/>
    <owl:onProperty rdf:resource="http://www.w3.org/2004/02/skos/core#altLabel"/>
  </rdf:Description>
  <rdf:Description rdf:about="https://w3id.org/tern/ontologies/tern/siteDescription">
    <skos:scopeNote>Value is usually a summary sentence of the site.</skos:scopeNote>
    <skos:definition>Contextual information is collected at each site. This includes measures of slope an aspect, surface strew and lithology, and information on the grazing and fire history of the site (Credit: TERN AusPlots).</skos:definition>
    <rdfs:label>site description</rdfs:label>
    <rdf:type rdf:resource="http://www.w3.org/1999/02/22-rdf-syntax-ns#Property"/>
    <skos:example rdf:resource="http://ozflux.org.au/monitoringsites/alicesprings/alicesprings_description.html"/>
  </rdf:Description>
  <rdf:Description rdf:about="https://w3id.org/tern/ontologies/tern/SuperSite">
    <rdf:type rdf:resource="http://www.w3.org/2002/07/owl#Class"/>
    <rdfs:subClassOf rdf:resource="https://w3id.org/tern/ontologies/tern/Site"/>
    <rdfs:label>SuperSite</rdfs:label>
    <skos:definition>TERN SuperSites are Long Term Ecological Research (LTER) sites co-located with TERN OzFlux eddy covariance towers, which deliver biological and environmental observations of flora, fauna, microbial biodiversity, soils and hydrology. TERN OzFlux delivers micrometeorological observations of energy, carbon and water exchange between the atmosphere and key Australian ecosystems. Each TERN SuperSite is located in a significant Australian biome and the network spans a wide range of environmental conditions. The SuperSite network collects detailed data sets on flora, fauna and biophysical processes from each SuperSite.</skos:definition>
    <rdfs:seeAlso rdf:resource="https://supersites.tern.org.au/"/>
  </rdf:Description>
  <rdf:Description rdf:about="https://w3id.org/tern/ontologies/tern/Parameter">
    <rdfs:label>Parameter</rdfs:label>
    <rdf:type rdf:resource="http://www.w3.org/2002/07/owl#Class"/>
    <skos:definition>A [FeatureOfInterest's](http://w3.org/ns/sosa/FeatureOfInterest) property or characteristic which an [Observation](#Observation) is measuring using some [Procedure](#Procedure).</skos:definition>
    <rdfs:subClassOf rdf:resource="http://www.w3.org/2004/02/skos/core#Concept"/>
  </rdf:Description>
  <rdf:Description rdf:nodeID="ub1bL386C19">
    <owl:maxQualifiedCardinality rdf:datatype="http://www.w3.org/2001/XMLSchema#nonNegativeInteger">1</owl:maxQualifiedCardinality>
    <owl:onDataRange rdf:resource="http://www.w3.org/2001/XMLSchema#string"/>
    <owl:onProperty rdf:resource="https://w3id.org/tern/ontologies/tern/purpose"/>
    <rdf:type rdf:resource="http://www.w3.org/2002/07/owl#Restriction"/>
  </rdf:Description>
  <rdf:Description rdf:about="https://w3id.org/tern/ontologies/tern/SiteTaxon">
    <rdfs:label>Site Taxon</rdfs:label>
    <rdfs:subClassOf rdf:resource="https://w3id.org/tern/ontologies/tern/Sample"/>
    <rdf:type rdf:resource="http://www.w3.org/2002/07/owl#Class"/>
    <rdfs:subClassOf rdf:nodeID="ub1bL1239C19"/>
  </rdf:Description>
  <rdf:Description rdf:nodeID="ub1bL640C19">
    <rdf:type rdf:resource="http://www.w3.org/2002/07/owl#Restriction"/>
    <owl:qualifiedCardinality rdf:datatype="http://www.w3.org/2001/XMLSchema#nonNegativeInteger">1</owl:qualifiedCardinality>
    <owl:onProperty rdf:resource="http://www.w3.org/ns/sosa/resultTime"/>
    <owl:onDataRange rdf:resource="http://www.w3.org/2001/XMLSchema#dateTime"/>
  </rdf:Description>
  <rdf:Description rdf:nodeID="ub1bL1298C19">
    <owl:onProperty rdf:resource="http://purl.org/dc/terms/identifier"/>
    <owl:qualifiedCardinality rdf:datatype="http://www.w3.org/2001/XMLSchema#nonNegativeInteger">1</owl:qualifiedCardinality>
    <owl:onClass rdf:resource="http://www.w3.org/2001/XMLSchema#string"/>
    <rdf:type rdf:resource="http://www.w3.org/2002/07/owl#Restriction"/>
  </rdf:Description>
  <rdf:Description rdf:about="https://w3id.org/tern/ontologies/tern/instructions">
    <skos:definition>Describe the instructions of the procedure/method.</skos:definition>
    <rdfs:label>instructions</rdfs:label>
    <rdfs:range rdf:resource="http://www.w3.org/2001/XMLSchema#string"/>
    <rdf:type rdf:resource="http://www.w3.org/2002/07/owl#DatatypeProperty"/>
  </rdf:Description>
  <rdf:Description rdf:about="https://w3id.org/tern/ontologies/tern/observationTheme">
    <rdfs:domain rdf:resource="https://w3id.org/tern/ontologies/tern/Observation"/>
    <rdf:type rdf:resource="http://www.w3.org/1999/02/22-rdf-syntax-ns#Property"/>
    <rdfs:subPropertyOf rdf:resource="http://purl.org/dc/terms/type"/>
    <rdfs:label>observation theme</rdfs:label>
    <skos:definition>Group observations into themes. See TERN's controlled list of &lt;a href="http://linked.data.gov.au/def/tern-cv/396192ae-3bd5-4050-b578-93107510129c"&gt;observation themes&lt;/a&gt; as example values.</skos:definition>
  </rdf:Description>
  <rdf:Description rdf:nodeID="ub1bL297C19">
    <owl:cardinality rdf:datatype="http://www.w3.org/2001/XMLSchema#nonNegativeInteger">1</owl:cardinality>
    <owl:onProperty rdf:resource="https://w3id.org/tern/ontologies/tern/length"/>
    <rdf:type rdf:resource="http://www.w3.org/2002/07/owl#Restriction"/>
  </rdf:Description>
  <rdf:Description rdf:about="https://w3id.org/tern/ontologies/tern/scope">
    <rdfs:range rdf:resource="http://www.w3.org/2001/XMLSchema#string"/>
    <rdfs:label>scope</rdfs:label>
    <skos:definition>Describe the scope of something.</skos:definition>
    <rdf:type rdf:resource="http://www.w3.org/2002/07/owl#DatatypeProperty"/>
  </rdf:Description>
  <rdf:Description rdf:nodeID="ub1bL1137C19">
    <owl:onClass rdf:resource="https://w3id.org/tern/ontologies/loc/Point"/>
    <owl:onProperty rdf:resource="https://w3id.org/tern/ontologies/tern/centroidPoint"/>
    <owl:maxQualifiedCardinality rdf:datatype="http://www.w3.org/2001/XMLSchema#nonNegativeInteger">1</owl:maxQualifiedCardinality>
    <rdf:type rdf:resource="http://www.w3.org/2002/07/owl#Restriction"/>
  </rdf:Description>
  <rdf:Description rdf:nodeID="ub1bL805C19">
    <owl:allValuesFrom rdf:resource="https://w3id.org/tern/ontologies/org/Person"/>
    <owl:onProperty rdf:resource="http://www.w3.org/ns/prov#wasAttributedTo"/>
    <rdf:type rdf:resource="http://www.w3.org/2002/07/owl#Restriction"/>
  </rdf:Description>
  <rdf:Description rdf:nodeID="ub1bL492C19">
    <owl:onDataRange rdf:resource="http://www.w3.org/2001/XMLSchema#string"/>
    <rdf:type rdf:resource="http://www.w3.org/2002/07/owl#Restriction"/>
    <owl:maxQualifiedCardinality rdf:datatype="http://www.w3.org/2001/XMLSchema#nonNegativeInteger">1</owl:maxQualifiedCardinality>
    <owl:onProperty rdf:resource="https://w3id.org/tern/ontologies/tern/instructions"/>
  </rdf:Description>
  <rdf:Description rdf:about="https://w3id.org/tern/ontologies/tern/globalVocabulary">
    <rdfs:label>global vocabulary</rdfs:label>
    <skos:definition>The global vocabulary refers to the main vocabulary, which takes precedence over other similar vocabularies to promote data harmonisation.</skos:definition>
    <rdf:type rdf:resource="http://www.w3.org/1999/02/22-rdf-syntax-ns#Property"/>
  </rdf:Description>
  <rdf:Description rdf:nodeID="ub1bL104C23">
    <schema-https:affiliation rdf:resource="https://w3id.org/tern/resources/a083902d-d821-41be-b663-1d7cb33eea66"/>
    <schema-https:name>Javier Sanchez Gonzalez</schema-https:name>
    <rdf:type rdf:resource="https://schema.org/Person"/>
    <schema-https:email>j.sanchezgonzalez@uq.edu.au</schema-https:email>
  </rdf:Description>
  <rdf:Description rdf:about="https://w3id.org/tern/ontologies/tern/SamplingPoint">
    <rdfs:subClassOf rdf:nodeID="ub1bL987C19"/>
    <rdfs:subClassOf rdf:resource="https://w3id.org/tern/ontologies/loc/Point"/>
    <rdfs:subClassOf rdf:nodeID="ub1bL993C19"/>
    <rdfs:subClassOf rdf:nodeID="ub1bL969C19"/>
    <rdfs:subClassOf rdf:nodeID="ub1bL999C19"/>
    <rdf:type rdf:resource="http://www.w3.org/2002/07/owl#Class"/>
    <rdfs:subClassOf rdf:nodeID="ub1bL981C19"/>
    <rdfs:label>Sampling Point</rdfs:label>
    <rdfs:subClassOf rdf:nodeID="ub1bL957C19"/>
    <skos:definition>A point in space where an [Observation](#Observation) or [Sampling](#Sampling) occurred. </skos:definition>
    <rdfs:subClassOf rdf:nodeID="ub1bL975C19"/>
    <rdfs:subClassOf rdf:nodeID="ub1bL963C19"/>
  </rdf:Description>
  <rdf:Description rdf:nodeID="ub1bL566C19">
    <rdf:type rdf:resource="http://www.w3.org/2002/07/owl#Restriction"/>
    <owl:onClass rdf:resource="https://w3id.org/tern/ontologies/tern/Parameter"/>
    <owl:onProperty rdf:resource="http://www.w3.org/1999/02/22-rdf-syntax-ns#value"/>
    <owl:qualifiedCardinality rdf:datatype="http://www.w3.org/2001/XMLSchema#nonNegativeInteger">1</owl:qualifiedCardinality>
  </rdf:Description>
  <rdf:Description rdf:about="https://w3id.org/tern/ontologies/tern/CORVEGSite">
    <dcterms:source rdf:resource="https://www.data.qld.gov.au/dataset/queensland-corveg-database"/>
    <rdf:type rdf:resource="http://www.w3.org/2002/07/owl#Class"/>
    <rdfs:subClassOf rdf:resource="https://w3id.org/tern/ontologies/tern/Site"/>
    <rdfs:label>CORVEG Site</rdfs:label>
    <skos:definition>A [CORVEG Site](#CORVEGSite) refers to a study location in Queensland that was visited since 1982 to collect data on physical and vegetation features, including structural and floristic attributes as well as descriptions of its landscape, soil and geological features.</skos:definition>
    <skos:example rdf:resource="http://linked.data.gov.au/dataset/corveg/site-12319"/>
    <skos:seeAlso rdf:resource="http://aekos.org.au/collection/qld.gov.au/corveg"/>
  </rdf:Description>
  <rdf:Description rdf:about="https://w3id.org/tern/ontologies/tern/ObservableProperty">
    <rdf:type rdf:resource="http://www.w3.org/2002/07/owl#Class"/>
    <rdfs:subClassOf rdf:nodeID="ub1bL538C19"/>
    <rdfs:subClassOf rdf:nodeID="ub1bL560C19"/>
    <rdfs:subClassOf rdf:nodeID="ub1bL555C19"/>
    <skos:definition>An observable quality (property, characteristic) of a [FeatureOfInterest](http://w3.org/ns/sosa/FeatureOfInterest). A feature-of-interest refers to a feature whose properties are measured or observed. </skos:definition>
    <skos:example>Sampling depth, bulk density, pH are examples of properties of a 
soil sample, and the soil sample is the feature-of-interest, 
representative of the area from which it is collected.</skos:example>
    <rdfs:subClassOf rdf:resource="http://www.w3.org/ns/sosa/ObservableProperty"/>
    <rdfs:label>Observable Property</rdfs:label>
    <rdfs:subClassOf rdf:nodeID="ub1bL566C19"/>
    <rdfs:subClassOf rdf:nodeID="ub1bL550C19"/>
  </rdf:Description>
  <rdf:Description rdf:nodeID="ub1bL242C19">
    <rdf:type rdf:resource="http://www.w3.org/2002/07/owl#Restriction"/>
    <owl:onProperty rdf:resource="http://www.w3.org/2004/02/skos/core#definition"/>
    <owl:allValuesFrom rdf:resource="http://www.w3.org/2001/XMLSchema#string"/>
  </rdf:Description>
  <rdf:Description rdf:nodeID="ub1bL1392C19">
    <rdf:type rdf:resource="http://www.w3.org/2002/07/owl#Restriction"/>
    <owl:onProperty rdf:resource="http://www.opengis.net/ont/geosparql#hasGeometry"/>
    <owl:onClass rdf:resource="https://w3id.org/tern/ontologies/loc/LineString"/>
    <owl:qualifiedCardinality rdf:datatype="http://www.w3.org/2001/XMLSchema#nonNegativeInteger">1</owl:qualifiedCardinality>
  </rdf:Description>
  <rdf:Description rdf:nodeID="ub1bL604C19">
    <owl:onClass rdf:resource="https://w3id.org/tern/ontologies/tern/Result"/>
    <rdf:type rdf:resource="http://www.w3.org/2002/07/owl#Restriction"/>
    <owl:onProperty rdf:resource="http://www.w3.org/ns/sosa/hasResult"/>
    <owl:minQualifiedCardinality rdf:datatype="http://www.w3.org/2001/XMLSchema#nonNegativeInteger">1</owl:minQualifiedCardinality>
  </rdf:Description>
  <rdf:Description rdf:about="https://w3id.org/tern/ontologies/tern/DerivedObservation">
    <rdfs:label>Derived Observation</rdfs:label>
    <rdf:type rdf:resource="http://www.w3.org/2002/07/owl#Class"/>
    <skos:definition>A derived observation.</skos:definition>
    <rdfs:subClassOf rdf:resource="https://w3id.org/tern/ontologies/tern/Observation"/>
  </rdf:Description>
  <rdf:Description rdf:nodeID="ub1bL307C19">
    <owl:onProperty rdf:resource="http://linked.data.gov.au/def/datatype/unit"/>
    <owl:qualifiedCardinality rdf:datatype="http://www.w3.org/2001/XMLSchema#nonNegativeInteger">1</owl:qualifiedCardinality>
    <rdf:type rdf:resource="http://www.w3.org/2002/07/owl#Restriction"/>
    <owl:onClass rdf:resource="http://qudt.org/schema/qudt/Unit"/>
  </rdf:Description>
  <rdf:Description rdf:nodeID="ub1bL1022C19">
    <owl:onProperty rdf:resource="http://www.w3.org/ns/sosa/isHostedBy"/>
    <rdf:type rdf:resource="http://www.w3.org/2002/07/owl#Restriction"/>
    <owl:allValuesFrom rdf:resource="https://w3id.org/tern/ontologies/tern/Platform"/>
  </rdf:Description>
  <rdf:Description rdf:nodeID="ub1bL444C25">
    <owl:unionOf rdf:nodeID="f5a816f5a0f7a4e439059a4ae4caf6ab4b5"/>
    <rdf:type rdf:resource="http://www.w3.org/2002/07/owl#Class"/>
  </rdf:Description>
  <rdf:Description rdf:nodeID="ub1bL116C23">
    <schema-https:email>t.parkhurst@uq.edu.au</schema-https:email>
    <rdf:type rdf:resource="https://schema.org/Person"/>
    <schema-https:name>Tina Parkhurst</schema-https:name>
    <schema-https:affiliation rdf:resource="https://w3id.org/tern/resources/a083902d-d821-41be-b663-1d7cb33eea66"/>
  </rdf:Description>
  <rdf:Description rdf:about="https://w3id.org/tern/ontologies/tern/SAR">
    <skos:altLabel>SAR</skos:altLabel>
    <rdf:type rdf:resource="http://www.w3.org/2002/07/owl#Class"/>
    <rdfs:label>Synthetic Aperture Radar</rdfs:label>
    <skos:altLabel>Synthetic-aperture radar</skos:altLabel>
    <rdfs:seeAlso rdf:resource="https://earthdata.nasa.gov/learn/backgrounders/what-is-sar"/>
    <rdfs:subClassOf rdf:resource="https://w3id.org/tern/ontologies/tern/Sensor"/>
  </rdf:Description>
  <rdf:Description rdf:nodeID="ub1bL363C19">
    <owl:allValuesFrom rdf:resource="http://www.w3.org/2001/XMLSchema#string"/>
    <rdf:type rdf:resource="http://www.w3.org/2002/07/owl#Restriction"/>
    <owl:onProperty rdf:resource="http://www.w3.org/2000/01/rdf-schema#comment"/>
  </rdf:Description>
  <rdf:Description rdf:nodeID="f5a816f5a0f7a4e439059a4ae4caf6ab4b23">
    <rdf:rest rdf:resource="http://www.w3.org/1999/02/22-rdf-syntax-ns#nil"/>
    <rdf:first rdf:resource="http://www.w3.org/2001/XMLSchema#int"/>
  </rdf:Description>
  <rdf:Description rdf:about="https://w3id.org/tern/ontologies/tern/MobilePlatform">
    <skos:definition>A moving mobile platform on land, in water or in space.</skos:definition>
    <rdfs:subClassOf rdf:resource="https://w3id.org/tern/ontologies/tern/Platform"/>
    <rdfs:label>Mobile Platform</rdfs:label>
    <rdf:type rdf:resource="http://www.w3.org/2002/07/owl#Class"/>
  </rdf:Description>
  <rdf:Description rdf:about="https://w3id.org/tern/ontologies/tern/transectStartPoint">
    <rdfs:label>transect start point</rdfs:label>
    <skos:definition>Refers to the [tern-loc:Point](https://w3id.org/tern/ontologies/loc/Point) representing the start of a transect.</skos:definition>
    <rdfs:domain rdf:resource="https://w3id.org/tern/ontologies/tern/Transect"/>
    <rdf:type rdf:resource="http://www.w3.org/1999/02/22-rdf-syntax-ns#Property"/>
  </rdf:Description>
  <rdf:Description rdf:nodeID="f5a816f5a0f7a4e439059a4ae4caf6ab4b9">
    <rdf:rest rdf:nodeID="f5a816f5a0f7a4e439059a4ae4caf6ab4b10"/>
    <rdf:first rdf:resource="http://www.w3.org/2001/XMLSchema#string"/>
  </rdf:Description>
  <rdf:Description rdf:about="https://w3id.org/tern/ontologies/tern/domain">
    <rdf:type rdf:resource="http://www.w3.org/1999/02/22-rdf-syntax-ns#Property"/>
    <skos:example>Vegetation, soil, disturbance, landform, etc.</skos:example>
    <rdfs:label>domain</rdfs:label>
    <skos:definition>The domain of the observation.</skos:definition>
  </rdf:Description>
  <rdf:Description rdf:nodeID="ub1bL1075C19">
    <rdf:type rdf:resource="http://www.w3.org/2002/07/owl#Restriction"/>
    <owl:allValuesFrom rdf:resource="https://w3id.org/tern/ontologies/tern/SiteVisit"/>
    <owl:onProperty rdf:resource="https://w3id.org/tern/ontologies/tern/siteVisit"/>
  </rdf:Description>
  <rdf:Description rdf:nodeID="ub1bL634C19">
    <owl:onProperty rdf:resource="http://www.w3.org/ns/sosa/usedProcedure"/>
    <owl:qualifiedCardinality rdf:datatype="http://www.w3.org/2001/XMLSchema#nonNegativeInteger">1</owl:qualifiedCardinality>
    <rdf:type rdf:resource="http://www.w3.org/2002/07/owl#Restriction"/>
    <owl:onClass rdf:resource="https://w3id.org/tern/ontologies/tern/Procedure"/>
  </rdf:Description>
  <rdf:Description rdf:nodeID="ub1bL1216C19">
    <rdf:type rdf:resource="http://www.w3.org/2002/07/owl#Restriction"/>
    <owl:minQualifiedCardinality rdf:datatype="http://www.w3.org/2001/XMLSchema#nonNegativeInteger">1</owl:minQualifiedCardinality>
    <owl:onClass rdf:resource="https://w3id.org/tern/ontologies/tern/SiteStratum"/>
    <owl:onProperty rdf:resource="http://www.w3.org/ns/sosa/isSampleOf"/>
  </rdf:Description>
  <rdf:Description rdf:nodeID="ub1bL1060C19">
    <owl:allValuesFrom rdf:resource="https://w3id.org/tern/ontologies/tern/PropertyValue"/>
    <rdf:type rdf:resource="http://www.w3.org/2002/07/owl#Restriction"/>
    <owl:onProperty rdf:resource="http://schema.org/additionalProperty"/>
  </rdf:Description>
  <rdf:Description rdf:about="https://w3id.org/tern/ontologies/tern/Spectroradiometer">
    <rdf:type rdf:resource="http://www.w3.org/2002/07/owl#Class"/>
    <rdfs:seeAlso rdf:resource="https://en.wikipedia.org/wiki/Spectroradiometer"/>
    <rdfs:comment>A spectroradiometer is a light measurement tool that is able to measure both the wavelength and amplitude of the light emitted from a light source.</rdfs:comment>
    <rdfs:subClassOf rdf:resource="https://w3id.org/tern/ontologies/tern/Sensor"/>
    <rdfs:label>Spectroradiometer</rdfs:label>
  </rdf:Description>
  <rdf:Description rdf:nodeID="ub1bL963C19">
    <owl:onClass rdf:resource="http://linked.data.gov.au/def/datatype/QuantitativeMeasure"/>
    <owl:maxQualifiedCardinality rdf:datatype="http://www.w3.org/2001/XMLSchema#nonNegativeInteger">1</owl:maxQualifiedCardinality>
    <owl:onProperty rdf:resource="https://w3id.org/tern/ontologies/loc/depth"/>
    <rdf:type rdf:resource="http://www.w3.org/2002/07/owl#Restriction"/>
  </rdf:Description>
  <rdf:Description rdf:about="https://w3id.org/tern/ontologies/tern/cardinalDirection">
    <rdfs:label>cardinal direction</rdfs:label>
    <skos:definition>The cardinal direction of the *thing* represented as a string and expressed by cardinal and intercardinal points. </skos:definition>
    <skos:example>NNE, W, SE, etc.</skos:example>
    <rdf:type rdf:resource="http://www.w3.org/1999/02/22-rdf-syntax-ns#Property"/>
    <rdfs:range rdf:resource="http://www.w3.org/2001/XMLSchema#string"/>
  </rdf:Description>
  <rdf:Description rdf:nodeID="ub1bL1125C19">
    <rdf:type rdf:resource="http://www.w3.org/2002/07/owl#Restriction"/>
    <owl:maxQualifiedCardinality rdf:datatype="http://www.w3.org/2001/XMLSchema#nonNegativeInteger">1</owl:maxQualifiedCardinality>
    <owl:onProperty rdf:resource="https://w3id.org/tern/ontologies/tern/siteDescription"/>
    <owl:onClass rdf:resource="http://www.w3.org/2001/XMLSchema#string"/>
  </rdf:Description>
  <rdf:Description rdf:about="https://w3id.org/tern/ontologies/tern/locationProcedure">
    <rdfs:label>location procedure</rdfs:label>
    <rdfs:subPropertyOf rdf:resource="https://w3id.org/tern/ontologies/tern/hasMethod"/>
    <skos:definition>Link to a procedure used to obtain the location.</skos:definition>
    <rdf:type rdf:resource="http://www.w3.org/1999/02/22-rdf-syntax-ns#Property"/>
  </rdf:Description>
  <rdf:Description rdf:nodeID="ub1bL1228C19">
    <owl:onProperty rdf:resource="https://w3id.org/tern/ontologies/tern/taxon"/>
    <rdf:type rdf:resource="http://www.w3.org/2002/07/owl#Restriction"/>
    <owl:qualifiedCardinality rdf:datatype="http://www.w3.org/2001/XMLSchema#nonNegativeInteger">1</owl:qualifiedCardinality>
    <owl:onClass rdf:resource="https://w3id.org/tern/ontologies/sd/StateTaxon"/>
  </rdf:Description>
  <rdf:Description rdf:nodeID="ub1bL368C19">
    <owl:onClass rdf:resource="http://www.w3.org/2001/XMLSchema#date"/>
    <owl:maxQualifiedCardinality rdf:datatype="http://www.w3.org/2001/XMLSchema#nonNegativeInteger">1</owl:maxQualifiedCardinality>
    <rdf:type rdf:resource="http://www.w3.org/2002/07/owl#Restriction"/>
    <owl:onProperty rdf:resource="https://w3id.org/tern/ontologies/tern/dateDecommissioned"/>
  </rdf:Description>
  <rdf:Description rdf:nodeID="ub1bL172C23">
    <rdf:type rdf:resource="http://www.w3.org/ns/prov#Activity"/>
    <rdf:type rdf:resource="http://usefulinc.com/ns/doap#Project"/>
    <doap:repository rdf:resource="https://github.com/ternaustralia/ontology_tern"/>
  </rdf:Description>
  <rdf:Description rdf:nodeID="ub1bL374C19">
    <owl:maxQualifiedCardinality rdf:datatype="http://www.w3.org/2001/XMLSchema#nonNegativeInteger">1</owl:maxQualifiedCardinality>
    <owl:onClass rdf:resource="http://www.w3.org/2001/XMLSchema#string"/>
    <owl:onProperty rdf:resource="https://w3id.org/tern/ontologies/tern/fluxnetID"/>
    <rdf:type rdf:resource="http://www.w3.org/2002/07/owl#Restriction"/>
  </rdf:Description>
  <rdf:Description rdf:nodeID="ub1bL45C19">
    <owl:cardinality rdf:datatype="http://www.w3.org/2001/XMLSchema#nonNegativeInteger">1</owl:cardinality>
    <owl:onProperty rdf:resource="https://w3id.org/tern/ontologies/tern/globalValue"/>
    <rdf:type rdf:resource="http://www.w3.org/2002/07/owl#Restriction"/>
  </rdf:Description>
  <rdf:Description rdf:about="http://rs.tdwg.org/dwc/terms/MaterialSample">
    <rdfs:label>Material Sample</rdfs:label>
    <skos:example>A whole organism preserved in a collection. 
A part of an organism isolated for some purpose. A soil sample. A marine microbial sample.</skos:example>
    <rdf:type rdf:resource="http://www.w3.org/2002/07/owl#Class"/>
    <rdfs:isDefinedBy rdf:resource="http://rs.tdwg.org/dwc/terms/"/>
    <rdfs:comment>A physical result of a sampling (or subsampling) event. In biological collections, the material sample is typically collected, and either preserved or destructively processed.</rdfs:comment>
  </rdf:Description>
  <rdf:Description rdf:nodeID="ub1bL734C19">
    <rdf:type rdf:resource="http://www.w3.org/2002/07/owl#Restriction"/>
    <owl:maxQualifiedCardinality rdf:datatype="http://www.w3.org/2001/XMLSchema#nonNegativeInteger">1</owl:maxQualifiedCardinality>
    <owl:onClass rdf:resource="https://w3id.org/tern/ontologies/tern/Input"/>
    <owl:onProperty rdf:resource="http://www.w3.org/ns/ssn/hasInput"/>
  </rdf:Description>
  <rdf:Description rdf:about="https://w3id.org/tern/ontologies/tern/isSubActivityOf">
    <rdfs:label>is sub activity of</rdfs:label>
    <skos:definition>A property that links an activity to its parent activity.</skos:definition>
    <rdf:type rdf:resource="http://www.w3.org/1999/02/22-rdf-syntax-ns#Property"/>
  </rdf:Description>
  <rdf:Description rdf:about="https://w3id.org/tern/ontologies/tern/locationDescription">
    <skos:definition>The description of the location.</skos:definition>
    <skos:example>Location description of the AusPlots site NTABRT0004 in the Alice Mulga SuperSite: 
Pine Hill Station. 25km South East of Ti-Tree. 20km East of Stuart Highway. 
South west corner of the site is 200m north west of proposed supersite flux tower</skos:example>
    <rdf:type rdf:resource="http://www.w3.org/1999/02/22-rdf-syntax-ns#Property"/>
    <rdfs:label>location description</rdfs:label>
  </rdf:Description>
  <rdf:Description rdf:about="http://linked.data.gov.au/def/datatype/PercentRange">
    <rdfs:subClassOf rdf:resource="https://w3id.org/tern/ontologies/tern/Result"/>
  </rdf:Description>
  <rdf:Description rdf:nodeID="ub1bL498C19">
    <owl:onDataRange rdf:resource="http://www.w3.org/2001/XMLSchema#string"/>
    <rdf:type rdf:resource="http://www.w3.org/2002/07/owl#Restriction"/>
    <owl:maxQualifiedCardinality rdf:datatype="http://www.w3.org/2001/XMLSchema#nonNegativeInteger">1</owl:maxQualifiedCardinality>
    <owl:onProperty rdf:resource="https://w3id.org/tern/ontologies/tern/purpose"/>
  </rdf:Description>
  <rdf:Description rdf:nodeID="ub1bL1222C19">
    <owl:minQualifiedCardinality rdf:datatype="http://www.w3.org/2001/XMLSchema#nonNegativeInteger">1</owl:minQualifiedCardinality>
    <owl:onClass rdf:resource="https://w3id.org/tern/ontologies/tern/SiteTaxon"/>
    <rdf:type rdf:resource="http://www.w3.org/2002/07/owl#Restriction"/>
    <owl:onProperty rdf:resource="http://www.w3.org/ns/sosa/isSampleOf"/>
  </rdf:Description>
  <rdf:Description rdf:nodeID="ub1bL628C19">
    <owl:qualifiedCardinality rdf:datatype="http://www.w3.org/2001/XMLSchema#nonNegativeInteger">1</owl:qualifiedCardinality>
    <rdf:type rdf:resource="http://www.w3.org/2002/07/owl#Restriction"/>
    <owl:onClass rdf:resource="https://w3id.org/tern/ontologies/tern/ObservableProperty"/>
    <owl:onProperty rdf:resource="http://www.w3.org/ns/sosa/observedProperty"/>
  </rdf:Description>
  <rdf:Description rdf:nodeID="ub1bL1344C19">
    <owl:allValuesFrom rdf:resource="http://linked.data.gov.au/def/datatype/Text"/>
    <owl:onProperty rdf:resource="https://w3id.org/tern/ontologies/tern/soilClassification"/>
    <rdf:type rdf:resource="http://www.w3.org/2002/07/owl#Restriction"/>
  </rdf:Description>
  <rdf:Description rdf:nodeID="ub1bL1707C1">
    <owl:unionOf rdf:nodeID="f5a816f5a0f7a4e439059a4ae4caf6ab4b20"/>
    <rdf:type rdf:resource="http://www.w3.org/2002/07/owl#Class"/>
  </rdf:Description>
  <rdf:Description rdf:nodeID="f5a816f5a0f7a4e439059a4ae4caf6ab4b11">
    <rdf:first rdf:resource="http://www.w3.org/2004/02/skos/core#ConceptScheme"/>
    <rdf:rest rdf:nodeID="f5a816f5a0f7a4e439059a4ae4caf6ab4b12"/>
  </rdf:Description>
  <rdf:Description rdf:nodeID="ub1bL587C19">
    <owl:allValuesFrom rdf:resource="https://w3id.org/tern/ontologies/org/Person"/>
    <rdf:type rdf:resource="http://www.w3.org/2002/07/owl#Restriction"/>
    <owl:onProperty rdf:resource="http://www.w3.org/ns/prov#wasAttributedTo"/>
  </rdf:Description>
  <rdf:Description rdf:nodeID="ub1bL98C23">
    <schema-https:affiliation rdf:resource="https://w3id.org/tern/resources/a083902d-d821-41be-b663-1d7cb33eea66"/>
    <schema-https:name>Habacuc Flores Moreno</schema-https:name>
    <schema-https:email>h.floresmoreno@uq.edu.au</schema-https:email>
    <rdf:type rdf:resource="https://schema.org/Person"/>
  </rdf:Description>
  <rdf:Description rdf:nodeID="ub1bL92C23">
    <schema-https:email>a.devaraju@uq.edu.au</schema-https:email>
    <rdf:type rdf:resource="https://schema.org/Person"/>
    <schema-https:affiliation rdf:resource="https://w3id.org/tern/resources/a083902d-d821-41be-b663-1d7cb33eea66"/>
    <schema-https:name>Anusuriya Devaraju</schema-https:name>
  </rdf:Description>
  <rdf:Description rdf:nodeID="ub1bL257C19">
    <owl:minQualifiedCardinality rdf:datatype="http://www.w3.org/2001/XMLSchema#nonNegativeInteger">1</owl:minQualifiedCardinality>
    <owl:onProperty rdf:resource="http://purl.org/dc/terms/source"/>
    <owl:onClass rdf:resource="http://www.w3.org/2001/XMLSchema#string"/>
    <rdf:type rdf:resource="http://www.w3.org/2002/07/owl#Restriction"/>
  </rdf:Description>
  <rdf:Description rdf:nodeID="ub1bL1310C19">
    <owl:onProperty rdf:resource="https://w3id.org/tern/ontologies/tern/site"/>
    <rdf:type rdf:resource="http://www.w3.org/2002/07/owl#Restriction"/>
    <owl:onClass rdf:resource="https://w3id.org/tern/ontologies/tern/Site"/>
    <owl:qualifiedCardinality rdf:datatype="http://www.w3.org/2001/XMLSchema#nonNegativeInteger">1</owl:qualifiedCardinality>
  </rdf:Description>
  <rdf:Description rdf:nodeID="ub1bL1131C19">
    <owl:onClass rdf:resource="http://www.w3.org/2004/02/skos/core#Concept"/>
    <owl:onProperty rdf:resource="https://w3id.org/tern/ontologies/tern/siteShape"/>
    <owl:maxQualifiedCardinality rdf:datatype="http://www.w3.org/2001/XMLSchema#nonNegativeInteger">1</owl:maxQualifiedCardinality>
    <rdf:type rdf:resource="http://www.w3.org/2002/07/owl#Restriction"/>
  </rdf:Description>
  <rdf:Description rdf:nodeID="ub1bL928C19">
    <owl:onClass rdf:resource="https://w3id.org/tern/ontologies/tern/Procedure"/>
    <owl:onProperty rdf:resource="http://www.w3.org/ns/sosa/usedProcedure"/>
    <rdf:type rdf:resource="http://www.w3.org/2002/07/owl#Restriction"/>
    <owl:qualifiedCardinality rdf:datatype="http://www.w3.org/2001/XMLSchema#nonNegativeInteger">1</owl:qualifiedCardinality>
  </rdf:Description>
  <rdf:Description rdf:nodeID="ub1bL136C19">
    <schema-https:memberOf rdf:nodeID="ub1bL140C29"/>
    <rdf:type rdf:resource="https://schema.org/Person"/>
    <schema-https:identifier rdf:resource="https://orcid.org/0000-0002-3884-3420"/>
    <schema-https:email>simon.cox@csiro.au</schema-https:email>
    <schema-https:name>Simon J.D.Cox</schema-https:name>
  </rdf:Description>
  <rdf:Description rdf:about="https://w3id.org/tern/ontologies/tern/site">
    <skos:definition>A property that links, e.g., a [SiteVisit](#EcologicalSiteVisit) to a [Site](#EcologicalSite).</skos:definition>
    <rdfs:range rdf:resource="https://w3id.org/tern/ontologies/tern/Site"/>
    <rdfs:label>site</rdfs:label>
    <rdf:type rdf:resource="http://www.w3.org/1999/02/22-rdf-syntax-ns#Property"/>
  </rdf:Description>
  <rdf:Description rdf:about="https://w3id.org/tern/ontologies/tern/AutomaticWeatherStation">
    <rdfs:label>Automatic Weather Station</rdfs:label>
    <rdf:type rdf:resource="http://www.w3.org/2002/07/owl#Class"/>
    <rdfs:subClassOf rdf:resource="https://w3id.org/tern/ontologies/tern/FixedPlatform"/>
  </rdf:Description>
  <rdf:Description rdf:nodeID="ub1bL872C19">
    <rdf:type rdf:resource="http://www.w3.org/2002/07/owl#Restriction"/>
    <owl:onClass rdf:resource="https://w3id.org/tern/ontologies/tern/Sampling"/>
    <owl:onProperty rdf:resource="http://www.w3.org/ns/sosa/isResultOf"/>
    <owl:maxQualifiedCardinality rdf:datatype="http://www.w3.org/2001/XMLSchema#nonNegativeInteger">1</owl:maxQualifiedCardinality>
  </rdf:Description>
  <rdf:Description rdf:about="https://w3id.org/tern/ontologies/tern/EnvironmentalCharacteristic">
    <rdfs:subClassOf rdf:resource="http://www.w3.org/ns/sosa/FeatureOfInterest"/>
    <skos:definition>The environment characteristics  is a [FeatureOfInterest](http://w3.org/ns/sosa/FeatureOfInterest) of a location where [Observations](#Observation) such as the annual mean rainfall or the annual mean temperature are made.</skos:definition>
    <rdfs:label>Environmental Characteristic</rdfs:label>
    <rdf:type rdf:resource="http://www.w3.org/2002/07/owl#Class"/>
    <rdfs:subClassOf rdf:nodeID="ub1bL332C19"/>
  </rdf:Description>
  <rdf:Description rdf:nodeID="f5a816f5a0f7a4e439059a4ae4caf6ab4b3">
    <rdf:first rdf:resource="http://www.w3.org/2001/XMLSchema#decimal"/>
    <rdf:rest rdf:nodeID="f5a816f5a0f7a4e439059a4ae4caf6ab4b4"/>
  </rdf:Description>
  <rdf:Description rdf:nodeID="ub1bL999C19">
    <rdf:type rdf:resource="http://www.w3.org/2002/07/owl#Restriction"/>
    <owl:onProperty rdf:resource="http://www.opengis.net/ont/geosparql#asWKT"/>
    <owl:qualifiedCardinality rdf:datatype="http://www.w3.org/2001/XMLSchema#nonNegativeInteger">1</owl:qualifiedCardinality>
    <owl:onDataRange rdf:resource="https://w3id.org/tern/ontologies/loc/wktLiteral"/>
  </rdf:Description>
  <rdf:Description rdf:nodeID="ub1bL610C19">
    <owl:onProperty rdf:resource="http://www.w3.org/2000/01/rdf-schema#label"/>
    <rdf:type rdf:resource="http://www.w3.org/2002/07/owl#Restriction"/>
    <owl:onClass rdf:resource="http://www.w3.org/2001/XMLSchema#string"/>
    <owl:qualifiedCardinality rdf:datatype="http://www.w3.org/2001/XMLSchema#nonNegativeInteger">1</owl:qualifiedCardinality>
  </rdf:Description>
  <rdf:Description rdf:about="https://w3id.org/tern/ontologies/tern/taxon">
    <skos:scopeNote>Value should be from a controlled vocabulary identified by a URI.</skos:scopeNote>
    <rdfs:label>taxon</rdfs:label>
    <skos:definition>Taxon classification.</skos:definition>
    <rdf:type rdf:resource="http://www.w3.org/1999/02/22-rdf-syntax-ns#Property"/>
  </rdf:Description>
  <rdf:Description rdf:about="https://w3id.org/tern/ontologies/tern/EcosystemProcessesSite">
    <skos:definition>An ecological [Site](#EcologicalSite) that usually hosts a [FluxTower](#FluxTower).</skos:definition>
    <rdfs:label>Ecosystem Processes Site</rdfs:label>
    <rdf:type rdf:resource="http://www.w3.org/2002/07/owl#Class"/>
    <rdfs:subClassOf rdf:resource="https://w3id.org/tern/ontologies/tern/Site"/>
  </rdf:Description>
  <rdf:Description rdf:nodeID="f5a816f5a0f7a4e439059a4ae4caf6ab4b5">
    <rdf:first rdf:resource="http://www.w3.org/2004/02/skos/core#Concept"/>
    <rdf:rest rdf:nodeID="f5a816f5a0f7a4e439059a4ae4caf6ab4b6"/>
  </rdf:Description>
  <rdf:Description rdf:about="https://w3id.org/tern/ontologies/tern/SiteStratumTaxon">
    <rdfs:label>Site Stratum Taxon</rdfs:label>
    <rdf:type rdf:resource="http://www.w3.org/2002/07/owl#Class"/>
    <rdfs:subClassOf rdf:nodeID="ub1bL1222C19"/>
    <rdfs:subClassOf rdf:nodeID="ub1bL1228C19"/>
    <rdfs:subClassOf rdf:nodeID="ub1bL1216C19"/>
    <rdfs:subClassOf rdf:resource="https://w3id.org/tern/ontologies/tern/Sample"/>
  </rdf:Description>
  <rdf:Description rdf:nodeID="ub1bL821C19">
    <rdf:type rdf:resource="http://www.w3.org/2002/07/owl#Restriction"/>
    <owl:onProperty rdf:resource="http://www.w3.org/ns/sosa/isResultOf"/>
    <owl:cardinality rdf:datatype="http://www.w3.org/2001/XMLSchema#nonNegativeInteger">1</owl:cardinality>
  </rdf:Description>
  <rdf:Description rdf:about="https://w3id.org/tern/ontologies/tern/width">
    <rdfs:label>width</rdfs:label>
    <rdfs:seeAlso rdf:resource="http://qudt.org/vocab/quantitykind/Width"/>
    <skos:definition>The measurement or extent of something from side to side.</skos:definition>
    <rdf:type rdf:resource="http://www.w3.org/1999/02/22-rdf-syntax-ns#Property"/>
  </rdf:Description>
  <rdf:Description rdf:nodeID="ub1bL1184C19">
    <owl:onProperty rdf:resource="http://www.w3.org/ns/dcat#dataset"/>
    <rdf:type rdf:resource="http://www.w3.org/2002/07/owl#Restriction"/>
    <owl:onClass rdf:resource="http://www.w3.org/ns/dcat#Dataset"/>
    <owl:qualifiedCardinality rdf:datatype="http://www.w3.org/2001/XMLSchema#nonNegativeInteger">1</owl:qualifiedCardinality>
  </rdf:Description>
  <rdf:Description rdf:about="https://w3id.org/tern/ontologies/tern/dateCommissioned">
    <rdf:type rdf:resource="http://www.w3.org/1999/02/22-rdf-syntax-ns#Property"/>
    <skos:definition>The date when, e.g., a [Site](#EcologicalSite) is ready to commence its operations, after it is successfully installed and tested.</skos:definition>
    <skos:scopeNote>Use ISO 8601 international standard for representing dates and times. Missing start date may be set to the first of the month.</skos:scopeNote>
    <rdfs:label>date commissioned</rdfs:label>
    <skos:example>1 August 2017 is the date commisioned of the 
[Collie flux station](http://ozflux.org.au/monitoringsites/collie/index.html)</skos:example>
  </rdf:Description>
  <rdf:Description rdf:nodeID="ub1bL598C19">
    <rdf:type rdf:resource="http://www.w3.org/2002/07/owl#Restriction"/>
    <owl:onProperty rdf:resource="https://w3id.org/tern/ontologies/tern/isSubActivityOf"/>
    <owl:maxQualifiedCardinality rdf:datatype="http://www.w3.org/2001/XMLSchema#nonNegativeInteger">1</owl:maxQualifiedCardinality>
    <owl:onClass rdf:resource="https://w3id.org/tern/ontologies/tern/SiteVisit"/>
  </rdf:Description>
  <rdf:Description rdf:nodeID="ub1bL1387C19">
    <owl:maxCardinality rdf:datatype="http://www.w3.org/2001/XMLSchema#nonNegativeInteger">1</owl:maxCardinality>
    <rdf:type rdf:resource="http://www.w3.org/2002/07/owl#Restriction"/>
    <owl:onProperty rdf:resource="https://w3id.org/tern/ontologies/tern/transectDirection"/>
  </rdf:Description>
  <rdf:Description rdf:nodeID="ub1bL332C19">
    <owl:onClass rdf:resource="https://w3id.org/tern/ontologies/tern/Observation"/>
    <rdf:type rdf:resource="http://www.w3.org/2002/07/owl#Restriction"/>
    <owl:minQualifiedCardinality rdf:datatype="http://www.w3.org/2001/XMLSchema#nonNegativeInteger">1</owl:minQualifiedCardinality>
    <owl:onProperty rdf:resource="http://www.w3.org/ns/sosa/isFeatureOfInterestOf"/>
  </rdf:Description>
  <rdf:Description rdf:nodeID="ub1bL582C19">
    <owl:onProperty rdf:resource="http://www.w3.org/2000/01/rdf-schema#comment"/>
    <owl:allValuesFrom rdf:resource="http://www.w3.org/2001/XMLSchema#string"/>
    <rdf:type rdf:resource="http://www.w3.org/2002/07/owl#Restriction"/>
  </rdf:Description>
  <rdf:Description rdf:nodeID="ub1bL957C19">
    <owl:onClass rdf:resource="http://linked.data.gov.au/def/datatype/QuantitativeMeasure"/>
    <rdf:type rdf:resource="http://www.w3.org/2002/07/owl#Restriction"/>
    <owl:onProperty rdf:resource="https://w3id.org/tern/ontologies/loc/altitude"/>
    <owl:maxQualifiedCardinality rdf:datatype="http://www.w3.org/2001/XMLSchema#nonNegativeInteger">1</owl:maxQualifiedCardinality>
  </rdf:Description>
  <rdf:Description rdf:about="http://linked.data.gov.au/def/datatype/Boolean">
    <rdfs:subClassOf rdf:resource="https://w3id.org/tern/ontologies/tern/Result"/>
  </rdf:Description>
  <rdf:Description rdf:nodeID="ub1bL1012C19">
    <owl:onProperty rdf:resource="http://www.w3.org/ns/sosa/observes"/>
    <rdf:type rdf:resource="http://www.w3.org/2002/07/owl#Restriction"/>
    <owl:allValuesFrom rdf:resource="https://w3id.org/tern/ontologies/tern/ObservableProperty"/>
  </rdf:Description>
  <rdf:Description rdf:nodeID="ub1bL404C19">
    <owl:onProperty rdf:resource="https://w3id.org/tern/ontologies/tern/centroidPoint"/>
    <owl:onClass rdf:resource="https://w3id.org/tern/ontologies/loc/Point"/>
    <owl:qualifiedCardinality rdf:datatype="http://www.w3.org/2001/XMLSchema#nonNegativeInteger">1</owl:qualifiedCardinality>
    <rdf:type rdf:resource="http://www.w3.org/2002/07/owl#Restriction"/>
  </rdf:Description>
  <rdf:Description rdf:nodeID="ub1bL398C19">
    <owl:qualifiedCardinality rdf:datatype="http://www.w3.org/2001/XMLSchema#nonNegativeInteger">1</owl:qualifiedCardinality>
    <rdf:type rdf:resource="http://www.w3.org/2002/07/owl#Restriction"/>
    <owl:onClass rdf:resource="http://www.w3.org/2001/XMLSchema#string"/>
    <owl:onProperty rdf:resource="http://www.w3.org/2000/01/rdf-schema#label"/>
  </rdf:Description>
  <rdf:Description rdf:about="https://w3id.org/tern/ontologies/tern/AffiliateSuperSite">
    <rdfs:subClassOf rdf:resource="https://w3id.org/tern/ontologies/tern/SuperSite"/>
    <rdf:type rdf:resource="http://www.w3.org/2002/07/owl#Class"/>
    <rdfs:seeAlso rdf:resource="https://supersites.tern.org.au/"/>
    <rdfs:label>Affiliate SuperSite</rdfs:label>
    <skos:example rdf:resource="https://w3id.org/tern/resources/a05a51c0-2daa-4369-aa2b-08c3638efa7a"/>
    <skos:example>Samford Peri-urban Affiliate SuperSite</skos:example>
  </rdf:Description>
  <rdf:Description rdf:nodeID="f5a816f5a0f7a4e439059a4ae4caf6ab4b21">
    <rdf:first rdf:resource="http://www.w3.org/2001/XMLSchema#int"/>
    <rdf:rest rdf:resource="http://www.w3.org/1999/02/22-rdf-syntax-ns#nil"/>
  </rdf:Description>
  <rdf:Description rdf:nodeID="ub1bL1040C19">
    <owl:onProperty rdf:resource="http://www.opengis.net/ont/geosparql#sfWithin"/>
    <rdf:type rdf:resource="http://www.w3.org/2002/07/owl#Restriction"/>
    <owl:allValuesFrom rdf:resource="http://www.opengis.net/ont/geosparql#Feature"/>
  </rdf:Description>
  <rdf:Description rdf:nodeID="ub1bL1714C1">
    <rdf:type rdf:resource="http://www.w3.org/2002/07/owl#Class"/>
    <owl:unionOf rdf:nodeID="f5a816f5a0f7a4e439059a4ae4caf6ab4b22"/>
  </rdf:Description>
  <rdf:Description rdf:about="https://w3id.org/tern/ontologies/tern/Sensor">
    <rdfs:subClassOf rdf:nodeID="ub1bL1017C19"/>
    <rdfs:subClassOf rdf:nodeID="ub1bL1022C19"/>
    <rdfs:subClassOf rdf:resource="http://www.w3.org/ns/sosa/Sensor"/>
    <rdfs:subClassOf rdf:nodeID="ub1bL1027C19"/>
    <skos:definition>Device, agent (including humans), or software (simulation) involved in, or implementing, a Procedure. Sensors respond to a stimulus, e.g., a change in the environment, or input data composed from the results of prior Observations, and generate a Result. Sensors can be hosted by Platforms.</skos:definition>
    <rdfs:subClassOf rdf:nodeID="ub1bL1012C19"/>
    <rdf:type rdf:resource="http://www.w3.org/2002/07/owl#Class"/>
    <rdfs:subClassOf rdf:resource="https://w3id.org/tern/ontologies/tern/Instrument"/>
    <rdfs:label>Sensor</rdfs:label>
  </rdf:Description>
  <rdf:Description rdf:nodeID="ub1bL1265C19">
    <owl:allValuesFrom rdf:resource="https://w3id.org/tern/ontologies/tern/PhysicalSpecimen"/>
    <owl:onProperty rdf:resource="http://www.w3.org/ns/sosa/hasSample"/>
    <rdf:type rdf:resource="http://www.w3.org/2002/07/owl#Restriction"/>
  </rdf:Description>
  <rdf:Description rdf:nodeID="ub1bL1198C19">
    <owl:qualifiedCardinality rdf:datatype="http://www.w3.org/2001/XMLSchema#nonNegativeInteger">1</owl:qualifiedCardinality>
    <rdf:type rdf:resource="http://www.w3.org/2002/07/owl#Restriction"/>
    <owl:onClass rdf:resource="http://www.w3.org/2004/02/skos/core#Concept"/>
    <owl:onProperty rdf:resource="https://w3id.org/tern/ontologies/tern/stratum"/>
  </rdf:Description>
  <rdf:Description rdf:nodeID="f5a816f5a0f7a4e439059a4ae4caf6ab4b20">
    <rdf:first rdf:resource="http://www.w3.org/2001/XMLSchema#string"/>
    <rdf:rest rdf:nodeID="f5a816f5a0f7a4e439059a4ae4caf6ab4b21"/>
  </rdf:Description>
  <rdf:Description rdf:about="https://w3id.org/tern/ontologies/tern/transectDirection">
    <skos:definition>Describes the direction of the transect.</skos:definition>
    <rdfs:range rdf:resource="http://www.w3.org/2001/XMLSchema#string"/>
    <rdfs:domain rdf:resource="https://w3id.org/tern/ontologies/tern/Transect"/>
    <rdfs:label>transect direction</rdfs:label>
    <rdf:type rdf:resource="http://www.w3.org/1999/02/22-rdf-syntax-ns#Property"/>
    <skos:example>S-W</skos:example>
  </rdf:Description>
  <rdf:Description rdf:about="https://w3id.org/tern/ontologies/tern/globalMatch">
    <skos:definition>Link a concept to an upper concept (in the closed system).</skos:definition>
    <skos:scopeNote>Use in between controlled vocabularies.</skos:scopeNote>
    <owl:inverseOf rdf:resource="https://w3id.org/tern/ontologies/tern/isGlobalMatchOf"/>
    <rdf:type rdf:resource="http://www.w3.org/1999/02/22-rdf-syntax-ns#Property"/>
    <rdfs:subPropertyOf rdf:resource="http://www.w3.org/2004/02/skos/core#exactMatch"/>
    <rdfs:label>global match</rdfs:label>
  </rdf:Description>
  <rdf:Description rdf:nodeID="ub1bL288C25">
    <owl:unionOf rdf:nodeID="f5a816f5a0f7a4e439059a4ae4caf6ab4b3"/>
    <rdf:type rdf:resource="http://www.w3.org/2002/07/owl#Class"/>
  </rdf:Description>
  <rdf:Description rdf:nodeID="ub1bL1161C19">
    <owl:onProperty rdf:resource="http://www.opengis.net/ont/geosparql#hasGeometry"/>
    <owl:minCardinality rdf:datatype="http://www.w3.org/2001/XMLSchema#nonNegativeInteger">1</owl:minCardinality>
    <rdf:type rdf:resource="http://www.w3.org/2002/07/owl#Restriction"/>
  </rdf:Description>
  <rdf:Description rdf:nodeID="ub1bL560C19">
    <rdf:type rdf:resource="http://www.w3.org/2002/07/owl#Restriction"/>
    <owl:onProperty rdf:resource="https://w3id.org/tern/ontologies/tern/globalValue"/>
    <owl:maxQualifiedCardinality rdf:datatype="http://www.w3.org/2001/XMLSchema#nonNegativeInteger">1</owl:maxQualifiedCardinality>
    <owl:onClass rdf:resource="http://www.w3.org/2004/02/skos/core#Concept"/>
  </rdf:Description>
  <rdf:Description rdf:nodeID="ub1bL471C25">
    <owl:unionOf rdf:nodeID="f5a816f5a0f7a4e439059a4ae4caf6ab4b9"/>
    <rdf:type rdf:resource="http://www.w3.org/2002/07/owl#Class"/>
  </rdf:Description>
  <rdf:Description rdf:nodeID="f5a816f5a0f7a4e439059a4ae4caf6ab4b22">
    <rdf:rest rdf:nodeID="f5a816f5a0f7a4e439059a4ae4caf6ab4b23"/>
    <rdf:first rdf:resource="http://www.w3.org/2001/XMLSchema#string"/>
  </rdf:Description>
  <rdf:Description rdf:about="https://w3id.org/tern/ontologies/tern/length">
    <rdf:type rdf:resource="http://www.w3.org/1999/02/22-rdf-syntax-ns#Property"/>
    <rdfs:seeAlso rdf:resource="http://qudt.org/vocab/quantitykind/Length"/>
    <skos:definition>A measure of distance.</skos:definition>
    <rdfs:label>length</rdfs:label>
  </rdf:Description>
  <rdf:Description rdf:nodeID="ub1bL252C19">
    <owl:minCardinality rdf:datatype="http://www.w3.org/2001/XMLSchema#nonNegativeInteger">1</owl:minCardinality>
    <rdf:type rdf:resource="http://www.w3.org/2002/07/owl#Restriction"/>
    <owl:onProperty rdf:resource="http://www.w3.org/2004/02/skos/core#prefLabel"/>
  </rdf:Description>
  <rdf:Description rdf:nodeID="ub1bL892C19">
    <owl:onClass rdf:resource="https://w3id.org/tern/ontologies/tern/Procedure"/>
    <owl:minQualifiedCardinality rdf:datatype="http://www.w3.org/2001/XMLSchema#nonNegativeInteger">1</owl:minQualifiedCardinality>
    <owl:onProperty rdf:resource="http://www.w3.org/ns/ssn/implements"/>
    <rdf:type rdf:resource="http://www.w3.org/2002/07/owl#Restriction"/>
  </rdf:Description>
  <rdf:Description rdf:about="https://w3id.org/tern/ontologies/tern/RadiationSensor">
    <rdfs:label>Radiation sensor</rdfs:label>
    <rdfs:subClassOf rdf:resource="https://w3id.org/tern/ontologies/tern/Sensor"/>
    <rdf:type rdf:resource="http://www.w3.org/2002/07/owl#Class"/>
  </rdf:Description>
  <rdf:Description rdf:nodeID="ub1bL847C19">
    <owl:onProperty rdf:resource="http://www.w3.org/ns/prov#wasAttributedTo"/>
    <owl:allValuesFrom rdf:resource="https://w3id.org/tern/ontologies/org/Person"/>
    <rdf:type rdf:resource="http://www.w3.org/2002/07/owl#Restriction"/>
  </rdf:Description>
  <rdf:Description rdf:about="https://w3id.org/tern/ontologies/tern/AusPlotsSite">
    <rdfs:subClassOf rdf:resource="https://w3id.org/tern/ontologies/tern/Site"/>
    <skos:seeAlso rdf:resource="http://www.ausplots.org/"/>
    <rdfs:label>AusPlots Site</rdfs:label>
    <skos:example rdf:resource="http://linked.data.gov.au/dataset/ausplots/site-QDABBN0001"/>
    <skos:definition>AusPlots is a plot-based surveillance monitoring program delivered by TERN Surveillance. An [AusPlot Site](#AusPlotsSite) refers to a [site](#EcologicalSite) where AusPlots Rangelands or Forests method has been implemented.</skos:definition>
    <rdf:type rdf:resource="http://www.w3.org/2002/07/owl#Class"/>
  </rdf:Description>
  <rdf:Description rdf:nodeID="ub1bL1096C19">
    <rdf:type rdf:resource="http://www.w3.org/2002/07/owl#Restriction"/>
    <owl:onProperty rdf:resource="https://w3id.org/tern/ontologies/tern/hasEnvironmentalCharacteristic"/>
    <owl:maxCardinality rdf:datatype="http://www.w3.org/2001/XMLSchema#nonNegativeInteger">1</owl:maxCardinality>
  </rdf:Description>
  <rdf:Description rdf:about="https://w3id.org/tern/ontologies/tern/Radiometer">
    <rdfs:seeAlso rdf:resource="https://en.wikipedia.org/wiki/Radiometer"/>
    <rdfs:label>Radiometer</rdfs:label>
    <rdfs:subClassOf rdf:resource="https://w3id.org/tern/ontologies/tern/RadiationSensor"/>
    <rdfs:comment>A radiometer or roentgenometer is a device for measuring the radiant flux (power) of electromagnetic radiation. Generally, a radiometer is an infrared radiation detector or an ultraviolet detector.</rdfs:comment>
    <rdf:type rdf:resource="http://www.w3.org/2002/07/owl#Class"/>
  </rdf:Description>
  <rdf:Description rdf:nodeID="ub1bL1327C19">
    <rdf:type rdf:resource="http://www.w3.org/2002/07/owl#Restriction"/>
    <owl:onProperty rdf:resource="https://w3id.org/tern/ontologies/tern/soilHorizonClassifier"/>
    <owl:allValuesFrom rdf:resource="http://linked.data.gov.au/def/datatype/Text"/>
  </rdf:Description>
  <rdf:Description rdf:nodeID="ub1bL1166C19">
    <owl:qualifiedCardinality rdf:datatype="http://www.w3.org/2001/XMLSchema#nonNegativeInteger">1</owl:qualifiedCardinality>
    <rdf:type rdf:resource="http://www.w3.org/2002/07/owl#Restriction"/>
    <owl:onProperty rdf:resource="https://w3id.org/tern/ontologies/tern/dateCommissioned"/>
    <owl:onClass rdf:resource="http://www.w3.org/2001/XMLSchema#date"/>
  </rdf:Description>
  <rdf:Description rdf:about="https://w3id.org/tern/ontologies/tern/methodType">
    <rdf:type rdf:resource="http://www.w3.org/1999/02/22-rdf-syntax-ns#Property"/>
    <rdfs:label>method type</rdfs:label>
    <skos:definition>A particular method type used to conduct some survey.</skos:definition>
  </rdf:Description>
  <rdf:Description rdf:nodeID="f5a816f5a0f7a4e439059a4ae4caf6ab4b7">
    <rdf:first rdf:resource="http://www.w3.org/2000/01/rdf-schema#Class"/>
    <rdf:rest rdf:nodeID="f5a816f5a0f7a4e439059a4ae4caf6ab4b8"/>
  </rdf:Description>
  <rdf:Description rdf:nodeID="ub1bL1017C19">
    <rdf:type rdf:resource="http://www.w3.org/2002/07/owl#Restriction"/>
    <owl:allValuesFrom rdf:resource="https://w3id.org/tern/ontologies/tern/Observation"/>
    <owl:onProperty rdf:resource="http://www.w3.org/ns/sosa/madeObservation"/>
  </rdf:Description>
  <rdf:Description rdf:nodeID="ub1bL302C19">
    <owl:cardinality rdf:datatype="http://www.w3.org/2001/XMLSchema#nonNegativeInteger">1</owl:cardinality>
    <owl:onProperty rdf:resource="https://w3id.org/tern/ontologies/tern/width"/>
    <rdf:type rdf:resource="http://www.w3.org/2002/07/owl#Restriction"/>
  </rdf:Description>
  <rdf:Description rdf:about="https://w3id.org/tern/ontologies/tern/soilHorizonClassifier">
    <rdf:type rdf:resource="http://www.w3.org/1999/02/22-rdf-syntax-ns#Property"/>
    <skos:definition>Soil horizon classifier as defined in the Australian Soil and Land Survey Field Handbook on page 148.</skos:definition>
    <rdfs:label>soil horizon classifier</rdfs:label>
  </rdf:Description>
  <rdf:Description rdf:nodeID="f5a816f5a0f7a4e439059a4ae4caf6ab4b17">
    <rdf:first rdf:resource="https://w3id.org/tern/ontologies/loc/Polygon"/>
    <rdf:rest rdf:resource="http://www.w3.org/1999/02/22-rdf-syntax-ns#nil"/>
  </rdf:Description>
  <rdf:Description rdf:nodeID="ub1bL677C19">
    <owl:allValuesFrom rdf:resource="http://www.w3.org/2001/XMLSchema#string"/>
    <owl:onProperty rdf:resource="http://www.w3.org/2000/01/rdf-schema#label"/>
    <rdf:type rdf:resource="http://www.w3.org/2002/07/owl#Restriction"/>
  </rdf:Description>
  <rdf:Description rdf:nodeID="f5a816f5a0f7a4e439059a4ae4caf6ab4b16">
    <rdf:rest rdf:nodeID="f5a816f5a0f7a4e439059a4ae4caf6ab4b17"/>
    <rdf:first rdf:resource="https://w3id.org/tern/ontologies/loc/Point"/>
  </rdf:Description>
  <rdf:Description rdf:nodeID="f5a816f5a0f7a4e439059a4ae4caf6ab4b13">
    <rdf:first rdf:resource="http://www.w3.org/2002/07/owl#Ontology"/>
    <rdf:rest rdf:resource="http://www.w3.org/1999/02/22-rdf-syntax-ns#nil"/>
  </rdf:Description>
  <rdf:Description rdf:about="http://linked.data.gov.au/def/datatype/QuantitativeRange">
    <rdfs:subClassOf rdf:resource="https://w3id.org/tern/ontologies/tern/Result"/>
  </rdf:Description>
  <rdf:Description rdf:nodeID="ub1bL455C19">
    <owl:onProperty rdf:resource="http://purl.org/dc/terms/type"/>
    <rdf:type rdf:resource="http://www.w3.org/2002/07/owl#Restriction"/>
    <owl:cardinality rdf:datatype="http://www.w3.org/2001/XMLSchema#nonNegativeInteger">1</owl:cardinality>
  </rdf:Description>
  <rdf:Description rdf:nodeID="ub1bL140C29">
    <rdf:type rdf:resource="https://schema.org/Organization"/>
    <schema-https:identifier rdf:resource="https://w3id.org/tern/resources/276dd611-5d74-4555-b20f-12f0f0b618a1"/>
    <schema-https:name>CSIRO</schema-https:name>
  </rdf:Description>
  <rdf:Description rdf:nodeID="f5a816f5a0f7a4e439059a4ae4caf6ab4b6">
    <rdf:first rdf:resource="http://www.w3.org/2002/07/owl#Class"/>
    <rdf:rest rdf:nodeID="f5a816f5a0f7a4e439059a4ae4caf6ab4b7"/>
  </rdf:Description>
  <rdf:Description rdf:about="https://w3id.org/tern/ontologies/tern/hasMethod">
    <rdfs:label>has method</rdfs:label>
    <rdf:type rdf:resource="http://www.w3.org/1999/02/22-rdf-syntax-ns#Property"/>
    <skos:definition>A property that links a concept to a method.</skos:definition>
    <rdfs:subPropertyOf rdf:resource="http://www.w3.org/2004/02/skos/core#relatedMatch"/>
  </rdf:Description>
  <rdf:Description rdf:nodeID="ub1bL286C19">
    <owl:onProperty rdf:resource="https://w3id.org/tern/ontologies/tern/width"/>
    <owl:allValuesFrom rdf:nodeID="ub1bL288C25"/>
    <rdf:type rdf:resource="http://www.w3.org/2002/07/owl#Restriction"/>
  </rdf:Description>
  <rdf:Description rdf:nodeID="ub1bL392C19">
    <owl:qualifiedCardinality rdf:datatype="http://www.w3.org/2001/XMLSchema#nonNegativeInteger">1</owl:qualifiedCardinality>
    <owl:onProperty rdf:resource="https://w3id.org/tern/ontologies/tern/dateCommissioned"/>
    <owl:onClass rdf:resource="http://www.w3.org/2001/XMLSchema#date"/>
    <rdf:type rdf:resource="http://www.w3.org/2002/07/owl#Restriction"/>
  </rdf:Description>
  <rdf:Description rdf:about="https://w3id.org/tern/ontologies/tern/hasSamplingPoint">
    <rdfs:label>has sampling point</rdfs:label>
    <owl:inverseOf rdf:resource="https://w3id.org/tern/ontologies/tern/isSamplingPointOf"/>
    <skos:definition>A property that links, e.g., a [Sampling](#Sampling) to a [SamplingPoint](#SamplingPoint).</skos:definition>
    <rdf:type rdf:resource="http://www.w3.org/1999/02/22-rdf-syntax-ns#Property"/>
    <rdfs:range rdf:resource="https://w3id.org/tern/ontologies/tern/SamplingPoint"/>
  </rdf:Description>
  <rdf:Description rdf:about="http://linked.data.gov.au/def/datatype/Text">
    <rdfs:subClassOf rdf:resource="https://w3id.org/tern/ontologies/tern/Result"/>
  </rdf:Description>
  <rdf:Description rdf:nodeID="ub1bL1304C19">
    <owl:onProperty rdf:resource="http://www.w3.org/2000/01/rdf-schema#label"/>
    <owl:qualifiedCardinality rdf:datatype="http://www.w3.org/2001/XMLSchema#nonNegativeInteger">1</owl:qualifiedCardinality>
    <owl:onClass rdf:resource="http://www.w3.org/2001/XMLSchema#string"/>
    <rdf:type rdf:resource="http://www.w3.org/2002/07/owl#Restriction"/>
  </rdf:Description>
  <rdf:Description rdf:nodeID="ub1bL1082C25">
    <rdf:type rdf:resource="http://www.w3.org/2002/07/owl#Class"/>
    <owl:unionOf rdf:nodeID="f5a816f5a0f7a4e439059a4ae4caf6ab4b16"/>
  </rdf:Description>
  <rdf:Description rdf:nodeID="ub1bL916C19">
    <rdf:type rdf:resource="http://www.w3.org/2002/07/owl#Restriction"/>
    <owl:onProperty rdf:resource="https://w3id.org/tern/ontologies/tern/hasSamplingPoint"/>
    <owl:maxQualifiedCardinality rdf:datatype="http://www.w3.org/2001/XMLSchema#nonNegativeInteger">1</owl:maxQualifiedCardinality>
    <owl:onClass rdf:resource="https://w3id.org/tern/ontologies/tern/SamplingPoint"/>
  </rdf:Description>
  <rdf:Description rdf:nodeID="f5a816f5a0f7a4e439059a4ae4caf6ab4b8">
    <rdf:first rdf:resource="http://www.w3.org/2002/07/owl#NamedIndividual"/>
    <rdf:rest rdf:resource="http://www.w3.org/1999/02/22-rdf-syntax-ns#nil"/>
  </rdf:Description>
  <rdf:Description rdf:about="https://w3id.org/tern/ontologies/tern/area">
    <rdf:type rdf:resource="http://www.w3.org/1999/02/22-rdf-syntax-ns#Property"/>
    <skos:definition>The extent of a [Site](#EcologicalSite) area, e.g., in m2</skos:definition>
    <rdfs:label>area</rdfs:label>
    <skos:example> The area of the Mitchell Grass Rangeland SuperSite Supersite is approximately 47 M (million) ha.</skos:example>
  </rdf:Description>
  <rdf:Description rdf:nodeID="ub1bL1055C19">
    <owl:onProperty rdf:resource="https://w3id.org/tern/ontologies/tern/locationProcedure"/>
    <rdf:type rdf:resource="http://www.w3.org/2002/07/owl#Restriction"/>
    <owl:allValuesFrom rdf:resource="https://w3id.org/tern/ontologies/tern/Procedure"/>
  </rdf:Description>
  <rdf:Description rdf:about="https://w3id.org/tern/ontologies/tern/CosmOzStation">
    <rdfs:label>CosmOz Station</rdfs:label>
    <rdfs:seeAlso rdf:resource="https://cosmoz.csiro.au"/>
    <rdf:type rdf:resource="http://www.w3.org/2002/07/owl#Class"/>
    <skos:definition>CosmOz is the Australian Cosmic-Ray Neutron Soil Moisture Monitoring Network

Beginning in October 2010, CSIRO Land and Water installed cosmic-ray probes at a number of locations around Australia to form the inaugural CosmOz network. These sites were established at instrumented research sites operated by CSIRO and University collaborators to test and validate the operation of this new technology.

These novel probes use cosmic rays originating from outer space to measure average soil moisture over an area of about 30 hectares to depths in the soil of between 10 to 50 cm. This constitutes a quantum leap over conventional on-ground soil moisture sensing technology that can only measure soil moisture content within small volumes of soil.

Each system is comprised of a data logger, neutron detector, satellite telemetry, tipping bucket rain gauge, temperature humidity and pressure sensors and three surface moisture (TDR) probes. The system requires minimal maintenance and is powered by a solar charging system. The entire system is installed on a single mast. Data is logged and transmitted every 60 minutes to the CosmOz database.</skos:definition>
    <rdfs:subClassOf rdf:resource="https://w3id.org/tern/ontologies/tern/FixedPlatform"/>
  </rdf:Description>
  <rdf:Description rdf:nodeID="ub1bL1045C19">
    <owl:onProperty rdf:resource="http://www.w3.org/2000/01/rdf-schema#comment"/>
    <owl:allValuesFrom rdf:resource="http://www.w3.org/2001/XMLSchema#string"/>
    <rdf:type rdf:resource="http://www.w3.org/2002/07/owl#Restriction"/>
  </rdf:Description>
  <rdf:Description rdf:nodeID="ub1bL538C19">
    <owl:onProperty rdf:resource="https://w3id.org/tern/ontologies/tern/globalVocabulary"/>
    <rdf:type rdf:resource="http://www.w3.org/2002/07/owl#Restriction"/>
    <owl:allValuesFrom rdf:nodeID="ub1bL540C25"/>
  </rdf:Description>
  <rdf:Description rdf:nodeID="f5a816f5a0f7a4e439059a4ae4caf6ab4b10">
    <rdf:first rdf:resource="http://www.w3.org/2001/XMLSchema#anyURI"/>
    <rdf:rest rdf:resource="http://www.w3.org/1999/02/22-rdf-syntax-ns#nil"/>
  </rdf:Description>
  <rdf:Description rdf:about="https://w3id.org/tern/resources/a083902d-d821-41be-b663-1d7cb33eea66">
    <schema-https:name>TERN</schema-https:name>
    <schema-https:identifier rdf:resource="https://w3id.org/tern/resources/a083902d-d821-41be-b663-1d7cb33eea66"/>
    <rdf:type rdf:resource="https://schema.org/Organization"/>
  </rdf:Description>
  <rdf:Description rdf:nodeID="f5a816f5a0f7a4e439059a4ae4caf6ab4b12">
    <rdf:first rdf:resource="http://www.w3.org/2004/02/skos/core#Collection"/>
    <rdf:rest rdf:nodeID="f5a816f5a0f7a4e439059a4ae4caf6ab4b13"/>
  </rdf:Description>
  <rdf:Description rdf:nodeID="ub1bL1050C19">
    <rdf:type rdf:resource="http://www.w3.org/2002/07/owl#Restriction"/>
    <owl:allValuesFrom rdf:resource="https://w3id.org/tern/ontologies/tern/PhysicalSpecimen"/>
    <owl:onProperty rdf:resource="http://www.w3.org/ns/sosa/hasSample"/>
  </rdf:Description>
  <rdf:Description rdf:nodeID="ub1bL129C19">
    <schema-https:name>Siddeswara Guru</schema-https:name>
    <schema-https:email>s.guru@uq.edu.au</schema-https:email>
    <rdf:type rdf:resource="https://schema.org/Person"/>
    <schema-https:identifier rdf:resource="https://orcid.org/0000-0002-3903-254X"/>
    <schema-https:affiliation rdf:resource="https://w3id.org/tern/resources/a083902d-d821-41be-b663-1d7cb33eea66"/>
  </rdf:Description>
  <rdf:Description rdf:nodeID="ub1bL1239C19">
    <rdf:type rdf:resource="http://www.w3.org/2002/07/owl#Restriction"/>
    <owl:qualifiedCardinality rdf:datatype="http://www.w3.org/2001/XMLSchema#nonNegativeInteger">1</owl:qualifiedCardinality>
    <owl:onClass rdf:resource="https://w3id.org/tern/ontologies/sd/StateTaxon"/>
    <owl:onProperty rdf:resource="https://w3id.org/tern/ontologies/tern/taxon"/>
  </rdf:Description>
  <rdf:Description rdf:nodeID="ub1bL247C19">
    <rdf:type rdf:resource="http://www.w3.org/2002/07/owl#Restriction"/>
    <owl:minCardinality rdf:datatype="http://www.w3.org/2001/XMLSchema#nonNegativeInteger">1</owl:minCardinality>
    <owl:onProperty rdf:resource="http://schema.org/model"/>
  </rdf:Description>
  <rdf:Description rdf:nodeID="f5a816f5a0f7a4e439059a4ae4caf6ab4b4">
    <rdf:first rdf:resource="http://www.w3.org/2001/XMLSchema#integer"/>
    <rdf:rest rdf:resource="http://www.w3.org/1999/02/22-rdf-syntax-ns#nil"/>
  </rdf:Description>
  <rdf:Description rdf:nodeID="ub1bL862C19">
    <owl:allValuesFrom rdf:resource="https://w3id.org/tern/ontologies/tern/Sample"/>
    <owl:onProperty rdf:resource="http://www.w3.org/ns/sosa/isSampleOf"/>
    <rdf:type rdf:resource="http://www.w3.org/2002/07/owl#Restriction"/>
  </rdf:Description>
  <rdf:Description rdf:about="https://w3id.org/tern/ontologies/tern/soilClassification">
    <skos:definition>The term used to classify the SoilProfile.</skos:definition>
    <rdf:type rdf:resource="http://www.w3.org/1999/02/22-rdf-syntax-ns#Property"/>
    <rdfs:label>soil classification</rdfs:label>
  </rdf:Description>
  <rdf:Description rdf:nodeID="ub1bL510C19">
    <owl:onClass rdf:resource="http://www.w3.org/2001/XMLSchema#string"/>
    <rdf:type rdf:resource="http://www.w3.org/2002/07/owl#Restriction"/>
    <owl:qualifiedCardinality rdf:datatype="http://www.w3.org/2001/XMLSchema#nonNegativeInteger">1</owl:qualifiedCardinality>
    <owl:onProperty rdf:resource="http://www.w3.org/2004/02/skos/core#prefLabel"/>
  </rdf:Description>
  <rdf:Description rdf:nodeID="ub1bL1404C19">
    <owl:onClass rdf:resource="https://w3id.org/tern/ontologies/loc/Point"/>
    <rdf:type rdf:resource="http://www.w3.org/2002/07/owl#Restriction"/>
    <owl:qualifiedCardinality rdf:datatype="http://www.w3.org/2001/XMLSchema#nonNegativeInteger">1</owl:qualifiedCardinality>
    <owl:onProperty rdf:resource="https://w3id.org/tern/ontologies/tern/transectStartPoint"/>
  </rdf:Description>
  <rdf:Description rdf:nodeID="ub1bL682C19">
    <rdf:type rdf:resource="http://www.w3.org/2002/07/owl#Restriction"/>
    <owl:allValuesFrom rdf:resource="https://w3id.org/tern/ontologies/tern/Platform"/>
    <owl:onProperty rdf:resource="http://www.w3.org/ns/sosa/isHostedBy"/>
  </rdf:Description>
  <rdf:Description rdf:nodeID="ub1bL277C25">
    <owl:unionOf rdf:nodeID="f5a816f5a0f7a4e439059a4ae4caf6ab4b1"/>
    <rdf:type rdf:resource="http://www.w3.org/2002/07/owl#Class"/>
  </rdf:Description>
  <rdf:Description rdf:about="https://w3id.org/tern/ontologies/tern/transectEndPoint">
    <rdf:type rdf:resource="http://www.w3.org/1999/02/22-rdf-syntax-ns#Property"/>
    <rdfs:label>transect end point</rdfs:label>
    <skos:definition>Refers to the [tern-loc:Point](https://w3id.org/tern/ontologies/loc/Point) representing the end of a transect.</skos:definition>
  </rdf:Description>
  <rdf:Description rdf:about="http://linked.data.gov.au/def/datatype/Count">
    <rdfs:subClassOf rdf:resource="https://w3id.org/tern/ontologies/tern/Result"/>
  </rdf:Description>
  <rdf:Description rdf:nodeID="ub1bL1277C25">
    <owl:unionOf rdf:nodeID="f5a816f5a0f7a4e439059a4ae4caf6ab4b18"/>
    <rdf:type rdf:resource="http://www.w3.org/2002/07/owl#Class"/>
  </rdf:Description>
  <rdf:Description rdf:nodeID="ub1bL540C25">
    <owl:unionOf rdf:nodeID="f5a816f5a0f7a4e439059a4ae4caf6ab4b11"/>
    <rdf:type rdf:resource="http://www.w3.org/2002/07/owl#Class"/>
  </rdf:Description>
  <rdf:Description rdf:about="http://linked.data.gov.au/def/datatype/Percent">
    <rdfs:subClassOf rdf:resource="https://w3id.org/tern/ontologies/tern/Result"/>
  </rdf:Description>
  <rdf:Description rdf:nodeID="f5a816f5a0f7a4e439059a4ae4caf6ab4b1">
    <rdf:first rdf:resource="http://www.w3.org/2001/XMLSchema#decimal"/>
    <rdf:rest rdf:nodeID="f5a816f5a0f7a4e439059a4ae4caf6ab4b2"/>
  </rdf:Description>
  <rdf:Description rdf:nodeID="ub1bL1250C19">
    <rdf:type rdf:resource="http://www.w3.org/2002/07/owl#Restriction"/>
    <owl:allValuesFrom rdf:resource="http://www.w3.org/2001/XMLSchema#dateTime"/>
    <owl:onProperty rdf:resource="http://www.w3.org/ns/prov#endedAtTime"/>
  </rdf:Description>
  <rdf:Description rdf:about="http://linked.data.gov.au/def/datatype/QuantitativeMeasure">
    <rdfs:subClassOf rdf:resource="https://w3id.org/tern/ontologies/tern/Result"/>
  </rdf:Description>
  <rdf:Description rdf:nodeID="f5a816f5a0f7a4e439059a4ae4caf6ab4b15">
    <rdf:rest rdf:resource="http://www.w3.org/1999/02/22-rdf-syntax-ns#nil"/>
    <rdf:first rdf:resource="https://w3id.org/tern/ontologies/tern/Sampling"/>
  </rdf:Description>
</rdf:RDF>
