<?xml version="1.0" encoding="UTF-8"?>
<rdf:RDF
   xmlns:dcterms="http://purl.org/dc/terms/"
   xmlns:doap="http://usefulinc.com/ns/doap#"
   xmlns:owl="http://www.w3.org/2002/07/owl#"
   xmlns:prov="http://www.w3.org/ns/prov#"
   xmlns:rdf="http://www.w3.org/1999/02/22-rdf-syntax-ns#"
   xmlns:rdfs="http://www.w3.org/2000/01/rdf-schema#"
   xmlns:schema="http://schema.org/"
   xmlns:skos="http://www.w3.org/2004/02/skos/core#"
>
  <rdf:Description rdf:about="https://w3id.org/tern/ontologies/tern/Sampling">
    <rdf:type rdf:resource="http://www.w3.org/2002/07/owl#Class"/>
    <rdfs:subClassOf rdf:nodeID="ub1bL813C19"/>
    <rdfs:subClassOf rdf:nodeID="ub1bL841C19"/>
    <rdfs:subClassOf rdf:nodeID="ub1bL818C19"/>
    <rdfs:subClassOf rdf:resource="http://www.w3.org/ns/sosa/Sampling"/>
    <skos:definition>*Sampling* - An act of [Sampling](#Sampling) carries out a (Sampling) [Procedure](#Procedure) to create or transform one or more [Samples](#Sample).</skos:definition>
    <skos:scopeNote>Crushing a rock sample in a ball mill.
Digging a pit through a soil sequence.
Dividing a field site into quadrants.
Drawing blood from a patient.
Drilling an observation well.
Establishing a station for environmental monitoring.
Registering an image of the landscape.
Sieving a powder to separate the subset finer than 100-mesh.
Selecting a subset of a population.
Splitting a piece of drill-core to create two new samples.
Taking a diamond-drill core from a rock outcrop.</skos:scopeNote>
    <rdfs:subClassOf rdf:nodeID="ub1bL835C19"/>
    <rdfs:subClassOf rdf:nodeID="ub1bL829C19"/>
    <rdfs:subClassOf rdf:nodeID="ub1bL823C19"/>
    <rdfs:subClassOf rdf:resource="http://www.w3.org/ns/prov#Activity"/>
    <rdfs:label>Sampling</rdfs:label>
  </rdf:Description>
  <rdf:Description rdf:about="https://w3id.org/tern/ontologies/tern/Transect">
    <skos:definition>A straight line or narrow section through an object or natural feature or across the earth's surface, along which observations are made or measurements taken.</skos:definition>
    <rdfs:subClassOf rdf:nodeID="ub1bL1259C19"/>
    <rdfs:subClassOf rdf:nodeID="ub1bL1248C19"/>
    <rdfs:subClassOf rdf:nodeID="ub1bL1243C19"/>
    <rdf:type rdf:resource="http://www.w3.org/2002/07/owl#Class"/>
    <rdfs:label>Transect</rdfs:label>
    <rdfs:subClassOf rdf:nodeID="ub1bL1265C19"/>
    <rdfs:subClassOf rdf:nodeID="ub1bL1253C19"/>
    <rdfs:subClassOf rdf:resource="https://w3id.org/tern/ontologies/tern/Sample"/>
  </rdf:Description>
  <rdf:Description rdf:nodeID="ub1bL1134C19">
    <owl:qualifiedCardinality rdf:datatype="http://www.w3.org/2001/XMLSchema#nonNegativeInteger">1</owl:qualifiedCardinality>
    <rdf:type rdf:resource="http://www.w3.org/2002/07/owl#Restriction"/>
    <owl:onProperty rdf:resource="https://w3id.org/tern/ontologies/tern/taxon"/>
    <owl:onClass rdf:resource="https://w3id.org/tern/ontologies/sd/StateTaxon"/>
  </rdf:Description>
  <rdf:Description rdf:about="https://w3id.org/tern/ontologies/tern/siteShape">
    <rdfs:domain rdf:resource="https://w3id.org/tern/ontologies/tern/Site"/>
    <skos:definition>The shape of the site. The value is expected to be from a controlled vocabulary with a persistent URI identifier.</skos:definition>
    <rdfs:label>site shape</rdfs:label>
    <rdf:type rdf:resource="http://www.w3.org/1999/02/22-rdf-syntax-ns#Property"/>
  </rdf:Description>
  <rdf:Description rdf:about="https://w3id.org/tern/ontologies/tern/SiteVisit">
    <skos:definition>A discrete time-bounded visit to a site, during which sampling or observation activities are undertaken.</skos:definition>
    <rdfs:subClassOf rdf:nodeID="ub1bL1199C19"/>
    <rdfs:subClassOf rdf:nodeID="ub1bL1145C19"/>
    <rdfs:subClassOf rdf:nodeID="ub1bL1155C19"/>
    <rdfs:subClassOf rdf:nodeID="ub1bL1150C19"/>
    <rdfs:subClassOf rdf:nodeID="ub1bL1187C19"/>
    <rdfs:subClassOf rdf:nodeID="ub1bL1205C19"/>
    <rdfs:subClassOf rdf:nodeID="ub1bL1193C19"/>
    <rdfs:subClassOf rdf:nodeID="ub1bL1160C19"/>
    <rdf:type rdf:resource="http://www.w3.org/2002/07/owl#Class"/>
    <rdfs:subClassOf rdf:resource="http://www.w3.org/ns/prov#Activity"/>
    <rdfs:subClassOf rdf:nodeID="ub1bL1181C19"/>
    <rdfs:subClassOf rdf:nodeID="ub1bL1165C19"/>
    <rdfs:label>Site Visit</rdfs:label>
    <rdfs:subClassOf rdf:nodeID="ub1bL1170C19"/>
  </rdf:Description>
  <rdf:Description rdf:about="https://w3id.org/tern/ontologies/tern/transectStartPoint">
    <skos:definition>Link to a [tern-loc:Point](https://w3id.org/tern/ontologies/loc/Point) representing the start of the transect.</skos:definition>
    <rdfs:label>transect start point</rdfs:label>
    <rdf:type rdf:resource="http://www.w3.org/1999/02/22-rdf-syntax-ns#Property"/>
    <rdfs:domain rdf:resource="https://w3id.org/tern/ontologies/tern/Transect"/>
  </rdf:Description>
  <rdf:Description rdf:about="https://w3id.org/tern/ontologies/tern/FluxTower">
    <rdfs:subClassOf rdf:resource="https://w3id.org/tern/ontologies/tern/FixedPlatform"/>
    <rdfs:subClassOf rdf:nodeID="ub1bL384C19"/>
    <rdfs:subClassOf rdf:nodeID="ub1bL366C19"/>
    <rdfs:label>Flux Tower</rdfs:label>
    <rdf:type rdf:resource="http://www.w3.org/2002/07/owl#Class"/>
    <rdfs:subClassOf rdf:nodeID="ub1bL372C19"/>
    <skos:definition>Across the globe, towers stand among the landscape, with sensors monitoring these eddies for carbon dioxide, water vapor and other gasses.  These so-called “flux towers” collect data on carbon dioxide exchange rates between the earth and atmosphere.</skos:definition>
    <rdfs:subClassOf rdf:nodeID="ub1bL354C19"/>
    <rdfs:subClassOf rdf:nodeID="ub1bL360C19"/>
    <rdfs:subClassOf rdf:nodeID="ub1bL378C19"/>
    <rdfs:subClassOf rdf:nodeID="ub1bL344C19"/>
    <rdfs:subClassOf rdf:nodeID="ub1bL349C19"/>
  </rdf:Description>
  <rdf:Description rdf:about="https://w3id.org/tern/ontologies/tern/Input">
    <rdfs:subClassOf rdf:resource="http://www.w3.org/ns/ssn/Input"/>
    <rdfs:subClassOf rdf:nodeID="ub1bL396C19"/>
    <skos:definition>*Input* - Any information that is provided to a [Procedure](#Procedure) for its use.</skos:definition>
    <rdf:type rdf:resource="http://www.w3.org/2002/07/owl#Class"/>
    <rdfs:subClassOf rdf:nodeID="ub1bL401C19"/>
    <rdfs:label>Input</rdfs:label>
    <rdfs:subClassOf rdf:nodeID="ub1bL406C19"/>
    <skos:scopeNote>&lt;a href="#Input"&gt;Input&lt;/a&gt; can be used to capture any input values for a procedure, such as the input value of the basal wedge to estimate the basal area per hectare.</skos:scopeNote>
  </rdf:Description>
  <rdf:Description rdf:about="https://w3id.org/tern/ontologies/tern/SiteStratumTaxon">
    <rdfs:subClassOf rdf:nodeID="ub1bL1123C19"/>
    <rdfs:label>Site Stratum Taxon</rdfs:label>
    <rdf:type rdf:resource="http://www.w3.org/2002/07/owl#Class"/>
    <rdfs:subClassOf rdf:nodeID="ub1bL1111C19"/>
    <rdfs:subClassOf rdf:resource="https://w3id.org/tern/ontologies/tern/Sample"/>
    <rdfs:subClassOf rdf:nodeID="ub1bL1117C19"/>
  </rdf:Description>
  <rdf:Description rdf:about="https://w3id.org/tern/ontologies/tern/">
    <owl:imports rdf:resource="http://www.w3.org/2004/02/skos/core#"/>
    <dcterms:modified rdf:datatype="http://www.w3.org/2001/XMLSchema#date">2020-12-07</dcterms:modified>
    <owl:imports rdf:resource="https://w3id.org/tern/ontologies/loc/"/>
    <dcterms:contributor rdf:nodeID="ub1bL89C23"/>
    <rdfs:seeAlso rdf:resource="https://www.w3.org/TR/vocab-ssn-ext/"/>
    <dcterms:license rdf:resource="http://creativecommons.org/publicdomain/zero/1.0/"/>
    <dcterms:creator rdf:nodeID="ub1bL121C19"/>
    <dcterms:contributor rdf:nodeID="ub1bL95C23"/>
    <owl:imports rdf:resource="file:///Users/uqechuc/TBCMEWorkspace/projects/external_imports/schemaorg-current-http.ttl"/>
    <owl:versionInfo>0.1.2</owl:versionInfo>
    <owl:imports rdf:resource="https://raw.githubusercontent.com/AGLDWG/datatype-ont/master/rdf/datatype.rdf"/>
    <dcterms:creator rdf:nodeID="ub1bL107C19"/>
    <owl:imports rdf:resource="http://www.w3.org/ns/dcat#"/>
    <owl:imports rdf:resource="http://www.w3.org/2006/time#"/>
    <rdfs:seeAlso rdf:resource="https://www.w3.org/ns/ssn/"/>
    <rdfs:label>TERN Ontology</rdfs:label>
    <owl:imports rdf:resource="http://www.w3.org/ns/prov#"/>
    <owl:imports rdf:resource="http://www.w3.org/ns/sosa/"/>
    <owl:imports rdf:resource="http://www.w3.org/ns/ssn/"/>
    <dcterms:creator rdf:nodeID="ub1bL114C19"/>
    <dcterms:publisher rdf:resource="https://w3id.org/tern/resources/a083902d-d821-41be-b663-1d7cb33eea66"/>
    <rdfs:seeAlso rdf:resource="https://www.publish.csiro.au/book/5230/"/>
    <owl:versionIRI rdf:resource="http://linked.data.gov.au/def/plot/0.1.2"/>
    <prov:wasGeneratedBy rdf:nodeID="ub1bL155C23"/>
    <dcterms:contributor rdf:nodeID="ub1bL101C23"/>
    <owl:imports rdf:resource="http://qudt.org/schema/qudt/"/>
    <owl:imports rdf:resource="https://w3id.org/tern/ontologies/org/"/>
    <owl:imports rdf:resource="https://w3id.org/tern/ontologies/sd/"/>
    <rdfs:comment>A set of vocabularies based largely on SOSA/SSN to site-based ecological survey data. It is primary related to vegetation surveys, following the methodologies outlined in the Australian Soil and Land Survey Field Handbook.</rdfs:comment>
    <rdf:type rdf:resource="http://www.w3.org/2002/07/owl#Ontology"/>
    <owl:imports rdf:resource="http://datashapes.org/dash"/>
  </rdf:Description>
  <rdf:Description rdf:nodeID="ub1bL1093C19">
    <owl:onClass rdf:resource="http://www.w3.org/2004/02/skos/core#Concept"/>
    <owl:onProperty rdf:resource="https://w3id.org/tern/ontologies/tern/stratum"/>
    <rdf:type rdf:resource="http://www.w3.org/2002/07/owl#Restriction"/>
    <owl:qualifiedCardinality rdf:datatype="http://www.w3.org/2001/XMLSchema#nonNegativeInteger">1</owl:qualifiedCardinality>
  </rdf:Description>
  <rdf:Description rdf:nodeID="ub1bL1068C19">
    <owl:onClass rdf:resource="http://www.w3.org/2001/XMLSchema#string"/>
    <owl:qualifiedCardinality rdf:datatype="http://www.w3.org/2001/XMLSchema#nonNegativeInteger">1</owl:qualifiedCardinality>
    <owl:onProperty rdf:resource="http://purl.org/dc/terms/identifier"/>
    <rdf:type rdf:resource="http://www.w3.org/2002/07/owl#Restriction"/>
  </rdf:Description>
  <rdf:Description rdf:about="https://w3id.org/tern/ontologies/tern/siteDescription">
    <rdf:type rdf:resource="http://www.w3.org/1999/02/22-rdf-syntax-ns#Property"/>
    <skos:definition>The description of the site.</skos:definition>
    <rdfs:label>site description</rdfs:label>
  </rdf:Description>
  <rdf:Description rdf:about="https://w3id.org/tern/ontologies/tern/PropertyValue">
    <rdf:type rdf:resource="http://www.w3.org/2002/07/owl#Class"/>
    <rdfs:subClassOf rdf:resource="http://schema.org/PropertyValue"/>
    <rdfs:subClassOf rdf:nodeID="ub1bL674C19"/>
    <rdfs:label>Property Value</rdfs:label>
    <rdfs:subClassOf rdf:nodeID="ub1bL669C19"/>
    <skos:definition>A property-value pair. Use the [schema:name](http://schema.org/name) property for the name of the property. If there is an additional human-readable version of the value, put that into the [schema:description](http://schema.org/description) property.</skos:definition>
    <rdfs:subClassOf rdf:nodeID="ub1bL680C19"/>
    <skos:example>@prefix tern: &lt;https://w3id.org/tern/ontologies/tern/&gt; .
@prefix schema: &lt;http://schema.org/&gt; .
@prefix data: &lt;http://linked.data.gov.au/def/datatype/&gt; .
@prefix sosa: &lt;http://w3.org/ns/sosa/&gt; .

&lt;example&gt; a tern:PropertyValue ;
	schema:name "AUSPLOTS_RANGELANDS.SITE.PROPERTY" ;
	schema:description "The property name" ;
	sosa:hasResult [
		a data:Text ;
		data:value "Great Victoria Desert Nature Reserve" ;
	] .</skos:example>
  </rdf:Description>
  <rdf:Description rdf:about="https://w3id.org/tern/ontologies/tern/Site">
    <rdfs:subClassOf rdf:nodeID="ub1bL1080C19"/>
    <rdfs:subClassOf rdf:nodeID="ub1bL1021C19"/>
    <rdfs:subClassOf rdf:nodeID="ub1bL956C19"/>
    <rdfs:subClassOf rdf:nodeID="ub1bL987C19"/>
    <rdfs:subClassOf rdf:nodeID="ub1bL992C19"/>
    <rdfs:subClassOf rdf:nodeID="ub1bL971C19"/>
    <rdfs:subClassOf rdf:nodeID="ub1bL1015C19"/>
    <rdf:type rdf:resource="http://www.w3.org/2002/07/owl#Class"/>
    <rdfs:subClassOf rdf:nodeID="ub1bL951C19"/>
    <rdfs:subClassOf rdf:nodeID="ub1bL946C19"/>
    <rdfs:subClassOf rdf:nodeID="ub1bL936C19"/>
    <rdfs:subClassOf rdf:nodeID="ub1bL966C19"/>
    <rdfs:subClassOf rdf:nodeID="ub1bL976C19"/>
    <rdfs:subClassOf rdf:nodeID="ub1bL1039C19"/>
    <rdfs:subClassOf rdf:nodeID="ub1bL997C19"/>
    <rdfs:subClassOf rdf:nodeID="ub1bL1033C19"/>
    <rdfs:subClassOf rdf:nodeID="ub1bL1068C19"/>
    <skos:definition>Location where observations may be made. This is a subclass of [Sample](#Sample) because a site should be designed to be representative of an environmental system (which may be an ecosystem or bioregion) or zone (which may be a zone such as a parcel or tract).</skos:definition>
    <skos:scopeNote>Use [dcterms:hasPart](http://purl.org/dc/terms/hasPart) and [dcterms:isPartOf](http://purl.org/dc/terms/isPartOf) to model [Site](#Site) and [Subsite](#Site) relationships. E.g. In TERN, there are SuperSites that contain multiple core 1 ha subsites.</skos:scopeNote>
    <rdfs:subClassOf rdf:nodeID="ub1bL1074C19"/>
    <rdfs:subClassOf rdf:nodeID="ub1bL961C19"/>
    <rdfs:subClassOf rdf:nodeID="ub1bL1027C19"/>
    <rdfs:subClassOf rdf:nodeID="ub1bL1057C19"/>
    <rdfs:subClassOf rdf:nodeID="ub1bL1045C19"/>
    <rdfs:subClassOf rdf:nodeID="ub1bL941C19"/>
    <rdfs:subClassOf rdf:nodeID="ub1bL1003C19"/>
    <rdfs:subClassOf rdf:resource="https://w3id.org/tern/ontologies/tern/Sample"/>
    <rdfs:label>Site</rdfs:label>
    <rdfs:subClassOf rdf:resource="https://w3id.org/tern/ontologies/tern/Platform"/>
    <rdfs:subClassOf rdf:nodeID="ub1bL1009C19"/>
    <rdfs:subClassOf rdf:nodeID="ub1bL1062C19"/>
    <rdfs:subClassOf rdf:nodeID="ub1bL1051C19"/>
  </rdf:Description>
  <rdf:Description rdf:nodeID="ub1bL554C19">
    <owl:minQualifiedCardinality rdf:datatype="http://www.w3.org/2001/XMLSchema#nonNegativeInteger">1</owl:minQualifiedCardinality>
    <owl:onProperty rdf:resource="http://www.w3.org/ns/sosa/hasResult"/>
    <rdf:type rdf:resource="http://www.w3.org/2002/07/owl#Restriction"/>
    <owl:onClass rdf:resource="https://w3id.org/tern/ontologies/tern/Result"/>
  </rdf:Description>
  <rdf:Description rdf:nodeID="ub1bL1057C19">
    <owl:onProperty rdf:resource="http://www.opengis.net/ont/geosparql#hasGeometry"/>
    <owl:minCardinality rdf:datatype="http://www.w3.org/2001/XMLSchema#nonNegativeInteger">1</owl:minCardinality>
    <rdf:type rdf:resource="http://www.w3.org/2002/07/owl#Restriction"/>
  </rdf:Description>
  <rdf:Description rdf:about="https://w3id.org/tern/ontologies/tern/globalVocabulary">
    <rdf:type rdf:resource="http://www.w3.org/1999/02/22-rdf-syntax-ns#Property"/>
    <rdfs:label>global vocabulary</rdfs:label>
    <skos:definition>The global vocabulary which the global:value belongs to (in the closed system).</skos:definition>
  </rdf:Description>
  <rdf:Description rdf:nodeID="ub1bL468C19">
    <rdf:type rdf:resource="http://www.w3.org/2002/07/owl#Restriction"/>
    <owl:onClass rdf:resource="http://www.w3.org/2001/XMLSchema#string"/>
    <owl:qualifiedCardinality rdf:datatype="http://www.w3.org/2001/XMLSchema#nonNegativeInteger">1</owl:qualifiedCardinality>
    <owl:onProperty rdf:resource="http://www.w3.org/2004/02/skos/core#prefLabel"/>
  </rdf:Description>
  <rdf:Description rdf:about="http://rs.tdwg.org/dwc/terms/MaterialSample">
    <rdf:type rdf:resource="http://www.w3.org/2002/07/owl#Class"/>
    <rdfs:isDefinedBy rdf:resource="http://rs.tdwg.org/dwc/terms/"/>
    <skos:example>A whole organism preserved in a collection. A part of an organism isolated for some purpose. A soil sample. A marine microbial sample.</skos:example>
    <rdfs:comment>A physical result of a sampling (or subsampling) event. In biological collections, the material sample is typically collected, and either preserved or destructively processed.</rdfs:comment>
    <rdfs:label>Material Sample</rdfs:label>
  </rdf:Description>
  <rdf:Description rdf:about="https://w3id.org/tern/ontologies/tern/Observation">
    <rdfs:subClassOf rdf:resource="http://www.w3.org/ns/prov#Activity"/>
    <rdfs:subClassOf rdf:nodeID="ub1bL542C19"/>
    <rdfs:subClassOf rdf:nodeID="ub1bL566C19"/>
    <rdfs:subClassOf rdf:nodeID="ub1bL532C19"/>
    <rdfs:subClassOf rdf:nodeID="ub1bL572C19"/>
    <rdfs:subClassOf rdf:nodeID="ub1bL590C19"/>
    <rdfs:subClassOf rdf:nodeID="ub1bL537C19"/>
    <rdfs:subClassOf rdf:nodeID="ub1bL548C19"/>
    <rdfs:subClassOf rdf:resource="http://www.w3.org/ns/sosa/Observation"/>
    <rdfs:subClassOf rdf:nodeID="ub1bL578C19"/>
    <rdfs:label>Observation</rdfs:label>
    <rdfs:subClassOf rdf:nodeID="ub1bL554C19"/>
    <rdf:type rdf:resource="http://www.w3.org/2002/07/owl#Class"/>
    <rdfs:subClassOf rdf:nodeID="ub1bL560C19"/>
    <rdfs:subClassOf rdf:nodeID="ub1bL584C19"/>
    <skos:definition>*Observation* - Act of carrying out an (Observation) [Procedure](#Procedure) to estimate or calculate a value of a property of a [FeatureOfInterest](http://w3.org/ns/sosa/FeatureOfInterest). Links to a [Sensor](http://w3.org/ns/sosa/Sensor) to describe what made the [Observation](#Observation) and how; links to an [ObservableProperty](#ObservableProperty) to describe what the result is an estimate of, and to a [FeatureOfInterest](http://w3.org/ns/sosa/FeatureOfInterest) to detail what that property was associated with.</skos:definition>
  </rdf:Description>
  <rdf:Description rdf:about="https://w3id.org/tern/ontologies/tern/SamplingPoint">
    <rdfs:label>Sampling Point</rdfs:label>
    <rdfs:subClassOf rdf:nodeID="ub1bL888C19"/>
    <rdfs:subClassOf rdf:nodeID="ub1bL900C19"/>
    <rdf:type rdf:resource="http://www.w3.org/2002/07/owl#Class"/>
    <rdfs:subClassOf rdf:nodeID="ub1bL882C19"/>
    <rdfs:subClassOf rdf:resource="https://w3id.org/tern/ontologies/loc/Point"/>
    <rdfs:subClassOf rdf:nodeID="ub1bL864C19"/>
    <rdfs:subClassOf rdf:nodeID="ub1bL906C19"/>
    <rdfs:subClassOf rdf:nodeID="ub1bL894C19"/>
    <rdfs:subClassOf rdf:nodeID="ub1bL870C19"/>
    <rdfs:subClassOf rdf:nodeID="ub1bL876C19"/>
    <skos:definition>A point in space where an [Observation](#Observation) or [Sampling](#Sampling) occurred. </skos:definition>
  </rdf:Description>
  <rdf:Description rdf:about="http://linked.data.gov.au/def/datatype/Percent">
    <rdfs:subClassOf rdf:resource="https://w3id.org/tern/ontologies/tern/Result"/>
  </rdf:Description>
  <rdf:Description rdf:nodeID="ub1bL669C19">
    <owl:allValuesFrom rdf:resource="http://www.w3.org/2001/XMLSchema#string"/>
    <owl:onProperty rdf:resource="http://schema.org/description"/>
    <rdf:type rdf:resource="http://www.w3.org/2002/07/owl#Restriction"/>
  </rdf:Description>
  <rdf:Description rdf:nodeID="ub1bL888C19">
    <rdf:type rdf:resource="http://www.w3.org/2002/07/owl#Restriction"/>
    <owl:onClass rdf:resource="https://w3id.org/tern/ontologies/tern/Transect"/>
    <owl:maxQualifiedCardinality rdf:datatype="http://www.w3.org/2001/XMLSchema#nonNegativeInteger">1</owl:maxQualifiedCardinality>
    <owl:onProperty rdf:resource="https://w3id.org/tern/ontologies/tern/isSamplingPointOf"/>
  </rdf:Description>
  <rdf:Description rdf:nodeID="ub1bL95C23">
    <schema:email>mosheh.eliyahu@adelaide.edu.au</schema:email>
    <schema:name>Mosheh Eliyahu</schema:name>
    <schema:affiliation rdf:resource="https://w3id.org/tern/resources/a083902d-d821-41be-b663-1d7cb33eea66"/>
    <rdf:type rdf:resource="http://schema.org/Person"/>
  </rdf:Description>
  <rdf:Description rdf:about="https://w3id.org/tern/ontologies/tern/dateCommissioned">
    <skos:definition>The date when something was commissioned, e.g. a [Site](#Site).</skos:definition>
    <rdfs:label>date commissioned</rdfs:label>
    <rdf:type rdf:resource="http://www.w3.org/1999/02/22-rdf-syntax-ns#Property"/>
  </rdf:Description>
  <rdf:Description rdf:about="https://w3id.org/tern/ontologies/tern/Sampler">
    <rdf:type rdf:resource="http://www.w3.org/2002/07/owl#Class"/>
    <skos:definition>*Sampler* - A device that is used by, or implements, a (Sampling) [Procedure](#Procedure) to create or transform one or more samples.</skos:definition>
    <rdfs:subClassOf rdf:nodeID="ub1bL800C19"/>
    <rdfs:subClassOf rdf:nodeID="ub1bL795C19"/>
    <rdfs:subClassOf rdf:resource="https://w3id.org/tern/ontologies/tern/Instrument"/>
    <rdfs:subClassOf rdf:resource="http://www.w3.org/ns/sosa/Sampler"/>
    <rdfs:label>Sampler</rdfs:label>
  </rdf:Description>
  <rdf:Description rdf:about="https://w3id.org/tern/ontologies/tern/EcosystemProcessesSite">
    <rdfs:label>Ecosystem Processes Site</rdfs:label>
    <rdfs:subClassOf rdf:resource="https://w3id.org/tern/ontologies/tern/Site"/>
    <rdf:type rdf:resource="http://www.w3.org/2002/07/owl#Class"/>
    <skos:definition>An ecological [Site](#Site) that usually hosts a [FluxTower](#FluxTower).</skos:definition>
  </rdf:Description>
  <rdf:Description rdf:nodeID="ub1bL519C19">
    <owl:qualifiedCardinality rdf:datatype="http://www.w3.org/2001/XMLSchema#nonNegativeInteger">1</owl:qualifiedCardinality>
    <rdf:type rdf:resource="http://www.w3.org/2002/07/owl#Restriction"/>
    <owl:onClass rdf:resource="https://w3id.org/tern/ontologies/tern/Parameter"/>
    <owl:onProperty rdf:resource="http://www.w3.org/1999/02/22-rdf-syntax-ns#value"/>
  </rdf:Description>
  <rdf:Description rdf:about="http://linked.data.gov.au/def/datatype/PercentRange">
    <rdfs:subClassOf rdf:resource="https://w3id.org/tern/ontologies/tern/Result"/>
  </rdf:Description>
  <rdf:Description rdf:nodeID="ub1bL241C19">
    <owl:onProperty rdf:resource="http://schema.org/model"/>
    <owl:minCardinality rdf:datatype="http://www.w3.org/2001/XMLSchema#nonNegativeInteger">1</owl:minCardinality>
    <rdf:type rdf:resource="http://www.w3.org/2002/07/owl#Restriction"/>
  </rdf:Description>
  <rdf:Description rdf:about="https://w3id.org/tern/ontologies/tern/transectDirection">
    <rdfs:label>transect direction</rdfs:label>
    <rdf:type rdf:resource="http://www.w3.org/1999/02/22-rdf-syntax-ns#Property"/>
    <rdfs:range rdf:resource="http://www.w3.org/2001/XMLSchema#string"/>
    <skos:example>S-W</skos:example>
    <rdfs:domain rdf:resource="https://w3id.org/tern/ontologies/tern/Transect"/>
    <skos:definition>Describe the direction of the transect.</skos:definition>
  </rdf:Description>
  <rdf:Description rdf:nodeID="ub1bL1181C19">
    <owl:onClass rdf:resource="http://www.w3.org/2001/XMLSchema#string"/>
    <rdf:type rdf:resource="http://www.w3.org/2002/07/owl#Restriction"/>
    <owl:maxQualifiedCardinality rdf:datatype="http://www.w3.org/2001/XMLSchema#nonNegativeInteger">1</owl:maxQualifiedCardinality>
    <owl:onProperty rdf:resource="https://w3id.org/tern/ontologies/tern/locationDescription"/>
  </rdf:Description>
  <rdf:Description rdf:nodeID="ub1bL578C19">
    <rdf:type rdf:resource="http://www.w3.org/2002/07/owl#Restriction"/>
    <owl:onClass rdf:resource="https://w3id.org/tern/ontologies/tern/ObservableProperty"/>
    <owl:onProperty rdf:resource="http://www.w3.org/ns/sosa/observedProperty"/>
    <owl:qualifiedCardinality rdf:datatype="http://www.w3.org/2001/XMLSchema#nonNegativeInteger">1</owl:qualifiedCardinality>
  </rdf:Description>
  <rdf:Description rdf:nodeID="ub1bL882C19">
    <owl:onClass rdf:resource="http://www.w3.org/2001/XMLSchema#string"/>
    <owl:maxQualifiedCardinality rdf:datatype="http://www.w3.org/2001/XMLSchema#nonNegativeInteger">1</owl:maxQualifiedCardinality>
    <owl:onProperty rdf:resource="http://purl.org/dc/terms/identifier"/>
    <rdf:type rdf:resource="http://www.w3.org/2002/07/owl#Restriction"/>
  </rdf:Description>
  <rdf:Description rdf:about="https://w3id.org/tern/ontologies/tern/AutomaticWeatherStation">
    <rdfs:label>Automatic Weather Station</rdfs:label>
    <rdfs:subClassOf rdf:resource="https://w3id.org/tern/ontologies/tern/FixedPlatform"/>
    <rdf:type rdf:resource="http://www.w3.org/2002/07/owl#Class"/>
  </rdf:Description>
  <rdf:Description rdf:about="https://w3id.org/tern/ontologies/tern/Result">
    <rdfs:subClassOf rdf:nodeID="ub1bL721C19"/>
    <skos:definition>*Result* - The result of an [Observation](#Observation), [Actuation](http://w3.org/ns/sosa/Actuation), or act of [Sampling](#Sampling). To store an observation's simple result value one can use the [hasSimpleResult](http://w3.org/ns/sosa/hasSimpleResult) property.</skos:definition>
    <skos:example>The value 20 as the height of a certain tree together with the unit, e.g., Meter.</skos:example>
    <rdfs:subClassOf rdf:nodeID="ub1bL716C19"/>
    <rdfs:subClassOf rdf:resource="http://www.w3.org/ns/sosa/Result"/>
    <rdfs:subClassOf rdf:nodeID="ub1bL732C19"/>
    <rdf:type rdf:resource="http://www.w3.org/2002/07/owl#Class"/>
    <rdfs:label>Result</rdfs:label>
  </rdf:Description>
  <rdf:Description rdf:about="https://w3id.org/tern/ontologies/tern/equipment">
    <rdf:type rdf:resource="http://www.w3.org/2002/07/owl#DatatypeProperty"/>
    <rdfs:range rdf:resource="http://www.w3.org/2001/XMLSchema#string"/>
    <rdfs:label>equipment</rdfs:label>
    <skos:definition>Describe the equipment used as text.</skos:definition>
  </rdf:Description>
  <rdf:Description rdf:about="https://w3id.org/tern/ontologies/tern/CORVEGSite">
    <rdfs:subClassOf rdf:resource="https://w3id.org/tern/ontologies/tern/Site"/>
    <rdf:type rdf:resource="http://www.w3.org/2002/07/owl#Class"/>
    <rdfs:label>CORVEG Site</rdfs:label>
  </rdf:Description>
  <rdf:Description rdf:nodeID="ub1bL537C19">
    <owl:allValuesFrom rdf:resource="https://w3id.org/tern/ontologies/org/Person"/>
    <rdf:type rdf:resource="http://www.w3.org/2002/07/owl#Restriction"/>
    <owl:onProperty rdf:resource="http://www.w3.org/ns/prov#wasAttributedTo"/>
  </rdf:Description>
  <rdf:Description rdf:about="https://w3id.org/tern/ontologies/tern/locationProcedure">
    <rdf:type rdf:resource="http://www.w3.org/1999/02/22-rdf-syntax-ns#Property"/>
    <rdfs:label>location procedure</rdfs:label>
    <skos:definition>Link to a procedure used to obtain the location.</skos:definition>
    <rdfs:subPropertyOf rdf:resource="https://w3id.org/tern/ontologies/tern/hasMethod"/>
  </rdf:Description>
  <rdf:Description rdf:about="https://w3id.org/tern/ontologies/tern/Sensor">
    <rdfs:subClassOf rdf:nodeID="ub1bL924C19"/>
    <rdfs:subClassOf rdf:nodeID="ub1bL919C19"/>
    <skos:definition>Device, agent (including humans), or software (simulation) involved in, or implementing, a Procedure. Sensors respond to a stimulus, e.g., a change in the environment, or input data composed from the results of prior Observations, and generate a Result. Sensors can be hosted by Platforms.</skos:definition>
    <rdfs:label>Sensor</rdfs:label>
    <rdf:type rdf:resource="http://www.w3.org/2002/07/owl#Class"/>
    <rdfs:subClassOf rdf:resource="http://www.w3.org/ns/sosa/Sensor"/>
    <rdfs:subClassOf rdf:resource="https://w3id.org/tern/ontologies/tern/Instrument"/>
  </rdf:Description>
  <rdf:Description rdf:about="https://w3id.org/tern/ontologies/tern/hasMethod">
    <rdf:type rdf:resource="http://www.w3.org/1999/02/22-rdf-syntax-ns#Property"/>
    <rdfs:subPropertyOf rdf:resource="http://www.w3.org/2004/02/skos/core#relatedMatch"/>
    <skos:definition>Link a concept to a method.</skos:definition>
    <rdfs:label>has method</rdfs:label>
  </rdf:Description>
  <rdf:Description rdf:nodeID="ub1bL572C19">
    <owl:qualifiedCardinality rdf:datatype="http://www.w3.org/2001/XMLSchema#nonNegativeInteger">1</owl:qualifiedCardinality>
    <rdf:type rdf:resource="http://www.w3.org/2002/07/owl#Restriction"/>
    <owl:onProperty rdf:resource="http://www.w3.org/ns/sosa/hasFeatureOfInterest"/>
    <owl:onClass rdf:resource="http://www.w3.org/ns/sosa/FeatureOfInterest"/>
  </rdf:Description>
  <rdf:Description rdf:nodeID="ub1bL438C19">
    <owl:onProperty rdf:resource="http://www.w3.org/2004/02/skos/core#definition"/>
    <owl:onClass rdf:resource="http://www.w3.org/2001/XMLSchema#string"/>
    <owl:maxQualifiedCardinality rdf:datatype="http://www.w3.org/2001/XMLSchema#nonNegativeInteger">1</owl:maxQualifiedCardinality>
    <rdf:type rdf:resource="http://www.w3.org/2002/07/owl#Restriction"/>
  </rdf:Description>
  <rdf:Description rdf:nodeID="fe114e3c19c6e4b2e8a8d1297357cbc21b18">
    <rdf:rest rdf:nodeID="fe114e3c19c6e4b2e8a8d1297357cbc21b19"/>
    <rdf:first rdf:resource="http://www.w3.org/2001/XMLSchema#string"/>
  </rdf:Description>
  <rdf:Description rdf:nodeID="ub1bL44C19">
    <owl:onProperty rdf:resource="https://w3id.org/tern/ontologies/tern/globalValue"/>
    <rdf:type rdf:resource="http://www.w3.org/2002/07/owl#Restriction"/>
    <owl:cardinality rdf:datatype="http://www.w3.org/2001/XMLSchema#nonNegativeInteger">1</owl:cardinality>
  </rdf:Description>
  <rdf:Description rdf:about="https://w3id.org/tern/ontologies/tern/stratum">
    <rdfs:subPropertyOf rdf:resource="http://purl.org/dc/terms/type"/>
    <skos:definition>Stratum classification.</skos:definition>
    <skos:scopeNote>Value should be from a controlled vocabulary identified by a URI.</skos:scopeNote>
    <rdfs:label>stratum</rdfs:label>
    <rdf:type rdf:resource="http://www.w3.org/1999/02/22-rdf-syntax-ns#Property"/>
  </rdf:Description>
  <rdf:Description rdf:nodeID="ub1bL1009C19">
    <owl:onProperty rdf:resource="https://w3id.org/tern/ontologies/tern/cardinalDirection"/>
    <rdf:type rdf:resource="http://www.w3.org/2002/07/owl#Restriction"/>
    <owl:onClass rdf:resource="http://www.w3.org/2001/XMLSchema#string"/>
    <owl:maxQualifiedCardinality rdf:datatype="http://www.w3.org/2001/XMLSchema#nonNegativeInteger">1</owl:maxQualifiedCardinality>
  </rdf:Description>
  <rdf:Description rdf:nodeID="fe114e3c19c6e4b2e8a8d1297357cbc21b3">
    <rdf:rest rdf:nodeID="fe114e3c19c6e4b2e8a8d1297357cbc21b4"/>
    <rdf:first rdf:resource="http://www.w3.org/2001/XMLSchema#decimal"/>
  </rdf:Description>
  <rdf:Description rdf:nodeID="ub1bL823C19">
    <owl:maxQualifiedCardinality rdf:datatype="http://www.w3.org/2001/XMLSchema#nonNegativeInteger">1</owl:maxQualifiedCardinality>
    <owl:onClass rdf:resource="https://w3id.org/tern/ontologies/tern/SamplingPoint"/>
    <rdf:type rdf:resource="http://www.w3.org/2002/07/owl#Restriction"/>
    <owl:onProperty rdf:resource="https://w3id.org/tern/ontologies/tern/hasSamplingPoint"/>
  </rdf:Description>
  <rdf:Description rdf:nodeID="ub1bL997C19">
    <owl:onClass rdf:resource="http://linked.data.gov.au/def/datatype/QuantitativeMeasure"/>
    <owl:onProperty rdf:resource="https://w3id.org/tern/ontologies/tern/area"/>
    <owl:maxQualifiedCardinality rdf:datatype="http://www.w3.org/2001/XMLSchema#nonNegativeInteger">1</owl:maxQualifiedCardinality>
    <rdf:type rdf:resource="http://www.w3.org/2002/07/owl#Restriction"/>
  </rdf:Description>
  <rdf:Description rdf:about="https://w3id.org/tern/ontologies/tern/hasParameter">
    <skos:definition>Link a concept to a parameter.</skos:definition>
    <rdfs:label>has parameter</rdfs:label>
    <rdf:type rdf:resource="http://www.w3.org/1999/02/22-rdf-syntax-ns#Property"/>
    <rdfs:subPropertyOf rdf:resource="http://www.w3.org/2004/02/skos/core#relatedMatch"/>
  </rdf:Description>
  <rdf:Description rdf:nodeID="ub1bL1080C19">
    <rdf:type rdf:resource="http://www.w3.org/2002/07/owl#Restriction"/>
    <owl:qualifiedCardinality rdf:datatype="http://www.w3.org/2001/XMLSchema#nonNegativeInteger">1</owl:qualifiedCardinality>
    <owl:onClass rdf:resource="http://www.w3.org/ns/dcat#Dataset"/>
    <owl:onProperty rdf:resource="http://www.w3.org/ns/dcat#dataset"/>
  </rdf:Description>
  <rdf:Description rdf:about="https://w3id.org/tern/ontologies/tern/SAR">
    <rdf:type rdf:resource="http://www.w3.org/2002/07/owl#Class"/>
    <rdfs:subClassOf rdf:resource="https://w3id.org/tern/ontologies/tern/Sensor"/>
    <rdfs:seeAlso rdf:resource="https://earthdata.nasa.gov/learn/backgrounders/what-is-sar"/>
    <rdfs:label>Synthetic Aperture Radar</rdfs:label>
    <skos:altLabel>SAR</skos:altLabel>
    <skos:altLabel>Synthetic-aperture radar</skos:altLabel>
  </rdf:Description>
  <rdf:Description rdf:about="https://w3id.org/tern/ontologies/tern/dimension">
    <rdfs:label>dimension</rdfs:label>
    <skos:definition>Link to a [Dimension](#Dimension).</skos:definition>
    <rdf:type rdf:resource="http://www.w3.org/1999/02/22-rdf-syntax-ns#Property"/>
  </rdf:Description>
  <rdf:Description rdf:about="https://w3id.org/tern/ontologies/tern/site">
    <rdf:type rdf:resource="http://www.w3.org/1999/02/22-rdf-syntax-ns#Property"/>
    <rdfs:label>site</rdfs:label>
    <skos:definition>Link to a [Site](#Site).</skos:definition>
    <rdfs:range rdf:resource="https://w3id.org/tern/ontologies/tern/Site"/>
  </rdf:Description>
  <rdf:Description rdf:nodeID="ub1bL231C19">
    <owl:allValuesFrom rdf:resource="http://www.w3.org/2001/XMLSchema#string"/>
    <rdf:type rdf:resource="http://www.w3.org/2002/07/owl#Restriction"/>
    <owl:onProperty rdf:resource="http://www.w3.org/2004/02/skos/core#altLabel"/>
  </rdf:Description>
  <rdf:Description rdf:about="https://w3id.org/tern/ontologies/tern/SuperSite">
    <rdf:type rdf:resource="http://www.w3.org/2002/07/owl#Class"/>
    <rdfs:subClassOf rdf:resource="https://w3id.org/tern/ontologies/tern/Site"/>
    <rdfs:seeAlso rdf:resource="https://supersites.tern.org.au/"/>
    <skos:definition>TERN SuperSites are Long Term Ecological Research (LTER) sites co-located with TERN OzFlux eddy covariance towers, which deliver biological and environmental observations of flora, fauna, microbial biodiversity, soils and hydrology. TERN OzFlux delivers micrometeorological observations of energy, carbon and water exchange between the atmosphere and key Australian ecosystems. Each TERN SuperSite is located in a significant Australian biome and the network spans a wide range of environmental conditions. The SuperSite network collects detailed data sets on flora, fauna and biophysical processes from each SuperSite.</skos:definition>
    <rdfs:label>SuperSite</rdfs:label>
  </rdf:Description>
  <rdf:Description rdf:about="https://w3id.org/tern/ontologies/tern/hasEnvironmentalCharacteristic">
    <rdf:type rdf:resource="http://www.w3.org/2002/07/owl#ObjectProperty"/>
    <rdfs:label>has environmental characteristic</rdfs:label>
    <rdfs:range rdf:resource="https://w3id.org/tern/ontologies/tern/EnvironmentalCharacteristic"/>
  </rdf:Description>
  <rdf:Description rdf:about="https://w3id.org/tern/ontologies/tern/DigitalCamera">
    <rdfs:subClassOf rdf:resource="http://www.w3.org/2004/02/skos/core#Concept"/>
    <rdfs:subClassOf rdf:nodeID="ub1bL231C19"/>
    <rdfs:subClassOf rdf:nodeID="ub1bL246C19"/>
    <rdfs:subClassOf rdf:nodeID="ub1bL236C19"/>
    <rdfs:subClassOf rdf:nodeID="ub1bL251C19"/>
    <skos:example>E.g. EOS 350D</skos:example>
    <rdf:type rdf:resource="http://www.w3.org/2002/07/owl#Class"/>
    <rdfs:subClassOf rdf:nodeID="ub1bL241C19"/>
    <skos:definition>The model as defined by the manufacturer.</skos:definition>
    <rdfs:subClassOf rdf:resource="https://w3id.org/tern/ontologies/tern/Sampler"/>
    <rdfs:subClassOf rdf:nodeID="ub1bL257C19"/>
    <rdfs:label>Digital Camera</rdfs:label>
  </rdf:Description>
  <rdf:Description rdf:nodeID="ub1bL246C19">
    <owl:minCardinality rdf:datatype="http://www.w3.org/2001/XMLSchema#nonNegativeInteger">1</owl:minCardinality>
    <owl:onProperty rdf:resource="http://www.w3.org/2004/02/skos/core#prefLabel"/>
    <rdf:type rdf:resource="http://www.w3.org/2002/07/owl#Restriction"/>
  </rdf:Description>
  <rdf:Description rdf:nodeID="ub1bL1155C19">
    <rdf:type rdf:resource="http://www.w3.org/2002/07/owl#Restriction"/>
    <owl:onProperty rdf:resource="http://www.w3.org/2000/01/rdf-schema#comment"/>
    <owl:allValuesFrom rdf:resource="http://www.w3.org/2001/XMLSchema#string"/>
  </rdf:Description>
  <rdf:Description rdf:nodeID="ub1bL906C19">
    <owl:onProperty rdf:resource="http://www.opengis.net/ont/geosparql#asWKT"/>
    <owl:onDataRange rdf:resource="https://w3id.org/tern/ontologies/loc/wktLiteral"/>
    <rdf:type rdf:resource="http://www.w3.org/2002/07/owl#Restriction"/>
    <owl:qualifiedCardinality rdf:datatype="http://www.w3.org/2001/XMLSchema#nonNegativeInteger">1</owl:qualifiedCardinality>
  </rdf:Description>
  <rdf:Description rdf:about="https://w3id.org/tern/ontologies/tern/length">
    <rdfs:label>length</rdfs:label>
    <skos:definition>The measurement or extent of something from end to end.</skos:definition>
    <rdf:type rdf:resource="http://www.w3.org/1999/02/22-rdf-syntax-ns#Property"/>
  </rdf:Description>
  <rdf:Description rdf:about="https://w3id.org/tern/ontologies/tern/Sample">
    <rdfs:subClassOf rdf:resource="http://www.w3.org/ns/sosa/Sample"/>
    <rdfs:subClassOf rdf:nodeID="ub1bL752C19"/>
    <rdfs:label>Sample</rdfs:label>
    <rdfs:subClassOf rdf:nodeID="ub1bL762C19"/>
    <skos:definition>*Sample* - Feature which is intended to be representative of a [FeatureOfInterest](http://w3.org/ns/sosa/FeatureOfInterest) on which [Observations](#Observation) may be made.</skos:definition>
    <rdf:type rdf:resource="http://www.w3.org/2002/07/owl#Class"/>
    <rdfs:subClassOf rdf:nodeID="ub1bL757C19"/>
    <rdfs:subClassOf rdf:nodeID="ub1bL767C19"/>
    <rdfs:subClassOf rdf:nodeID="ub1bL772C19"/>
    <rdfs:subClassOf rdf:nodeID="ub1bL782C19"/>
    <rdfs:subClassOf rdf:nodeID="ub1bL777C19"/>
  </rdf:Description>
  <rdf:Description rdf:nodeID="ub1bL193C19">
    <owl:onProperty rdf:resource="http://rs.tdwg.org/dwc/terms/materialSampleID"/>
    <rdf:type rdf:resource="http://www.w3.org/2002/07/owl#Restriction"/>
    <owl:cardinality rdf:datatype="http://www.w3.org/2001/XMLSchema#nonNegativeInteger">1</owl:cardinality>
  </rdf:Description>
  <rdf:Description rdf:nodeID="ub1bL1021C19">
    <rdf:type rdf:resource="http://www.w3.org/2002/07/owl#Restriction"/>
    <owl:onClass rdf:resource="http://www.w3.org/2001/XMLSchema#string"/>
    <owl:onProperty rdf:resource="https://w3id.org/tern/ontologies/tern/siteDescription"/>
    <owl:maxQualifiedCardinality rdf:datatype="http://www.w3.org/2001/XMLSchema#nonNegativeInteger">1</owl:maxQualifiedCardinality>
  </rdf:Description>
  <rdf:Description rdf:nodeID="ub1bL650C19">
    <owl:maxQualifiedCardinality rdf:datatype="http://www.w3.org/2001/XMLSchema#nonNegativeInteger">1</owl:maxQualifiedCardinality>
    <owl:onClass rdf:resource="https://w3id.org/tern/ontologies/tern/Input"/>
    <rdf:type rdf:resource="http://www.w3.org/2002/07/owl#Restriction"/>
    <owl:onProperty rdf:resource="http://www.w3.org/ns/ssn/hasInput"/>
  </rdf:Description>
  <rdf:Description rdf:about="https://w3id.org/tern/ontologies/tern/Radiometer">
    <rdf:type rdf:resource="http://www.w3.org/2002/07/owl#Class"/>
    <rdfs:seeAlso rdf:resource="https://en.wikipedia.org/wiki/Radiometer"/>
    <rdfs:comment>A radiometer or roentgenometer is a device for measuring the radiant flux (power) of electromagnetic radiation. Generally, a radiometer is an infrared radiation detector or an ultraviolet detector.</rdfs:comment>
    <rdfs:label>Radiometer</rdfs:label>
    <rdfs:subClassOf rdf:resource="https://w3id.org/tern/ontologies/tern/RadiationSensor"/>
  </rdf:Description>
  <rdf:Description rdf:nodeID="fe114e3c19c6e4b2e8a8d1297357cbc21b4">
    <rdf:rest rdf:resource="http://www.w3.org/1999/02/22-rdf-syntax-ns#nil"/>
    <rdf:first rdf:resource="http://www.w3.org/2001/XMLSchema#integer"/>
  </rdf:Description>
  <rdf:Description rdf:nodeID="ub1bL1117C19">
    <owl:onProperty rdf:resource="http://www.w3.org/ns/sosa/isSampleOf"/>
    <owl:minQualifiedCardinality rdf:datatype="http://www.w3.org/2001/XMLSchema#nonNegativeInteger">1</owl:minQualifiedCardinality>
    <rdf:type rdf:resource="http://www.w3.org/2002/07/owl#Restriction"/>
    <owl:onClass rdf:resource="https://w3id.org/tern/ontologies/tern/SiteTaxon"/>
  </rdf:Description>
  <rdf:Description rdf:nodeID="ub1bL732C19">
    <owl:cardinality rdf:datatype="http://www.w3.org/2001/XMLSchema#nonNegativeInteger">1</owl:cardinality>
    <rdf:type rdf:resource="http://www.w3.org/2002/07/owl#Restriction"/>
    <owl:onProperty rdf:resource="http://www.w3.org/ns/sosa/isResultOf"/>
  </rdf:Description>
  <rdf:Description rdf:nodeID="ub1bL584C19">
    <owl:qualifiedCardinality rdf:datatype="http://www.w3.org/2001/XMLSchema#nonNegativeInteger">1</owl:qualifiedCardinality>
    <owl:onProperty rdf:resource="http://www.w3.org/ns/sosa/usedProcedure"/>
    <owl:onClass rdf:resource="https://w3id.org/tern/ontologies/tern/Procedure"/>
    <rdf:type rdf:resource="http://www.w3.org/2002/07/owl#Restriction"/>
  </rdf:Description>
  <rdf:Description rdf:about="https://w3id.org/tern/ontologies/tern/hasObservationTheme">
    <rdfs:subPropertyOf rdf:resource="http://www.w3.org/2004/02/skos/core#relatedMatch"/>
    <skos:definition>Link a concept to an observation theme.</skos:definition>
    <rdfs:label>has observation theme</rdfs:label>
    <rdf:type rdf:resource="http://www.w3.org/1999/02/22-rdf-syntax-ns#Property"/>
  </rdf:Description>
  <rdf:Description rdf:about="https://w3id.org/tern/ontologies/tern/isSamplingPointOf">
    <rdf:type rdf:resource="http://www.w3.org/1999/02/22-rdf-syntax-ns#Property"/>
    <rdfs:label>is sampling point of</rdfs:label>
    <skos:definition>Link to the parent of the [SamplingPoint](#SamplingPoint),.</skos:definition>
  </rdf:Description>
  <rdf:Description rdf:nodeID="ub1bL354C19">
    <owl:onClass rdf:resource="http://www.w3.org/2001/XMLSchema#date"/>
    <owl:onProperty rdf:resource="https://w3id.org/tern/ontologies/tern/dateDecommissioned"/>
    <owl:maxQualifiedCardinality rdf:datatype="http://www.w3.org/2001/XMLSchema#nonNegativeInteger">1</owl:maxQualifiedCardinality>
    <rdf:type rdf:resource="http://www.w3.org/2002/07/owl#Restriction"/>
  </rdf:Description>
  <rdf:Description rdf:about="https://w3id.org/tern/ontologies/tern/area">
    <skos:definition>The extent or measurement of a surface or piece of land.</skos:definition>
    <rdf:type rdf:resource="http://www.w3.org/1999/02/22-rdf-syntax-ns#Property"/>
    <rdfs:label>area</rdfs:label>
  </rdf:Description>
  <rdf:Description rdf:nodeID="ub1bL542C19">
    <rdf:type rdf:resource="http://www.w3.org/2002/07/owl#Restriction"/>
    <owl:onClass rdf:resource="https://w3id.org/tern/ontologies/tern/Site"/>
    <owl:onProperty rdf:resource="https://w3id.org/tern/ontologies/tern/site"/>
    <owl:maxQualifiedCardinality rdf:datatype="http://www.w3.org/2001/XMLSchema#nonNegativeInteger">1</owl:maxQualifiedCardinality>
  </rdf:Description>
  <rdf:Description rdf:nodeID="ub1bL800C19">
    <owl:onClass rdf:resource="https://w3id.org/tern/ontologies/tern/Procedure"/>
    <owl:onProperty rdf:resource="http://www.w3.org/ns/ssn/implements"/>
    <rdf:type rdf:resource="http://www.w3.org/2002/07/owl#Restriction"/>
    <owl:minQualifiedCardinality rdf:datatype="http://www.w3.org/2001/XMLSchema#nonNegativeInteger">1</owl:minQualifiedCardinality>
  </rdf:Description>
  <rdf:Description rdf:about="https://w3id.org/tern/ontologies/tern/AffiliateSuperSite">
    <rdf:type rdf:resource="http://www.w3.org/2002/07/owl#Class"/>
    <rdfs:subClassOf rdf:resource="https://w3id.org/tern/ontologies/tern/SuperSite"/>
    <rdfs:seeAlso rdf:resource="https://supersites.tern.org.au/"/>
    <rdfs:label>Affiliate SuperSite</rdfs:label>
  </rdf:Description>
  <rdf:Description rdf:nodeID="ub1bL560C19">
    <rdf:type rdf:resource="http://www.w3.org/2002/07/owl#Restriction"/>
    <owl:qualifiedCardinality rdf:datatype="http://www.w3.org/2001/XMLSchema#nonNegativeInteger">1</owl:qualifiedCardinality>
    <owl:onProperty rdf:resource="http://www.w3.org/2000/01/rdf-schema#label"/>
    <owl:onClass rdf:resource="http://www.w3.org/2001/XMLSchema#string"/>
  </rdf:Description>
  <rdf:Description rdf:nodeID="ub1bL326C19">
    <owl:onProperty rdf:resource="http://www.w3.org/ns/sosa/isFeatureOfInterestOf"/>
    <rdf:type rdf:resource="http://www.w3.org/2002/07/owl#Restriction"/>
    <owl:onClass rdf:resource="https://w3id.org/tern/ontologies/tern/Observation"/>
    <owl:minQualifiedCardinality rdf:datatype="http://www.w3.org/2001/XMLSchema#nonNegativeInteger">1</owl:minQualifiedCardinality>
  </rdf:Description>
  <rdf:Description rdf:nodeID="ub1bL829C19">
    <owl:qualifiedCardinality rdf:datatype="http://www.w3.org/2001/XMLSchema#nonNegativeInteger">1</owl:qualifiedCardinality>
    <owl:onProperty rdf:resource="http://www.w3.org/2000/01/rdf-schema#label"/>
    <rdf:type rdf:resource="http://www.w3.org/2002/07/owl#Restriction"/>
    <owl:onClass rdf:resource="http://www.w3.org/2001/XMLSchema#string"/>
  </rdf:Description>
  <rdf:Description rdf:nodeID="ub1bL924C19">
    <owl:onProperty rdf:resource="http://www.w3.org/ns/sosa/madeObservation"/>
    <owl:allValuesFrom rdf:resource="https://w3id.org/tern/ontologies/tern/Observation"/>
    <rdf:type rdf:resource="http://www.w3.org/2002/07/owl#Restriction"/>
  </rdf:Description>
  <rdf:Description rdf:nodeID="ub1bL1111C19">
    <owl:onProperty rdf:resource="http://www.w3.org/ns/sosa/isSampleOf"/>
    <owl:onClass rdf:resource="https://w3id.org/tern/ontologies/tern/SiteStratum"/>
    <rdf:type rdf:resource="http://www.w3.org/2002/07/owl#Restriction"/>
    <owl:minQualifiedCardinality rdf:datatype="http://www.w3.org/2001/XMLSchema#nonNegativeInteger">1</owl:minQualifiedCardinality>
  </rdf:Description>
  <rdf:Description rdf:nodeID="ub1bL360C19">
    <owl:onProperty rdf:resource="https://w3id.org/tern/ontologies/tern/fluxnetID"/>
    <rdf:type rdf:resource="http://www.w3.org/2002/07/owl#Restriction"/>
    <owl:onClass rdf:resource="http://www.w3.org/2001/XMLSchema#string"/>
    <owl:maxQualifiedCardinality rdf:datatype="http://www.w3.org/2001/XMLSchema#nonNegativeInteger">1</owl:maxQualifiedCardinality>
  </rdf:Description>
  <rdf:Description rdf:nodeID="ub1bL301C19">
    <owl:onClass rdf:resource="http://qudt.org/schema/qudt/Unit"/>
    <rdf:type rdf:resource="http://www.w3.org/2002/07/owl#Restriction"/>
    <owl:onProperty rdf:resource="http://linked.data.gov.au/def/datatype/unit"/>
    <owl:qualifiedCardinality rdf:datatype="http://www.w3.org/2001/XMLSchema#nonNegativeInteger">1</owl:qualifiedCardinality>
  </rdf:Description>
  <rdf:Description rdf:nodeID="ub1bL680C19">
    <owl:onClass rdf:resource="https://w3id.org/tern/ontologies/tern/Result"/>
    <owl:qualifiedCardinality rdf:datatype="http://www.w3.org/2001/XMLSchema#nonNegativeInteger">1</owl:qualifiedCardinality>
    <rdf:type rdf:resource="http://www.w3.org/2002/07/owl#Restriction"/>
    <owl:onProperty rdf:resource="http://www.w3.org/ns/sosa/hasResult"/>
  </rdf:Description>
  <rdf:Description rdf:nodeID="ub1bL757C19">
    <owl:onProperty rdf:resource="http://www.w3.org/ns/prov#wasAttributedTo"/>
    <owl:allValuesFrom rdf:resource="https://w3id.org/tern/ontologies/org/Person"/>
    <rdf:type rdf:resource="http://www.w3.org/2002/07/owl#Restriction"/>
  </rdf:Description>
  <rdf:Description rdf:nodeID="ub1bL1160C19">
    <owl:allValuesFrom rdf:resource="https://w3id.org/tern/ontologies/tern/CollectedSample"/>
    <rdf:type rdf:resource="http://www.w3.org/2002/07/owl#Restriction"/>
    <owl:onProperty rdf:resource="http://www.w3.org/ns/sosa/hasSample"/>
  </rdf:Description>
  <rdf:Description rdf:nodeID="fe114e3c19c6e4b2e8a8d1297357cbc21b6">
    <rdf:first rdf:resource="http://www.w3.org/2001/XMLSchema#anyURI"/>
    <rdf:rest rdf:resource="http://www.w3.org/1999/02/22-rdf-syntax-ns#nil"/>
  </rdf:Description>
  <rdf:Description rdf:nodeID="ub1bL625C19">
    <owl:allValuesFrom rdf:resource="https://w3id.org/tern/ontologies/tern/Platform"/>
    <owl:onProperty rdf:resource="http://www.w3.org/ns/sosa/isHostedBy"/>
    <rdf:type rdf:resource="http://www.w3.org/2002/07/owl#Restriction"/>
  </rdf:Description>
  <rdf:Description rdf:nodeID="ub1bL462C19">
    <owl:maxQualifiedCardinality rdf:datatype="http://www.w3.org/2001/XMLSchema#nonNegativeInteger">1</owl:maxQualifiedCardinality>
    <rdf:type rdf:resource="http://www.w3.org/2002/07/owl#Restriction"/>
    <owl:onProperty rdf:resource="https://w3id.org/tern/ontologies/tern/scope"/>
    <owl:onDataRange rdf:resource="http://www.w3.org/2001/XMLSchema#string"/>
  </rdf:Description>
  <rdf:Description rdf:about="https://w3id.org/tern/ontologies/tern/hasSamplingPoint">
    <skos:definition>Link to a [SamplingPoint](#SamplingPoint).</skos:definition>
    <rdfs:range rdf:resource="https://w3id.org/tern/ontologies/tern/SamplingPoint"/>
    <rdf:type rdf:resource="http://www.w3.org/1999/02/22-rdf-syntax-ns#Property"/>
    <rdfs:label>has sampling point</rdfs:label>
  </rdf:Description>
  <rdf:Description rdf:about="https://w3id.org/tern/ontologies/tern/transectEndPoint">
    <rdf:type rdf:resource="http://www.w3.org/1999/02/22-rdf-syntax-ns#Property"/>
    <rdfs:label>transect end point</rdfs:label>
    <skos:definition>Link to a [tern-loc:Point](https://w3id.org/tern/ontologies/loc/Point) representing the end of the transect.</skos:definition>
  </rdf:Description>
  <rdf:Description rdf:about="https://w3id.org/tern/ontologies/tern/EnvironmentalCharacteristic">
    <rdfs:label>Environmental Characteristic</rdfs:label>
    <rdfs:subClassOf rdf:nodeID="ub1bL326C19"/>
    <rdfs:subClassOf rdf:resource="http://www.w3.org/ns/sosa/FeatureOfInterest"/>
    <rdf:type rdf:resource="http://www.w3.org/2002/07/owl#Class"/>
    <skos:definition>The environment characteristics  is a [FeatureOfInterest](http://w3.org/ns/sosa/FeatureOfInterest) of a location where [Observations](#Observation) such as the annual mean rainfall or the annual mean temperature are made.</skos:definition>
  </rdf:Description>
  <rdf:Description rdf:nodeID="ub1bL491C19">
    <owl:allValuesFrom rdf:nodeID="ub1bL493C25"/>
    <owl:onProperty rdf:resource="https://w3id.org/tern/ontologies/tern/globalVocabulary"/>
    <rdf:type rdf:resource="http://www.w3.org/2002/07/owl#Restriction"/>
  </rdf:Description>
  <rdf:Description rdf:nodeID="ub1bL125C23">
    <schema:name>CSIRO</schema:name>
    <rdf:type rdf:resource="http://schema.org/Organization"/>
    <schema:identifier rdf:resource="http://catalogue.linked.data.gov.au/def/csiro"/>
  </rdf:Description>
  <rdf:Description rdf:nodeID="ub1bL590C19">
    <owl:qualifiedCardinality rdf:datatype="http://www.w3.org/2001/XMLSchema#nonNegativeInteger">1</owl:qualifiedCardinality>
    <owl:onProperty rdf:resource="http://www.w3.org/ns/sosa/resultTime"/>
    <owl:onDataRange rdf:resource="http://www.w3.org/2001/XMLSchema#dateTime"/>
    <rdf:type rdf:resource="http://www.w3.org/2002/07/owl#Restriction"/>
  </rdf:Description>
  <rdf:Description rdf:about="https://w3id.org/tern/ontologies/tern/PhenologyCamera">
    <skos:altLabel>Phenocam</skos:altLabel>
    <skos:definition>A "phenocam" is a digital camera capturing time-lapse images of foliage which can be used to generate quantitative measures of plant phenology. Over time, these data provide a near-continuous visual record of canopy change and environmental conditions.</skos:definition>
    <rdf:type rdf:resource="http://www.w3.org/2002/07/owl#Class"/>
    <rdfs:label>Phenology Camera</rdfs:label>
    <rdfs:subClassOf rdf:nodeID="ub1bL625C19"/>
    <rdfs:subClassOf rdf:nodeID="ub1bL615C19"/>
    <rdfs:seeAlso rdf:resource="https://www.neonscience.org/data-collection/phenocams"/>
    <skos:altLabel>Phenocamera</skos:altLabel>
    <rdfs:subClassOf rdf:nodeID="ub1bL620C19"/>
    <rdfs:subClassOf rdf:resource="https://w3id.org/tern/ontologies/tern/Sampler"/>
  </rdf:Description>
  <rdf:Description rdf:nodeID="fe114e3c19c6e4b2e8a8d1297357cbc21b8">
    <rdf:rest rdf:nodeID="fe114e3c19c6e4b2e8a8d1297357cbc21b9"/>
    <rdf:first rdf:resource="http://www.w3.org/2004/02/skos/core#Collection"/>
  </rdf:Description>
  <rdf:Description rdf:about="https://w3id.org/tern/ontologies/tern/width">
    <rdfs:label>width</rdfs:label>
    <skos:definition>The measurement or extent of something from side to side.</skos:definition>
    <rdf:type rdf:resource="http://www.w3.org/1999/02/22-rdf-syntax-ns#Property"/>
  </rdf:Description>
  <rdf:Description rdf:about="https://w3id.org/tern/ontologies/tern/CosmOzStation">
    <rdf:type rdf:resource="http://www.w3.org/2002/07/owl#Class"/>
    <rdfs:label>CosmOz Station</rdfs:label>
    <rdfs:seeAlso rdf:resource="https://cosmoz.csiro.au"/>
    <rdfs:subClassOf rdf:resource="https://w3id.org/tern/ontologies/tern/FixedPlatform"/>
    <skos:definition>CosmOz is the Australian Cosmic-Ray Neutron Soil Moisture Monitoring Network

Beginning in October 2010, CSIRO Land and Water installed cosmic-ray probes at a number of locations around Australia to form the inaugural CosmOz network. These sites were established at instrumented research sites operated by CSIRO and University collaborators to test and validate the operation of this new technology.

These novel probes use cosmic rays originating from outer space to measure average soil moisture over an area of about 30 hectares to depths in the soil of between 10 to 50 cm. This constitutes a quantum leap over conventional on-ground soil moisture sensing technology that can only measure soil moisture content within small volumes of soil.

Each system is comprised of a data logger, neutron detector, satellite telemetry, tipping bucket rain gauge, temperature humidity and pressure sensors and three surface moisture (TDR) probes. The system requires minimal maintenance and is powered by a solar charging system. The entire system is installed on a single mast. Data is logged and transmitted every 60 minutes to the CosmOz database.</skos:definition>
  </rdf:Description>
  <rdf:Description rdf:about="http://rs.tdwg.org/dwc/terms/materialSampleID">
    <rdf:type rdf:resource="http://www.w3.org/1999/02/22-rdf-syntax-ns#Property"/>
    <rdfs:isDefinedBy rdf:resource="http://rs.tdwg.org/dwc/terms/"/>
    <skos:example>06809dc5-f143-459a-be1a-6f03e63fc083</skos:example>
    <rdfs:label>material sample ID</rdfs:label>
    <rdfs:comment>An identifier for the MaterialSample (as opposed to a particular digital record of the material sample). In the absence of a persistent global unique identifier, construct one from a combination of identifiers in the record that will most closely make the materialSampleID globally unique.</rdfs:comment>
  </rdf:Description>
  <rdf:Description rdf:nodeID="ub1bL444C19">
    <rdf:type rdf:resource="http://www.w3.org/2002/07/owl#Restriction"/>
    <owl:onDataRange rdf:resource="http://www.w3.org/2001/XMLSchema#string"/>
    <owl:maxQualifiedCardinality rdf:datatype="http://www.w3.org/2001/XMLSchema#nonNegativeInteger">1</owl:maxQualifiedCardinality>
    <owl:onProperty rdf:resource="https://w3id.org/tern/ontologies/tern/equipment"/>
  </rdf:Description>
  <rdf:Description rdf:about="https://w3id.org/tern/ontologies/tern/CollectedSample">
    <skos:example>Soil sample or plant sample from the field.</skos:example>
    <rdfs:subClassOf rdf:resource="https://w3id.org/tern/ontologies/tern/Sample"/>
    <rdfs:subClassOf rdf:resource="http://rs.tdwg.org/dwc/terms/MaterialSample"/>
    <rdf:type rdf:resource="http://www.w3.org/2002/07/owl#Class"/>
    <rdfs:subClassOf rdf:nodeID="ub1bL198C19"/>
    <skos:definition>A [Collected Sample](#CollectedSample) is a [Sample](#Sample) which has been collected in the field. </skos:definition>
    <rdfs:label>Collected Sample</rdfs:label>
    <rdfs:subClassOf rdf:nodeID="ub1bL193C19"/>
  </rdf:Description>
  <rdf:Description rdf:about="https://w3id.org/tern/ontologies/tern/AusPlotsSite">
    <rdf:type rdf:resource="http://www.w3.org/2002/07/owl#Class"/>
    <rdfs:label>AusPlots Site</rdfs:label>
    <rdfs:subClassOf rdf:resource="https://w3id.org/tern/ontologies/tern/Site"/>
  </rdf:Description>
  <rdf:Description rdf:nodeID="ub1bL992C19">
    <rdf:type rdf:resource="http://www.w3.org/2002/07/owl#Restriction"/>
    <owl:maxCardinality rdf:datatype="http://www.w3.org/2001/XMLSchema#nonNegativeInteger">1</owl:maxCardinality>
    <owl:onProperty rdf:resource="https://w3id.org/tern/ontologies/tern/hasEnvironmentalCharacteristic"/>
  </rdf:Description>
  <rdf:Description rdf:about="https://w3id.org/tern/ontologies/tern/isGlobalMatchOf">
    <rdfs:subPropertyOf rdf:resource="http://www.w3.org/2004/02/skos/core#exactMatch"/>
    <rdf:type rdf:resource="http://www.w3.org/1999/02/22-rdf-syntax-ns#Property"/>
    <skos:definition>Link an upper concept to a concept (in the closed system).</skos:definition>
    <rdfs:label>is global match of</rdfs:label>
  </rdf:Description>
  <rdf:Description rdf:about="https://w3id.org/tern/ontologies/tern/Parameter">
    <rdfs:subClassOf rdf:resource="http://www.w3.org/2004/02/skos/core#Concept"/>
    <skos:definition>A [FeatureOfInterest's](http://w3.org/ns/sosa/FeatureOfInterest) property or characteristic which an [Observation](#Observation) is measuring using some [Procedure](#Procedure).</skos:definition>
    <rdf:type rdf:resource="http://www.w3.org/2002/07/owl#Class"/>
    <rdfs:label>Parameter</rdfs:label>
  </rdf:Description>
  <rdf:Description rdf:nodeID="ub1bL532C19">
    <owl:onProperty rdf:resource="http://www.w3.org/2000/01/rdf-schema#comment"/>
    <owl:allValuesFrom rdf:resource="http://www.w3.org/2001/XMLSchema#string"/>
    <rdf:type rdf:resource="http://www.w3.org/2002/07/owl#Restriction"/>
  </rdf:Description>
  <rdf:Description rdf:nodeID="ub1bL656C19">
    <owl:onProperty rdf:resource="http://www.w3.org/1999/02/22-rdf-syntax-ns#value"/>
    <rdf:type rdf:resource="http://www.w3.org/2002/07/owl#Restriction"/>
    <owl:onClass rdf:resource="https://w3id.org/tern/ontologies/tern/Method"/>
    <owl:qualifiedCardinality rdf:datatype="http://www.w3.org/2001/XMLSchema#nonNegativeInteger">1</owl:qualifiedCardinality>
  </rdf:Description>
  <rdf:Description rdf:nodeID="ub1bL795C19">
    <owl:allValuesFrom rdf:resource="https://w3id.org/tern/ontologies/tern/Sampling"/>
    <owl:onProperty rdf:resource="http://www.w3.org/ns/sosa/madeSampling"/>
    <rdf:type rdf:resource="http://www.w3.org/2002/07/owl#Restriction"/>
  </rdf:Description>
  <rdf:Description rdf:nodeID="ub1bL1027C19">
    <owl:onProperty rdf:resource="https://w3id.org/tern/ontologies/tern/siteShape"/>
    <rdf:type rdf:resource="http://www.w3.org/2002/07/owl#Restriction"/>
    <owl:onClass rdf:resource="http://www.w3.org/2004/02/skos/core#Concept"/>
    <owl:maxQualifiedCardinality rdf:datatype="http://www.w3.org/2001/XMLSchema#nonNegativeInteger">1</owl:maxQualifiedCardinality>
  </rdf:Description>
  <rdf:Description rdf:nodeID="ub1bL721C19">
    <rdf:type rdf:resource="http://www.w3.org/2002/07/owl#Restriction"/>
    <owl:onProperty rdf:resource="http://www.w3.org/ns/sosa/isResultOf"/>
    <owl:allValuesFrom rdf:nodeID="ub1bL723C25"/>
  </rdf:Description>
  <rdf:Description rdf:about="https://w3id.org/tern/ontologies/tern/SiteTaxon">
    <rdfs:subClassOf rdf:resource="https://w3id.org/tern/ontologies/tern/Sample"/>
    <rdf:type rdf:resource="http://www.w3.org/2002/07/owl#Class"/>
    <rdfs:label>Site Taxon</rdfs:label>
    <rdfs:subClassOf rdf:nodeID="ub1bL1134C19"/>
  </rdf:Description>
  <rdf:Description rdf:nodeID="ub1bL1253C19">
    <owl:qualifiedCardinality rdf:datatype="http://www.w3.org/2001/XMLSchema#nonNegativeInteger">1</owl:qualifiedCardinality>
    <owl:onProperty rdf:resource="http://www.opengis.net/ont/geosparql#hasGeometry"/>
    <rdf:type rdf:resource="http://www.w3.org/2002/07/owl#Restriction"/>
    <owl:onClass rdf:resource="https://w3id.org/tern/ontologies/loc/LineString"/>
  </rdf:Description>
  <rdf:Description rdf:nodeID="ub1bL946C19">
    <rdf:type rdf:resource="http://www.w3.org/2002/07/owl#Restriction"/>
    <owl:allValuesFrom rdf:resource="https://w3id.org/tern/ontologies/tern/CollectedSample"/>
    <owl:onProperty rdf:resource="http://www.w3.org/ns/sosa/hasSample"/>
  </rdf:Description>
  <rdf:Description rdf:nodeID="ub1bL1150C19">
    <owl:onProperty rdf:resource="http://www.w3.org/ns/prov#startedAtTime"/>
    <rdf:type rdf:resource="http://www.w3.org/2002/07/owl#Restriction"/>
    <owl:allValuesFrom rdf:resource="http://www.w3.org/2001/XMLSchema#dateTime"/>
  </rdf:Description>
  <rdf:Description rdf:nodeID="ub1bL1045C19">
    <owl:onClass rdf:resource="https://w3id.org/tern/ontologies/loc/Polygon"/>
    <owl:maxQualifiedCardinality rdf:datatype="http://www.w3.org/2001/XMLSchema#nonNegativeInteger">1</owl:maxQualifiedCardinality>
    <rdf:type rdf:resource="http://www.w3.org/2002/07/owl#Restriction"/>
    <owl:onProperty rdf:resource="https://w3id.org/tern/ontologies/tern/polygon"/>
  </rdf:Description>
  <rdf:Description rdf:about="https://w3id.org/tern/ontologies/tern/cardinalDirection">
    <skos:definition>The cardinal direction of the *thing* represented as a string and expressed by cardinal and intercardinal points. </skos:definition>
    <skos:example>NNE, W, SE, etc.</skos:example>
    <rdfs:label>cardinal direction</rdfs:label>
    <rdf:type rdf:resource="http://www.w3.org/1999/02/22-rdf-syntax-ns#Property"/>
    <rdfs:range rdf:resource="http://www.w3.org/2001/XMLSchema#string"/>
  </rdf:Description>
  <rdf:Description rdf:about="https://w3id.org/tern/ontologies/tern/Procedure">
    <rdfs:label>Procedure</rdfs:label>
    <skos:scopeNote>[Input](#Input) can be used to capture any input values for a procedure, such as the input value of the basal wedge to estimate the basal area per hectare.</skos:scopeNote>
    <skos:definition>*Procedure* - A workflow, protocol, plan, algorithm, or computational method specifying how to make an [Observation](#Observation), create a [Sample](#Sample), or make a change to the state of the world (via an [Actuator](http://w3.org/ns/sosa/Actuator). A [Procedure](#Procedure) is re-usable, and might be involved in many [Observations](#Observation), [Samplings](#Samplings), or [Actuations](http://w3.org/ns/sosa/Actuation). it explains the steps to be carried out to arrive at reproducible [Results](#Result).</skos:definition>
    <rdfs:subClassOf rdf:nodeID="ub1bL645C19"/>
    <rdf:type rdf:resource="http://www.w3.org/2002/07/owl#Class"/>
    <rdfs:subClassOf rdf:nodeID="ub1bL650C19"/>
    <rdfs:subClassOf rdf:nodeID="ub1bL656C19"/>
    <rdfs:subClassOf rdf:resource="http://www.w3.org/ns/sosa/Procedure"/>
  </rdf:Description>
  <rdf:Description rdf:about="https://w3id.org/tern/ontologies/tern/instructions">
    <rdf:type rdf:resource="http://www.w3.org/2002/07/owl#DatatypeProperty"/>
    <skos:definition>Describe the instructions of the procedure/method.</skos:definition>
    <rdfs:label>instructions</rdfs:label>
    <rdfs:range rdf:resource="http://www.w3.org/2001/XMLSchema#string"/>
  </rdf:Description>
  <rdf:Description rdf:nodeID="ub1bL503C19">
    <owl:cardinality rdf:datatype="http://www.w3.org/2001/XMLSchema#nonNegativeInteger">1</owl:cardinality>
    <rdf:type rdf:resource="http://www.w3.org/2002/07/owl#Restriction"/>
    <owl:onProperty rdf:resource="http://linked.data.gov.au/def/datatype/vocabulary"/>
  </rdf:Description>
  <rdf:Description rdf:about="https://w3id.org/tern/ontologies/tern/Instrument">
    <rdf:type rdf:resource="http://www.w3.org/2002/07/owl#Class"/>
    <rdfs:label>Instrument</rdfs:label>
    <skos:definition>A thing to measure or produce a sample.</skos:definition>
    <rdfs:subClassOf rdf:resource="http://www.w3.org/ns/ssn/System"/>
  </rdf:Description>
  <rdf:Description rdf:about="http://linked.data.gov.au/def/datatype/Concept">
    <rdfs:subClassOf rdf:resource="https://w3id.org/tern/ontologies/tern/Result"/>
    <rdfs:subClassOf rdf:nodeID="ub1bL49C19"/>
    <rdf:type rdf:resource="http://www.w3.org/2002/07/owl#Class"/>
    <rdfs:subClassOf rdf:nodeID="ub1bL44C19"/>
  </rdf:Description>
  <rdf:Description rdf:about="https://w3id.org/tern/ontologies/tern/OEHSite">
    <rdf:type rdf:resource="http://www.w3.org/2002/07/owl#Class"/>
    <rdfs:label>OEH Site</rdfs:label>
    <rdfs:subClassOf rdf:resource="https://w3id.org/tern/ontologies/tern/Site"/>
  </rdf:Description>
  <rdf:Description rdf:nodeID="ub1bL121C19">
    <schema:memberOf rdf:nodeID="ub1bL125C23"/>
    <schema:email>simon.cox@csiro.au</schema:email>
    <rdf:type rdf:resource="http://schema.org/Person"/>
    <schema:identifier rdf:resource="https://orcid.org/0000-0002-3884-3420"/>
    <schema:name>Simon J.D.Cox</schema:name>
  </rdf:Description>
  <rdf:Description rdf:nodeID="ub1bL951C19">
    <owl:onProperty rdf:resource="https://w3id.org/tern/ontologies/tern/locationProcedure"/>
    <rdf:type rdf:resource="http://www.w3.org/2002/07/owl#Restriction"/>
    <owl:allValuesFrom rdf:resource="https://w3id.org/tern/ontologies/tern/Procedure"/>
  </rdf:Description>
  <rdf:Description rdf:nodeID="ub1bL427C19">
    <owl:onProperty rdf:resource="http://purl.org/dc/terms/source"/>
    <rdf:type rdf:resource="http://www.w3.org/2002/07/owl#Restriction"/>
    <owl:allValuesFrom rdf:nodeID="ub1bL429C25"/>
  </rdf:Description>
  <rdf:Description rdf:nodeID="fe114e3c19c6e4b2e8a8d1297357cbc21b17">
    <rdf:rest rdf:resource="http://www.w3.org/1999/02/22-rdf-syntax-ns#nil"/>
    <rdf:first rdf:resource="http://www.w3.org/2001/XMLSchema#int"/>
  </rdf:Description>
  <rdf:Description rdf:about="https://w3id.org/tern/ontologies/tern/DerivedObservation">
    <rdfs:label>Derived Observation</rdfs:label>
    <rdf:type rdf:resource="http://www.w3.org/2002/07/owl#Class"/>
    <rdfs:subClassOf rdf:resource="https://w3id.org/tern/ontologies/tern/Observation"/>
    <skos:definition>A derived observation.</skos:definition>
  </rdf:Description>
  <rdf:Description rdf:about="https://w3id.org/tern/ontologies/tern/Method">
    <rdfs:subClassOf rdf:nodeID="ub1bL450C19"/>
    <rdfs:subClassOf rdf:nodeID="ub1bL438C19"/>
    <rdfs:subClassOf rdf:nodeID="ub1bL456C19"/>
    <rdfs:seeAlso rdf:resource="https://3yn1j14c4twk1bmdg82226en-wpengine.netdna-ssl.com/wp-content/uploads/2016/08/iso-9001-procedure.pdf"/>
    <rdfs:label>Method</rdfs:label>
    <rdfs:subClassOf rdf:resource="http://www.w3.org/2004/02/skos/core#Concept"/>
    <rdfs:subClassOf rdf:nodeID="ub1bL427C19"/>
    <rdfs:seeAlso rdf:resource="https://the9000store.com/iso-9001-2015-requirements/iso-9001-2015-context-of-the-organization/processes-procedures-work-instructions/"/>
    <rdfs:subClassOf rdf:nodeID="ub1bL468C19"/>
    <rdf:type rdf:resource="http://www.w3.org/2002/07/owl#Class"/>
    <rdfs:subClassOf rdf:nodeID="ub1bL462C19"/>
    <skos:definition>A Method describes in detailed steps how a workflow, protocol, plan or algorithm is carried out to make an [Observation](#Observation) or a [Sample](#Sample). It explains the steps to be carried out to arrive at reproducible [Result](#Result).</skos:definition>
    <rdfs:subClassOf rdf:nodeID="ub1bL444C19"/>
  </rdf:Description>
  <rdf:Description rdf:nodeID="ub1bL864C19">
    <owl:onProperty rdf:resource="https://w3id.org/tern/ontologies/loc/altitude"/>
    <owl:onClass rdf:resource="http://linked.data.gov.au/def/datatype/QuantitativeMeasure"/>
    <rdf:type rdf:resource="http://www.w3.org/2002/07/owl#Restriction"/>
    <owl:maxQualifiedCardinality rdf:datatype="http://www.w3.org/2001/XMLSchema#nonNegativeInteger">1</owl:maxQualifiedCardinality>
  </rdf:Description>
  <rdf:Description rdf:nodeID="ub1bL841C19">
    <owl:onClass rdf:resource="https://w3id.org/tern/ontologies/tern/Sample"/>
    <rdf:type rdf:resource="http://www.w3.org/2002/07/owl#Restriction"/>
    <owl:qualifiedCardinality rdf:datatype="http://www.w3.org/2001/XMLSchema#nonNegativeInteger">1</owl:qualifiedCardinality>
    <owl:onProperty rdf:resource="http://www.w3.org/ns/sosa/hasResult"/>
  </rdf:Description>
  <rdf:Description rdf:nodeID="ub1bL1062C19">
    <owl:qualifiedCardinality rdf:datatype="http://www.w3.org/2001/XMLSchema#nonNegativeInteger">1</owl:qualifiedCardinality>
    <owl:onProperty rdf:resource="https://w3id.org/tern/ontologies/tern/dateCommissioned"/>
    <rdf:type rdf:resource="http://www.w3.org/2002/07/owl#Restriction"/>
    <owl:onClass rdf:resource="http://www.w3.org/2001/XMLSchema#date"/>
  </rdf:Description>
  <rdf:Description rdf:nodeID="ub1bL772C19">
    <rdf:type rdf:resource="http://www.w3.org/2002/07/owl#Restriction"/>
    <owl:allValuesFrom rdf:resource="https://w3id.org/tern/ontologies/tern/Sample"/>
    <owl:onProperty rdf:resource="http://www.w3.org/ns/sosa/isSampleOf"/>
  </rdf:Description>
  <rdf:Description rdf:nodeID="ub1bL1265C19">
    <owl:qualifiedCardinality rdf:datatype="http://www.w3.org/2001/XMLSchema#nonNegativeInteger">1</owl:qualifiedCardinality>
    <rdf:type rdf:resource="http://www.w3.org/2002/07/owl#Restriction"/>
    <owl:onProperty rdf:resource="https://w3id.org/tern/ontologies/tern/transectStartPoint"/>
    <owl:onClass rdf:resource="https://w3id.org/tern/ontologies/loc/Point"/>
  </rdf:Description>
  <rdf:Description rdf:about="https://w3id.org/tern/ontologies/tern/MobilePlatform">
    <rdfs:subClassOf rdf:resource="https://w3id.org/tern/ontologies/tern/Platform"/>
    <rdfs:label>Mobile Platform</rdfs:label>
    <rdf:type rdf:resource="http://www.w3.org/2002/07/owl#Class"/>
    <skos:definition>A moving mobile platform on land, in water or in space.</skos:definition>
  </rdf:Description>
  <rdf:Description rdf:about="https://w3id.org/tern/ontologies/tern/CategoricalValue">
    <skos:definition>A [Categorical Value](#CategoricalValue) to categorise some [FeatureOfInterest](http://w3.org/ns/sosa/FeatureOfInterest)</skos:definition>
    <rdfs:subClassOf rdf:resource="http://www.w3.org/2004/02/skos/core#Concept"/>
    <rdfs:label>Categorical Value</rdfs:label>
    <rdf:type rdf:resource="http://www.w3.org/2002/07/owl#Class"/>
  </rdf:Description>
  <rdf:Description rdf:about="https://w3id.org/tern/ontologies/tern/polygon">
    <skos:definition>The polygon of the subject.</skos:definition>
    <rdfs:label>polygon</rdfs:label>
    <rdf:type rdf:resource="http://www.w3.org/1999/02/22-rdf-syntax-ns#Property"/>
    <rdfs:subPropertyOf rdf:resource="http://www.opengis.net/ont/geosparql#hasGeometry"/>
    <rdfs:range rdf:resource="https://w3id.org/tern/ontologies/loc/Polygon"/>
  </rdf:Description>
  <rdf:Description rdf:nodeID="fe114e3c19c6e4b2e8a8d1297357cbc21b19">
    <rdf:first rdf:resource="http://www.w3.org/2001/XMLSchema#int"/>
    <rdf:rest rdf:resource="http://www.w3.org/1999/02/22-rdf-syntax-ns#nil"/>
  </rdf:Description>
  <rdf:Description rdf:nodeID="ub1bL1015C19">
    <owl:maxQualifiedCardinality rdf:datatype="http://www.w3.org/2001/XMLSchema#nonNegativeInteger">1</owl:maxQualifiedCardinality>
    <owl:onProperty rdf:resource="https://w3id.org/tern/ontologies/tern/locationDescription"/>
    <rdf:type rdf:resource="http://www.w3.org/2002/07/owl#Restriction"/>
    <owl:onClass rdf:resource="http://www.w3.org/2001/XMLSchema#string"/>
  </rdf:Description>
  <rdf:Description rdf:nodeID="ub1bL1145C19">
    <owl:allValuesFrom rdf:resource="http://www.w3.org/2001/XMLSchema#dateTime"/>
    <owl:onProperty rdf:resource="http://www.w3.org/ns/prov#endedAtTime"/>
    <rdf:type rdf:resource="http://www.w3.org/2002/07/owl#Restriction"/>
  </rdf:Description>
  <rdf:Description rdf:nodeID="ub1bL987C19">
    <owl:onProperty rdf:resource="http://www.w3.org/ns/prov#generatedAtTime"/>
    <rdf:type rdf:resource="http://www.w3.org/2002/07/owl#Restriction"/>
    <owl:maxCardinality rdf:datatype="http://www.w3.org/2001/XMLSchema#nonNegativeInteger">1</owl:maxCardinality>
  </rdf:Description>
  <rdf:Description rdf:nodeID="ub1bL372C19">
    <owl:qualifiedCardinality rdf:datatype="http://www.w3.org/2001/XMLSchema#nonNegativeInteger">1</owl:qualifiedCardinality>
    <owl:onProperty rdf:resource="https://w3id.org/tern/ontologies/tern/dateCommissioned"/>
    <rdf:type rdf:resource="http://www.w3.org/2002/07/owl#Restriction"/>
    <owl:onClass rdf:resource="http://www.w3.org/2001/XMLSchema#date"/>
  </rdf:Description>
  <rdf:Description rdf:nodeID="ub1bL280C19">
    <owl:allValuesFrom rdf:nodeID="ub1bL282C25"/>
    <owl:onProperty rdf:resource="https://w3id.org/tern/ontologies/tern/width"/>
    <rdf:type rdf:resource="http://www.w3.org/2002/07/owl#Restriction"/>
  </rdf:Description>
  <rdf:Description rdf:nodeID="ub1bL513C19">
    <rdf:type rdf:resource="http://www.w3.org/2002/07/owl#Restriction"/>
    <owl:onClass rdf:resource="http://www.w3.org/2004/02/skos/core#Concept"/>
    <owl:maxQualifiedCardinality rdf:datatype="http://www.w3.org/2001/XMLSchema#nonNegativeInteger">1</owl:maxQualifiedCardinality>
    <owl:onProperty rdf:resource="https://w3id.org/tern/ontologies/tern/globalValue"/>
  </rdf:Description>
  <rdf:Description rdf:nodeID="ub1bL620C19">
    <owl:onProperty rdf:resource="http://www.w3.org/2000/01/rdf-schema#label"/>
    <rdf:type rdf:resource="http://www.w3.org/2002/07/owl#Restriction"/>
    <owl:allValuesFrom rdf:resource="http://www.w3.org/2001/XMLSchema#string"/>
  </rdf:Description>
  <rdf:Description rdf:nodeID="ub1bL566C19">
    <owl:onClass rdf:resource="http://www.w3.org/2006/time#Instant"/>
    <rdf:type rdf:resource="http://www.w3.org/2002/07/owl#Restriction"/>
    <owl:qualifiedCardinality rdf:datatype="http://www.w3.org/2001/XMLSchema#nonNegativeInteger">1</owl:qualifiedCardinality>
    <owl:onProperty rdf:resource="http://www.w3.org/ns/sosa/phenomenonTime"/>
  </rdf:Description>
  <rdf:Description rdf:about="http://linked.data.gov.au/def/datatype/Boolean">
    <rdfs:subClassOf rdf:resource="https://w3id.org/tern/ontologies/tern/Result"/>
  </rdf:Description>
  <rdf:Description rdf:nodeID="ub1bL1243C19">
    <owl:allValuesFrom rdf:resource="https://w3id.org/tern/ontologies/tern/SamplingPoint"/>
    <rdf:type rdf:resource="http://www.w3.org/2002/07/owl#Restriction"/>
    <owl:onProperty rdf:resource="https://w3id.org/tern/ontologies/tern/hasSamplingPoint"/>
  </rdf:Description>
  <rdf:Description rdf:nodeID="ub1bL282C25">
    <owl:unionOf rdf:nodeID="fe114e3c19c6e4b2e8a8d1297357cbc21b3"/>
    <rdf:type rdf:resource="http://www.w3.org/2002/07/owl#Class"/>
  </rdf:Description>
  <rdf:Description rdf:nodeID="ub1bL548C19">
    <owl:onProperty rdf:resource="https://w3id.org/tern/ontologies/tern/wasSubActivityOf"/>
    <owl:maxQualifiedCardinality rdf:datatype="http://www.w3.org/2001/XMLSchema#nonNegativeInteger">1</owl:maxQualifiedCardinality>
    <owl:onClass rdf:resource="https://w3id.org/tern/ontologies/tern/SiteVisit"/>
    <rdf:type rdf:resource="http://www.w3.org/2002/07/owl#Restriction"/>
  </rdf:Description>
  <rdf:Description rdf:nodeID="ub1bL894C19">
    <owl:qualifiedCardinality rdf:datatype="http://www.w3.org/2001/XMLSchema#nonNegativeInteger">1</owl:qualifiedCardinality>
    <rdf:type rdf:resource="http://www.w3.org/2002/07/owl#Restriction"/>
    <owl:onClass rdf:resource="http://linked.data.gov.au/def/datatype/QuantitativeMeasure"/>
    <owl:onProperty rdf:resource="https://w3id.org/tern/ontologies/loc/latitude"/>
  </rdf:Description>
  <rdf:Description rdf:nodeID="ub1bL107C19">
    <rdf:type rdf:resource="http://schema.org/Person"/>
    <schema:email>e.chuc@uq.edu.au</schema:email>
    <schema:identifier>https://orcid.org/0000-0002-6047-9864</schema:identifier>
    <schema:name>Edmond Chuc</schema:name>
    <schema:affiliation rdf:resource="https://w3id.org/tern/resources/a083902d-d821-41be-b663-1d7cb33eea66"/>
  </rdf:Description>
  <rdf:Description rdf:about="https://w3id.org/tern/ontologies/tern/SoilSampling">
    <skos:definition>An act of [Sampling](#Sampling) on soil.</skos:definition>
    <rdf:type rdf:resource="http://www.w3.org/2002/07/owl#Class"/>
    <rdfs:label>Soil Sampling</rdfs:label>
    <rdfs:subClassOf rdf:resource="https://w3id.org/tern/ontologies/tern/Sampling"/>
  </rdf:Description>
  <rdf:Description rdf:nodeID="ub1bL114C19">
    <schema:affiliation rdf:resource="https://w3id.org/tern/resources/a083902d-d821-41be-b663-1d7cb33eea66"/>
    <schema:email>s.guru@uq.edu.au</schema:email>
    <schema:name>Siddeswara Guru</schema:name>
    <schema:identifier>https://orcid.org/0000-0002-3903-254X</schema:identifier>
    <rdf:type rdf:resource="http://schema.org/Person"/>
  </rdf:Description>
  <rdf:Description rdf:nodeID="ub1bL429C25">
    <owl:unionOf rdf:nodeID="fe114e3c19c6e4b2e8a8d1297357cbc21b5"/>
    <rdf:type rdf:resource="http://www.w3.org/2002/07/owl#Class"/>
  </rdf:Description>
  <rdf:Description rdf:about="https://w3id.org/tern/ontologies/tern/observationTheme">
    <rdf:type rdf:resource="http://www.w3.org/1999/02/22-rdf-syntax-ns#Property"/>
    <skos:definition>Group observations into themes. See TERN's controlled list of &lt;a href="http://linked.data.gov.au/def/tern-cv/396192ae-3bd5-4050-b578-93107510129c"&gt;observation themes&lt;/a&gt; as example values.</skos:definition>
    <rdfs:subPropertyOf rdf:resource="http://purl.org/dc/terms/type"/>
    <rdfs:domain rdf:resource="https://w3id.org/tern/ontologies/tern/Observation"/>
    <rdfs:label>observation theme</rdfs:label>
  </rdf:Description>
  <rdf:Description rdf:nodeID="fe114e3c19c6e4b2e8a8d1297357cbc21b7">
    <rdf:rest rdf:nodeID="fe114e3c19c6e4b2e8a8d1297357cbc21b8"/>
    <rdf:first rdf:resource="http://www.w3.org/2004/02/skos/core#ConceptScheme"/>
  </rdf:Description>
  <rdf:Description rdf:nodeID="ub1bL236C19">
    <owl:onProperty rdf:resource="http://www.w3.org/2004/02/skos/core#definition"/>
    <owl:allValuesFrom rdf:resource="http://www.w3.org/2001/XMLSchema#string"/>
    <rdf:type rdf:resource="http://www.w3.org/2002/07/owl#Restriction"/>
  </rdf:Description>
  <rdf:Description rdf:nodeID="ub1bL450C19">
    <owl:maxQualifiedCardinality rdf:datatype="http://www.w3.org/2001/XMLSchema#nonNegativeInteger">1</owl:maxQualifiedCardinality>
    <owl:onProperty rdf:resource="https://w3id.org/tern/ontologies/tern/instructions"/>
    <rdf:type rdf:resource="http://www.w3.org/2002/07/owl#Restriction"/>
    <owl:onDataRange rdf:resource="http://www.w3.org/2001/XMLSchema#string"/>
  </rdf:Description>
  <rdf:Description rdf:nodeID="fe114e3c19c6e4b2e8a8d1297357cbc21b16">
    <rdf:first rdf:resource="http://www.w3.org/2001/XMLSchema#string"/>
    <rdf:rest rdf:nodeID="fe114e3c19c6e4b2e8a8d1297357cbc21b17"/>
  </rdf:Description>
  <rdf:Description rdf:about="https://w3id.org/tern/ontologies/tern/sampleStorageLocation">
    <rdfs:label>sample storage location</rdfs:label>
    <rdf:type rdf:resource="http://www.w3.org/1999/02/22-rdf-syntax-ns#Property"/>
    <skos:definition>Link a [CollectedSample](#CollectedSample) to the location [Point](https://w3id.org/tern/ontologies/loc/Point) of where it is stored.</skos:definition>
    <rdfs:subPropertyOf rdf:resource="http://www.opengis.net/ont/geosparql#hasGeometry"/>
  </rdf:Description>
  <rdf:Description rdf:nodeID="ub1bL818C19">
    <owl:allValuesFrom rdf:resource="https://w3id.org/tern/ontologies/org/Person"/>
    <owl:onProperty rdf:resource="http://www.w3.org/ns/prov#wasAttributedTo"/>
    <rdf:type rdf:resource="http://www.w3.org/2002/07/owl#Restriction"/>
  </rdf:Description>
  <rdf:Description rdf:about="https://w3id.org/tern/ontologies/tern/fluxnetID">
    <skos:definition>The unique identifier for flux towers registered with FLUXNET.</skos:definition>
    <rdfs:label>fluxnet ID</rdfs:label>
    <skos:example>AU-ASM</skos:example>
    <rdfs:seeAlso rdf:resource="https://fluxnet.org/"/>
    <rdf:type rdf:resource="http://www.w3.org/1999/02/22-rdf-syntax-ns#Property"/>
  </rdf:Description>
  <rdf:Description rdf:nodeID="ub1bL870C19">
    <owl:onClass rdf:resource="http://linked.data.gov.au/def/datatype/QuantitativeMeasure"/>
    <rdf:type rdf:resource="http://www.w3.org/2002/07/owl#Restriction"/>
    <owl:onProperty rdf:resource="https://w3id.org/tern/ontologies/loc/depth"/>
    <owl:maxQualifiedCardinality rdf:datatype="http://www.w3.org/2001/XMLSchema#nonNegativeInteger">1</owl:maxQualifiedCardinality>
  </rdf:Description>
  <rdf:Description rdf:nodeID="ub1bL752C19">
    <owl:onProperty rdf:resource="http://www.w3.org/2000/01/rdf-schema#comment"/>
    <owl:allValuesFrom rdf:resource="http://www.w3.org/2001/XMLSchema#string"/>
    <rdf:type rdf:resource="http://www.w3.org/2002/07/owl#Restriction"/>
  </rdf:Description>
  <rdf:Description rdf:nodeID="ub1bL961C19">
    <owl:allValuesFrom rdf:resource="https://w3id.org/tern/ontologies/tern/Site"/>
    <rdf:type rdf:resource="http://www.w3.org/2002/07/owl#Restriction"/>
    <owl:onProperty rdf:resource="http://purl.org/dc/terms/hasPart"/>
  </rdf:Description>
  <rdf:Description rdf:nodeID="ub1bL1193C19">
    <owl:onProperty rdf:resource="http://purl.org/dc/terms/identifier"/>
    <rdf:type rdf:resource="http://www.w3.org/2002/07/owl#Restriction"/>
    <owl:onClass rdf:resource="http://www.w3.org/2001/XMLSchema#string"/>
    <owl:qualifiedCardinality rdf:datatype="http://www.w3.org/2001/XMLSchema#nonNegativeInteger">1</owl:qualifiedCardinality>
  </rdf:Description>
  <rdf:Description rdf:nodeID="fe114e3c19c6e4b2e8a8d1297357cbc21b11">
    <rdf:rest rdf:resource="http://www.w3.org/1999/02/22-rdf-syntax-ns#nil"/>
    <rdf:first rdf:resource="https://w3id.org/tern/ontologies/tern/Sampling"/>
  </rdf:Description>
  <rdf:Description rdf:nodeID="ub1bL1123C19">
    <rdf:type rdf:resource="http://www.w3.org/2002/07/owl#Restriction"/>
    <owl:onProperty rdf:resource="https://w3id.org/tern/ontologies/tern/taxon"/>
    <owl:onClass rdf:resource="https://w3id.org/tern/ontologies/sd/StateTaxon"/>
    <owl:qualifiedCardinality rdf:datatype="http://www.w3.org/2001/XMLSchema#nonNegativeInteger">1</owl:qualifiedCardinality>
  </rdf:Description>
  <rdf:Description rdf:nodeID="ub1bL978C25">
    <rdf:type rdf:resource="http://www.w3.org/2002/07/owl#Class"/>
    <owl:unionOf rdf:nodeID="fe114e3c19c6e4b2e8a8d1297357cbc21b12"/>
  </rdf:Description>
  <rdf:Description rdf:nodeID="fe114e3c19c6e4b2e8a8d1297357cbc21b10">
    <rdf:rest rdf:nodeID="fe114e3c19c6e4b2e8a8d1297357cbc21b11"/>
    <rdf:first rdf:resource="https://w3id.org/tern/ontologies/tern/Observation"/>
  </rdf:Description>
  <rdf:Description rdf:nodeID="fe114e3c19c6e4b2e8a8d1297357cbc21b1">
    <rdf:rest rdf:nodeID="fe114e3c19c6e4b2e8a8d1297357cbc21b2"/>
    <rdf:first rdf:resource="http://www.w3.org/2001/XMLSchema#decimal"/>
  </rdf:Description>
  <rdf:Description rdf:nodeID="ub1bL919C19">
    <owl:onProperty rdf:resource="http://www.w3.org/ns/sosa/observes"/>
    <owl:allValuesFrom rdf:resource="https://w3id.org/tern/ontologies/tern/ObservableProperty"/>
    <rdf:type rdf:resource="http://www.w3.org/2002/07/owl#Restriction"/>
  </rdf:Description>
  <rdf:Description rdf:about="http://linked.data.gov.au/def/datatype/QuantitativeMeasure">
    <rdfs:subClassOf rdf:resource="https://w3id.org/tern/ontologies/tern/Result"/>
  </rdf:Description>
  <rdf:Description rdf:about="https://w3id.org/tern/ontologies/tern/hadSubActivity">
    <rdf:type rdf:resource="http://www.w3.org/1999/02/22-rdf-syntax-ns#Property"/>
    <rdfs:label>had sub activity</rdfs:label>
    <skos:definition>Link to an [Observation](#Observation) or [Sampling](#Sampling).</skos:definition>
  </rdf:Description>
  <rdf:Description rdf:about="https://w3id.org/tern/ontologies/tern/ObservableProperty">
    <rdfs:subClassOf rdf:nodeID="ub1bL513C19"/>
    <rdf:type rdf:resource="http://www.w3.org/2002/07/owl#Class"/>
    <rdfs:subClassOf rdf:nodeID="ub1bL503C19"/>
    <rdfs:subClassOf rdf:nodeID="ub1bL519C19"/>
    <rdfs:subClassOf rdf:nodeID="ub1bL508C19"/>
    <skos:definition>&lt;i&gt;Observable Property&lt;/i&gt; - An observable quality (property, characteristic) of a &lt;a href="http://w3.org/ns/sosa/FeatureOfInterest"&gt;FeatureOfInterest&lt;/a&gt;.</skos:definition>
    <rdfs:subClassOf rdf:nodeID="ub1bL491C19"/>
    <rdfs:subClassOf rdf:resource="http://www.w3.org/ns/sosa/ObservableProperty"/>
    <rdfs:label>Observable Property</rdfs:label>
  </rdf:Description>
  <rdf:Description rdf:nodeID="ub1bL508C19">
    <owl:onProperty rdf:resource="https://w3id.org/tern/ontologies/tern/globalVocabulary"/>
    <rdf:type rdf:resource="http://www.w3.org/2002/07/owl#Restriction"/>
    <owl:maxCardinality rdf:datatype="http://www.w3.org/2001/XMLSchema#nonNegativeInteger">1</owl:maxCardinality>
  </rdf:Description>
  <rdf:Description rdf:nodeID="ub1bL1033C19">
    <owl:onClass rdf:resource="https://w3id.org/tern/ontologies/loc/Point"/>
    <owl:onProperty rdf:resource="https://w3id.org/tern/ontologies/tern/centroidPoint"/>
    <rdf:type rdf:resource="http://www.w3.org/2002/07/owl#Restriction"/>
    <owl:maxQualifiedCardinality rdf:datatype="http://www.w3.org/2001/XMLSchema#nonNegativeInteger">1</owl:maxQualifiedCardinality>
  </rdf:Description>
  <rdf:Description rdf:about="https://w3id.org/tern/ontologies/tern/TERNDerivedObservation">
    <rdfs:label>TERN Derived Observation</rdfs:label>
    <rdf:type rdf:resource="http://www.w3.org/2002/07/owl#Class"/>
    <rdfs:subClassOf rdf:resource="https://w3id.org/tern/ontologies/tern/DerivedObservation"/>
    <skos:definition>A derived observation created by TERN.</skos:definition>
  </rdf:Description>
  <rdf:Description rdf:nodeID="ub1bL876C19">
    <rdf:type rdf:resource="http://www.w3.org/2002/07/owl#Restriction"/>
    <owl:onClass rdf:resource="http://linked.data.gov.au/def/datatype/QuantitativeMeasure"/>
    <owl:onProperty rdf:resource="https://w3id.org/tern/ontologies/loc/elevation"/>
    <owl:maxQualifiedCardinality rdf:datatype="http://www.w3.org/2001/XMLSchema#nonNegativeInteger">1</owl:maxQualifiedCardinality>
  </rdf:Description>
  <rdf:Description rdf:about="https://w3id.org/tern/ontologies/tern/hasCategoricalCollection">
    <rdfs:label>has categorical collection</rdfs:label>
    <rdf:type rdf:resource="http://www.w3.org/1999/02/22-rdf-syntax-ns#Property"/>
    <skos:definition>Link a concept to a collection containing categorical values.</skos:definition>
  </rdf:Description>
  <rdf:Description rdf:nodeID="ub1bL101C23">
    <rdf:type rdf:resource="http://schema.org/Person"/>
    <schema:email>t.parkhurst@uq.edu.au</schema:email>
    <schema:name>Tina Parkhurst</schema:name>
    <schema:affiliation rdf:resource="https://w3id.org/tern/resources/a083902d-d821-41be-b663-1d7cb33eea66"/>
  </rdf:Description>
  <rdf:Description rdf:nodeID="ub1bL349C19">
    <owl:onProperty rdf:resource="http://www.w3.org/2000/01/rdf-schema#comment"/>
    <owl:allValuesFrom rdf:resource="http://www.w3.org/2001/XMLSchema#string"/>
    <rdf:type rdf:resource="http://www.w3.org/2002/07/owl#Restriction"/>
  </rdf:Description>
  <rdf:Description rdf:nodeID="ub1bL813C19">
    <rdf:type rdf:resource="http://www.w3.org/2002/07/owl#Restriction"/>
    <owl:onProperty rdf:resource="http://www.w3.org/2000/01/rdf-schema#comment"/>
    <owl:allValuesFrom rdf:resource="http://www.w3.org/2001/XMLSchema#string"/>
  </rdf:Description>
  <rdf:Description rdf:nodeID="ub1bL271C25">
    <rdf:type rdf:resource="http://www.w3.org/2002/07/owl#Class"/>
    <owl:unionOf rdf:nodeID="fe114e3c19c6e4b2e8a8d1297357cbc21b1"/>
  </rdf:Description>
  <rdf:Description rdf:about="https://w3id.org/tern/ontologies/tern/EarthObservationSatellite">
    <rdfs:subClassOf rdf:resource="https://w3id.org/tern/ontologies/tern/MobilePlatform"/>
    <rdfs:label>Earth Observation Satellite</rdfs:label>
    <rdfs:seeAlso rdf:resource="https://gcmd.earthdata.nasa.gov/kms/concept/3466eed1-2fbb-49bf-ab0b-dc08731d502b"/>
    <skos:definition>Earth observation satellites are satellites specifically designed to observe Earth from orbit, similar to spy satellites but intended for non-military uses such as environmental monitoring, meteorology, map making etc. Source: Wikipedia, http://en.wikipedia.org/wiki/Earth_observation_satellite Group: Platform_Details Entry_ID: Earth Observation Satellites Group: Platform_Identification Platform_Category: Earth Observation Satellites Short_Name: Earth Observation Satellites End_Group End_Group</skos:definition>
    <rdf:type rdf:resource="http://www.w3.org/2002/07/owl#Class"/>
  </rdf:Description>
  <rdf:Description rdf:nodeID="ub1bL615C19">
    <owl:allValuesFrom rdf:resource="http://www.w3.org/2001/XMLSchema#string"/>
    <owl:onProperty rdf:resource="http://schema.org/serialNumber"/>
    <rdf:type rdf:resource="http://www.w3.org/2002/07/owl#Restriction"/>
  </rdf:Description>
  <rdf:Description rdf:nodeID="ub1bL251C19">
    <rdf:type rdf:resource="http://www.w3.org/2002/07/owl#Restriction"/>
    <owl:minQualifiedCardinality rdf:datatype="http://www.w3.org/2001/XMLSchema#nonNegativeInteger">1</owl:minQualifiedCardinality>
    <owl:onProperty rdf:resource="http://purl.org/dc/terms/source"/>
    <owl:onClass rdf:resource="http://www.w3.org/2001/XMLSchema#string"/>
  </rdf:Description>
  <rdf:Description rdf:about="https://w3id.org/tern/ontologies/tern/wasSubActivityOf">
    <rdfs:label>was sub activity of</rdfs:label>
    <rdf:type rdf:resource="http://www.w3.org/1999/02/22-rdf-syntax-ns#Property"/>
    <skos:definition>Link to parent activity.</skos:definition>
  </rdf:Description>
  <rdf:Description rdf:nodeID="ub1bL89C23">
    <rdf:type rdf:resource="http://schema.org/Person"/>
    <schema:email>j.sanchezgonzalez@uq.edu.au</schema:email>
    <schema:affiliation rdf:resource="https://w3id.org/tern/resources/a083902d-d821-41be-b663-1d7cb33eea66"/>
    <schema:name>Javier Sanchez Gonzalez</schema:name>
  </rdf:Description>
  <rdf:Description rdf:nodeID="ub1bL384C19">
    <owl:onProperty rdf:resource="https://w3id.org/tern/ontologies/tern/centroidPoint"/>
    <rdf:type rdf:resource="http://www.w3.org/2002/07/owl#Restriction"/>
    <owl:qualifiedCardinality rdf:datatype="http://www.w3.org/2001/XMLSchema#nonNegativeInteger">1</owl:qualifiedCardinality>
    <owl:onClass rdf:resource="https://w3id.org/tern/ontologies/loc/Point"/>
  </rdf:Description>
  <rdf:Description rdf:about="https://w3id.org/tern/ontologies/tern/centroidPoint">
    <rdfs:label>centroid point</rdfs:label>
    <rdfs:subPropertyOf rdf:resource="http://www.opengis.net/ont/geosparql#hasGeometry"/>
    <rdf:type rdf:resource="http://www.w3.org/1999/02/22-rdf-syntax-ns#Property"/>
    <skos:definition>The centroid point of the subject.</skos:definition>
    <rdfs:range rdf:resource="https://w3id.org/tern/ontologies/loc/Point"/>
  </rdf:Description>
  <rdf:Description rdf:nodeID="ub1bL1259C19">
    <owl:qualifiedCardinality rdf:datatype="http://www.w3.org/2001/XMLSchema#nonNegativeInteger">1</owl:qualifiedCardinality>
    <owl:onClass rdf:resource="https://w3id.org/tern/ontologies/loc/Point"/>
    <owl:onProperty rdf:resource="https://w3id.org/tern/ontologies/tern/transectEndPoint"/>
    <rdf:type rdf:resource="http://www.w3.org/2002/07/owl#Restriction"/>
  </rdf:Description>
  <rdf:Description rdf:nodeID="ub1bL782C19">
    <owl:onProperty rdf:resource="http://www.w3.org/ns/sosa/isResultOf"/>
    <rdf:type rdf:resource="http://www.w3.org/2002/07/owl#Restriction"/>
    <owl:maxQualifiedCardinality rdf:datatype="http://www.w3.org/2001/XMLSchema#nonNegativeInteger">1</owl:maxQualifiedCardinality>
    <owl:onClass rdf:resource="https://w3id.org/tern/ontologies/tern/Sampling"/>
  </rdf:Description>
  <rdf:Description rdf:about="https://w3id.org/tern/ontologies/tern/dateDecommissioned">
    <rdf:type rdf:resource="http://www.w3.org/1999/02/22-rdf-syntax-ns#Property"/>
    <rdfs:label>date decommissioned</rdfs:label>
    <skos:definition>The date when something was decommissioned, e.g. a [Site](#Site).</skos:definition>
  </rdf:Description>
  <rdf:Description rdf:nodeID="ub1bL456C19">
    <owl:maxQualifiedCardinality rdf:datatype="http://www.w3.org/2001/XMLSchema#nonNegativeInteger">1</owl:maxQualifiedCardinality>
    <owl:onProperty rdf:resource="https://w3id.org/tern/ontologies/tern/purpose"/>
    <rdf:type rdf:resource="http://www.w3.org/2002/07/owl#Restriction"/>
    <owl:onDataRange rdf:resource="http://www.w3.org/2001/XMLSchema#string"/>
  </rdf:Description>
  <rdf:Description rdf:nodeID="ub1bL1519C1">
    <rdf:type rdf:resource="http://www.w3.org/2002/07/owl#Class"/>
    <owl:unionOf rdf:nodeID="fe114e3c19c6e4b2e8a8d1297357cbc21b18"/>
  </rdf:Description>
  <rdf:Description rdf:nodeID="ub1bL366C19">
    <owl:onProperty rdf:resource="http://www.w3.org/ns/sosa/isHostedBy"/>
    <rdf:type rdf:resource="http://www.w3.org/2002/07/owl#Restriction"/>
    <owl:maxQualifiedCardinality rdf:datatype="http://www.w3.org/2001/XMLSchema#nonNegativeInteger">1</owl:maxQualifiedCardinality>
    <owl:onClass rdf:resource="https://w3id.org/tern/ontologies/tern/Site"/>
  </rdf:Description>
  <rdf:Description rdf:about="https://w3id.org/tern/ontologies/tern/ObservationTheme">
    <rdfs:subClassOf rdf:resource="http://www.w3.org/2004/02/skos/core#Concept"/>
    <skos:definition>An [Observation Theme](#ObservationTheme) categorises [Parameters](#Parameter) based on domain.</skos:definition>
    <rdfs:label>Observation Theme</rdfs:label>
    <rdf:type rdf:resource="http://www.w3.org/2002/07/owl#Class"/>
  </rdf:Description>
  <rdf:Description rdf:nodeID="ub1bL1172C25">
    <rdf:type rdf:resource="http://www.w3.org/2002/07/owl#Class"/>
    <owl:unionOf rdf:nodeID="fe114e3c19c6e4b2e8a8d1297357cbc21b14"/>
  </rdf:Description>
  <rdf:Description rdf:nodeID="ub1bL401C19">
    <rdf:type rdf:resource="http://www.w3.org/2002/07/owl#Restriction"/>
    <owl:onProperty rdf:resource="http://linked.data.gov.au/def/datatype/value"/>
    <owl:cardinality rdf:datatype="http://www.w3.org/2001/XMLSchema#nonNegativeInteger">1</owl:cardinality>
  </rdf:Description>
  <rdf:Description rdf:about="https://w3id.org/tern/ontologies/tern/swPoint">
    <skos:definition>The south-west point of the subject.</skos:definition>
    <rdfs:subPropertyOf rdf:resource="http://www.opengis.net/ont/geosparql#hasGeometry"/>
    <rdf:type rdf:resource="http://www.w3.org/1999/02/22-rdf-syntax-ns#Property"/>
    <rdfs:label>sw point</rdfs:label>
    <rdfs:range rdf:resource="https://w3id.org/tern/ontologies/loc/Point"/>
  </rdf:Description>
  <rdf:Description rdf:about="http://linked.data.gov.au/def/datatype/QuantitativeRange">
    <rdfs:subClassOf rdf:resource="https://w3id.org/tern/ontologies/tern/Result"/>
  </rdf:Description>
  <rdf:Description rdf:nodeID="ub1bL1074C19">
    <owl:qualifiedCardinality rdf:datatype="http://www.w3.org/2001/XMLSchema#nonNegativeInteger">1</owl:qualifiedCardinality>
    <owl:onProperty rdf:resource="http://www.w3.org/2000/01/rdf-schema#label"/>
    <rdf:type rdf:resource="http://www.w3.org/2002/07/owl#Restriction"/>
    <owl:onClass rdf:resource="http://www.w3.org/2001/XMLSchema#string"/>
  </rdf:Description>
  <rdf:Description rdf:nodeID="fe114e3c19c6e4b2e8a8d1297357cbc21b14">
    <rdf:first rdf:resource="https://w3id.org/tern/ontologies/tern/Observation"/>
    <rdf:rest rdf:nodeID="fe114e3c19c6e4b2e8a8d1297357cbc21b15"/>
  </rdf:Description>
  <rdf:Description rdf:nodeID="ub1bL767C19">
    <rdf:type rdf:resource="http://www.w3.org/2002/07/owl#Restriction"/>
    <owl:allValuesFrom rdf:resource="https://w3id.org/tern/ontologies/tern/Sample"/>
    <owl:onProperty rdf:resource="http://www.w3.org/ns/sosa/hasSample"/>
  </rdf:Description>
  <rdf:Description rdf:nodeID="ub1bL1051C19">
    <owl:maxQualifiedCardinality rdf:datatype="http://www.w3.org/2001/XMLSchema#nonNegativeInteger">1</owl:maxQualifiedCardinality>
    <owl:onProperty rdf:resource="https://w3id.org/tern/ontologies/tern/dimension"/>
    <rdf:type rdf:resource="http://www.w3.org/2002/07/owl#Restriction"/>
    <owl:onClass rdf:resource="https://w3id.org/tern/ontologies/tern/Dimension"/>
  </rdf:Description>
  <rdf:Description rdf:about="https://w3id.org/tern/ontologies/tern/Platform">
    <rdfs:subClassOf rdf:resource="http://www.w3.org/ns/sosa/Platform"/>
    <skos:example>A post, buoy, vehicle, ship, aircraft, satellite, cell-phone, human or animal may act as platforms for (technical or biological) sensors or actuators.</skos:example>
    <rdfs:label>Platform</rdfs:label>
    <rdf:type rdf:resource="http://www.w3.org/2002/07/owl#Class"/>
    <skos:definition>A Platform is an entity that hosts other entities, particularly Sensors, Actuators, Samplers, and other Platforms.</skos:definition>
  </rdf:Description>
  <rdf:Description rdf:nodeID="ub1bL645C19">
    <owl:cardinality rdf:datatype="http://www.w3.org/2001/XMLSchema#nonNegativeInteger">1</owl:cardinality>
    <owl:onProperty rdf:resource="http://linked.data.gov.au/def/datatype/vocabulary"/>
    <rdf:type rdf:resource="http://www.w3.org/2002/07/owl#Restriction"/>
  </rdf:Description>
  <rdf:Description rdf:nodeID="ub1bL493C25">
    <owl:unionOf rdf:nodeID="fe114e3c19c6e4b2e8a8d1297357cbc21b7"/>
    <rdf:type rdf:resource="http://www.w3.org/2002/07/owl#Class"/>
  </rdf:Description>
  <rdf:Description rdf:about="https://w3id.org/tern/ontologies/tern/RadiationSensor">
    <rdfs:label>Radiation sensor</rdfs:label>
    <rdf:type rdf:resource="http://www.w3.org/2002/07/owl#Class"/>
    <rdfs:subClassOf rdf:resource="https://w3id.org/tern/ontologies/tern/Sensor"/>
  </rdf:Description>
  <rdf:Description rdf:nodeID="ub1bL674C19">
    <rdf:type rdf:resource="http://www.w3.org/2002/07/owl#Restriction"/>
    <owl:onClass rdf:resource="http://www.w3.org/2001/XMLSchema#string"/>
    <owl:qualifiedCardinality rdf:datatype="http://www.w3.org/2001/XMLSchema#nonNegativeInteger">1</owl:qualifiedCardinality>
    <owl:onProperty rdf:resource="http://schema.org/name"/>
  </rdf:Description>
  <rdf:Description rdf:nodeID="ub1bL835C19">
    <owl:qualifiedCardinality rdf:datatype="http://www.w3.org/2001/XMLSchema#nonNegativeInteger">1</owl:qualifiedCardinality>
    <owl:onProperty rdf:resource="http://www.w3.org/ns/sosa/usedProcedure"/>
    <owl:onClass rdf:resource="https://w3id.org/tern/ontologies/tern/Procedure"/>
    <rdf:type rdf:resource="http://www.w3.org/2002/07/owl#Restriction"/>
  </rdf:Description>
  <rdf:Description rdf:nodeID="ub1bL1512C1">
    <owl:unionOf rdf:nodeID="fe114e3c19c6e4b2e8a8d1297357cbc21b16"/>
    <rdf:type rdf:resource="http://www.w3.org/2002/07/owl#Class"/>
  </rdf:Description>
  <rdf:Description rdf:nodeID="ub1bL257C19">
    <rdf:type rdf:resource="http://www.w3.org/2002/07/owl#Restriction"/>
    <owl:minQualifiedCardinality rdf:datatype="http://www.w3.org/2001/XMLSchema#nonNegativeInteger">1</owl:minQualifiedCardinality>
    <owl:onClass rdf:resource="http://www.w3.org/2001/XMLSchema#string"/>
    <owl:onProperty rdf:resource="http://schema.org/manufacturer"/>
  </rdf:Description>
  <rdf:Description rdf:about="https://w3id.org/tern/ontologies/tern/Dimension">
    <rdfs:subClassOf rdf:nodeID="ub1bL301C19"/>
    <rdfs:subClassOf rdf:nodeID="ub1bL291C19"/>
    <rdf:type rdf:resource="http://www.w3.org/2002/07/owl#Class"/>
    <rdfs:subClassOf rdf:nodeID="ub1bL269C19"/>
    <rdfs:subClassOf rdf:nodeID="ub1bL296C19"/>
    <rdfs:subClassOf rdf:nodeID="ub1bL280C19"/>
    <rdfs:label>Dimension</rdfs:label>
    <skos:definition>The dimension of a 2D square or rectangular feature. Example, the dimension of a rectangular plot [Site](#Site). This class should perhaps have specialised classes to express not just square or rectangular features but also others such as circular features.</skos:definition>
  </rdf:Description>
  <rdf:Description rdf:nodeID="ub1bL269C19">
    <owl:onProperty rdf:resource="https://w3id.org/tern/ontologies/tern/length"/>
    <owl:allValuesFrom rdf:nodeID="ub1bL271C25"/>
    <rdf:type rdf:resource="http://www.w3.org/2002/07/owl#Restriction"/>
  </rdf:Description>
  <rdf:Description rdf:nodeID="ub1bL1099C19">
    <owl:onClass rdf:resource="https://w3id.org/tern/ontologies/tern/Site"/>
    <rdf:type rdf:resource="http://www.w3.org/2002/07/owl#Restriction"/>
    <owl:qualifiedCardinality rdf:datatype="http://www.w3.org/2001/XMLSchema#nonNegativeInteger">1</owl:qualifiedCardinality>
    <owl:onProperty rdf:resource="http://www.w3.org/ns/sosa/isSampleOf"/>
  </rdf:Description>
  <rdf:Description rdf:about="https://w3id.org/tern/ontologies/tern/siteVisit">
    <rdfs:range rdf:resource="https://w3id.org/tern/ontologies/tern/SiteVisit"/>
    <rdf:type rdf:resource="http://www.w3.org/1999/02/22-rdf-syntax-ns#Property"/>
    <rdfs:label>site visit</rdfs:label>
    <skos:definition>Link to a [Site Visit](#SiteVisit).</skos:definition>
  </rdf:Description>
  <rdf:Description rdf:nodeID="ub1bL971C19">
    <owl:onProperty rdf:resource="https://w3id.org/tern/ontologies/tern/siteVisit"/>
    <rdf:type rdf:resource="http://www.w3.org/2002/07/owl#Restriction"/>
    <owl:allValuesFrom rdf:resource="https://w3id.org/tern/ontologies/tern/SiteVisit"/>
  </rdf:Description>
  <rdf:Description rdf:nodeID="ub1bL1187C19">
    <owl:onClass rdf:resource="http://www.w3.org/2001/XMLSchema#string"/>
    <rdf:type rdf:resource="http://www.w3.org/2002/07/owl#Restriction"/>
    <owl:onProperty rdf:resource="https://w3id.org/tern/ontologies/tern/siteDescription"/>
    <owl:maxQualifiedCardinality rdf:datatype="http://www.w3.org/2001/XMLSchema#nonNegativeInteger">1</owl:maxQualifiedCardinality>
  </rdf:Description>
  <rdf:Description rdf:nodeID="ub1bL1199C19">
    <owl:onProperty rdf:resource="http://www.w3.org/2000/01/rdf-schema#label"/>
    <rdf:type rdf:resource="http://www.w3.org/2002/07/owl#Restriction"/>
    <owl:onClass rdf:resource="http://www.w3.org/2001/XMLSchema#string"/>
    <owl:qualifiedCardinality rdf:datatype="http://www.w3.org/2001/XMLSchema#nonNegativeInteger">1</owl:qualifiedCardinality>
  </rdf:Description>
  <rdf:Description rdf:nodeID="fe114e3c19c6e4b2e8a8d1297357cbc21b5">
    <rdf:first rdf:resource="http://www.w3.org/2001/XMLSchema#string"/>
    <rdf:rest rdf:nodeID="fe114e3c19c6e4b2e8a8d1297357cbc21b6"/>
  </rdf:Description>
  <rdf:Description rdf:about="http://linked.data.gov.au/def/datatype/Count">
    <rdfs:subClassOf rdf:resource="https://w3id.org/tern/ontologies/tern/Result"/>
  </rdf:Description>
  <rdf:Description rdf:nodeID="fe114e3c19c6e4b2e8a8d1297357cbc21b12">
    <rdf:first rdf:resource="https://w3id.org/tern/ontologies/loc/Point"/>
    <rdf:rest rdf:nodeID="fe114e3c19c6e4b2e8a8d1297357cbc21b13"/>
  </rdf:Description>
  <rdf:Description rdf:nodeID="ub1bL155C23">
    <doap:repository rdf:resource="https://github.com/ternaustralia/ontology_tern"/>
    <rdf:type rdf:resource="http://usefulinc.com/ns/doap#Project"/>
    <rdf:type rdf:resource="http://www.w3.org/ns/prov#Activity"/>
  </rdf:Description>
  <rdf:Description rdf:nodeID="fe114e3c19c6e4b2e8a8d1297357cbc21b2">
    <rdf:rest rdf:resource="http://www.w3.org/1999/02/22-rdf-syntax-ns#nil"/>
    <rdf:first rdf:resource="http://www.w3.org/2001/XMLSchema#integer"/>
  </rdf:Description>
  <rdf:Description rdf:nodeID="ub1bL956C19">
    <rdf:type rdf:resource="http://www.w3.org/2002/07/owl#Restriction"/>
    <owl:onProperty rdf:resource="http://schema.org/additionalProperty"/>
    <owl:allValuesFrom rdf:resource="https://w3id.org/tern/ontologies/tern/PropertyValue"/>
  </rdf:Description>
  <rdf:Description rdf:nodeID="fe114e3c19c6e4b2e8a8d1297357cbc21b15">
    <rdf:first rdf:resource="https://w3id.org/tern/ontologies/tern/Sampling"/>
    <rdf:rest rdf:resource="http://www.w3.org/1999/02/22-rdf-syntax-ns#nil"/>
  </rdf:Description>
  <rdf:Description rdf:nodeID="ub1bL198C19">
    <rdf:type rdf:resource="http://www.w3.org/2002/07/owl#Restriction"/>
    <owl:onProperty rdf:resource="https://w3id.org/tern/ontologies/tern/sampleStorageLocation"/>
    <owl:maxQualifiedCardinality rdf:datatype="http://www.w3.org/2001/XMLSchema#nonNegativeInteger">1</owl:maxQualifiedCardinality>
    <owl:onClass rdf:resource="https://w3id.org/tern/ontologies/loc/Point"/>
  </rdf:Description>
  <rdf:Description rdf:about="https://w3id.org/tern/ontologies/tern/FixedPlatform">
    <rdfs:subClassOf rdf:resource="https://w3id.org/tern/ontologies/tern/Platform"/>
    <rdf:type rdf:resource="http://www.w3.org/2002/07/owl#Class"/>
    <rdfs:label>Fixed Platform</rdfs:label>
    <skos:definition>A fixed platform based on land.</skos:definition>
  </rdf:Description>
  <rdf:Description rdf:about="https://w3id.org/tern/ontologies/tern/purpose">
    <rdfs:label>purpose</rdfs:label>
    <skos:definition>Describe the purpose of something.</skos:definition>
    <rdf:type rdf:resource="http://www.w3.org/2002/07/owl#DatatypeProperty"/>
    <rdfs:range rdf:resource="http://www.w3.org/2001/XMLSchema#string"/>
  </rdf:Description>
  <rdf:Description rdf:nodeID="ub1bL1170C19">
    <owl:allValuesFrom rdf:nodeID="ub1bL1172C25"/>
    <owl:onProperty rdf:resource="https://w3id.org/tern/ontologies/tern/hadSubActivity"/>
    <rdf:type rdf:resource="http://www.w3.org/2002/07/owl#Restriction"/>
  </rdf:Description>
  <rdf:Description rdf:nodeID="ub1bL291C19">
    <owl:cardinality rdf:datatype="http://www.w3.org/2001/XMLSchema#nonNegativeInteger">1</owl:cardinality>
    <rdf:type rdf:resource="http://www.w3.org/2002/07/owl#Restriction"/>
    <owl:onProperty rdf:resource="https://w3id.org/tern/ontologies/tern/length"/>
  </rdf:Description>
  <rdf:Description rdf:nodeID="ub1bL716C19">
    <rdf:type rdf:resource="http://www.w3.org/2002/07/owl#Restriction"/>
    <owl:onProperty rdf:resource="http://www.w3.org/ns/prov#wasAttributedTo"/>
    <owl:allValuesFrom rdf:resource="https://w3id.org/tern/ontologies/org/Person"/>
  </rdf:Description>
  <rdf:Description rdf:nodeID="ub1bL941C19">
    <owl:onProperty rdf:resource="http://www.w3.org/2000/01/rdf-schema#comment"/>
    <owl:allValuesFrom rdf:resource="http://www.w3.org/2001/XMLSchema#string"/>
    <rdf:type rdf:resource="http://www.w3.org/2002/07/owl#Restriction"/>
  </rdf:Description>
  <rdf:Description rdf:about="https://w3id.org/tern/ontologies/tern/globalMatch">
    <rdfs:subPropertyOf rdf:resource="http://www.w3.org/2004/02/skos/core#exactMatch"/>
    <rdfs:label>global match</rdfs:label>
    <rdf:type rdf:resource="http://www.w3.org/1999/02/22-rdf-syntax-ns#Property"/>
    <skos:definition>Link a concept to an upper concept (in the closed system).</skos:definition>
  </rdf:Description>
  <rdf:Description rdf:nodeID="ub1bL936C19">
    <rdf:type rdf:resource="http://www.w3.org/2002/07/owl#Restriction"/>
    <owl:onProperty rdf:resource="http://www.opengis.net/ont/geosparql#sfWithin"/>
    <owl:allValuesFrom rdf:resource="http://www.opengis.net/ont/geosparql#Feature"/>
  </rdf:Description>
  <rdf:Description rdf:nodeID="ub1bL49C19">
    <owl:cardinality rdf:datatype="http://www.w3.org/2001/XMLSchema#nonNegativeInteger">1</owl:cardinality>
    <owl:onProperty rdf:resource="https://w3id.org/tern/ontologies/tern/globalVocabulary"/>
    <rdf:type rdf:resource="http://www.w3.org/2002/07/owl#Restriction"/>
  </rdf:Description>
  <rdf:Description rdf:nodeID="ub1bL966C19">
    <owl:allValuesFrom rdf:resource="https://w3id.org/tern/ontologies/tern/Site"/>
    <rdf:type rdf:resource="http://www.w3.org/2002/07/owl#Restriction"/>
    <owl:onProperty rdf:resource="http://purl.org/dc/terms/isPartOf"/>
  </rdf:Description>
  <rdf:Description rdf:about="https://w3id.org/tern/ontologies/tern/SiteStratum">
    <rdfs:subClassOf rdf:nodeID="ub1bL1099C19"/>
    <rdfs:subClassOf rdf:resource="https://w3id.org/tern/ontologies/tern/Sample"/>
    <rdfs:subClassOf rdf:nodeID="ub1bL1093C19"/>
    <rdf:type rdf:resource="http://www.w3.org/2002/07/owl#Class"/>
    <rdfs:label>Site Stratum</rdfs:label>
    <skos:definition>Structural element covering a recognisable height range in vegetation ecosystem occurring at an observation [Site](#Site).</skos:definition>
  </rdf:Description>
  <rdf:Description rdf:nodeID="ub1bL777C19">
    <owl:onProperty rdf:resource="http://www.w3.org/2000/01/rdf-schema#label"/>
    <rdf:type rdf:resource="http://www.w3.org/2002/07/owl#Restriction"/>
    <owl:cardinality rdf:datatype="http://www.w3.org/2001/XMLSchema#nonNegativeInteger">1</owl:cardinality>
  </rdf:Description>
  <rdf:Description rdf:nodeID="ub1bL1165C19">
    <owl:onProperty rdf:resource="http://schema.org/additionalProperty"/>
    <rdf:type rdf:resource="http://www.w3.org/2002/07/owl#Restriction"/>
    <owl:allValuesFrom rdf:resource="https://w3id.org/tern/ontologies/tern/PropertyValue"/>
  </rdf:Description>
  <rdf:Description rdf:nodeID="ub1bL1205C19">
    <owl:onClass rdf:resource="https://w3id.org/tern/ontologies/tern/Site"/>
    <rdf:type rdf:resource="http://www.w3.org/2002/07/owl#Restriction"/>
    <owl:onProperty rdf:resource="https://w3id.org/tern/ontologies/tern/site"/>
    <owl:qualifiedCardinality rdf:datatype="http://www.w3.org/2001/XMLSchema#nonNegativeInteger">1</owl:qualifiedCardinality>
  </rdf:Description>
  <rdf:Description rdf:nodeID="ub1bL1003C19">
    <owl:onProperty rdf:resource="https://w3id.org/tern/ontologies/tern/dateDecommissioned"/>
    <owl:maxQualifiedCardinality rdf:datatype="http://www.w3.org/2001/XMLSchema#nonNegativeInteger">1</owl:maxQualifiedCardinality>
    <owl:onClass rdf:resource="http://www.w3.org/2001/XMLSchema#date"/>
    <rdf:type rdf:resource="http://www.w3.org/2002/07/owl#Restriction"/>
  </rdf:Description>
  <rdf:Description rdf:about="https://w3id.org/tern/ontologies/tern/globalValue">
    <rdfs:label>global value</rdfs:label>
    <skos:definition>The global controlled vocabulary concept (in the closed system).</skos:definition>
    <rdf:type rdf:resource="http://www.w3.org/1999/02/22-rdf-syntax-ns#Property"/>
  </rdf:Description>
  <rdf:Description rdf:nodeID="ub1bL396C19">
    <owl:allValuesFrom rdf:resource="http://www.w3.org/2001/XMLSchema#string"/>
    <owl:onProperty rdf:resource="http://purl.org/dc/terms/description"/>
    <rdf:type rdf:resource="http://www.w3.org/2002/07/owl#Restriction"/>
  </rdf:Description>
  <rdf:Description rdf:nodeID="ub1bL406C19">
    <rdf:type rdf:resource="http://www.w3.org/2002/07/owl#Restriction"/>
    <owl:onProperty rdf:resource="http://www.w3.org/2000/01/rdf-schema#label"/>
    <owl:onClass rdf:resource="http://www.w3.org/2001/XMLSchema#string"/>
    <owl:qualifiedCardinality rdf:datatype="http://www.w3.org/2001/XMLSchema#nonNegativeInteger">1</owl:qualifiedCardinality>
  </rdf:Description>
  <rdf:Description rdf:nodeID="ub1bL1039C19">
    <rdf:type rdf:resource="http://www.w3.org/2002/07/owl#Restriction"/>
    <owl:maxQualifiedCardinality rdf:datatype="http://www.w3.org/2001/XMLSchema#nonNegativeInteger">1</owl:maxQualifiedCardinality>
    <owl:onProperty rdf:resource="https://w3id.org/tern/ontologies/tern/swPoint"/>
    <owl:onClass rdf:resource="https://w3id.org/tern/ontologies/loc/Point"/>
  </rdf:Description>
  <rdf:Description rdf:nodeID="ub1bL1248C19">
    <owl:maxCardinality rdf:datatype="http://www.w3.org/2001/XMLSchema#nonNegativeInteger">1</owl:maxCardinality>
    <rdf:type rdf:resource="http://www.w3.org/2002/07/owl#Restriction"/>
    <owl:onProperty rdf:resource="https://w3id.org/tern/ontologies/tern/transectDirection"/>
  </rdf:Description>
  <rdf:Description rdf:nodeID="ub1bL378C19">
    <owl:qualifiedCardinality rdf:datatype="http://www.w3.org/2001/XMLSchema#nonNegativeInteger">1</owl:qualifiedCardinality>
    <rdf:type rdf:resource="http://www.w3.org/2002/07/owl#Restriction"/>
    <owl:onProperty rdf:resource="http://www.w3.org/2000/01/rdf-schema#label"/>
    <owl:onClass rdf:resource="http://www.w3.org/2001/XMLSchema#string"/>
  </rdf:Description>
  <rdf:Description rdf:nodeID="ub1bL296C19">
    <owl:onProperty rdf:resource="https://w3id.org/tern/ontologies/tern/width"/>
    <rdf:type rdf:resource="http://www.w3.org/2002/07/owl#Restriction"/>
    <owl:cardinality rdf:datatype="http://www.w3.org/2001/XMLSchema#nonNegativeInteger">1</owl:cardinality>
  </rdf:Description>
  <rdf:Description rdf:about="https://w3id.org/tern/ontologies/tern/Spectroradiometer">
    <rdfs:seeAlso rdf:resource="https://en.wikipedia.org/wiki/Spectroradiometer"/>
    <rdf:type rdf:resource="http://www.w3.org/2002/07/owl#Class"/>
    <rdfs:comment>A spectroradiometer is a light measurement tool that is able to measure both the wavelength and amplitude of the light emitted from a light source.</rdfs:comment>
    <rdfs:subClassOf rdf:resource="https://w3id.org/tern/ontologies/tern/Sensor"/>
    <rdfs:label>Spectroradiometer</rdfs:label>
  </rdf:Description>
  <rdf:Description rdf:nodeID="ub1bL900C19">
    <owl:onProperty rdf:resource="https://w3id.org/tern/ontologies/loc/longitude"/>
    <rdf:type rdf:resource="http://www.w3.org/2002/07/owl#Restriction"/>
    <owl:onClass rdf:resource="http://linked.data.gov.au/def/datatype/QuantitativeMeasure"/>
    <owl:qualifiedCardinality rdf:datatype="http://www.w3.org/2001/XMLSchema#nonNegativeInteger">1</owl:qualifiedCardinality>
  </rdf:Description>
  <rdf:Description rdf:nodeID="ub1bL344C19">
    <owl:onProperty rdf:resource="http://purl.org/dc/terms/description"/>
    <rdf:type rdf:resource="http://www.w3.org/2002/07/owl#Restriction"/>
    <owl:allValuesFrom rdf:resource="http://www.w3.org/2001/XMLSchema#string"/>
  </rdf:Description>
  <rdf:Description rdf:about="https://w3id.org/tern/ontologies/tern/scope">
    <rdfs:label>scope</rdfs:label>
    <rdf:type rdf:resource="http://www.w3.org/2002/07/owl#DatatypeProperty"/>
    <rdfs:range rdf:resource="http://www.w3.org/2001/XMLSchema#string"/>
    <skos:definition>Describe the scope of something.</skos:definition>
  </rdf:Description>
  <rdf:Description rdf:about="https://w3id.org/tern/ontologies/tern/taxon">
    <rdfs:label>taxon</rdfs:label>
    <rdf:type rdf:resource="http://www.w3.org/1999/02/22-rdf-syntax-ns#Property"/>
    <skos:scopeNote>Value should be from a controlled vocabulary identified by a URI.</skos:scopeNote>
    <skos:definition>Taxon classification.</skos:definition>
  </rdf:Description>
  <rdf:Description rdf:nodeID="fe114e3c19c6e4b2e8a8d1297357cbc21b13">
    <rdf:rest rdf:resource="http://www.w3.org/1999/02/22-rdf-syntax-ns#nil"/>
    <rdf:first rdf:resource="https://w3id.org/tern/ontologies/loc/Polygon"/>
  </rdf:Description>
  <rdf:Description rdf:about="https://w3id.org/tern/ontologies/tern/locationDescription">
    <skos:definition>The description of the location.</skos:definition>
    <rdf:type rdf:resource="http://www.w3.org/1999/02/22-rdf-syntax-ns#Property"/>
    <rdfs:label>location description</rdfs:label>
  </rdf:Description>
  <rdf:Description rdf:nodeID="ub1bL762C19">
    <owl:allValuesFrom rdf:resource="https://w3id.org/tern/ontologies/tern/Observation"/>
    <owl:onProperty rdf:resource="http://www.w3.org/ns/sosa/isFeatureOfInterestOf"/>
    <rdf:type rdf:resource="http://www.w3.org/2002/07/owl#Restriction"/>
  </rdf:Description>
  <rdf:Description rdf:nodeID="ub1bL723C25">
    <rdf:type rdf:resource="http://www.w3.org/2002/07/owl#Class"/>
    <owl:unionOf rdf:nodeID="fe114e3c19c6e4b2e8a8d1297357cbc21b10"/>
  </rdf:Description>
  <rdf:Description rdf:nodeID="fe114e3c19c6e4b2e8a8d1297357cbc21b9">
    <rdf:first rdf:resource="http://www.w3.org/2002/07/owl#Ontology"/>
    <rdf:rest rdf:resource="http://www.w3.org/1999/02/22-rdf-syntax-ns#nil"/>
  </rdf:Description>
  <rdf:Description rdf:nodeID="ub1bL976C19">
    <owl:allValuesFrom rdf:nodeID="ub1bL978C25"/>
    <rdf:type rdf:resource="http://www.w3.org/2002/07/owl#Restriction"/>
    <owl:onProperty rdf:resource="http://www.opengis.net/ont/geosparql#hasGeometry"/>
  </rdf:Description>
  <rdf:Description rdf:about="http://linked.data.gov.au/def/datatype/Text">
    <rdfs:subClassOf rdf:resource="https://w3id.org/tern/ontologies/tern/Result"/>
  </rdf:Description>
</rdf:RDF>
