<?xml version="1.0" encoding="UTF-8"?>
<rdf:RDF
   xmlns:dcterms="http://purl.org/dc/terms/"
   xmlns:doap="http://usefulinc.com/ns/doap#"
   xmlns:owl="http://www.w3.org/2002/07/owl#"
   xmlns:prov="http://www.w3.org/ns/prov#"
   xmlns:rdf="http://www.w3.org/1999/02/22-rdf-syntax-ns#"
   xmlns:rdfs="http://www.w3.org/2000/01/rdf-schema#"
   xmlns:schema-https="https://schema.org/"
   xmlns:skos="http://www.w3.org/2004/02/skos/core#"
>
  <rdf:Description rdf:nodeID="ub1bL568C19">
    <owl:onProperty rdf:resource="https://w3id.org/tern/ontologies/tern/site"/>
    <owl:maxQualifiedCardinality rdf:datatype="http://www.w3.org/2001/XMLSchema#nonNegativeInteger">1</owl:maxQualifiedCardinality>
    <owl:onClass rdf:resource="https://w3id.org/tern/ontologies/tern/Site"/>
    <rdf:type rdf:resource="http://www.w3.org/2002/07/owl#Restriction"/>
  </rdf:Description>
  <rdf:Description rdf:about="https://w3id.org/tern/ontologies/tern/SiteVisit">
    <rdfs:label>Site Visit</rdfs:label>
    <rdf:type rdf:resource="http://www.w3.org/2002/07/owl#Class"/>
    <rdfs:subClassOf rdf:nodeID="ub1bL1275C19"/>
    <rdfs:subClassOf rdf:nodeID="ub1bL1235C19"/>
    <rdfs:subClassOf rdf:nodeID="ub1bL1225C19"/>
    <rdfs:subClassOf rdf:nodeID="ub1bL1269C19"/>
    <rdfs:subClassOf rdf:nodeID="ub1bL1240C19"/>
    <rdfs:subClassOf rdf:nodeID="ub1bL1215C19"/>
    <rdfs:subClassOf rdf:resource="http://www.w3.org/ns/prov#Activity"/>
    <rdfs:subClassOf rdf:nodeID="ub1bL1257C19"/>
    <rdfs:subClassOf rdf:nodeID="ub1bL1220C19"/>
    <rdfs:subClassOf rdf:nodeID="ub1bL1230C19"/>
    <skos:definition>A discrete time-bounded visit to a site, during which sampling or observation activities are undertaken.</skos:definition>
    <rdfs:subClassOf rdf:nodeID="ub1bL1263C19"/>
    <rdfs:subClassOf rdf:nodeID="ub1bL1251C19"/>
  </rdf:Description>
  <rdf:Description rdf:about="https://w3id.org/tern/ontologies/tern/DigitalCamera">
    <skos:definition>The model as defined by the manufacturer.</skos:definition>
    <rdfs:subClassOf rdf:nodeID="ub1bL257C19"/>
    <rdfs:subClassOf rdf:nodeID="ub1bL237C19"/>
    <rdfs:subClassOf rdf:resource="https://w3id.org/tern/ontologies/tern/Sampler"/>
    <rdfs:subClassOf rdf:nodeID="ub1bL247C19"/>
    <rdfs:subClassOf rdf:nodeID="ub1bL263C19"/>
    <rdfs:subClassOf rdf:nodeID="ub1bL252C19"/>
    <rdfs:subClassOf rdf:nodeID="ub1bL242C19"/>
    <skos:example>E.g. EOS 350D</skos:example>
    <rdf:type rdf:resource="http://www.w3.org/2002/07/owl#Class"/>
    <rdfs:label>Digital Camera</rdfs:label>
    <rdfs:subClassOf rdf:resource="http://www.w3.org/2004/02/skos/core#Concept"/>
  </rdf:Description>
  <rdf:Description rdf:about="https://w3id.org/tern/ontologies/tern/hasSubActivity">
    <rdf:type rdf:resource="http://www.w3.org/1999/02/22-rdf-syntax-ns#Property"/>
    <rdfs:label>has sub activity</rdfs:label>
    <skos:definition>Link to an [Observation](#Observation) or [Sampling](#Sampling).</skos:definition>
  </rdf:Description>
  <rdf:Description rdf:nodeID="ub1bL574C19">
    <owl:onClass rdf:resource="https://w3id.org/tern/ontologies/tern/SiteVisit"/>
    <owl:maxQualifiedCardinality rdf:datatype="http://www.w3.org/2001/XMLSchema#nonNegativeInteger">1</owl:maxQualifiedCardinality>
    <owl:onProperty rdf:resource="https://w3id.org/tern/ontologies/tern/isSubActivityOf"/>
    <rdf:type rdf:resource="http://www.w3.org/2002/07/owl#Restriction"/>
  </rdf:Description>
  <rdf:Description rdf:about="http://linked.data.gov.au/def/datatype/Concept">
    <rdfs:subClassOf rdf:nodeID="ub1bL50C19"/>
    <rdfs:subClassOf rdf:resource="https://w3id.org/tern/ontologies/tern/Result"/>
    <rdfs:subClassOf rdf:nodeID="ub1bL45C19"/>
    <rdf:type rdf:resource="http://www.w3.org/2002/07/owl#Class"/>
  </rdf:Description>
  <rdf:Description rdf:about="https://w3id.org/tern/ontologies/tern/Dimension">
    <rdfs:label>Dimension</rdfs:label>
    <skos:definition>The dimension of a 2D square or rectangular feature. Example, the dimension of a rectangular plot [Site](#EcologicalSite). This class should perhaps have specialised classes to express not just square or rectangular features but also others such as circular features.</skos:definition>
    <rdfs:subClassOf rdf:nodeID="ub1bL302C19"/>
    <rdfs:subClassOf rdf:nodeID="ub1bL286C19"/>
    <rdfs:subClassOf rdf:nodeID="ub1bL307C19"/>
    <rdf:type rdf:resource="http://www.w3.org/2002/07/owl#Class"/>
    <rdfs:subClassOf rdf:nodeID="ub1bL275C19"/>
    <rdfs:subClassOf rdf:nodeID="ub1bL297C19"/>
  </rdf:Description>
  <rdf:Description rdf:nodeID="ub1bL1263C19">
    <rdf:type rdf:resource="http://www.w3.org/2002/07/owl#Restriction"/>
    <owl:onClass rdf:resource="http://www.w3.org/2001/XMLSchema#string"/>
    <owl:qualifiedCardinality rdf:datatype="http://www.w3.org/2001/XMLSchema#nonNegativeInteger">1</owl:qualifiedCardinality>
    <owl:onProperty rdf:resource="http://purl.org/dc/terms/identifier"/>
  </rdf:Description>
  <rdf:Description rdf:about="https://w3id.org/tern/ontologies/tern/SamplingPoint">
    <rdfs:subClassOf rdf:nodeID="ub1bL933C19"/>
    <skos:definition>A point in space where an [Observation](#Observation) or [Sampling](#Sampling) occurred. </skos:definition>
    <rdf:type rdf:resource="http://www.w3.org/2002/07/owl#Class"/>
    <rdfs:label>Sampling Point</rdfs:label>
    <rdfs:subClassOf rdf:nodeID="ub1bL945C19"/>
    <rdfs:subClassOf rdf:nodeID="ub1bL939C19"/>
    <rdfs:subClassOf rdf:nodeID="ub1bL951C19"/>
    <rdfs:subClassOf rdf:resource="https://w3id.org/tern/ontologies/loc/Point"/>
    <rdfs:subClassOf rdf:nodeID="ub1bL963C19"/>
    <rdfs:subClassOf rdf:nodeID="ub1bL969C19"/>
    <rdfs:subClassOf rdf:nodeID="ub1bL975C19"/>
    <rdfs:subClassOf rdf:nodeID="ub1bL957C19"/>
  </rdf:Description>
  <rdf:Description rdf:about="https://w3id.org/tern/ontologies/tern/CORVEGSite">
    <skos:definition>A [CORVEG Site](#CORVEGSite) refers to a study location in Queensland that was visited since 1982 to collect data on physical and vegetation features, including structural and floristic attributes as well as descriptions of its landscape, soil and geological features.</skos:definition>
    <skos:example rdf:resource="http://linked.data.gov.au/dataset/corveg/site-12319"/>
    <skos:seeAlso rdf:resource="http://aekos.org.au/collection/qld.gov.au/corveg"/>
    <rdfs:label>CORVEG Site</rdfs:label>
    <dcterms:source rdf:resource="https://www.data.qld.gov.au/dataset/queensland-corveg-database"/>
    <rdfs:subClassOf rdf:resource="https://w3id.org/tern/ontologies/tern/Site"/>
    <rdf:type rdf:resource="http://www.w3.org/2002/07/owl#Class"/>
  </rdf:Description>
  <rdf:Description rdf:about="https://w3id.org/tern/ontologies/tern/domain">
    <rdf:type rdf:resource="http://www.w3.org/1999/02/22-rdf-syntax-ns#Property"/>
    <skos:definition>The domain of the observation.</skos:definition>
    <rdfs:label>domain</rdfs:label>
    <skos:example>Vegetation, soil, disturbance, landform, etc.</skos:example>
  </rdf:Description>
  <rdf:Description rdf:about="https://w3id.org/tern/ontologies/tern/soilClassification">
    <rdf:type rdf:resource="http://www.w3.org/1999/02/22-rdf-syntax-ns#Property"/>
    <rdfs:label>soil classification</rdfs:label>
    <skos:definition>The term used to classify the SoilProfile.</skos:definition>
  </rdf:Description>
  <rdf:Description rdf:nodeID="ub1bL263C19">
    <owl:onClass rdf:resource="http://www.w3.org/2001/XMLSchema#string"/>
    <rdf:type rdf:resource="http://www.w3.org/2002/07/owl#Restriction"/>
    <owl:onProperty rdf:resource="http://schema.org/manufacturer"/>
    <owl:minQualifiedCardinality rdf:datatype="http://www.w3.org/2001/XMLSchema#nonNegativeInteger">1</owl:minQualifiedCardinality>
  </rdf:Description>
  <rdf:Description rdf:nodeID="ub1bL297C19">
    <rdf:type rdf:resource="http://www.w3.org/2002/07/owl#Restriction"/>
    <owl:cardinality rdf:datatype="http://www.w3.org/2001/XMLSchema#nonNegativeInteger">1</owl:cardinality>
    <owl:onProperty rdf:resource="https://w3id.org/tern/ontologies/tern/length"/>
  </rdf:Description>
  <rdf:Description rdf:nodeID="ub1bL1193C19">
    <owl:onClass rdf:resource="https://w3id.org/tern/ontologies/sd/StateTaxon"/>
    <owl:onProperty rdf:resource="https://w3id.org/tern/ontologies/tern/taxon"/>
    <owl:qualifiedCardinality rdf:datatype="http://www.w3.org/2001/XMLSchema#nonNegativeInteger">1</owl:qualifiedCardinality>
    <rdf:type rdf:resource="http://www.w3.org/2002/07/owl#Restriction"/>
  </rdf:Description>
  <rdf:Description rdf:about="https://w3id.org/tern/ontologies/tern/dateCommissioned">
    <skos:example>1 August 2017 is the date commisioned of the 
[Collie flux station](http://ozflux.org.au/monitoringsites/collie/index.html)</skos:example>
    <rdfs:label>date commissioned</rdfs:label>
    <skos:definition>The date when, e.g., a [Site](#EcologicalSite) is ready to commence its operations, after it is successfully installed and tested.</skos:definition>
    <rdf:type rdf:resource="http://www.w3.org/1999/02/22-rdf-syntax-ns#Property"/>
    <skos:scopeNote>Use ISO 8601 international standard for representing dates and times. Missing start date may be set to the first of the month.</skos:scopeNote>
  </rdf:Description>
  <rdf:Description rdf:nodeID="ub1bL969C19">
    <owl:onClass rdf:resource="http://linked.data.gov.au/def/datatype/QuantitativeMeasure"/>
    <owl:onProperty rdf:resource="https://w3id.org/tern/ontologies/loc/longitude"/>
    <rdf:type rdf:resource="http://www.w3.org/2002/07/owl#Restriction"/>
    <owl:qualifiedCardinality rdf:datatype="http://www.w3.org/2001/XMLSchema#nonNegativeInteger">1</owl:qualifiedCardinality>
  </rdf:Description>
  <rdf:Description rdf:nodeID="ub1bL486C19">
    <owl:onClass rdf:resource="http://www.w3.org/2001/XMLSchema#string"/>
    <rdf:type rdf:resource="http://www.w3.org/2002/07/owl#Restriction"/>
    <owl:qualifiedCardinality rdf:datatype="http://www.w3.org/2001/XMLSchema#nonNegativeInteger">1</owl:qualifiedCardinality>
    <owl:onProperty rdf:resource="http://www.w3.org/2004/02/skos/core#prefLabel"/>
  </rdf:Description>
  <rdf:Description rdf:nodeID="ub1bL734C19">
    <rdf:type rdf:resource="http://www.w3.org/2002/07/owl#Restriction"/>
    <owl:allValuesFrom rdf:resource="http://www.w3.org/2001/XMLSchema#string"/>
    <owl:onProperty rdf:resource="http://schema.org/description"/>
  </rdf:Description>
  <rdf:Description rdf:about="https://w3id.org/tern/ontologies/tern/EarthObservationSatellite">
    <rdfs:label>Earth Observation Satellite</rdfs:label>
    <rdfs:seeAlso rdf:resource="https://gcmd.earthdata.nasa.gov/kms/concept/3466eed1-2fbb-49bf-ab0b-dc08731d502b"/>
    <rdf:type rdf:resource="http://www.w3.org/2002/07/owl#Class"/>
    <rdfs:subClassOf rdf:resource="https://w3id.org/tern/ontologies/tern/MobilePlatform"/>
    <skos:definition>Earth observation satellites are satellites specifically designed to observe Earth from orbit, similar to spy satellites but intended for non-military uses such as environmental monitoring, meteorology, map making etc. Source: Wikipedia, http://en.wikipedia.org/wiki/Earth_observation_satellite Group: Platform_Details Entry_ID: Earth Observation Satellites Group: Platform_Identification Platform_Category: Earth Observation Satellites Short_Name: Earth Observation Satellites End_Group End_Group</skos:definition>
  </rdf:Description>
  <rdf:Description rdf:about="https://w3id.org/tern/ontologies/tern/globalMatch">
    <skos:scopeNote>Use in between controlled vocabularies.</skos:scopeNote>
    <rdfs:subPropertyOf rdf:resource="http://www.w3.org/2004/02/skos/core#exactMatch"/>
    <rdf:type rdf:resource="http://www.w3.org/1999/02/22-rdf-syntax-ns#Property"/>
    <rdfs:label>global match</rdfs:label>
    <skos:definition>Link a concept to an upper concept (in the closed system).</skos:definition>
    <owl:inverseOf rdf:resource="https://w3id.org/tern/ontologies/tern/isGlobalMatchOf"/>
  </rdf:Description>
  <rdf:Description rdf:nodeID="ub1bL462C19">
    <rdf:type rdf:resource="http://www.w3.org/2002/07/owl#Restriction"/>
    <owl:onProperty rdf:resource="https://w3id.org/tern/ontologies/tern/equipment"/>
    <owl:maxQualifiedCardinality rdf:datatype="http://www.w3.org/2001/XMLSchema#nonNegativeInteger">1</owl:maxQualifiedCardinality>
    <owl:onDataRange rdf:resource="http://www.w3.org/2001/XMLSchema#string"/>
  </rdf:Description>
  <rdf:Description rdf:about="https://w3id.org/tern/ontologies/tern/FluxTower">
    <rdf:type rdf:resource="http://www.w3.org/2002/07/owl#Class"/>
    <rdfs:subClassOf rdf:nodeID="ub1bL380C19"/>
    <skos:example rdf:resource="https://w3id.org/tern/resources/fd2809a2-e705-4961-b09c-7e9ae1ffa87e"/>
    <rdfs:label>Flux Tower</rdfs:label>
    <rdfs:subClassOf rdf:nodeID="ub1bL386C19"/>
    <skos:definition>Across the globe, towers stand among the landscape, with sensors monitoring these eddies for carbon dioxide, water vapor and other gasses.  These so-called flux towers collect data on carbon dioxide exchange rates between the earth and atmosphere.</skos:definition>
    <rdfs:subClassOf rdf:nodeID="ub1bL398C19"/>
    <rdfs:subClassOf rdf:resource="https://w3id.org/tern/ontologies/tern/FixedPlatform"/>
    <rdfs:subClassOf rdf:nodeID="ub1bL392C19"/>
    <rdfs:subClassOf rdf:nodeID="ub1bL363C19"/>
    <rdfs:subClassOf rdf:nodeID="ub1bL358C19"/>
    <rdfs:subClassOf rdf:nodeID="ub1bL368C19"/>
    <skos:example>Alice Springs Mulga flux tower</skos:example>
    <rdfs:subClassOf rdf:nodeID="ub1bL374C19"/>
  </rdf:Description>
  <rdf:Description rdf:nodeID="ub1bL1040C19">
    <rdf:type rdf:resource="http://www.w3.org/2002/07/owl#Restriction"/>
    <owl:onProperty rdf:resource="https://w3id.org/tern/ontologies/tern/siteVisit"/>
    <owl:allValuesFrom rdf:resource="https://w3id.org/tern/ontologies/tern/SiteVisit"/>
  </rdf:Description>
  <rdf:Description rdf:nodeID="ub1bL1275C19">
    <rdf:type rdf:resource="http://www.w3.org/2002/07/owl#Restriction"/>
    <owl:onProperty rdf:resource="https://w3id.org/tern/ontologies/tern/site"/>
    <owl:qualifiedCardinality rdf:datatype="http://www.w3.org/2001/XMLSchema#nonNegativeInteger">1</owl:qualifiedCardinality>
    <owl:onClass rdf:resource="https://w3id.org/tern/ontologies/tern/Site"/>
  </rdf:Description>
  <rdf:Description rdf:nodeID="ub1bL1363C19">
    <owl:onProperty rdf:resource="https://w3id.org/tern/ontologies/tern/transectEndPoint"/>
    <owl:qualifiedCardinality rdf:datatype="http://www.w3.org/2001/XMLSchema#nonNegativeInteger">1</owl:qualifiedCardinality>
    <owl:onClass rdf:resource="https://w3id.org/tern/ontologies/loc/Point"/>
    <rdf:type rdf:resource="http://www.w3.org/2002/07/owl#Restriction"/>
  </rdf:Description>
  <rdf:Description rdf:about="https://w3id.org/tern/ontologies/tern/centroidPoint">
    <rdfs:label>centroid point</rdfs:label>
    <rdfs:subPropertyOf rdf:resource="http://www.opengis.net/ont/geosparql#hasGeometry"/>
    <rdf:type rdf:resource="http://www.w3.org/1999/02/22-rdf-syntax-ns#Property"/>
    <skos:definition>The centroid point of an object-of-interest.</skos:definition>
    <skos:example>The geometric center of 1-ha vegetation plot expressed 
as [tern-loc:Point](https://w3id.org/tern/ontologies/loc/Point).</skos:example>
    <rdfs:seeAlso rdf:resource="https://en.wikipedia.org/wiki/List_of_centroids"/>
    <rdfs:range rdf:resource="https://w3id.org/tern/ontologies/loc/Point"/>
  </rdf:Description>
  <rdf:Description rdf:about="https://w3id.org/tern/ontologies/tern/SiteStratumTaxon">
    <rdfs:subClassOf rdf:nodeID="ub1bL1187C19"/>
    <rdfs:subClassOf rdf:resource="https://w3id.org/tern/ontologies/tern/Sample"/>
    <rdf:type rdf:resource="http://www.w3.org/2002/07/owl#Class"/>
    <rdfs:subClassOf rdf:nodeID="ub1bL1193C19"/>
    <rdfs:label>Site Stratum Taxon</rdfs:label>
    <rdfs:subClassOf rdf:nodeID="ub1bL1181C19"/>
  </rdf:Description>
  <rdf:Description rdf:about="https://w3id.org/tern/ontologies/tern/hasCategoricalCollection">
    <rdfs:label>has categorical collection</rdfs:label>
    <skos:definition>A property that links a concept to a collection containing its categorical values.</skos:definition>
    <rdf:type rdf:resource="http://www.w3.org/1999/02/22-rdf-syntax-ns#Property"/>
  </rdf:Description>
  <rdf:Description rdf:about="https://w3id.org/tern/ontologies/tern/dimension">
    <skos:definition>A property that links, e.g., a [Site](#EcologicalSite) to its [Dimension](#Dimension).</skos:definition>
    <rdfs:label>dimension</rdfs:label>
    <rdf:type rdf:resource="http://www.w3.org/1999/02/22-rdf-syntax-ns#Property"/>
  </rdf:Description>
  <rdf:Description rdf:about="https://w3id.org/tern/ontologies/tern/Method">
    <skos:example>Borehole logging is a field method in which 
in situ physical measurements (e.g., temperature) are made down the 
length of a borehole by lowering measurement instruments down the borehole via cable. (Credit: PaST Thesaurus)</skos:example>
    <rdfs:subClassOf rdf:resource="http://www.w3.org/2004/02/skos/core#Concept"/>
    <skos:definition>A Method describes in detailed steps how a workflow, protocol, plan or algorithm is carried out to make an [Observation](#Observation) or a [Sample](#Sample). It explains the steps to be carried out to arrive at reproducible [Result](#Result).</skos:definition>
    <rdfs:subClassOf rdf:nodeID="ub1bL486C19"/>
    <rdfs:label>Method</rdfs:label>
    <rdfs:scopeNote>We recommend representing the method information following [ISO 9001 Processes, Procedures and Work Instructions](https://3yn1j14c4twk1bmdg82226en-wpengine.netdna-ssl.com/wp-content/uploads/2016/08/iso-9001-procedure.pdf)</rdfs:scopeNote>
    <rdfs:subClassOf rdf:nodeID="ub1bL462C19"/>
    <rdfs:subClassOf rdf:nodeID="ub1bL468C19"/>
    <rdfs:subClassOf rdf:nodeID="ub1bL480C19"/>
    <rdf:type rdf:resource="http://www.w3.org/2002/07/owl#Class"/>
    <rdfs:seeAlso rdf:resource="https://apps.usgs.gov/thesaurus/term-simple.php?thcode=2&amp;code=376"/>
    <rdfs:subClassOf rdf:nodeID="ub1bL474C19"/>
    <rdfs:subClassOf rdf:nodeID="ub1bL445C19"/>
    <rdfs:seeAlso rdf:resource="https://the9000store.com/iso-9001-2015-requirements/iso-9001-2015-context-of-the-organization/processes-procedures-work-instructions/"/>
    <rdfs:subClassOf rdf:nodeID="ub1bL456C19"/>
  </rdf:Description>
  <rdf:Description rdf:about="https://w3id.org/tern/ontologies/tern/MobilePlatform">
    <rdfs:subClassOf rdf:resource="https://w3id.org/tern/ontologies/tern/Platform"/>
    <rdfs:label>Mobile Platform</rdfs:label>
    <skos:definition>A moving mobile platform on land, in water or in space.</skos:definition>
    <rdf:type rdf:resource="http://www.w3.org/2002/07/owl#Class"/>
  </rdf:Description>
  <rdf:Description rdf:nodeID="ub1bL516C25">
    <rdf:type rdf:resource="http://www.w3.org/2002/07/owl#Class"/>
    <owl:unionOf rdf:nodeID="fcf4ebf340cd54dc4871b974b242da6f5b7"/>
  </rdf:Description>
  <rdf:Description rdf:about="https://w3id.org/tern/ontologies/tern/Site">
    <rdf:type rdf:resource="http://www.w3.org/2002/07/owl#Class"/>
    <rdfs:subClassOf rdf:nodeID="ub1bL1114C19"/>
    <rdfs:subClassOf rdf:nodeID="ub1bL1030C19"/>
    <rdfs:subClassOf rdf:nodeID="ub1bL1078C19"/>
    <rdfs:subClassOf rdf:nodeID="ub1bL1020C19"/>
    <rdfs:subClassOf rdf:nodeID="ub1bL1005C19"/>
    <rdfs:subClassOf rdf:nodeID="ub1bL1045C19"/>
    <rdfs:subClassOf rdf:nodeID="ub1bL1143C19"/>
    <rdfs:subClassOf rdf:nodeID="ub1bL1056C19"/>
    <rdfs:subClassOf rdf:nodeID="ub1bL1126C19"/>
    <rdfs:label>Ecological Site</rdfs:label>
    <rdfs:subClassOf rdf:nodeID="ub1bL1120C19"/>
    <rdfs:subClassOf rdf:resource="https://w3id.org/tern/ontologies/tern/Sample"/>
    <rdfs:subClassOf rdf:nodeID="ub1bL1035C19"/>
    <rdfs:subClassOf rdf:nodeID="ub1bL1072C19"/>
    <skos:scopeNote>Use [dcterms:hasPart](http://purl.org/dc/terms/hasPart) and [dcterms:isPartOf](http://purl.org/dc/terms/isPartOf) to model [Site](#EcologicalSite) and [Subsite](#EcologicalSite) relationships. E.g. In TERN, there are SuperSites that contain multiple core 1 ha subsites.</skos:scopeNote>
    <rdfs:subClassOf rdf:nodeID="ub1bL1015C19"/>
    <rdfs:subClassOf rdf:resource="https://w3id.org/tern/ontologies/tern/Platform"/>
    <rdfs:subClassOf rdf:nodeID="ub1bL1084C19"/>
    <rdfs:subClassOf rdf:nodeID="ub1bL1102C19"/>
    <rdfs:subClassOf rdf:nodeID="ub1bL1108C19"/>
    <rdfs:subClassOf rdf:nodeID="ub1bL1096C19"/>
    <rdfs:subClassOf rdf:nodeID="ub1bL1061C19"/>
    <rdfs:subClassOf rdf:nodeID="ub1bL1066C19"/>
    <rdfs:subClassOf rdf:nodeID="ub1bL1040C19"/>
    <rdfs:subClassOf rdf:nodeID="ub1bL1131C19"/>
    <skos:definition>Location where observations may be made. This is a subclass of [Sample](#Sample) because a site should be designed to be representative of an environmental system (which may be an ecosystem or bioregion) or zone (which may be a zone such as a parcel or tract).</skos:definition>
    <rdfs:subClassOf rdf:nodeID="ub1bL1137C19"/>
    <rdfs:subClassOf rdf:nodeID="ub1bL1025C19"/>
    <rdfs:subClassOf rdf:nodeID="ub1bL1090C19"/>
    <skos:example>Ausplots Rangelands Site 59858 (Site Name: WAACOO0011)</skos:example>
    <rdfs:subClassOf rdf:nodeID="ub1bL1149C19"/>
    <rdfs:subClassOf rdf:nodeID="ub1bL1010C19"/>
  </rdf:Description>
  <rdf:Description rdf:about="https://w3id.org/tern/ontologies/tern/AffiliateSuperSite">
    <skos:example rdf:resource="https://w3id.org/tern/resources/a05a51c0-2daa-4369-aa2b-08c3638efa7a"/>
    <skos:example>Samford Peri-urban Affiliate SuperSite</skos:example>
    <rdfs:seeAlso rdf:resource="https://supersites.tern.org.au/"/>
    <rdfs:label>Affiliate SuperSite</rdfs:label>
    <rdf:type rdf:resource="http://www.w3.org/2002/07/owl#Class"/>
    <rdfs:subClassOf rdf:resource="https://w3id.org/tern/ontologies/tern/SuperSite"/>
  </rdf:Description>
  <rdf:Description rdf:nodeID="ub1bL1181C19">
    <owl:minQualifiedCardinality rdf:datatype="http://www.w3.org/2001/XMLSchema#nonNegativeInteger">1</owl:minQualifiedCardinality>
    <owl:onClass rdf:resource="https://w3id.org/tern/ontologies/tern/SiteStratum"/>
    <owl:onProperty rdf:resource="http://www.w3.org/ns/sosa/isSampleOf"/>
    <rdf:type rdf:resource="http://www.w3.org/2002/07/owl#Restriction"/>
  </rdf:Description>
  <rdf:Description rdf:about="https://w3id.org/tern/ontologies/tern/observationTheme">
    <rdfs:subPropertyOf rdf:resource="http://purl.org/dc/terms/type"/>
    <skos:definition>Group observations into themes. See TERN's controlled list of &lt;a href="http://linked.data.gov.au/def/tern-cv/396192ae-3bd5-4050-b578-93107510129c"&gt;observation themes&lt;/a&gt; as example values.</skos:definition>
    <rdf:type rdf:resource="http://www.w3.org/1999/02/22-rdf-syntax-ns#Property"/>
    <rdfs:label>observation theme</rdfs:label>
    <rdfs:domain rdf:resource="https://w3id.org/tern/ontologies/tern/Observation"/>
  </rdf:Description>
  <rdf:Description rdf:about="https://w3id.org/tern/ontologies/tern/polygon">
    <skos:definition>The polygon of the subject.</skos:definition>
    <rdfs:label>polygon</rdfs:label>
    <rdfs:range rdf:resource="https://w3id.org/tern/ontologies/loc/Polygon"/>
    <rdfs:subPropertyOf rdf:resource="http://www.opengis.net/ont/geosparql#hasGeometry"/>
    <rdf:type rdf:resource="http://www.w3.org/1999/02/22-rdf-syntax-ns#Property"/>
  </rdf:Description>
  <rdf:Description rdf:about="https://w3id.org/tern/ontologies/tern/ObservationTheme">
    <skos:example>Field observations can be categorized into themes 
such as vegetation communities, landscape features, 
soil features and fauna populations.</skos:example>
    <rdf:type rdf:resource="http://www.w3.org/2002/07/owl#Class"/>
    <rdfs:subClassOf rdf:resource="http://www.w3.org/2004/02/skos/core#Concept"/>
    <skos:scopeNote>This concept is more commonly used at the application level and is usually mappable to a [FeatureOfInterest](http://w3.org/ns/sosa/FeatureOfInterest).</skos:scopeNote>
    <rdfs:label>Observation Theme</rdfs:label>
    <skos:definition>An [Observation Theme](#ObservationTheme) categorises [Parameters](#Parameter) (i.e., properties observed) based on a topic of interest.</skos:definition>
  </rdf:Description>
  <rdf:Description rdf:nodeID="ub1bL110C23">
    <schema-https:name>Mosheh Eliyahu</schema-https:name>
    <schema-https:affiliation rdf:resource="https://w3id.org/tern/resources/a083902d-d821-41be-b663-1d7cb33eea66"/>
    <schema-https:email>mosheh.eliyahu@adelaide.edu.au</schema-https:email>
    <rdf:type rdf:resource="https://schema.org/Person"/>
  </rdf:Description>
  <rdf:Description rdf:about="https://w3id.org/tern/ontologies/tern/transectStartPoint">
    <rdfs:label>transect start point</rdfs:label>
    <rdf:type rdf:resource="http://www.w3.org/1999/02/22-rdf-syntax-ns#Property"/>
    <rdfs:domain rdf:resource="https://w3id.org/tern/ontologies/tern/Transect"/>
    <skos:definition>Refers to the [tern-loc:Point](https://w3id.org/tern/ontologies/loc/Point) representing the start of a transect.</skos:definition>
  </rdf:Description>
  <rdf:Description rdf:nodeID="fcf4ebf340cd54dc4871b974b242da6f5b18">
    <rdf:rest rdf:nodeID="fcf4ebf340cd54dc4871b974b242da6f5b19"/>
    <rdf:first rdf:resource="http://www.w3.org/2001/XMLSchema#string"/>
  </rdf:Description>
  <rdf:Description rdf:nodeID="ub1bL1072C19">
    <rdf:type rdf:resource="http://www.w3.org/2002/07/owl#Restriction"/>
    <owl:onClass rdf:resource="http://www.w3.org/2001/XMLSchema#date"/>
    <owl:maxQualifiedCardinality rdf:datatype="http://www.w3.org/2001/XMLSchema#nonNegativeInteger">1</owl:maxQualifiedCardinality>
    <owl:onProperty rdf:resource="https://w3id.org/tern/ontologies/tern/dateDecommissioned"/>
  </rdf:Description>
  <rdf:Description rdf:about="https://w3id.org/tern/ontologies/tern/locationProcedure">
    <rdfs:label>location procedure</rdfs:label>
    <rdf:type rdf:resource="http://www.w3.org/1999/02/22-rdf-syntax-ns#Property"/>
    <rdfs:subPropertyOf rdf:resource="https://w3id.org/tern/ontologies/tern/hasMethod"/>
    <skos:definition>Link to a procedure used to obtain the location.</skos:definition>
  </rdf:Description>
  <rdf:Description rdf:about="https://w3id.org/tern/ontologies/tern/Observation">
    <skos:definition>Act of carrying out an (Observation) [Procedure](#Procedure) to estimate or calculate a value of a property of a [FeatureOfInterest](http://w3.org/ns/sosa/FeatureOfInterest). Links to a [Sensor](http://w3.org/ns/sosa/Sensor) to describe what made the [Observation](#Observation) and how; links to an [ObservableProperty](#ObservableProperty) to describe what the result is an estimate of, and to a [FeatureOfInterest](http://w3.org/ns/sosa/FeatureOfInterest) to detail what that property was associated with.</skos:definition>
    <rdfs:subClassOf rdf:nodeID="ub1bL580C19"/>
    <rdfs:subClassOf rdf:nodeID="ub1bL563C19"/>
    <rdfs:subClassOf rdf:nodeID="ub1bL568C19"/>
    <skos:example>The activity of measuring properties such as wind speed and direction by 
an anemometer sensor. The results of the observation are the measurement values 
of the properties estimated by the sensor.</skos:example>
    <rdfs:subClassOf rdf:nodeID="ub1bL586C19"/>
    <rdfs:subClassOf rdf:nodeID="ub1bL616C19"/>
    <rdfs:subClassOf rdf:nodeID="ub1bL610C19"/>
    <rdfs:subClassOf rdf:nodeID="ub1bL574C19"/>
    <rdfs:subClassOf rdf:nodeID="ub1bL598C19"/>
    <rdfs:subClassOf rdf:resource="http://www.w3.org/ns/prov#Activity"/>
    <rdfs:subClassOf rdf:nodeID="ub1bL592C19"/>
    <rdfs:subClassOf rdf:resource="http://www.w3.org/ns/sosa/Observation"/>
    <rdfs:label>Observation</rdfs:label>
    <rdfs:subClassOf rdf:nodeID="ub1bL558C19"/>
    <rdf:type rdf:resource="http://www.w3.org/2002/07/owl#Class"/>
    <rdfs:subClassOf rdf:nodeID="ub1bL604C19"/>
  </rdf:Description>
  <rdf:Description rdf:nodeID="ub1bL252C19">
    <owl:onProperty rdf:resource="http://www.w3.org/2004/02/skos/core#prefLabel"/>
    <rdf:type rdf:resource="http://www.w3.org/2002/07/owl#Restriction"/>
    <owl:minCardinality rdf:datatype="http://www.w3.org/2001/XMLSchema#nonNegativeInteger">1</owl:minCardinality>
  </rdf:Description>
  <rdf:Description rdf:about="http://linked.data.gov.au/def/datatype/Boolean">
    <rdfs:subClassOf rdf:resource="https://w3id.org/tern/ontologies/tern/Result"/>
  </rdf:Description>
  <rdf:Description rdf:nodeID="ub1bL716C19">
    <rdf:type rdf:resource="http://www.w3.org/2002/07/owl#Restriction"/>
    <owl:onProperty rdf:resource="http://www.w3.org/1999/02/22-rdf-syntax-ns#value"/>
    <owl:qualifiedCardinality rdf:datatype="http://www.w3.org/2001/XMLSchema#nonNegativeInteger">1</owl:qualifiedCardinality>
    <owl:onClass rdf:resource="https://w3id.org/tern/ontologies/tern/Method"/>
  </rdf:Description>
  <rdf:Description rdf:about="https://w3id.org/tern/ontologies/tern/">
    <owl:imports rdf:resource="https://raw.githubusercontent.com/AGLDWG/datatype-ont/master/rdf/datatype.rdf"/>
    <dcterms:creator rdf:nodeID="ub1bL122C19"/>
    <rdfs:seeAlso rdf:resource="https://www.publish.csiro.au/book/5230/"/>
    <rdf:type rdf:resource="http://www.w3.org/2002/07/owl#Ontology"/>
    <rdfs:seeAlso rdf:resource="https://www.w3.org/ns/ssn/"/>
    <owl:imports rdf:resource="http://www.w3.org/2006/time#"/>
    <owl:versionIRI rdf:resource="http://linked.data.gov.au/def/plot/0.2.0"/>
    <owl:imports rdf:resource="https://w3id.org/tern/ontologies/org/"/>
    <dcterms:contributor rdf:nodeID="ub1bL92C23"/>
    <owl:imports rdf:resource="http://www.w3.org/ns/prov#"/>
    <dcterms:creator rdf:nodeID="ub1bL136C19"/>
    <prov:wasGeneratedBy rdf:nodeID="ub1bL172C23"/>
    <dcterms:contributor rdf:nodeID="ub1bL110C23"/>
    <dcterms:license rdf:resource="http://creativecommons.org/publicdomain/zero/1.0/"/>
    <rdfs:comment>The TERN Ontology comprises a set of vocabularies for representing plot-based ecological data. It was developed primarily based on the SOSA (Sensor, Observation, Sample, and Actuator) ontology. The TERN Ontology's classes and properties have been tailored to describe terrestrial ecology survey data including flora, vegetation and soil, following the methodologies outlined in the Australian Soil and Land Survey Field Handbook.
  
  
  </rdfs:comment>
    <dcterms:contributor rdf:nodeID="ub1bL116C23"/>
    <dcterms:modified rdf:datatype="http://www.w3.org/2001/XMLSchema#date">2020-12-07</dcterms:modified>
    <owl:imports rdf:resource="https://w3id.org/tern/ontologies/loc/"/>
    <owl:imports rdf:resource="http://www.w3.org/ns/ssn/"/>
    <dcterms:contributor rdf:nodeID="ub1bL104C23"/>
    <rdfs:label>TERN Ontology</rdfs:label>
    <owl:imports rdf:resource="http://www.w3.org/2004/02/skos/core#"/>
    <dcterms:contributor rdf:nodeID="ub1bL98C23"/>
    <owl:versionInfo>0.2.0</owl:versionInfo>
    <owl:imports rdf:resource="http://www.w3.org/ns/dcat#"/>
    <owl:imports rdf:resource="http://datashapes.org/dash"/>
    <owl:imports rdf:resource="https://w3id.org/tern/ontologies/sd/"/>
    <rdfs:seeAlso rdf:resource="https://www.w3.org/TR/vocab-ssn-ext/"/>
    <dcterms:creator rdf:nodeID="ub1bL129C19"/>
    <dcterms:publisher rdf:resource="https://w3id.org/tern/resources/a083902d-d821-41be-b663-1d7cb33eea66"/>
    <owl:imports rdf:resource="http://www.w3.org/ns/sosa/"/>
    <owl:imports rdf:resource="http://qudt.org/schema/qudt/"/>
  </rdf:Description>
  <rdf:Description rdf:nodeID="ub1bL1025C19">
    <owl:allValuesFrom rdf:resource="https://w3id.org/tern/ontologies/tern/PropertyValue"/>
    <rdf:type rdf:resource="http://www.w3.org/2002/07/owl#Restriction"/>
    <owl:onProperty rdf:resource="http://schema.org/additionalProperty"/>
  </rdf:Description>
  <rdf:Description rdf:about="https://w3id.org/tern/ontologies/tern/siteDescription">
    <rdf:type rdf:resource="http://www.w3.org/1999/02/22-rdf-syntax-ns#Property"/>
    <skos:example rdf:resource="http://ozflux.org.au/monitoringsites/alicesprings/alicesprings_description.html"/>
    <rdfs:label>site description</rdfs:label>
    <skos:scopeNote>Value is usually a summary sentence of the site.</skos:scopeNote>
    <skos:definition>Contextual information is collected at each site. This includes measures of slope an aspect, surface strew and lithology, and information on the grazing and fire history of the site (Credit: TERN AusPlots).</skos:definition>
  </rdf:Description>
  <rdf:Description rdf:about="https://w3id.org/tern/ontologies/tern/SoilHorizon">
    <rdfs:subClassOf rdf:nodeID="ub1bL1292C19"/>
    <rdfs:subClassOf rdf:resource="https://w3id.org/tern/ontologies/tern/Sample"/>
    <rdf:type rdf:resource="http://www.w3.org/2002/07/owl#Class"/>
    <rdfs:label>Soil Horizon</rdfs:label>
    <skos:definition>A soil horizon is a layer of soil, approximately parallel to the land surface, with morphological properties different from layers below and/or above it. Tongues of material from one horizon may penetrate into adjacent horizons (Credit: Australian Soil and Land Survey Field Handbook).</skos:definition>
    <rdfs:subClassOf rdf:nodeID="ub1bL1297C19"/>
    <skos:example>C Horizon consists of weathering rock.</skos:example>
    <rdfs:subClassOf rdf:nodeID="ub1bL1287C19"/>
  </rdf:Description>
  <rdf:Description rdf:nodeID="ub1bL480C19">
    <rdf:type rdf:resource="http://www.w3.org/2002/07/owl#Restriction"/>
    <owl:onProperty rdf:resource="https://w3id.org/tern/ontologies/tern/scope"/>
    <owl:maxQualifiedCardinality rdf:datatype="http://www.w3.org/2001/XMLSchema#nonNegativeInteger">1</owl:maxQualifiedCardinality>
    <owl:onDataRange rdf:resource="http://www.w3.org/2001/XMLSchema#string"/>
  </rdf:Description>
  <rdf:Description rdf:nodeID="ub1bL843C19">
    <rdf:type rdf:resource="http://www.w3.org/2002/07/owl#Restriction"/>
    <owl:cardinality rdf:datatype="http://www.w3.org/2001/XMLSchema#nonNegativeInteger">1</owl:cardinality>
    <owl:onProperty rdf:resource="http://www.w3.org/2000/01/rdf-schema#label"/>
  </rdf:Description>
  <rdf:Description rdf:about="https://w3id.org/tern/ontologies/tern/SoilProfile">
    <rdfs:subClassOf rdf:resource="https://w3id.org/tern/ontologies/tern/Sample"/>
    <rdfs:label>Soil Profile</rdfs:label>
    <rdfs:subClassOf rdf:nodeID="ub1bL1309C19"/>
    <rdfs:subClassOf rdf:nodeID="ub1bL1314C19"/>
    <rdf:type rdf:resource="http://www.w3.org/2002/07/owl#Class"/>
    <skos:example rdf:resource="https://www.qld.gov.au/environment/land/management/soil/soil-explained/forms"/>
    <skos:definition>A soil profile is a vertical section of a soil from the soil surface through all its horizons to parent material, other consolidated substrate material or selected depth in unconsolidated material (Credit: Australian Soil and Land Survey Field Handbook).</skos:definition>
  </rdf:Description>
  <rdf:Description rdf:about="https://w3id.org/tern/ontologies/tern/Platform">
    <rdf:type rdf:resource="http://www.w3.org/2002/07/owl#Class"/>
    <rdfs:label>Platform</rdfs:label>
    <skos:definition>An entity that hosts other entities, particularly [Sensors](#Sensor), [Samplers](#Sampler), and other [Platforms](#Platform).</skos:definition>
    <skos:example>Ocean buoy is an example of platform that is equipped with 
an array of sensors such as GPS, current meters, atmospheric sensors and water 
quality monitors. Sensors measuring weather variables are attached to 
a weather station (a platform)</skos:example>
    <rdfs:subClassOf rdf:resource="http://www.w3.org/ns/sosa/Platform"/>
  </rdf:Description>
  <rdf:Description rdf:nodeID="ub1bL1215C19">
    <owl:allValuesFrom rdf:resource="http://www.w3.org/2001/XMLSchema#dateTime"/>
    <rdf:type rdf:resource="http://www.w3.org/2002/07/owl#Restriction"/>
    <owl:onProperty rdf:resource="http://www.w3.org/ns/prov#endedAtTime"/>
  </rdf:Description>
  <rdf:Description rdf:nodeID="ub1bL136C19">
    <schema-https:identifier rdf:resource="https://orcid.org/0000-0002-3884-3420"/>
    <schema-https:memberOf rdf:nodeID="ub1bL140C29"/>
    <schema-https:email>simon.cox@csiro.au</schema-https:email>
    <schema-https:name>Simon J.D.Cox</schema-https:name>
    <rdf:type rdf:resource="https://schema.org/Person"/>
  </rdf:Description>
  <rdf:Description rdf:nodeID="fcf4ebf340cd54dc4871b974b242da6f5b1">
    <rdf:first rdf:resource="http://www.w3.org/2001/XMLSchema#decimal"/>
    <rdf:rest rdf:nodeID="fcf4ebf340cd54dc4871b974b242da6f5b2"/>
  </rdf:Description>
  <rdf:Description rdf:about="http://linked.data.gov.au/def/datatype/Percent">
    <rdfs:subClassOf rdf:resource="https://w3id.org/tern/ontologies/tern/Result"/>
  </rdf:Description>
  <rdf:Description rdf:about="https://w3id.org/tern/ontologies/tern/stratum">
    <rdf:type rdf:resource="http://www.w3.org/1999/02/22-rdf-syntax-ns#Property"/>
    <skos:definition>A stratum is a distinct, easily seen, layer of foliage and branches of a measurable height.</skos:definition>
    <skos:scopeNote>Value should be from a controlled vocabulary identified by a URI.</skos:scopeNote>
    <rdfs:label>stratum</rdfs:label>
    <rdfs:subPropertyOf rdf:resource="http://purl.org/dc/terms/type"/>
  </rdf:Description>
  <rdf:Description rdf:nodeID="ub1bL672C19">
    <owl:cardinality rdf:datatype="http://www.w3.org/2001/XMLSchema#nonNegativeInteger">1</owl:cardinality>
    <rdf:type rdf:resource="http://www.w3.org/2002/07/owl#Restriction"/>
    <owl:onProperty rdf:resource="http://rs.tdwg.org/dwc/terms/materialSampleID"/>
  </rdf:Description>
  <rdf:Description rdf:about="https://w3id.org/tern/ontologies/tern/SiteTaxon">
    <rdfs:subClassOf rdf:nodeID="ub1bL1204C19"/>
    <rdfs:label>Site Taxon</rdfs:label>
    <rdfs:subClassOf rdf:resource="https://w3id.org/tern/ontologies/tern/Sample"/>
    <rdf:type rdf:resource="http://www.w3.org/2002/07/owl#Class"/>
  </rdf:Description>
  <rdf:Description rdf:about="https://w3id.org/tern/ontologies/tern/Sample">
    <rdfs:subClassOf rdf:nodeID="ub1bL838C19"/>
    <rdfs:subClassOf rdf:nodeID="ub1bL833C19"/>
    <skos:definition>*A feature which is intended to be representative of a [FeatureOfInterest](http://w3.org/ns/sosa/FeatureOfInterest) on which [Observations](#Observation) may be made. Physical samples are sometimes known as physical specimens.</skos:definition>
    <rdfs:subClassOf rdf:nodeID="ub1bL823C19"/>
    <rdfs:subClassOf rdf:nodeID="ub1bL828C19"/>
    <rdfs:subClassOf rdf:resource="https://w3id.org/tern/ontologies/tern/FeatureOfInterest"/>
    <rdfs:subClassOf rdf:nodeID="ub1bL843C19"/>
    <rdfs:label>Sample</rdfs:label>
    <rdf:type rdf:resource="http://www.w3.org/2002/07/owl#Class"/>
    <rdfs:subClassOf rdf:nodeID="ub1bL818C19"/>
    <skos:example>Plant, animal, soil and water are all 
examples of samples of some feature of interest.</skos:example>
    <rdfs:subClassOf rdf:nodeID="ub1bL848C19"/>
  </rdf:Description>
  <rdf:Description rdf:nodeID="ub1bL1143C19">
    <owl:onProperty rdf:resource="http://www.w3.org/2000/01/rdf-schema#label"/>
    <rdf:type rdf:resource="http://www.w3.org/2002/07/owl#Restriction"/>
    <owl:qualifiedCardinality rdf:datatype="http://www.w3.org/2001/XMLSchema#nonNegativeInteger">1</owl:qualifiedCardinality>
    <owl:onClass rdf:resource="http://www.w3.org/2001/XMLSchema#string"/>
  </rdf:Description>
  <rdf:Description rdf:nodeID="ub1bL838C19">
    <rdf:type rdf:resource="http://www.w3.org/2002/07/owl#Restriction"/>
    <owl:allValuesFrom rdf:resource="https://w3id.org/tern/ontologies/tern/Sample"/>
    <owl:onProperty rdf:resource="http://www.w3.org/ns/sosa/isSampleOf"/>
  </rdf:Description>
  <rdf:Description rdf:nodeID="ub1bL1679C1">
    <owl:unionOf rdf:nodeID="fcf4ebf340cd54dc4871b974b242da6f5b18"/>
    <rdf:type rdf:resource="http://www.w3.org/2002/07/owl#Class"/>
  </rdf:Description>
  <rdf:Description rdf:about="https://w3id.org/tern/ontologies/tern/SiteStratum">
    <rdfs:subClassOf rdf:nodeID="ub1bL1163C19"/>
    <skos:definition>Structural element covering a recognisable height range in vegetation ecosystem occurring at an observation [Site](#EcologicalSite).</skos:definition>
    <rdfs:subClassOf rdf:nodeID="ub1bL1169C19"/>
    <rdfs:label>Site Stratum</rdfs:label>
    <rdf:type rdf:resource="http://www.w3.org/2002/07/owl#Class"/>
    <rdfs:subClassOf rdf:resource="https://w3id.org/tern/ontologies/tern/Sample"/>
  </rdf:Description>
  <rdf:Description rdf:about="https://w3id.org/tern/ontologies/tern/siteVisit">
    <rdfs:label>site visit</rdfs:label>
    <rdfs:range rdf:resource="https://w3id.org/tern/ontologies/tern/SiteVisit"/>
    <rdf:type rdf:resource="http://www.w3.org/1999/02/22-rdf-syntax-ns#Property"/>
    <skos:definition>A property that links, e.g., a [Site](#EcologicalSite) to a [Site Visit](#EcologicalSiteVisit).</skos:definition>
  </rdf:Description>
  <rdf:Description rdf:nodeID="ub1bL1131C19">
    <rdf:type rdf:resource="http://www.w3.org/2002/07/owl#Restriction"/>
    <owl:onClass rdf:resource="http://www.w3.org/2001/XMLSchema#date"/>
    <owl:qualifiedCardinality rdf:datatype="http://www.w3.org/2001/XMLSchema#nonNegativeInteger">1</owl:qualifiedCardinality>
    <owl:onProperty rdf:resource="https://w3id.org/tern/ontologies/tern/dateCommissioned"/>
  </rdf:Description>
  <rdf:Description rdf:nodeID="ub1bL447C25">
    <owl:unionOf rdf:nodeID="fcf4ebf340cd54dc4871b974b242da6f5b5"/>
    <rdf:type rdf:resource="http://www.w3.org/2002/07/owl#Class"/>
  </rdf:Description>
  <rdf:Description rdf:nodeID="ub1bL358C19">
    <owl:allValuesFrom rdf:resource="http://www.w3.org/2001/XMLSchema#string"/>
    <rdf:type rdf:resource="http://www.w3.org/2002/07/owl#Restriction"/>
    <owl:onProperty rdf:resource="http://purl.org/dc/terms/description"/>
  </rdf:Description>
  <rdf:Description rdf:about="https://w3id.org/tern/ontologies/tern/isSamplingPointOf">
    <owl:inverseOf rdf:resource="https://w3id.org/tern/ontologies/tern/hasSamplingPoint"/>
    <rdfs:label>is sampling point of</rdfs:label>
    <rdf:type rdf:resource="http://www.w3.org/1999/02/22-rdf-syntax-ns#Property"/>
    <skos:definition>The inverse property [hasSamplingPoint](#hasSamplingPoint).</skos:definition>
  </rdf:Description>
  <rdf:Description rdf:nodeID="ub1bL710C19">
    <owl:maxQualifiedCardinality rdf:datatype="http://www.w3.org/2001/XMLSchema#nonNegativeInteger">1</owl:maxQualifiedCardinality>
    <owl:onClass rdf:resource="https://w3id.org/tern/ontologies/tern/Input"/>
    <owl:onProperty rdf:resource="http://www.w3.org/ns/ssn/hasInput"/>
    <rdf:type rdf:resource="http://www.w3.org/2002/07/owl#Restriction"/>
  </rdf:Description>
  <rdf:Description rdf:nodeID="ub1bL1204C19">
    <rdf:type rdf:resource="http://www.w3.org/2002/07/owl#Restriction"/>
    <owl:qualifiedCardinality rdf:datatype="http://www.w3.org/2001/XMLSchema#nonNegativeInteger">1</owl:qualifiedCardinality>
    <owl:onClass rdf:resource="https://w3id.org/tern/ontologies/sd/StateTaxon"/>
    <owl:onProperty rdf:resource="https://w3id.org/tern/ontologies/tern/taxon"/>
  </rdf:Description>
  <rdf:Description rdf:nodeID="ub1bL392C19">
    <owl:qualifiedCardinality rdf:datatype="http://www.w3.org/2001/XMLSchema#nonNegativeInteger">1</owl:qualifiedCardinality>
    <rdf:type rdf:resource="http://www.w3.org/2002/07/owl#Restriction"/>
    <owl:onClass rdf:resource="http://www.w3.org/2001/XMLSchema#string"/>
    <owl:onProperty rdf:resource="http://www.w3.org/2000/01/rdf-schema#label"/>
  </rdf:Description>
  <rdf:Description rdf:about="https://w3id.org/tern/ontologies/tern/hasSamplingPoint">
    <rdfs:label>has sampling point</rdfs:label>
    <owl:inverseOf rdf:resource="https://w3id.org/tern/ontologies/tern/isSamplingPointOf"/>
    <skos:definition>A property that links, e.g., a [Sampling](#Sampling) to a [SamplingPoint](#SamplingPoint).</skos:definition>
    <rdfs:range rdf:resource="https://w3id.org/tern/ontologies/tern/SamplingPoint"/>
    <rdf:type rdf:resource="http://www.w3.org/1999/02/22-rdf-syntax-ns#Property"/>
  </rdf:Description>
  <rdf:Description rdf:about="https://w3id.org/tern/ontologies/tern/width">
    <rdf:type rdf:resource="http://www.w3.org/1999/02/22-rdf-syntax-ns#Property"/>
    <skos:definition>The measurement or extent of something from side to side.</skos:definition>
    <rdfs:label>width</rdfs:label>
    <rdfs:seeAlso rdf:resource="http://qudt.org/vocab/quantitykind/Width"/>
  </rdf:Description>
  <rdf:Description rdf:about="https://w3id.org/tern/ontologies/tern/site">
    <skos:definition>A property that links, e.g., a [SiteVisit](#EcologicalSiteVisit) to a [Site](#EcologicalSite).</skos:definition>
    <rdf:type rdf:resource="http://www.w3.org/1999/02/22-rdf-syntax-ns#Property"/>
    <rdfs:range rdf:resource="https://w3id.org/tern/ontologies/tern/Site"/>
    <rdfs:label>site</rdfs:label>
  </rdf:Description>
  <rdf:Description rdf:nodeID="ub1bL892C19">
    <owl:maxQualifiedCardinality rdf:datatype="http://www.w3.org/2001/XMLSchema#nonNegativeInteger">1</owl:maxQualifiedCardinality>
    <rdf:type rdf:resource="http://www.w3.org/2002/07/owl#Restriction"/>
    <owl:onClass rdf:resource="https://w3id.org/tern/ontologies/tern/SamplingPoint"/>
    <owl:onProperty rdf:resource="https://w3id.org/tern/ontologies/tern/hasSamplingPoint"/>
  </rdf:Description>
  <rdf:Description rdf:nodeID="ub1bL975C19">
    <owl:onProperty rdf:resource="http://www.opengis.net/ont/geosparql#asWKT"/>
    <owl:qualifiedCardinality rdf:datatype="http://www.w3.org/2001/XMLSchema#nonNegativeInteger">1</owl:qualifiedCardinality>
    <owl:onDataRange rdf:resource="https://w3id.org/tern/ontologies/loc/wktLiteral"/>
    <rdf:type rdf:resource="http://www.w3.org/2002/07/owl#Restriction"/>
  </rdf:Description>
  <rdf:Description rdf:about="https://w3id.org/tern/ontologies/tern/EnvironmentalCharacteristic">
    <rdfs:subClassOf rdf:nodeID="ub1bL332C19"/>
    <skos:definition>The environment characteristics  is a [FeatureOfInterest](http://w3.org/ns/sosa/FeatureOfInterest) of a location where [Observations](#Observation) such as the annual mean rainfall or the annual mean temperature are made.</skos:definition>
    <rdfs:label>Environmental Characteristic</rdfs:label>
    <rdfs:subClassOf rdf:resource="http://www.w3.org/ns/sosa/FeatureOfInterest"/>
    <rdf:type rdf:resource="http://www.w3.org/2002/07/owl#Class"/>
  </rdf:Description>
  <rdf:Description rdf:about="http://rs.tdwg.org/dwc/terms/MaterialSample">
    <rdfs:label>Material Sample</rdfs:label>
    <rdf:type rdf:resource="http://www.w3.org/2002/07/owl#Class"/>
    <skos:example>A whole organism preserved in a collection. 
A part of an organism isolated for some purpose. A soil sample. A marine microbial sample.</skos:example>
    <rdfs:isDefinedBy rdf:resource="http://rs.tdwg.org/dwc/terms/"/>
    <rdfs:comment>A physical result of a sampling (or subsampling) event. In biological collections, the material sample is typically collected, and either preserved or destructively processed.</rdfs:comment>
  </rdf:Description>
  <rdf:Description rdf:nodeID="ub1bL1045C19">
    <owl:onProperty rdf:resource="http://www.opengis.net/ont/geosparql#hasGeometry"/>
    <rdf:type rdf:resource="http://www.w3.org/2002/07/owl#Restriction"/>
    <owl:allValuesFrom rdf:nodeID="ub1bL1047C25"/>
  </rdf:Description>
  <rdf:Description rdf:nodeID="ub1bL412C19">
    <owl:onProperty rdf:resource="http://purl.org/dc/terms/description"/>
    <owl:allValuesFrom rdf:resource="http://www.w3.org/2001/XMLSchema#string"/>
    <rdf:type rdf:resource="http://www.w3.org/2002/07/owl#Restriction"/>
  </rdf:Description>
  <rdf:Description rdf:about="https://w3id.org/tern/ontologies/tern/Instrument">
    <skos:definition>A device or instrument that is used for making measurements or observations.</skos:definition>
    <rdf:type rdf:resource="http://www.w3.org/2002/07/owl#Class"/>
    <rdfs:label>Instrument</rdfs:label>
    <rdfs:subClassOf rdf:resource="http://www.w3.org/ns/ssn/System"/>
  </rdf:Description>
  <rdf:Description rdf:about="https://w3id.org/tern/ontologies/tern/PropertyValue">
    <skos:example>@prefix tern: &lt;https://w3id.org/tern/ontologies/tern/&gt; .
@prefix schema: &lt;http://schema.org/&gt; .
@prefix data: &lt;http://linked.data.gov.au/def/datatype/&gt; .
@prefix sosa: &lt;http://w3.org/ns/sosa/&gt; .

&lt;example&gt; a tern:PropertyValue ;
	schema:name "AUSPLOTS_RANGELANDS.SITE.PROPERTY" ;
	schema:description "The property name" ;
	sosa:hasResult [
		a data:Text ;
		data:value "Great Victoria Desert Nature Reserve" ;
	] .</skos:example>
    <skos:definition>A property-value pair. Use the [schema:name](http://schema.org/name) property for the name of the property. If there is an additional human-readable version of the value, put that into the [schema:description](http://schema.org/description) property.</skos:definition>
    <rdfs:subClassOf rdf:nodeID="ub1bL734C19"/>
    <rdfs:subClassOf rdf:nodeID="ub1bL745C19"/>
    <rdfs:subClassOf rdf:nodeID="ub1bL739C19"/>
    <rdf:type rdf:resource="http://www.w3.org/2002/07/owl#Class"/>
    <rdfs:label>Property Value</rdfs:label>
    <rdfs:subClassOf rdf:resource="http://schema.org/PropertyValue"/>
  </rdf:Description>
  <rdf:Description rdf:nodeID="fcf4ebf340cd54dc4871b974b242da6f5b6">
    <rdf:rest rdf:resource="http://www.w3.org/1999/02/22-rdf-syntax-ns#nil"/>
    <rdf:first rdf:resource="http://www.w3.org/2001/XMLSchema#anyURI"/>
  </rdf:Description>
  <rdf:Description rdf:about="https://w3id.org/tern/ontologies/tern/SAR">
    <rdf:type rdf:resource="http://www.w3.org/2002/07/owl#Class"/>
    <rdfs:subClassOf rdf:resource="https://w3id.org/tern/ontologies/tern/Sensor"/>
    <skos:altLabel>SAR</skos:altLabel>
    <skos:altLabel>Synthetic-aperture radar</skos:altLabel>
    <rdfs:seeAlso rdf:resource="https://earthdata.nasa.gov/learn/backgrounders/what-is-sar"/>
    <rdfs:label>Synthetic Aperture Radar</rdfs:label>
  </rdf:Description>
  <rdf:Description rdf:nodeID="ub1bL237C19">
    <rdf:type rdf:resource="http://www.w3.org/2002/07/owl#Restriction"/>
    <owl:allValuesFrom rdf:resource="http://www.w3.org/2001/XMLSchema#string"/>
    <owl:onProperty rdf:resource="http://www.w3.org/2004/02/skos/core#altLabel"/>
  </rdf:Description>
  <rdf:Description rdf:nodeID="ub1bL700C19">
    <rdf:type rdf:resource="http://www.w3.org/2002/07/owl#Restriction"/>
    <owl:allValuesFrom rdf:resource="http://www.w3.org/2004/02/skos/core#Concept"/>
    <owl:onProperty rdf:resource="https://w3id.org/tern/ontologies/tern/methodType"/>
  </rdf:Description>
  <rdf:Description rdf:about="https://w3id.org/tern/ontologies/tern/fluxnetID">
    <rdfs:seeAlso rdf:resource="https://fluxnet.org/"/>
    <skos:definition>The unique identifier for flux towers registered with FLUXNET.</skos:definition>
    <rdf:type rdf:resource="http://www.w3.org/1999/02/22-rdf-syntax-ns#Property"/>
    <skos:example>AU-ASM</skos:example>
    <rdfs:label>fluxnet ID</rdfs:label>
  </rdf:Description>
  <rdf:Description rdf:nodeID="ub1bL993C19">
    <owl:onProperty rdf:resource="http://www.w3.org/ns/sosa/madeObservation"/>
    <owl:allValuesFrom rdf:resource="https://w3id.org/tern/ontologies/tern/Observation"/>
    <rdf:type rdf:resource="http://www.w3.org/2002/07/owl#Restriction"/>
  </rdf:Description>
  <rdf:Description rdf:nodeID="ub1bL786C19">
    <rdf:type rdf:resource="http://www.w3.org/2002/07/owl#Restriction"/>
    <owl:allValuesFrom rdf:nodeID="ub1bL788C25"/>
    <owl:onProperty rdf:resource="http://www.w3.org/ns/sosa/isResultOf"/>
  </rdf:Description>
  <rdf:Description rdf:about="https://w3id.org/tern/ontologies/tern/transectDirection">
    <rdf:type rdf:resource="http://www.w3.org/1999/02/22-rdf-syntax-ns#Property"/>
    <rdfs:domain rdf:resource="https://w3id.org/tern/ontologies/tern/Transect"/>
    <rdfs:range rdf:resource="http://www.w3.org/2001/XMLSchema#string"/>
    <skos:definition>Describes the direction of the transect.</skos:definition>
    <skos:example>S-W</skos:example>
    <rdfs:label>transect direction</rdfs:label>
  </rdf:Description>
  <rdf:Description rdf:nodeID="ub1bL823C19">
    <owl:allValuesFrom rdf:resource="https://w3id.org/tern/ontologies/org/Person"/>
    <rdf:type rdf:resource="http://www.w3.org/2002/07/owl#Restriction"/>
    <owl:onProperty rdf:resource="http://www.w3.org/ns/prov#wasAttributedTo"/>
  </rdf:Description>
  <rdf:Description rdf:nodeID="ub1bL247C19">
    <owl:minCardinality rdf:datatype="http://www.w3.org/2001/XMLSchema#nonNegativeInteger">1</owl:minCardinality>
    <rdf:type rdf:resource="http://www.w3.org/2002/07/owl#Restriction"/>
    <owl:onProperty rdf:resource="http://schema.org/model"/>
  </rdf:Description>
  <rdf:Description rdf:nodeID="ub1bL456C19">
    <owl:onProperty rdf:resource="http://www.w3.org/2004/02/skos/core#definition"/>
    <owl:maxQualifiedCardinality rdf:datatype="http://www.w3.org/2001/XMLSchema#nonNegativeInteger">1</owl:maxQualifiedCardinality>
    <owl:onClass rdf:resource="http://www.w3.org/2001/XMLSchema#string"/>
    <rdf:type rdf:resource="http://www.w3.org/2002/07/owl#Restriction"/>
  </rdf:Description>
  <rdf:Description rdf:nodeID="ub1bL1163C19">
    <owl:qualifiedCardinality rdf:datatype="http://www.w3.org/2001/XMLSchema#nonNegativeInteger">1</owl:qualifiedCardinality>
    <rdf:type rdf:resource="http://www.w3.org/2002/07/owl#Restriction"/>
    <owl:onProperty rdf:resource="https://w3id.org/tern/ontologies/tern/stratum"/>
    <owl:onClass rdf:resource="http://www.w3.org/2004/02/skos/core#Concept"/>
  </rdf:Description>
  <rdf:Description rdf:nodeID="ub1bL1269C19">
    <owl:onClass rdf:resource="http://www.w3.org/2001/XMLSchema#string"/>
    <rdf:type rdf:resource="http://www.w3.org/2002/07/owl#Restriction"/>
    <owl:onProperty rdf:resource="http://www.w3.org/2000/01/rdf-schema#label"/>
    <owl:qualifiedCardinality rdf:datatype="http://www.w3.org/2001/XMLSchema#nonNegativeInteger">1</owl:qualifiedCardinality>
  </rdf:Description>
  <rdf:Description rdf:about="https://w3id.org/tern/ontologies/tern/globalVocabulary">
    <skos:definition>The global vocabulary refers to the main vocabulary, which takes precedence over other similar vocabularies to promote data harmonisation.</skos:definition>
    <rdfs:label>global vocabulary</rdfs:label>
    <rdf:type rdf:resource="http://www.w3.org/1999/02/22-rdf-syntax-ns#Property"/>
  </rdf:Description>
  <rdf:Description rdf:about="https://w3id.org/tern/resources/a083902d-d821-41be-b663-1d7cb33eea66">
    <rdf:type rdf:resource="https://schema.org/Organization"/>
    <schema-https:name>TERN</schema-https:name>
    <schema-https:identifier rdf:resource="https://w3id.org/tern/resources/a083902d-d821-41be-b663-1d7cb33eea66"/>
  </rdf:Description>
  <rdf:Description rdf:nodeID="ub1bL307C19">
    <owl:onProperty rdf:resource="http://linked.data.gov.au/def/datatype/unit"/>
    <owl:qualifiedCardinality rdf:datatype="http://www.w3.org/2001/XMLSchema#nonNegativeInteger">1</owl:qualifiedCardinality>
    <rdf:type rdf:resource="http://www.w3.org/2002/07/owl#Restriction"/>
    <owl:onClass rdf:resource="http://qudt.org/schema/qudt/Unit"/>
  </rdf:Description>
  <rdf:Description rdf:nodeID="ub1bL781C19">
    <owl:allValuesFrom rdf:resource="https://w3id.org/tern/ontologies/org/Person"/>
    <rdf:type rdf:resource="http://www.w3.org/2002/07/owl#Restriction"/>
    <owl:onProperty rdf:resource="http://www.w3.org/ns/prov#wasAttributedTo"/>
  </rdf:Description>
  <rdf:Description rdf:about="https://w3id.org/tern/ontologies/tern/Spectroradiometer">
    <rdf:type rdf:resource="http://www.w3.org/2002/07/owl#Class"/>
    <rdfs:seeAlso rdf:resource="https://en.wikipedia.org/wiki/Spectroradiometer"/>
    <rdfs:subClassOf rdf:resource="https://w3id.org/tern/ontologies/tern/Sensor"/>
    <rdfs:comment>A spectroradiometer is a light measurement tool that is able to measure both the wavelength and amplitude of the light emitted from a light source.</rdfs:comment>
    <rdfs:label>Spectroradiometer</rdfs:label>
  </rdf:Description>
  <rdf:Description rdf:nodeID="ub1bL898C19">
    <owl:qualifiedCardinality rdf:datatype="http://www.w3.org/2001/XMLSchema#nonNegativeInteger">1</owl:qualifiedCardinality>
    <owl:onProperty rdf:resource="http://www.w3.org/2000/01/rdf-schema#label"/>
    <owl:onClass rdf:resource="http://www.w3.org/2001/XMLSchema#string"/>
    <rdf:type rdf:resource="http://www.w3.org/2002/07/owl#Restriction"/>
  </rdf:Description>
  <rdf:Description rdf:nodeID="ub1bL1369C19">
    <owl:onProperty rdf:resource="https://w3id.org/tern/ontologies/tern/transectStartPoint"/>
    <owl:qualifiedCardinality rdf:datatype="http://www.w3.org/2001/XMLSchema#nonNegativeInteger">1</owl:qualifiedCardinality>
    <rdf:type rdf:resource="http://www.w3.org/2002/07/owl#Restriction"/>
    <owl:onClass rdf:resource="https://w3id.org/tern/ontologies/loc/Point"/>
  </rdf:Description>
  <rdf:Description rdf:nodeID="ub1bL1149C19">
    <owl:onClass rdf:resource="http://www.w3.org/ns/dcat#Dataset"/>
    <rdf:type rdf:resource="http://www.w3.org/2002/07/owl#Restriction"/>
    <owl:qualifiedCardinality rdf:datatype="http://www.w3.org/2001/XMLSchema#nonNegativeInteger">1</owl:qualifiedCardinality>
    <owl:onProperty rdf:resource="http://www.w3.org/ns/dcat#dataset"/>
  </rdf:Description>
  <rdf:Description rdf:about="https://w3id.org/tern/ontologies/tern/Result">
    <skos:example>The value 20 as the height of a certain 
tree together with the unit, e.g., Meter.</skos:example>
    <rdfs:subClassOf rdf:nodeID="ub1bL797C19"/>
    <rdf:type rdf:resource="http://www.w3.org/2002/07/owl#Class"/>
    <rdfs:label>Result</rdfs:label>
    <rdfs:subClassOf rdf:resource="http://www.w3.org/ns/sosa/Result"/>
    <rdfs:subClassOf rdf:nodeID="ub1bL781C19"/>
    <skos:definition>The result of an [Observation](#Observation), [Actuation](http://w3.org/ns/sosa/Actuation), or act of [Sampling](#Sampling). To store an observation's simple result value one can use the [hasSimpleResult](http://w3.org/ns/sosa/hasSimpleResult) property.</skos:definition>
    <rdfs:subClassOf rdf:nodeID="ub1bL786C19"/>
  </rdf:Description>
  <rdf:Description rdf:nodeID="ub1bL257C19">
    <owl:onClass rdf:resource="http://www.w3.org/2001/XMLSchema#string"/>
    <owl:minQualifiedCardinality rdf:datatype="http://www.w3.org/2001/XMLSchema#nonNegativeInteger">1</owl:minQualifiedCardinality>
    <owl:onProperty rdf:resource="http://purl.org/dc/terms/source"/>
    <rdf:type rdf:resource="http://www.w3.org/2002/07/owl#Restriction"/>
  </rdf:Description>
  <rdf:Description rdf:about="http://linked.data.gov.au/def/datatype/PercentRange">
    <rdfs:subClassOf rdf:resource="https://w3id.org/tern/ontologies/tern/Result"/>
  </rdf:Description>
  <rdf:Description rdf:about="https://w3id.org/tern/ontologies/tern/scope">
    <rdf:type rdf:resource="http://www.w3.org/2002/07/owl#DatatypeProperty"/>
    <rdfs:label>scope</rdfs:label>
    <rdfs:range rdf:resource="http://www.w3.org/2001/XMLSchema#string"/>
    <skos:definition>Describe the scope of something.</skos:definition>
  </rdf:Description>
  <rdf:Description rdf:nodeID="ub1bL277C25">
    <rdf:type rdf:resource="http://www.w3.org/2002/07/owl#Class"/>
    <owl:unionOf rdf:nodeID="fcf4ebf340cd54dc4871b974b242da6f5b1"/>
  </rdf:Description>
  <rdf:Description rdf:nodeID="ub1bL648C19">
    <owl:onProperty rdf:resource="http://schema.org/serialNumber"/>
    <owl:allValuesFrom rdf:resource="http://www.w3.org/2001/XMLSchema#string"/>
    <rdf:type rdf:resource="http://www.w3.org/2002/07/owl#Restriction"/>
  </rdf:Description>
  <rdf:Description rdf:about="https://w3id.org/tern/ontologies/tern/equipment">
    <rdf:type rdf:resource="http://www.w3.org/2002/07/owl#DatatypeProperty"/>
    <rdfs:label>equipment</rdfs:label>
    <skos:definition>Describe the equipment used as text.</skos:definition>
    <rdfs:range rdf:resource="http://www.w3.org/2001/XMLSchema#string"/>
  </rdf:Description>
  <rdf:Description rdf:nodeID="ub1bL586C19">
    <rdf:type rdf:resource="http://www.w3.org/2002/07/owl#Restriction"/>
    <owl:qualifiedCardinality rdf:datatype="http://www.w3.org/2001/XMLSchema#nonNegativeInteger">1</owl:qualifiedCardinality>
    <owl:onProperty rdf:resource="http://www.w3.org/2000/01/rdf-schema#label"/>
    <owl:onClass rdf:resource="http://www.w3.org/2001/XMLSchema#string"/>
  </rdf:Description>
  <rdf:Description rdf:nodeID="ub1bL1225C19">
    <owl:onProperty rdf:resource="http://www.w3.org/2000/01/rdf-schema#comment"/>
    <rdf:type rdf:resource="http://www.w3.org/2002/07/owl#Restriction"/>
    <owl:allValuesFrom rdf:resource="http://www.w3.org/2001/XMLSchema#string"/>
  </rdf:Description>
  <rdf:Description rdf:about="https://w3id.org/tern/ontologies/tern/SuperSite">
    <skos:definition>TERN SuperSites are Long Term Ecological Research (LTER) sites co-located with TERN OzFlux eddy covariance towers, which deliver biological and environmental observations of flora, fauna, microbial biodiversity, soils and hydrology. TERN OzFlux delivers micrometeorological observations of energy, carbon and water exchange between the atmosphere and key Australian ecosystems. Each TERN SuperSite is located in a significant Australian biome and the network spans a wide range of environmental conditions. The SuperSite network collects detailed data sets on flora, fauna and biophysical processes from each SuperSite.</skos:definition>
    <rdf:type rdf:resource="http://www.w3.org/2002/07/owl#Class"/>
    <rdfs:subClassOf rdf:resource="https://w3id.org/tern/ontologies/tern/Site"/>
    <rdfs:seeAlso rdf:resource="https://supersites.tern.org.au/"/>
    <rdfs:label>SuperSite</rdfs:label>
  </rdf:Description>
  <rdf:Description rdf:nodeID="ub1bL122C19">
    <schema-https:affiliation rdf:resource="https://w3id.org/tern/resources/a083902d-d821-41be-b663-1d7cb33eea66"/>
    <schema-https:identifier rdf:resource="https://orcid.org/0000-0002-6047-9864"/>
    <rdf:type rdf:resource="https://schema.org/Person"/>
    <schema-https:email>e.chuc@uq.edu.au</schema-https:email>
    <schema-https:name>Edmond Chuc</schema-https:name>
  </rdf:Description>
  <rdf:Description rdf:nodeID="ub1bL1061C19">
    <owl:onProperty rdf:resource="https://w3id.org/tern/ontologies/tern/hasEnvironmentalCharacteristic"/>
    <owl:maxCardinality rdf:datatype="http://www.w3.org/2001/XMLSchema#nonNegativeInteger">1</owl:maxCardinality>
    <rdf:type rdf:resource="http://www.w3.org/2002/07/owl#Restriction"/>
  </rdf:Description>
  <rdf:Description rdf:nodeID="ub1bL242C19">
    <rdf:type rdf:resource="http://www.w3.org/2002/07/owl#Restriction"/>
    <owl:onProperty rdf:resource="http://www.w3.org/2004/02/skos/core#definition"/>
    <owl:allValuesFrom rdf:resource="http://www.w3.org/2001/XMLSchema#string"/>
  </rdf:Description>
  <rdf:Description rdf:nodeID="ub1bL1137C19">
    <owl:qualifiedCardinality rdf:datatype="http://www.w3.org/2001/XMLSchema#nonNegativeInteger">1</owl:qualifiedCardinality>
    <owl:onProperty rdf:resource="http://purl.org/dc/terms/identifier"/>
    <owl:onClass rdf:resource="http://www.w3.org/2001/XMLSchema#string"/>
    <rdf:type rdf:resource="http://www.w3.org/2002/07/owl#Restriction"/>
  </rdf:Description>
  <rdf:Description rdf:nodeID="ub1bL933C19">
    <owl:onProperty rdf:resource="https://w3id.org/tern/ontologies/loc/altitude"/>
    <owl:onClass rdf:resource="http://linked.data.gov.au/def/datatype/QuantitativeMeasure"/>
    <owl:maxQualifiedCardinality rdf:datatype="http://www.w3.org/2001/XMLSchema#nonNegativeInteger">1</owl:maxQualifiedCardinality>
    <rdf:type rdf:resource="http://www.w3.org/2002/07/owl#Restriction"/>
  </rdf:Description>
  <rdf:Description rdf:nodeID="ub1bL1015C19">
    <rdf:type rdf:resource="http://www.w3.org/2002/07/owl#Restriction"/>
    <owl:allValuesFrom rdf:resource="https://w3id.org/tern/ontologies/tern/PhysicalSpecimen"/>
    <owl:onProperty rdf:resource="http://www.w3.org/ns/sosa/hasSample"/>
  </rdf:Description>
  <rdf:Description rdf:nodeID="fcf4ebf340cd54dc4871b974b242da6f5b17">
    <rdf:rest rdf:resource="http://www.w3.org/1999/02/22-rdf-syntax-ns#nil"/>
    <rdf:first rdf:resource="http://www.w3.org/2001/XMLSchema#int"/>
  </rdf:Description>
  <rdf:Description rdf:nodeID="ub1bL386C19">
    <owl:onClass rdf:resource="http://www.w3.org/2001/XMLSchema#date"/>
    <owl:qualifiedCardinality rdf:datatype="http://www.w3.org/2001/XMLSchema#nonNegativeInteger">1</owl:qualifiedCardinality>
    <rdf:type rdf:resource="http://www.w3.org/2002/07/owl#Restriction"/>
    <owl:onProperty rdf:resource="https://w3id.org/tern/ontologies/tern/dateCommissioned"/>
  </rdf:Description>
  <rdf:Description rdf:nodeID="ub1bL50C19">
    <owl:cardinality rdf:datatype="http://www.w3.org/2001/XMLSchema#nonNegativeInteger">1</owl:cardinality>
    <rdf:type rdf:resource="http://www.w3.org/2002/07/owl#Restriction"/>
    <owl:onProperty rdf:resource="https://w3id.org/tern/ontologies/tern/globalVocabulary"/>
  </rdf:Description>
  <rdf:Description rdf:nodeID="ub1bL951C19">
    <owl:maxQualifiedCardinality rdf:datatype="http://www.w3.org/2001/XMLSchema#nonNegativeInteger">1</owl:maxQualifiedCardinality>
    <owl:onClass rdf:resource="http://www.w3.org/2001/XMLSchema#string"/>
    <rdf:type rdf:resource="http://www.w3.org/2002/07/owl#Restriction"/>
    <owl:onProperty rdf:resource="http://purl.org/dc/terms/identifier"/>
  </rdf:Description>
  <rdf:Description rdf:nodeID="ub1bL797C19">
    <rdf:type rdf:resource="http://www.w3.org/2002/07/owl#Restriction"/>
    <owl:onProperty rdf:resource="http://www.w3.org/ns/sosa/isResultOf"/>
    <owl:cardinality rdf:datatype="http://www.w3.org/2001/XMLSchema#nonNegativeInteger">1</owl:cardinality>
  </rdf:Description>
  <rdf:Description rdf:nodeID="ub1bL374C19">
    <rdf:type rdf:resource="http://www.w3.org/2002/07/owl#Restriction"/>
    <owl:onClass rdf:resource="http://www.w3.org/2001/XMLSchema#string"/>
    <owl:onProperty rdf:resource="https://w3id.org/tern/ontologies/tern/fluxnetID"/>
    <owl:maxQualifiedCardinality rdf:datatype="http://www.w3.org/2001/XMLSchema#nonNegativeInteger">1</owl:maxQualifiedCardinality>
  </rdf:Description>
  <rdf:Description rdf:nodeID="ub1bL745C19">
    <owl:qualifiedCardinality rdf:datatype="http://www.w3.org/2001/XMLSchema#nonNegativeInteger">1</owl:qualifiedCardinality>
    <owl:onClass rdf:resource="https://w3id.org/tern/ontologies/tern/Result"/>
    <rdf:type rdf:resource="http://www.w3.org/2002/07/owl#Restriction"/>
    <owl:onProperty rdf:resource="http://www.w3.org/ns/sosa/hasResult"/>
  </rdf:Description>
  <rdf:Description rdf:nodeID="ub1bL1120C19">
    <owl:maxQualifiedCardinality rdf:datatype="http://www.w3.org/2001/XMLSchema#nonNegativeInteger">1</owl:maxQualifiedCardinality>
    <rdf:type rdf:resource="http://www.w3.org/2002/07/owl#Restriction"/>
    <owl:onProperty rdf:resource="https://w3id.org/tern/ontologies/tern/dimension"/>
    <owl:onClass rdf:resource="https://w3id.org/tern/ontologies/tern/Dimension"/>
  </rdf:Description>
  <rdf:Description rdf:nodeID="ub1bL882C19">
    <owl:onProperty rdf:resource="http://www.w3.org/2000/01/rdf-schema#comment"/>
    <owl:allValuesFrom rdf:resource="http://www.w3.org/2001/XMLSchema#string"/>
    <rdf:type rdf:resource="http://www.w3.org/2002/07/owl#Restriction"/>
  </rdf:Description>
  <rdf:Description rdf:about="https://w3id.org/tern/ontologies/tern/locationDescription">
    <skos:example>Location description of the AusPlots site NTABRT0004 in the Alice Mulga SuperSite: 
Pine Hill Station. 25km South East of Ti-Tree. 20km East of Stuart Highway. 
South west corner of the site is 200m north west of proposed supersite flux tower</skos:example>
    <rdfs:label>location description</rdfs:label>
    <skos:definition>The description of the location.</skos:definition>
    <rdf:type rdf:resource="http://www.w3.org/1999/02/22-rdf-syntax-ns#Property"/>
  </rdf:Description>
  <rdf:Description rdf:nodeID="ub1bL1352C19">
    <owl:onProperty rdf:resource="https://w3id.org/tern/ontologies/tern/transectDirection"/>
    <owl:maxCardinality rdf:datatype="http://www.w3.org/2001/XMLSchema#nonNegativeInteger">1</owl:maxCardinality>
    <rdf:type rdf:resource="http://www.w3.org/2002/07/owl#Restriction"/>
  </rdf:Description>
  <rdf:Description rdf:about="https://w3id.org/tern/ontologies/tern/AutomaticWeatherStation">
    <rdf:type rdf:resource="http://www.w3.org/2002/07/owl#Class"/>
    <rdfs:label>Automatic Weather Station</rdfs:label>
    <rdfs:subClassOf rdf:resource="https://w3id.org/tern/ontologies/tern/FixedPlatform"/>
  </rdf:Description>
  <rdf:Description rdf:about="https://w3id.org/tern/ontologies/tern/TERNDerivedObservation">
    <rdfs:subClassOf rdf:resource="https://w3id.org/tern/ontologies/tern/DerivedObservation"/>
    <rdfs:label>TERN Derived Observation</rdfs:label>
    <skos:definition>A derived observation created by TERN.</skos:definition>
    <rdf:type rdf:resource="http://www.w3.org/2002/07/owl#Class"/>
  </rdf:Description>
  <rdf:Description rdf:about="https://w3id.org/tern/ontologies/tern/area">
    <skos:definition>The extent of a [Site](#EcologicalSite) area, e.g., in m2</skos:definition>
    <rdf:type rdf:resource="http://www.w3.org/1999/02/22-rdf-syntax-ns#Property"/>
    <rdfs:label>area</rdfs:label>
    <skos:example> The area of the Mitchell Grass Rangeland SuperSite Supersite is approximately 47 M (million) ha.</skos:example>
  </rdf:Description>
  <rdf:Description rdf:nodeID="ub1bL1242C25">
    <rdf:type rdf:resource="http://www.w3.org/2002/07/owl#Class"/>
    <owl:unionOf rdf:nodeID="fcf4ebf340cd54dc4871b974b242da6f5b14"/>
  </rdf:Description>
  <rdf:Description rdf:nodeID="ub1bL1287C19">
    <owl:onProperty rdf:resource="https://w3id.org/tern/ontologies/loc/depth"/>
    <owl:allValuesFrom rdf:resource="http://linked.data.gov.au/def/datatype/QuantitativeRange"/>
    <rdf:type rdf:resource="http://www.w3.org/2002/07/owl#Restriction"/>
  </rdf:Description>
  <rdf:Description rdf:nodeID="ub1bL526C19">
    <rdf:type rdf:resource="http://www.w3.org/2002/07/owl#Restriction"/>
    <owl:onProperty rdf:resource="http://linked.data.gov.au/def/datatype/vocabulary"/>
    <owl:cardinality rdf:datatype="http://www.w3.org/2001/XMLSchema#nonNegativeInteger">1</owl:cardinality>
  </rdf:Description>
  <rdf:Description rdf:about="https://w3id.org/tern/ontologies/tern/dateDecommissioned">
    <skos:scopeNote>Use ISO 8601 international standard for representing dates and times. Missing end date may be set to the end of the month.</skos:scopeNote>
    <rdfs:label>date decommissioned</rdfs:label>
    <rdf:type rdf:resource="http://www.w3.org/1999/02/22-rdf-syntax-ns#Property"/>
    <skos:definition>The date when, e.g., a [Site](#EcologicalSite) is decommissioned or stopped operating.</skos:definition>
    <skos:example>30 Nov 2019 is the date decommisioned of the 
[Collie flux station](http://ozflux.org.au/monitoringsites/collie/index.html)</skos:example>
  </rdf:Description>
  <rdf:Description rdf:about="https://w3id.org/tern/ontologies/tern/PhysicalSpecimen">
    <rdfs:label>Physical Specimen</rdfs:label>
    <rdfs:subClassOf rdf:resource="http://rs.tdwg.org/dwc/terms/MaterialSample"/>
    <rdfs:subClassOf rdf:resource="https://w3id.org/tern/ontologies/tern/Sample"/>
    <rdfs:subClassOf rdf:nodeID="ub1bL672C19"/>
    <skos:example>A soil specimen or a plant specimen are examples of physical specimens.</skos:example>
    <skos:definition>A [Physical Specimen](#PhysicalSpecimen) is a physical [specimen](#Sample) collected from the field. </skos:definition>
    <rdfs:subClassOf rdf:nodeID="ub1bL677C19"/>
    <rdf:type rdf:resource="http://www.w3.org/2002/07/owl#Class"/>
  </rdf:Description>
  <rdf:Description rdf:about="https://w3id.org/tern/ontologies/tern/DerivedObservation">
    <rdf:type rdf:resource="http://www.w3.org/2002/07/owl#Class"/>
    <rdfs:label>Derived Observation</rdfs:label>
    <rdfs:subClassOf rdf:resource="https://w3id.org/tern/ontologies/tern/Observation"/>
    <skos:definition>A derived observation.</skos:definition>
  </rdf:Description>
  <rdf:Description rdf:nodeID="ub1bL1102C19">
    <rdf:type rdf:resource="http://www.w3.org/2002/07/owl#Restriction"/>
    <owl:onClass rdf:resource="https://w3id.org/tern/ontologies/loc/Point"/>
    <owl:onProperty rdf:resource="https://w3id.org/tern/ontologies/tern/centroidPoint"/>
    <owl:maxQualifiedCardinality rdf:datatype="http://www.w3.org/2001/XMLSchema#nonNegativeInteger">1</owl:maxQualifiedCardinality>
  </rdf:Description>
  <rdf:Description rdf:nodeID="ub1bL1257C19">
    <rdf:type rdf:resource="http://www.w3.org/2002/07/owl#Restriction"/>
    <owl:onClass rdf:resource="http://www.w3.org/2001/XMLSchema#string"/>
    <owl:onProperty rdf:resource="https://w3id.org/tern/ontologies/tern/siteDescription"/>
    <owl:maxQualifiedCardinality rdf:datatype="http://www.w3.org/2001/XMLSchema#nonNegativeInteger">1</owl:maxQualifiedCardinality>
  </rdf:Description>
  <rdf:Description rdf:nodeID="ub1bL1108C19">
    <rdf:type rdf:resource="http://www.w3.org/2002/07/owl#Restriction"/>
    <owl:onClass rdf:resource="https://w3id.org/tern/ontologies/loc/Point"/>
    <owl:onProperty rdf:resource="https://w3id.org/tern/ontologies/tern/swPoint"/>
    <owl:maxQualifiedCardinality rdf:datatype="http://www.w3.org/2001/XMLSchema#nonNegativeInteger">1</owl:maxQualifiedCardinality>
  </rdf:Description>
  <rdf:Description rdf:about="https://w3id.org/tern/ontologies/tern/RadiationSensor">
    <rdfs:subClassOf rdf:resource="https://w3id.org/tern/ontologies/tern/Sensor"/>
    <rdf:type rdf:resource="http://www.w3.org/2002/07/owl#Class"/>
    <rdfs:label>Radiation sensor</rdfs:label>
  </rdf:Description>
  <rdf:Description rdf:nodeID="ub1bL904C19">
    <owl:onClass rdf:resource="https://w3id.org/tern/ontologies/tern/Procedure"/>
    <rdf:type rdf:resource="http://www.w3.org/2002/07/owl#Restriction"/>
    <owl:onProperty rdf:resource="http://www.w3.org/ns/sosa/usedProcedure"/>
    <owl:qualifiedCardinality rdf:datatype="http://www.w3.org/2001/XMLSchema#nonNegativeInteger">1</owl:qualifiedCardinality>
  </rdf:Description>
  <rdf:Description rdf:about="https://w3id.org/tern/ontologies/tern/AusPlotsSite">
    <skos:definition>AusPlots is a plot-based surveillance monitoring program delivered by TERN Surveillance. An [AusPlot Site](#AusPlotsSite) refers to a [site](#EcologicalSite) where AusPlots Rangelands or Forests method has been implemented.</skos:definition>
    <skos:seeAlso rdf:resource="http://www.ausplots.org/"/>
    <rdf:type rdf:resource="http://www.w3.org/2002/07/owl#Class"/>
    <rdfs:subClassOf rdf:resource="https://w3id.org/tern/ontologies/tern/Site"/>
    <skos:example rdf:resource="http://linked.data.gov.au/dataset/ausplots/site-QDABBN0001"/>
    <rdfs:label>AusPlots Site</rdfs:label>
  </rdf:Description>
  <rdf:Description rdf:nodeID="fcf4ebf340cd54dc4871b974b242da6f5b8">
    <rdf:rest rdf:nodeID="fcf4ebf340cd54dc4871b974b242da6f5b9"/>
    <rdf:first rdf:resource="http://www.w3.org/2004/02/skos/core#Collection"/>
  </rdf:Description>
  <rdf:Description rdf:about="https://w3id.org/tern/ontologies/tern/swPoint">
    <rdfs:range rdf:resource="https://w3id.org/tern/ontologies/loc/Point"/>
    <rdfs:subPropertyOf rdf:resource="http://www.opengis.net/ont/geosparql#hasGeometry"/>
    <rdf:type rdf:resource="http://www.w3.org/1999/02/22-rdf-syntax-ns#Property"/>
    <skos:definition>The south-west point of the subject.</skos:definition>
    <rdfs:label>sw point</rdfs:label>
  </rdf:Description>
  <rdf:Description rdf:about="https://w3id.org/tern/ontologies/tern/CosmOzStation">
    <rdf:type rdf:resource="http://www.w3.org/2002/07/owl#Class"/>
    <rdfs:label>CosmOz Station</rdfs:label>
    <rdfs:seeAlso rdf:resource="https://cosmoz.csiro.au"/>
    <skos:definition>CosmOz is the Australian Cosmic-Ray Neutron Soil Moisture Monitoring Network

Beginning in October 2010, CSIRO Land and Water installed cosmic-ray probes at a number of locations around Australia to form the inaugural CosmOz network. These sites were established at instrumented research sites operated by CSIRO and University collaborators to test and validate the operation of this new technology.

These novel probes use cosmic rays originating from outer space to measure average soil moisture over an area of about 30 hectares to depths in the soil of between 10 to 50 cm. This constitutes a quantum leap over conventional on-ground soil moisture sensing technology that can only measure soil moisture content within small volumes of soil.

Each system is comprised of a data logger, neutron detector, satellite telemetry, tipping bucket rain gauge, temperature humidity and pressure sensors and three surface moisture (TDR) probes. The system requires minimal maintenance and is powered by a solar charging system. The entire system is installed on a single mast. Data is logged and transmitted every 60 minutes to the CosmOz database.</skos:definition>
    <rdfs:subClassOf rdf:resource="https://w3id.org/tern/ontologies/tern/FixedPlatform"/>
  </rdf:Description>
  <rdf:Description rdf:nodeID="ub1bL542C19">
    <owl:qualifiedCardinality rdf:datatype="http://www.w3.org/2001/XMLSchema#nonNegativeInteger">1</owl:qualifiedCardinality>
    <owl:onProperty rdf:resource="http://www.w3.org/1999/02/22-rdf-syntax-ns#value"/>
    <rdf:type rdf:resource="http://www.w3.org/2002/07/owl#Restriction"/>
    <owl:onClass rdf:resource="https://w3id.org/tern/ontologies/tern/Parameter"/>
  </rdf:Description>
  <rdf:Description rdf:about="https://w3id.org/tern/ontologies/tern/Procedure">
    <rdfs:label>Procedure</rdfs:label>
    <rdfs:subClassOf rdf:nodeID="ub1bL710C19"/>
    <skos:definition>A workflow, protocol, plan, algorithm, or computational method specifying how to make an [Observation](#Observation), create a [Sample](#Sample), or make a change to the state of the world (via an [Actuator](http://w3.org/ns/sosa/Actuator). A [Procedure](#Procedure) is re-usable, and might be involved in many [Observations](#Observation), [Samplings](#Sampling), or [Actuations](http://w3.org/ns/sosa/Actuation). it explains the steps to be carried out to arrive at reproducible [Results](#Result).</skos:definition>
    <skos:scopeNote>[Input](#Input) can be used to capture any input values for a procedure, such as the input value of the basal wedge to estimate the basal area per hectare.</skos:scopeNote>
    <rdf:type rdf:resource="http://www.w3.org/2002/07/owl#Class"/>
    <rdfs:subClassOf rdf:nodeID="ub1bL705C19"/>
    <rdfs:subClassOf rdf:nodeID="ub1bL716C19"/>
    <skos:example>The procedure for collecting photopoints are specified in the 
[AusPlots Rangelands Survey Protocols Manual](http://dx.doi.org/10.13140/2.1.4287.3607).
The DEC Nature Conservation Service Biodiversity have defined 
[standard procedures](https://www.dpaw.wa.gov.au/images/documents/plants-animals/monitoring/sop/sop_establishingvegetationquadrats_20090818_v1.0.pdf)
for establishing quadrats for vegetation sampling.</skos:example>
    <rdfs:subClassOf rdf:resource="http://www.w3.org/ns/sosa/Procedure"/>
    <rdfs:subClassOf rdf:nodeID="ub1bL700C19"/>
  </rdf:Description>
  <rdf:Description rdf:nodeID="ub1bL558C19">
    <owl:allValuesFrom rdf:resource="http://www.w3.org/2001/XMLSchema#string"/>
    <owl:onProperty rdf:resource="http://www.w3.org/2000/01/rdf-schema#comment"/>
    <rdf:type rdf:resource="http://www.w3.org/2002/07/owl#Restriction"/>
  </rdf:Description>
  <rdf:Description rdf:nodeID="ub1bL887C19">
    <owl:allValuesFrom rdf:resource="https://w3id.org/tern/ontologies/org/Person"/>
    <owl:onProperty rdf:resource="http://www.w3.org/ns/prov#wasAttributedTo"/>
    <rdf:type rdf:resource="http://www.w3.org/2002/07/owl#Restriction"/>
  </rdf:Description>
  <rdf:Description rdf:nodeID="ub1bL1297C19">
    <owl:onProperty rdf:resource="http://www.w3.org/ns/sosa/isSampleOf"/>
    <owl:allValuesFrom rdf:resource="https://w3id.org/tern/ontologies/tern/SoilProfile"/>
    <rdf:type rdf:resource="http://www.w3.org/2002/07/owl#Restriction"/>
  </rdf:Description>
  <rdf:Description rdf:nodeID="ub1bL1078C19">
    <rdf:type rdf:resource="http://www.w3.org/2002/07/owl#Restriction"/>
    <owl:onProperty rdf:resource="https://w3id.org/tern/ontologies/tern/cardinalDirection"/>
    <owl:maxQualifiedCardinality rdf:datatype="http://www.w3.org/2001/XMLSchema#nonNegativeInteger">1</owl:maxQualifiedCardinality>
    <owl:onClass rdf:resource="http://www.w3.org/2001/XMLSchema#string"/>
  </rdf:Description>
  <rdf:Description rdf:about="https://w3id.org/tern/ontologies/tern/Input">
    <rdfs:subClassOf rdf:resource="http://www.w3.org/ns/ssn/Input"/>
    <rdfs:label>Input</rdfs:label>
    <rdf:type rdf:resource="http://www.w3.org/2002/07/owl#Class"/>
    <rdfs:subClassOf rdf:nodeID="ub1bL417C19"/>
    <rdfs:subClassOf rdf:nodeID="ub1bL422C19"/>
    <skos:example>A **wedge prism** or **relascope** can be used to estimate the Basal Area per hectare. 
The number of counted trees and the Basal Area Factor are inputs to estimate the Basal Area.</skos:example>
    <skos:definition>*Input* - Any information that is provided to a [Procedure](#Procedure) for its use.</skos:definition>
    <rdfs:subClassOf rdf:nodeID="ub1bL412C19"/>
  </rdf:Description>
  <rdf:Description rdf:about="https://w3id.org/tern/ontologies/tern/hasParameter">
    <skos:definition>A property that links a concept to a parameter.</skos:definition>
    <rdfs:label>has parameter</rdfs:label>
    <rdf:type rdf:resource="http://www.w3.org/1999/02/22-rdf-syntax-ns#Property"/>
    <rdfs:subPropertyOf rdf:resource="http://www.w3.org/2004/02/skos/core#relatedMatch"/>
  </rdf:Description>
  <rdf:Description rdf:nodeID="ub1bL604C19">
    <owl:onClass rdf:resource="https://w3id.org/tern/ontologies/tern/ObservableProperty"/>
    <owl:onProperty rdf:resource="http://www.w3.org/ns/sosa/observedProperty"/>
    <owl:qualifiedCardinality rdf:datatype="http://www.w3.org/2001/XMLSchema#nonNegativeInteger">1</owl:qualifiedCardinality>
    <rdf:type rdf:resource="http://www.w3.org/2002/07/owl#Restriction"/>
  </rdf:Description>
  <rdf:Description rdf:about="https://w3id.org/tern/ontologies/tern/Radiometer">
    <rdfs:comment>A radiometer or roentgenometer is a device for measuring the radiant flux (power) of electromagnetic radiation. Generally, a radiometer is an infrared radiation detector or an ultraviolet detector.</rdfs:comment>
    <rdfs:subClassOf rdf:resource="https://w3id.org/tern/ontologies/tern/RadiationSensor"/>
    <rdfs:label>Radiometer</rdfs:label>
    <rdfs:seeAlso rdf:resource="https://en.wikipedia.org/wiki/Radiometer"/>
    <rdf:type rdf:resource="http://www.w3.org/2002/07/owl#Class"/>
  </rdf:Description>
  <rdf:Description rdf:nodeID="ub1bL368C19">
    <owl:maxQualifiedCardinality rdf:datatype="http://www.w3.org/2001/XMLSchema#nonNegativeInteger">1</owl:maxQualifiedCardinality>
    <rdf:type rdf:resource="http://www.w3.org/2002/07/owl#Restriction"/>
    <owl:onProperty rdf:resource="https://w3id.org/tern/ontologies/tern/dateDecommissioned"/>
    <owl:onClass rdf:resource="http://www.w3.org/2001/XMLSchema#date"/>
  </rdf:Description>
  <rdf:Description rdf:nodeID="ub1bL104C23">
    <rdf:type rdf:resource="https://schema.org/Person"/>
    <schema-https:name>Javier Sanchez Gonzalez</schema-https:name>
    <schema-https:affiliation rdf:resource="https://w3id.org/tern/resources/a083902d-d821-41be-b663-1d7cb33eea66"/>
    <schema-https:email>j.sanchezgonzalez@uq.edu.au</schema-https:email>
  </rdf:Description>
  <rdf:Description rdf:nodeID="ub1bL788C25">
    <owl:unionOf rdf:nodeID="fcf4ebf340cd54dc4871b974b242da6f5b10"/>
    <rdf:type rdf:resource="http://www.w3.org/2002/07/owl#Class"/>
  </rdf:Description>
  <rdf:Description rdf:about="https://w3id.org/tern/ontologies/tern/Sampling">
    <rdfs:subClassOf rdf:nodeID="ub1bL898C19"/>
    <skos:example>Crushing a rock sample in a ball mill to create sub-samples of the rock.
Digging a pit through a soil sequence.
Dividing a field site into quadrants.
Drawing blood from a patient.
Drilling an observation well.
Establishing a station for environmental monitoring.
Registering an image of the landscape.
Sieving a powder to separate the subset finer than 100-mesh.
Selecting a subset of a population.
Splitting a piece of drill-core to create two new samples.
Taking a diamond-drill core from a rock outcrop.</skos:example>
    <rdfs:subClassOf rdf:nodeID="ub1bL904C19"/>
    <rdfs:label>Sampling</rdfs:label>
    <rdfs:subClassOf rdf:resource="http://www.w3.org/ns/sosa/Sampling"/>
    <rdfs:subClassOf rdf:nodeID="ub1bL887C19"/>
    <rdfs:subClassOf rdf:nodeID="ub1bL882C19"/>
    <rdf:type rdf:resource="http://www.w3.org/2002/07/owl#Class"/>
    <skos:definition>An activity of [Sampling](#Sampling) carries out a (Sampling) [Procedure](#Procedure) to create or transform one or more [Samples](#Sample).</skos:definition>
    <rdfs:subClassOf rdf:resource="http://www.w3.org/ns/prov#Activity"/>
    <rdfs:subClassOf rdf:nodeID="ub1bL910C19"/>
    <rdfs:subClassOf rdf:nodeID="ub1bL892C19"/>
  </rdf:Description>
  <rdf:Description rdf:about="https://w3id.org/tern/ontologies/tern/isSubActivityOf">
    <rdf:type rdf:resource="http://www.w3.org/1999/02/22-rdf-syntax-ns#Property"/>
    <skos:definition>A property that links an activity to its parent activity.</skos:definition>
    <rdfs:label>is sub activity of</rdfs:label>
  </rdf:Description>
  <rdf:Description rdf:nodeID="ub1bL1114C19">
    <rdf:type rdf:resource="http://www.w3.org/2002/07/owl#Restriction"/>
    <owl:onClass rdf:resource="https://w3id.org/tern/ontologies/loc/Polygon"/>
    <owl:onProperty rdf:resource="https://w3id.org/tern/ontologies/tern/polygon"/>
    <owl:maxQualifiedCardinality rdf:datatype="http://www.w3.org/2001/XMLSchema#nonNegativeInteger">1</owl:maxQualifiedCardinality>
  </rdf:Description>
  <rdf:Description rdf:about="https://w3id.org/tern/ontologies/tern/soilHorizonClassifier">
    <rdfs:label>soil horizon classifier</rdfs:label>
    <skos:definition>Soil horizon classifier as defined in the Australian Soil and Land Survey Field Handbook on page 148.</skos:definition>
    <rdf:type rdf:resource="http://www.w3.org/1999/02/22-rdf-syntax-ns#Property"/>
  </rdf:Description>
  <rdf:Description rdf:nodeID="ub1bL705C19">
    <owl:onProperty rdf:resource="http://linked.data.gov.au/def/datatype/vocabulary"/>
    <owl:cardinality rdf:datatype="http://www.w3.org/2001/XMLSchema#nonNegativeInteger">1</owl:cardinality>
    <rdf:type rdf:resource="http://www.w3.org/2002/07/owl#Restriction"/>
  </rdf:Description>
  <rdf:Description rdf:nodeID="ub1bL92C23">
    <schema-https:affiliation rdf:resource="https://w3id.org/tern/resources/a083902d-d821-41be-b663-1d7cb33eea66"/>
    <rdf:type rdf:resource="https://schema.org/Person"/>
    <schema-https:name>Anusuriya Devaraju</schema-https:name>
    <schema-https:email>a.devaraju@uq.edu.au</schema-https:email>
  </rdf:Description>
  <rdf:Description rdf:nodeID="ub1bL1010C19">
    <owl:onProperty rdf:resource="http://www.w3.org/2000/01/rdf-schema#comment"/>
    <rdf:type rdf:resource="http://www.w3.org/2002/07/owl#Restriction"/>
    <owl:allValuesFrom rdf:resource="http://www.w3.org/2001/XMLSchema#string"/>
  </rdf:Description>
  <rdf:Description rdf:nodeID="ub1bL945C19">
    <owl:onClass rdf:resource="http://linked.data.gov.au/def/datatype/QuantitativeMeasure"/>
    <owl:maxQualifiedCardinality rdf:datatype="http://www.w3.org/2001/XMLSchema#nonNegativeInteger">1</owl:maxQualifiedCardinality>
    <owl:onProperty rdf:resource="https://w3id.org/tern/ontologies/loc/elevation"/>
    <rdf:type rdf:resource="http://www.w3.org/2002/07/owl#Restriction"/>
  </rdf:Description>
  <rdf:Description rdf:nodeID="ub1bL286C19">
    <rdf:type rdf:resource="http://www.w3.org/2002/07/owl#Restriction"/>
    <owl:allValuesFrom rdf:nodeID="ub1bL288C25"/>
    <owl:onProperty rdf:resource="https://w3id.org/tern/ontologies/tern/width"/>
  </rdf:Description>
  <rdf:Description rdf:about="https://w3id.org/tern/ontologies/tern/PhenologyCamera">
    <rdfs:subClassOf rdf:resource="https://w3id.org/tern/ontologies/tern/Sampler"/>
    <rdfs:seeAlso rdf:resource="https://www.neonscience.org/data-collection/phenocams"/>
    <skos:definition>A "phenocam" is a digital camera capturing time-lapse images of foliage which can be used to generate quantitative measures of plant phenology. Over time, these data provide a near-continuous visual record of canopy change and environmental conditions.</skos:definition>
    <rdf:type rdf:resource="http://www.w3.org/2002/07/owl#Class"/>
    <skos:altLabel>Phenocam</skos:altLabel>
    <skos:altLabel>Phenocamera</skos:altLabel>
    <rdfs:subClassOf rdf:nodeID="ub1bL648C19"/>
    <rdfs:subClassOf rdf:nodeID="ub1bL653C19"/>
    <rdfs:subClassOf rdf:nodeID="ub1bL658C19"/>
    <rdfs:label>Phenology Camera</rdfs:label>
  </rdf:Description>
  <rdf:Description rdf:about="https://w3id.org/tern/ontologies/tern/hasEnvironmentalCharacteristic">
    <rdfs:label>has environmental characteristic</rdfs:label>
    <rdfs:range rdf:resource="https://w3id.org/tern/ontologies/tern/EnvironmentalCharacteristic"/>
    <skos:definition>The subject has some environmental characteristic. Points to a set of [Observations](#Observation) within an [EnvironmentalCharacteristic](#EnvironmentalCharacteristic).</skos:definition>
    <rdf:type rdf:resource="http://www.w3.org/2002/07/owl#ObjectProperty"/>
  </rdf:Description>
  <rdf:Description rdf:nodeID="ub1bL474C19">
    <owl:maxQualifiedCardinality rdf:datatype="http://www.w3.org/2001/XMLSchema#nonNegativeInteger">1</owl:maxQualifiedCardinality>
    <owl:onDataRange rdf:resource="http://www.w3.org/2001/XMLSchema#string"/>
    <rdf:type rdf:resource="http://www.w3.org/2002/07/owl#Restriction"/>
    <owl:onProperty rdf:resource="https://w3id.org/tern/ontologies/tern/purpose"/>
  </rdf:Description>
  <rdf:Description rdf:about="https://w3id.org/tern/ontologies/tern/FeatureOfInterest">
    <rdf:type rdf:resource="http://www.w3.org/2002/07/owl#Class"/>
    <rdfs:label>Feature of Interest</rdfs:label>
    <rdf:type rdf:resource="http://www.w3.org/2000/01/rdf-schema#Class"/>
    <skos:definition xml:lang="en">The thing whose property is being estimated or calculated in the course of an Observation to arrive at a Result or whose property is being manipulated by an Actuator, or which is being sampled or transformed in an act of Sampling.</skos:definition>
    <skos:example xml:lang="en">When measuring the height of a tree, the height is the observed ObservableProperty, 20m may be the Result of the Observation, and the tree is the FeatureOfInterest. A window is a FeatureOfInterest for an automatic window control Actuator.</skos:example>
    <rdfs:subClassOf rdf:resource="http://www.w3.org/ns/sosa/FeatureOfInterest"/>
  </rdf:Description>
  <rdf:Description rdf:nodeID="ub1bL332C19">
    <owl:onClass rdf:resource="https://w3id.org/tern/ontologies/tern/Observation"/>
    <rdf:type rdf:resource="http://www.w3.org/2002/07/owl#Restriction"/>
    <owl:onProperty rdf:resource="http://www.w3.org/ns/sosa/isFeatureOfInterestOf"/>
    <owl:minQualifiedCardinality rdf:datatype="http://www.w3.org/2001/XMLSchema#nonNegativeInteger">1</owl:minQualifiedCardinality>
  </rdf:Description>
  <rdf:Description rdf:nodeID="ub1bL833C19">
    <rdf:type rdf:resource="http://www.w3.org/2002/07/owl#Restriction"/>
    <owl:allValuesFrom rdf:resource="https://w3id.org/tern/ontologies/tern/Sample"/>
    <owl:onProperty rdf:resource="http://www.w3.org/ns/sosa/hasSample"/>
  </rdf:Description>
  <rdf:Description rdf:about="https://w3id.org/tern/ontologies/tern/Sensor">
    <skos:definition>Device, agent (including humans), or software (simulation) involved in, or implementing, a Procedure. Sensors respond to a stimulus, e.g., a change in the environment, or input data composed from the results of prior Observations, and generate a Result. Sensors can be hosted by Platforms.</skos:definition>
    <rdfs:subClassOf rdf:resource="https://w3id.org/tern/ontologies/tern/Instrument"/>
    <rdfs:subClassOf rdf:nodeID="ub1bL988C19"/>
    <rdf:type rdf:resource="http://www.w3.org/2002/07/owl#Class"/>
    <rdfs:label>Sensor</rdfs:label>
    <rdfs:subClassOf rdf:resource="http://www.w3.org/ns/sosa/Sensor"/>
    <rdfs:subClassOf rdf:nodeID="ub1bL993C19"/>
  </rdf:Description>
  <rdf:Description rdf:nodeID="ub1bL445C19">
    <rdf:type rdf:resource="http://www.w3.org/2002/07/owl#Restriction"/>
    <owl:onProperty rdf:resource="http://purl.org/dc/terms/source"/>
    <owl:allValuesFrom rdf:nodeID="ub1bL447C25"/>
  </rdf:Description>
  <rdf:Description rdf:about="https://w3id.org/tern/ontologies/tern/EcosystemProcessesSite">
    <rdf:type rdf:resource="http://www.w3.org/2002/07/owl#Class"/>
    <rdfs:subClassOf rdf:resource="https://w3id.org/tern/ontologies/tern/Site"/>
    <rdfs:label>Ecosystem Processes Site</rdfs:label>
    <skos:definition>An ecological [Site](#EcologicalSite) that usually hosts a [FluxTower](#FluxTower).</skos:definition>
  </rdf:Description>
  <rdf:Description rdf:about="https://w3id.org/tern/ontologies/tern/instructions">
    <rdfs:label>instructions</rdfs:label>
    <rdf:type rdf:resource="http://www.w3.org/2002/07/owl#DatatypeProperty"/>
    <skos:definition>Describe the instructions of the procedure/method.</skos:definition>
    <rdfs:range rdf:resource="http://www.w3.org/2001/XMLSchema#string"/>
  </rdf:Description>
  <rdf:Description rdf:nodeID="ub1bL302C19">
    <owl:onProperty rdf:resource="https://w3id.org/tern/ontologies/tern/width"/>
    <rdf:type rdf:resource="http://www.w3.org/2002/07/owl#Restriction"/>
    <owl:cardinality rdf:datatype="http://www.w3.org/2001/XMLSchema#nonNegativeInteger">1</owl:cardinality>
  </rdf:Description>
  <rdf:Description rdf:nodeID="fcf4ebf340cd54dc4871b974b242da6f5b3">
    <rdf:first rdf:resource="http://www.w3.org/2001/XMLSchema#decimal"/>
    <rdf:rest rdf:nodeID="fcf4ebf340cd54dc4871b974b242da6f5b4"/>
  </rdf:Description>
  <rdf:Description rdf:nodeID="ub1bL848C19">
    <owl:onProperty rdf:resource="http://www.w3.org/ns/sosa/isResultOf"/>
    <rdf:type rdf:resource="http://www.w3.org/2002/07/owl#Restriction"/>
    <owl:onClass rdf:resource="https://w3id.org/tern/ontologies/tern/Sampling"/>
    <owl:maxQualifiedCardinality rdf:datatype="http://www.w3.org/2001/XMLSchema#nonNegativeInteger">1</owl:maxQualifiedCardinality>
  </rdf:Description>
  <rdf:Description rdf:about="https://w3id.org/tern/ontologies/tern/globalValue">
    <rdfs:label>global value</rdfs:label>
    <rdf:type rdf:resource="http://www.w3.org/1999/02/22-rdf-syntax-ns#Property"/>
    <skos:definition>A property that links a concept from a vocabulary to another concept in an authoritative/endorsed vocabulary.</skos:definition>
    <skos:example>The concept dry soil colour is defined in two vocabularies, 
[CORVEG](http://linked.data.gov.au/def/corveg-cv/1842b772-72a4-430f-a264-dcfd6c2c23b4) and 
[Ausplots](http://linked.data.gov.au/def/ausplots-cv/aa11e5f7-aec2-4e92-95b8-6332911f0c4e). 
The property global value is used to map the concept from the two vocabularies to the relevant 
[concept](http://linked.data.gov.au/def/tern-cv/beceaa5a-a296-4385-a55a-3b8c8d5b2369) 
specified in the main vocabulary, i.e., TERN Vocabularies.</skos:example>
  </rdf:Description>
  <rdf:Description rdf:about="https://w3id.org/tern/ontologies/tern/sampleStorageLocation">
    <rdf:type rdf:resource="http://www.w3.org/1999/02/22-rdf-syntax-ns#Property"/>
    <skos:definition>A property that links a [PhysicalSpecimen](#PhysicalSpecimen) to the location [Point](https://w3id.org/tern/ontologies/loc/Point) of where it is stored.</skos:definition>
    <rdfs:label>sample storage location</rdfs:label>
    <rdfs:subPropertyOf rdf:resource="http://www.opengis.net/ont/geosparql#hasGeometry"/>
  </rdf:Description>
  <rdf:Description rdf:nodeID="ub1bL1357C19">
    <owl:onProperty rdf:resource="http://www.opengis.net/ont/geosparql#hasGeometry"/>
    <owl:onClass rdf:resource="https://w3id.org/tern/ontologies/loc/LineString"/>
    <owl:qualifiedCardinality rdf:datatype="http://www.w3.org/2001/XMLSchema#nonNegativeInteger">1</owl:qualifiedCardinality>
    <rdf:type rdf:resource="http://www.w3.org/2002/07/owl#Restriction"/>
  </rdf:Description>
  <rdf:Description rdf:nodeID="ub1bL1005C19">
    <rdf:type rdf:resource="http://www.w3.org/2002/07/owl#Restriction"/>
    <owl:onProperty rdf:resource="http://www.opengis.net/ont/geosparql#sfWithin"/>
    <owl:allValuesFrom rdf:resource="http://www.opengis.net/ont/geosparql#Feature"/>
  </rdf:Description>
  <rdf:Description rdf:nodeID="ub1bL677C19">
    <owl:onClass rdf:resource="https://w3id.org/tern/ontologies/loc/Point"/>
    <owl:maxQualifiedCardinality rdf:datatype="http://www.w3.org/2001/XMLSchema#nonNegativeInteger">1</owl:maxQualifiedCardinality>
    <owl:onProperty rdf:resource="https://w3id.org/tern/ontologies/tern/sampleStorageLocation"/>
    <rdf:type rdf:resource="http://www.w3.org/2002/07/owl#Restriction"/>
  </rdf:Description>
  <rdf:Description rdf:about="https://w3id.org/tern/ontologies/tern/Parameter">
    <rdfs:subClassOf rdf:resource="http://www.w3.org/2004/02/skos/core#Concept"/>
    <rdf:type rdf:resource="http://www.w3.org/2002/07/owl#Class"/>
    <rdfs:label>Parameter</rdfs:label>
    <skos:definition>A [FeatureOfInterest's](http://w3.org/ns/sosa/FeatureOfInterest) property or characteristic which an [Observation](#Observation) is measuring using some [Procedure](#Procedure).</skos:definition>
  </rdf:Description>
  <rdf:Description rdf:about="https://w3id.org/tern/ontologies/tern/transectEndPoint">
    <rdfs:label>transect end point</rdfs:label>
    <skos:definition>Refers to the [tern-loc:Point](https://w3id.org/tern/ontologies/loc/Point) representing the end of a transect.</skos:definition>
    <rdf:type rdf:resource="http://www.w3.org/1999/02/22-rdf-syntax-ns#Property"/>
  </rdf:Description>
  <rdf:Description rdf:about="https://w3id.org/tern/ontologies/tern/ObservableProperty">
    <skos:example>Sampling depth, bulk density, pH are examples of properties of a 
soil sample, and the soil sample is the feature-of-interest, 
representative of the area from which it is collected.</skos:example>
    <rdfs:label>Observable Property</rdfs:label>
    <rdfs:subClassOf rdf:nodeID="ub1bL526C19"/>
    <skos:definition>An observable quality (property, characteristic) of a [FeatureOfInterest](http://w3.org/ns/sosa/FeatureOfInterest). A feature-of-interest refers to a feature whose properties are measured or observed. </skos:definition>
    <rdfs:subClassOf rdf:nodeID="ub1bL514C19"/>
    <rdfs:subClassOf rdf:nodeID="ub1bL531C19"/>
    <rdfs:subClassOf rdf:nodeID="ub1bL536C19"/>
    <rdfs:subClassOf rdf:resource="http://www.w3.org/ns/sosa/ObservableProperty"/>
    <rdf:type rdf:resource="http://www.w3.org/2002/07/owl#Class"/>
    <rdfs:subClassOf rdf:nodeID="ub1bL542C19"/>
  </rdf:Description>
  <rdf:Description rdf:about="https://w3id.org/tern/ontologies/tern/Transect">
    <rdfs:subClassOf rdf:nodeID="ub1bL1357C19"/>
    <rdfs:subClassOf rdf:nodeID="ub1bL1363C19"/>
    <rdfs:subClassOf rdf:nodeID="ub1bL1352C19"/>
    <rdfs:subClassOf rdf:nodeID="ub1bL1347C19"/>
    <rdfs:subClassOf rdf:nodeID="ub1bL1369C19"/>
    <rdfs:subClassOf rdf:resource="https://w3id.org/tern/ontologies/tern/Sample"/>
    <skos:definition>A straight line or narrow section through an object or natural feature or across the earth's surface, along which observations are made or measurements taken.</skos:definition>
    <rdf:type rdf:resource="http://www.w3.org/2002/07/owl#Class"/>
    <rdfs:label>Transect</rdfs:label>
  </rdf:Description>
  <rdf:Description rdf:nodeID="ub1bL514C19">
    <rdf:type rdf:resource="http://www.w3.org/2002/07/owl#Restriction"/>
    <owl:allValuesFrom rdf:nodeID="ub1bL516C25"/>
    <owl:onProperty rdf:resource="https://w3id.org/tern/ontologies/tern/globalVocabulary"/>
  </rdf:Description>
  <rdf:Description rdf:nodeID="ub1bL468C19">
    <owl:maxQualifiedCardinality rdf:datatype="http://www.w3.org/2001/XMLSchema#nonNegativeInteger">1</owl:maxQualifiedCardinality>
    <owl:onDataRange rdf:resource="http://www.w3.org/2001/XMLSchema#string"/>
    <rdf:type rdf:resource="http://www.w3.org/2002/07/owl#Restriction"/>
    <owl:onProperty rdf:resource="https://w3id.org/tern/ontologies/tern/instructions"/>
  </rdf:Description>
  <rdf:Description rdf:nodeID="fcf4ebf340cd54dc4871b974b242da6f5b9">
    <rdf:first rdf:resource="http://www.w3.org/2002/07/owl#Ontology"/>
    <rdf:rest rdf:resource="http://www.w3.org/1999/02/22-rdf-syntax-ns#nil"/>
  </rdf:Description>
  <rdf:Description rdf:nodeID="ub1bL957C19">
    <owl:onProperty rdf:resource="https://w3id.org/tern/ontologies/tern/isSamplingPointOf"/>
    <owl:maxQualifiedCardinality rdf:datatype="http://www.w3.org/2001/XMLSchema#nonNegativeInteger">1</owl:maxQualifiedCardinality>
    <owl:onClass rdf:resource="https://w3id.org/tern/ontologies/tern/Transect"/>
    <rdf:type rdf:resource="http://www.w3.org/2002/07/owl#Restriction"/>
  </rdf:Description>
  <rdf:Description rdf:nodeID="ub1bL1169C19">
    <rdf:type rdf:resource="http://www.w3.org/2002/07/owl#Restriction"/>
    <owl:qualifiedCardinality rdf:datatype="http://www.w3.org/2001/XMLSchema#nonNegativeInteger">1</owl:qualifiedCardinality>
    <owl:onClass rdf:resource="https://w3id.org/tern/ontologies/tern/Site"/>
    <owl:onProperty rdf:resource="http://www.w3.org/ns/sosa/isSampleOf"/>
  </rdf:Description>
  <rdf:Description rdf:nodeID="ub1bL592C19">
    <owl:onClass rdf:resource="http://www.w3.org/2006/time#Instant"/>
    <owl:qualifiedCardinality rdf:datatype="http://www.w3.org/2001/XMLSchema#nonNegativeInteger">1</owl:qualifiedCardinality>
    <owl:onProperty rdf:resource="http://www.w3.org/ns/sosa/phenomenonTime"/>
    <rdf:type rdf:resource="http://www.w3.org/2002/07/owl#Restriction"/>
  </rdf:Description>
  <rdf:Description rdf:nodeID="fcf4ebf340cd54dc4871b974b242da6f5b4">
    <rdf:rest rdf:resource="http://www.w3.org/1999/02/22-rdf-syntax-ns#nil"/>
    <rdf:first rdf:resource="http://www.w3.org/2001/XMLSchema#integer"/>
  </rdf:Description>
  <rdf:Description rdf:nodeID="ub1bL45C19">
    <rdf:type rdf:resource="http://www.w3.org/2002/07/owl#Restriction"/>
    <owl:onProperty rdf:resource="https://w3id.org/tern/ontologies/tern/globalValue"/>
    <owl:cardinality rdf:datatype="http://www.w3.org/2001/XMLSchema#nonNegativeInteger">1</owl:cardinality>
  </rdf:Description>
  <rdf:Description rdf:about="https://w3id.org/tern/ontologies/tern/Sampler">
    <rdfs:subClassOf rdf:nodeID="ub1bL863C19"/>
    <rdf:type rdf:resource="http://www.w3.org/2002/07/owl#Class"/>
    <rdfs:subClassOf rdf:resource="http://www.w3.org/ns/sosa/Sampler"/>
    <rdfs:subClassOf rdf:nodeID="ub1bL868C19"/>
    <rdfs:label>Sampler</rdfs:label>
    <skos:definition>A device that is used by, or implements, a (Sampling) [Procedure](#Procedure) to create or transform one or more samples.</skos:definition>
    <skos:example>Soil probe is an example of device used to collect a soil core.</skos:example>
    <rdfs:subClassOf rdf:resource="https://w3id.org/tern/ontologies/tern/Instrument"/>
  </rdf:Description>
  <rdf:Description rdf:nodeID="ub1bL1240C19">
    <owl:onProperty rdf:resource="https://w3id.org/tern/ontologies/tern/hasSubActivity"/>
    <rdf:type rdf:resource="http://www.w3.org/2002/07/owl#Restriction"/>
    <owl:allValuesFrom rdf:nodeID="ub1bL1242C25"/>
  </rdf:Description>
  <rdf:Description rdf:about="http://rs.tdwg.org/dwc/terms/materialSampleID">
    <skos:example>IGSN:ASR000001 (Resulting URI: http://igsn.org/ASR000001) 
is a globally unique and persistent identifier of a soil sample.</skos:example>
    <rdfs:label>material sample ID</rdfs:label>
    <rdfs:isDefinedBy rdf:resource="http://rs.tdwg.org/dwc/terms/"/>
    <rdfs:comment>An identifier for the MaterialSample (as opposed to a particular digital record of the material sample). In the absence of a persistent global unique identifier, construct one from a combination of identifiers in the record that will most closely make the materialSampleID globally unique.</rdfs:comment>
    <rdf:type rdf:resource="http://www.w3.org/1999/02/22-rdf-syntax-ns#Property"/>
  </rdf:Description>
  <rdf:Description rdf:nodeID="ub1bL1220C19">
    <rdf:type rdf:resource="http://www.w3.org/2002/07/owl#Restriction"/>
    <owl:onProperty rdf:resource="http://www.w3.org/ns/prov#startedAtTime"/>
    <owl:allValuesFrom rdf:resource="http://www.w3.org/2001/XMLSchema#dateTime"/>
  </rdf:Description>
  <rdf:Description rdf:nodeID="ub1bL422C19">
    <owl:qualifiedCardinality rdf:datatype="http://www.w3.org/2001/XMLSchema#nonNegativeInteger">1</owl:qualifiedCardinality>
    <rdf:type rdf:resource="http://www.w3.org/2002/07/owl#Restriction"/>
    <owl:onProperty rdf:resource="http://www.w3.org/2000/01/rdf-schema#label"/>
    <owl:onClass rdf:resource="http://www.w3.org/2001/XMLSchema#string"/>
  </rdf:Description>
  <rdf:Description rdf:nodeID="ub1bL1096C19">
    <owl:maxQualifiedCardinality rdf:datatype="http://www.w3.org/2001/XMLSchema#nonNegativeInteger">1</owl:maxQualifiedCardinality>
    <rdf:type rdf:resource="http://www.w3.org/2002/07/owl#Restriction"/>
    <owl:onProperty rdf:resource="https://w3id.org/tern/ontologies/tern/siteShape"/>
    <owl:onClass rdf:resource="http://www.w3.org/2004/02/skos/core#Concept"/>
  </rdf:Description>
  <rdf:Description rdf:nodeID="ub1bL988C19">
    <owl:onProperty rdf:resource="http://www.w3.org/ns/sosa/observes"/>
    <owl:allValuesFrom rdf:resource="https://w3id.org/tern/ontologies/tern/ObservableProperty"/>
    <rdf:type rdf:resource="http://www.w3.org/2002/07/owl#Restriction"/>
  </rdf:Description>
  <rdf:Description rdf:nodeID="ub1bL140C29">
    <rdf:type rdf:resource="https://schema.org/Organization"/>
    <schema-https:identifier rdf:resource="https://w3id.org/tern/resources/276dd611-5d74-4555-b20f-12f0f0b618a1"/>
    <schema-https:name>CSIRO</schema-https:name>
  </rdf:Description>
  <rdf:Description rdf:about="https://w3id.org/tern/ontologies/tern/cardinalDirection">
    <skos:definition>The cardinal direction of the *thing* represented as a string and expressed by cardinal and intercardinal points. </skos:definition>
    <rdfs:label>cardinal direction</rdfs:label>
    <skos:example>NNE, W, SE, etc.</skos:example>
    <rdf:type rdf:resource="http://www.w3.org/1999/02/22-rdf-syntax-ns#Property"/>
    <rdfs:range rdf:resource="http://www.w3.org/2001/XMLSchema#string"/>
  </rdf:Description>
  <rdf:Description rdf:nodeID="ub1bL417C19">
    <rdf:type rdf:resource="http://www.w3.org/2002/07/owl#Restriction"/>
    <owl:onProperty rdf:resource="http://linked.data.gov.au/def/datatype/value"/>
    <owl:cardinality rdf:datatype="http://www.w3.org/2001/XMLSchema#nonNegativeInteger">1</owl:cardinality>
  </rdf:Description>
  <rdf:Description rdf:nodeID="ub1bL818C19">
    <owl:allValuesFrom rdf:resource="http://www.w3.org/2001/XMLSchema#string"/>
    <owl:onProperty rdf:resource="http://www.w3.org/2000/01/rdf-schema#comment"/>
    <rdf:type rdf:resource="http://www.w3.org/2002/07/owl#Restriction"/>
  </rdf:Description>
  <rdf:Description rdf:about="https://w3id.org/tern/ontologies/tern/OEHSite">
    <rdfs:label>OEH Site</rdfs:label>
    <skos:definition>A plot survey site managed by the NSW Office of Environment and Heritage (OEH).</skos:definition>
    <rdfs:seeAlso rdf:resource="https://www.environment.nsw.gov.au/surveys/AnimalAndPlantSurveys.htm"/>
    <rdf:type rdf:resource="http://www.w3.org/2002/07/owl#Class"/>
    <rdfs:subClassOf rdf:resource="https://w3id.org/tern/ontologies/tern/Site"/>
  </rdf:Description>
  <rdf:Description rdf:nodeID="ub1bL398C19">
    <owl:qualifiedCardinality rdf:datatype="http://www.w3.org/2001/XMLSchema#nonNegativeInteger">1</owl:qualifiedCardinality>
    <owl:onProperty rdf:resource="https://w3id.org/tern/ontologies/tern/centroidPoint"/>
    <owl:onClass rdf:resource="https://w3id.org/tern/ontologies/loc/Point"/>
    <rdf:type rdf:resource="http://www.w3.org/2002/07/owl#Restriction"/>
  </rdf:Description>
  <rdf:Description rdf:nodeID="ub1bL116C23">
    <rdf:type rdf:resource="https://schema.org/Person"/>
    <schema-https:email>t.parkhurst@uq.edu.au</schema-https:email>
    <schema-https:name>Tina Parkhurst</schema-https:name>
    <schema-https:affiliation rdf:resource="https://w3id.org/tern/resources/a083902d-d821-41be-b663-1d7cb33eea66"/>
  </rdf:Description>
  <rdf:Description rdf:nodeID="ub1bL1251C19">
    <owl:onProperty rdf:resource="https://w3id.org/tern/ontologies/tern/locationDescription"/>
    <owl:maxQualifiedCardinality rdf:datatype="http://www.w3.org/2001/XMLSchema#nonNegativeInteger">1</owl:maxQualifiedCardinality>
    <owl:onClass rdf:resource="http://www.w3.org/2001/XMLSchema#string"/>
    <rdf:type rdf:resource="http://www.w3.org/2002/07/owl#Restriction"/>
  </rdf:Description>
  <rdf:Description rdf:nodeID="ub1bL739C19">
    <owl:onProperty rdf:resource="http://schema.org/name"/>
    <rdf:type rdf:resource="http://www.w3.org/2002/07/owl#Restriction"/>
    <owl:onClass rdf:resource="http://www.w3.org/2001/XMLSchema#string"/>
    <owl:qualifiedCardinality rdf:datatype="http://www.w3.org/2001/XMLSchema#nonNegativeInteger">1</owl:qualifiedCardinality>
  </rdf:Description>
  <rdf:Description rdf:nodeID="ub1bL563C19">
    <owl:onProperty rdf:resource="http://www.w3.org/ns/prov#wasAttributedTo"/>
    <owl:allValuesFrom rdf:resource="https://w3id.org/tern/ontologies/org/Person"/>
    <rdf:type rdf:resource="http://www.w3.org/2002/07/owl#Restriction"/>
  </rdf:Description>
  <rdf:Description rdf:nodeID="fcf4ebf340cd54dc4871b974b242da6f5b19">
    <rdf:first rdf:resource="http://www.w3.org/2001/XMLSchema#int"/>
    <rdf:rest rdf:resource="http://www.w3.org/1999/02/22-rdf-syntax-ns#nil"/>
  </rdf:Description>
  <rdf:Description rdf:nodeID="ub1bL363C19">
    <rdf:type rdf:resource="http://www.w3.org/2002/07/owl#Restriction"/>
    <owl:onProperty rdf:resource="http://www.w3.org/2000/01/rdf-schema#comment"/>
    <owl:allValuesFrom rdf:resource="http://www.w3.org/2001/XMLSchema#string"/>
  </rdf:Description>
  <rdf:Description rdf:nodeID="ub1bL616C19">
    <owl:qualifiedCardinality rdf:datatype="http://www.w3.org/2001/XMLSchema#nonNegativeInteger">1</owl:qualifiedCardinality>
    <owl:onDataRange rdf:resource="http://www.w3.org/2001/XMLSchema#dateTime"/>
    <owl:onProperty rdf:resource="http://www.w3.org/ns/sosa/resultTime"/>
    <rdf:type rdf:resource="http://www.w3.org/2002/07/owl#Restriction"/>
  </rdf:Description>
  <rdf:Description rdf:nodeID="ub1bL1347C19">
    <rdf:type rdf:resource="http://www.w3.org/2002/07/owl#Restriction"/>
    <owl:allValuesFrom rdf:resource="https://w3id.org/tern/ontologies/tern/SamplingPoint"/>
    <owl:onProperty rdf:resource="https://w3id.org/tern/ontologies/tern/hasSamplingPoint"/>
  </rdf:Description>
  <rdf:Description rdf:about="https://w3id.org/tern/ontologies/tern/FixedPlatform">
    <skos:definition>A fixed platform based on land.</skos:definition>
    <rdf:type rdf:resource="http://www.w3.org/2002/07/owl#Class"/>
    <rdfs:label>Fixed Platform</rdfs:label>
    <rdfs:subClassOf rdf:resource="https://w3id.org/tern/ontologies/tern/Platform"/>
  </rdf:Description>
  <rdf:Description rdf:nodeID="ub1bL536C19">
    <owl:onProperty rdf:resource="https://w3id.org/tern/ontologies/tern/globalValue"/>
    <rdf:type rdf:resource="http://www.w3.org/2002/07/owl#Restriction"/>
    <owl:onClass rdf:resource="http://www.w3.org/2004/02/skos/core#Concept"/>
    <owl:maxQualifiedCardinality rdf:datatype="http://www.w3.org/2001/XMLSchema#nonNegativeInteger">1</owl:maxQualifiedCardinality>
  </rdf:Description>
  <rdf:Description rdf:nodeID="ub1bL1314C19">
    <owl:minQualifiedCardinality rdf:datatype="http://www.w3.org/2001/XMLSchema#nonNegativeInteger">1</owl:minQualifiedCardinality>
    <owl:onProperty rdf:resource="http://www.w3.org/ns/sosa/hasSample"/>
    <owl:onClass rdf:resource="https://w3id.org/tern/ontologies/tern/SoilHorizon"/>
    <rdf:type rdf:resource="http://www.w3.org/2002/07/owl#Restriction"/>
  </rdf:Description>
  <rdf:Description rdf:nodeID="ub1bL1672C1">
    <owl:unionOf rdf:nodeID="fcf4ebf340cd54dc4871b974b242da6f5b16"/>
    <rdf:type rdf:resource="http://www.w3.org/2002/07/owl#Class"/>
  </rdf:Description>
  <rdf:Description rdf:about="https://w3id.org/tern/ontologies/tern/siteShape">
    <skos:definition>The shape of the site. The value is expected to be from a controlled vocabulary with a persistent URI identifier.</skos:definition>
    <rdfs:label>site shape</rdfs:label>
    <rdf:type rdf:resource="http://www.w3.org/1999/02/22-rdf-syntax-ns#Property"/>
    <rdfs:domain rdf:resource="https://w3id.org/tern/ontologies/tern/Site"/>
  </rdf:Description>
  <rdf:Description rdf:nodeID="fcf4ebf340cd54dc4871b974b242da6f5b5">
    <rdf:rest rdf:nodeID="fcf4ebf340cd54dc4871b974b242da6f5b6"/>
    <rdf:first rdf:resource="http://www.w3.org/2001/XMLSchema#string"/>
  </rdf:Description>
  <rdf:Description rdf:nodeID="ub1bL598C19">
    <owl:qualifiedCardinality rdf:datatype="http://www.w3.org/2001/XMLSchema#nonNegativeInteger">1</owl:qualifiedCardinality>
    <owl:onProperty rdf:resource="http://www.w3.org/ns/sosa/hasFeatureOfInterest"/>
    <rdf:type rdf:resource="http://www.w3.org/2002/07/owl#Restriction"/>
    <owl:onClass rdf:resource="http://www.w3.org/ns/sosa/FeatureOfInterest"/>
  </rdf:Description>
  <rdf:Description rdf:nodeID="ub1bL863C19">
    <owl:allValuesFrom rdf:resource="https://w3id.org/tern/ontologies/tern/Sampling"/>
    <owl:onProperty rdf:resource="http://www.w3.org/ns/sosa/madeSampling"/>
    <rdf:type rdf:resource="http://www.w3.org/2002/07/owl#Restriction"/>
  </rdf:Description>
  <rdf:Description rdf:nodeID="ub1bL610C19">
    <owl:onClass rdf:resource="https://w3id.org/tern/ontologies/tern/Procedure"/>
    <rdf:type rdf:resource="http://www.w3.org/2002/07/owl#Restriction"/>
    <owl:onProperty rdf:resource="http://www.w3.org/ns/sosa/usedProcedure"/>
    <owl:qualifiedCardinality rdf:datatype="http://www.w3.org/2001/XMLSchema#nonNegativeInteger">1</owl:qualifiedCardinality>
  </rdf:Description>
  <rdf:Description rdf:nodeID="ub1bL910C19">
    <owl:onClass rdf:resource="https://w3id.org/tern/ontologies/tern/Sample"/>
    <owl:onProperty rdf:resource="http://www.w3.org/ns/sosa/hasResult"/>
    <owl:qualifiedCardinality rdf:datatype="http://www.w3.org/2001/XMLSchema#nonNegativeInteger">1</owl:qualifiedCardinality>
    <rdf:type rdf:resource="http://www.w3.org/2002/07/owl#Restriction"/>
  </rdf:Description>
  <rdf:Description rdf:nodeID="ub1bL1066C19">
    <owl:maxQualifiedCardinality rdf:datatype="http://www.w3.org/2001/XMLSchema#nonNegativeInteger">1</owl:maxQualifiedCardinality>
    <owl:onClass rdf:resource="http://linked.data.gov.au/def/datatype/QuantitativeMeasure"/>
    <rdf:type rdf:resource="http://www.w3.org/2002/07/owl#Restriction"/>
    <owl:onProperty rdf:resource="https://w3id.org/tern/ontologies/tern/area"/>
  </rdf:Description>
  <rdf:Description rdf:nodeID="ub1bL1126C19">
    <owl:onProperty rdf:resource="http://www.opengis.net/ont/geosparql#hasGeometry"/>
    <rdf:type rdf:resource="http://www.w3.org/2002/07/owl#Restriction"/>
    <owl:minCardinality rdf:datatype="http://www.w3.org/2001/XMLSchema#nonNegativeInteger">1</owl:minCardinality>
  </rdf:Description>
  <rdf:Description rdf:nodeID="ub1bL1187C19">
    <owl:onProperty rdf:resource="http://www.w3.org/ns/sosa/isSampleOf"/>
    <owl:onClass rdf:resource="https://w3id.org/tern/ontologies/tern/SiteTaxon"/>
    <rdf:type rdf:resource="http://www.w3.org/2002/07/owl#Restriction"/>
    <owl:minQualifiedCardinality rdf:datatype="http://www.w3.org/2001/XMLSchema#nonNegativeInteger">1</owl:minQualifiedCardinality>
  </rdf:Description>
  <rdf:Description rdf:nodeID="ub1bL1309C19">
    <rdf:type rdf:resource="http://www.w3.org/2002/07/owl#Restriction"/>
    <owl:allValuesFrom rdf:resource="http://linked.data.gov.au/def/datatype/Text"/>
    <owl:onProperty rdf:resource="https://w3id.org/tern/ontologies/tern/soilClassification"/>
  </rdf:Description>
  <rdf:Description rdf:nodeID="fcf4ebf340cd54dc4871b974b242da6f5b2">
    <rdf:rest rdf:resource="http://www.w3.org/1999/02/22-rdf-syntax-ns#nil"/>
    <rdf:first rdf:resource="http://www.w3.org/2001/XMLSchema#integer"/>
  </rdf:Description>
  <rdf:Description rdf:nodeID="ub1bL939C19">
    <owl:onProperty rdf:resource="https://w3id.org/tern/ontologies/loc/depth"/>
    <owl:maxQualifiedCardinality rdf:datatype="http://www.w3.org/2001/XMLSchema#nonNegativeInteger">1</owl:maxQualifiedCardinality>
    <owl:onClass rdf:resource="http://linked.data.gov.au/def/datatype/QuantitativeMeasure"/>
    <rdf:type rdf:resource="http://www.w3.org/2002/07/owl#Restriction"/>
  </rdf:Description>
  <rdf:Description rdf:nodeID="ub1bL380C19">
    <owl:onProperty rdf:resource="http://www.w3.org/ns/sosa/isHostedBy"/>
    <owl:maxQualifiedCardinality rdf:datatype="http://www.w3.org/2001/XMLSchema#nonNegativeInteger">1</owl:maxQualifiedCardinality>
    <owl:onClass rdf:resource="https://w3id.org/tern/ontologies/tern/Site"/>
    <rdf:type rdf:resource="http://www.w3.org/2002/07/owl#Restriction"/>
  </rdf:Description>
  <rdf:Description rdf:nodeID="ub1bL275C19">
    <rdf:type rdf:resource="http://www.w3.org/2002/07/owl#Restriction"/>
    <owl:allValuesFrom rdf:nodeID="ub1bL277C25"/>
    <owl:onProperty rdf:resource="https://w3id.org/tern/ontologies/tern/length"/>
  </rdf:Description>
  <rdf:Description rdf:about="https://w3id.org/tern/ontologies/tern/CategoricalValue">
    <rdf:type rdf:resource="http://www.w3.org/2002/07/owl#Class"/>
    <rdfs:subClassOf rdf:resource="http://www.w3.org/2004/02/skos/core#Concept"/>
    <rdfs:label>Categorical Value</rdfs:label>
  </rdf:Description>
  <rdf:Description rdf:about="https://w3id.org/tern/ontologies/tern/isGlobalMatchOf">
    <rdfs:subPropertyOf rdf:resource="http://www.w3.org/2004/02/skos/core#exactMatch"/>
    <skos:scopeNote>Use in between controlled vocabularies.</skos:scopeNote>
    <owl:inverseOf rdf:resource="https://w3id.org/tern/ontologies/tern/globalMatch"/>
    <rdfs:label>is global match of</rdfs:label>
    <skos:definition>An inverse property of [globalMatch](#globalMatch); Links an upper concept to a concept (in the closed system).</skos:definition>
    <rdf:type rdf:resource="http://www.w3.org/1999/02/22-rdf-syntax-ns#Property"/>
  </rdf:Description>
  <rdf:Description rdf:nodeID="ub1bL98C23">
    <schema-https:affiliation rdf:resource="https://w3id.org/tern/resources/a083902d-d821-41be-b663-1d7cb33eea66"/>
    <schema-https:email>h.floresmoreno@uq.edu.au</schema-https:email>
    <rdf:type rdf:resource="https://schema.org/Person"/>
    <schema-https:name>Habacuc Flores Moreno</schema-https:name>
  </rdf:Description>
  <rdf:Description rdf:about="http://linked.data.gov.au/def/datatype/QuantitativeRange">
    <rdfs:subClassOf rdf:resource="https://w3id.org/tern/ontologies/tern/Result"/>
  </rdf:Description>
  <rdf:Description rdf:about="https://w3id.org/tern/ontologies/tern/purpose">
    <rdfs:range rdf:resource="http://www.w3.org/2001/XMLSchema#string"/>
    <rdf:type rdf:resource="http://www.w3.org/2002/07/owl#DatatypeProperty"/>
    <rdfs:label>purpose</rdfs:label>
    <skos:definition>Describe the purpose of something.</skos:definition>
  </rdf:Description>
  <rdf:Description rdf:about="https://w3id.org/tern/ontologies/tern/hasObservationTheme">
    <rdf:type rdf:resource="http://www.w3.org/1999/02/22-rdf-syntax-ns#Property"/>
    <rdfs:label>has observation theme</rdfs:label>
    <skos:definition>Link a concept to an observation theme.</skos:definition>
    <rdfs:subPropertyOf rdf:resource="http://www.w3.org/2004/02/skos/core#relatedMatch"/>
  </rdf:Description>
  <rdf:Description rdf:nodeID="ub1bL1035C19">
    <owl:allValuesFrom rdf:resource="https://w3id.org/tern/ontologies/tern/Site"/>
    <rdf:type rdf:resource="http://www.w3.org/2002/07/owl#Restriction"/>
    <owl:onProperty rdf:resource="http://purl.org/dc/terms/isPartOf"/>
  </rdf:Description>
  <rdf:Description rdf:about="https://w3id.org/tern/ontologies/tern/length">
    <rdfs:label>length</rdfs:label>
    <rdfs:seeAlso rdf:resource="http://qudt.org/vocab/quantitykind/Length"/>
    <rdf:type rdf:resource="http://www.w3.org/1999/02/22-rdf-syntax-ns#Property"/>
    <skos:definition>A measure of distance.</skos:definition>
  </rdf:Description>
  <rdf:Description rdf:about="https://w3id.org/tern/ontologies/tern/hasMethod">
    <skos:definition>A property that links a concept to a method.</skos:definition>
    <rdfs:label>has method</rdfs:label>
    <rdf:type rdf:resource="http://www.w3.org/1999/02/22-rdf-syntax-ns#Property"/>
    <rdfs:subPropertyOf rdf:resource="http://www.w3.org/2004/02/skos/core#relatedMatch"/>
  </rdf:Description>
  <rdf:Description rdf:about="https://w3id.org/tern/ontologies/tern/methodType">
    <skos:definition>A particular method type used to conduct some survey.</skos:definition>
    <rdf:type rdf:resource="http://www.w3.org/1999/02/22-rdf-syntax-ns#Property"/>
    <rdfs:label>method type</rdfs:label>
  </rdf:Description>
  <rdf:Description rdf:nodeID="ub1bL288C25">
    <owl:unionOf rdf:nodeID="fcf4ebf340cd54dc4871b974b242da6f5b3"/>
    <rdf:type rdf:resource="http://www.w3.org/2002/07/owl#Class"/>
  </rdf:Description>
  <rdf:Description rdf:nodeID="fcf4ebf340cd54dc4871b974b242da6f5b11">
    <rdf:rest rdf:resource="http://www.w3.org/1999/02/22-rdf-syntax-ns#nil"/>
    <rdf:first rdf:resource="https://w3id.org/tern/ontologies/tern/Sampling"/>
  </rdf:Description>
  <rdf:Description rdf:about="http://linked.data.gov.au/def/datatype/QuantitativeMeasure">
    <rdfs:subClassOf rdf:resource="https://w3id.org/tern/ontologies/tern/Result"/>
  </rdf:Description>
  <rdf:Description rdf:nodeID="ub1bL963C19">
    <owl:onProperty rdf:resource="https://w3id.org/tern/ontologies/loc/latitude"/>
    <owl:qualifiedCardinality rdf:datatype="http://www.w3.org/2001/XMLSchema#nonNegativeInteger">1</owl:qualifiedCardinality>
    <owl:onClass rdf:resource="http://linked.data.gov.au/def/datatype/QuantitativeMeasure"/>
    <rdf:type rdf:resource="http://www.w3.org/2002/07/owl#Restriction"/>
  </rdf:Description>
  <rdf:Description rdf:nodeID="ub1bL580C19">
    <owl:onProperty rdf:resource="http://www.w3.org/ns/sosa/hasResult"/>
    <owl:onClass rdf:resource="https://w3id.org/tern/ontologies/tern/Result"/>
    <rdf:type rdf:resource="http://www.w3.org/2002/07/owl#Restriction"/>
    <owl:minQualifiedCardinality rdf:datatype="http://www.w3.org/2001/XMLSchema#nonNegativeInteger">1</owl:minQualifiedCardinality>
  </rdf:Description>
  <rdf:Description rdf:nodeID="ub1bL1235C19">
    <rdf:type rdf:resource="http://www.w3.org/2002/07/owl#Restriction"/>
    <owl:onProperty rdf:resource="http://schema.org/additionalProperty"/>
    <owl:allValuesFrom rdf:resource="https://w3id.org/tern/ontologies/tern/PropertyValue"/>
  </rdf:Description>
  <rdf:Description rdf:nodeID="ub1bL1020C19">
    <owl:allValuesFrom rdf:resource="https://w3id.org/tern/ontologies/tern/Procedure"/>
    <rdf:type rdf:resource="http://www.w3.org/2002/07/owl#Restriction"/>
    <owl:onProperty rdf:resource="https://w3id.org/tern/ontologies/tern/locationProcedure"/>
  </rdf:Description>
  <rdf:Description rdf:nodeID="fcf4ebf340cd54dc4871b974b242da6f5b16">
    <rdf:first rdf:resource="http://www.w3.org/2001/XMLSchema#string"/>
    <rdf:rest rdf:nodeID="fcf4ebf340cd54dc4871b974b242da6f5b17"/>
  </rdf:Description>
  <rdf:Description rdf:about="https://w3id.org/tern/ontologies/tern/taxon">
    <rdfs:label>taxon</rdfs:label>
    <skos:definition>Taxon classification.</skos:definition>
    <skos:scopeNote>Value should be from a controlled vocabulary identified by a URI.</skos:scopeNote>
    <rdf:type rdf:resource="http://www.w3.org/1999/02/22-rdf-syntax-ns#Property"/>
  </rdf:Description>
  <rdf:Description rdf:nodeID="ub1bL1292C19">
    <rdf:type rdf:resource="http://www.w3.org/2002/07/owl#Restriction"/>
    <owl:onProperty rdf:resource="https://w3id.org/tern/ontologies/tern/soilHorizonClassifier"/>
    <owl:allValuesFrom rdf:resource="http://linked.data.gov.au/def/datatype/Text"/>
  </rdf:Description>
  <rdf:Description rdf:nodeID="ub1bL1056C19">
    <owl:maxCardinality rdf:datatype="http://www.w3.org/2001/XMLSchema#nonNegativeInteger">1</owl:maxCardinality>
    <rdf:type rdf:resource="http://www.w3.org/2002/07/owl#Restriction"/>
    <owl:onProperty rdf:resource="http://www.w3.org/ns/prov#generatedAtTime"/>
  </rdf:Description>
  <rdf:Description rdf:nodeID="ub1bL531C19">
    <owl:maxCardinality rdf:datatype="http://www.w3.org/2001/XMLSchema#nonNegativeInteger">1</owl:maxCardinality>
    <rdf:type rdf:resource="http://www.w3.org/2002/07/owl#Restriction"/>
    <owl:onProperty rdf:resource="https://w3id.org/tern/ontologies/tern/globalVocabulary"/>
  </rdf:Description>
  <rdf:Description rdf:nodeID="ub1bL1084C19">
    <owl:maxQualifiedCardinality rdf:datatype="http://www.w3.org/2001/XMLSchema#nonNegativeInteger">1</owl:maxQualifiedCardinality>
    <rdf:type rdf:resource="http://www.w3.org/2002/07/owl#Restriction"/>
    <owl:onClass rdf:resource="http://www.w3.org/2001/XMLSchema#string"/>
    <owl:onProperty rdf:resource="https://w3id.org/tern/ontologies/tern/locationDescription"/>
  </rdf:Description>
  <rdf:Description rdf:nodeID="ub1bL129C19">
    <schema-https:affiliation rdf:resource="https://w3id.org/tern/resources/a083902d-d821-41be-b663-1d7cb33eea66"/>
    <rdf:type rdf:resource="https://schema.org/Person"/>
    <schema-https:name>Siddeswara Guru</schema-https:name>
    <schema-https:email>s.guru@uq.edu.au</schema-https:email>
    <schema-https:identifier rdf:resource="https://orcid.org/0000-0002-3903-254X"/>
  </rdf:Description>
  <rdf:Description rdf:nodeID="ub1bL828C19">
    <owl:allValuesFrom rdf:resource="https://w3id.org/tern/ontologies/tern/Observation"/>
    <rdf:type rdf:resource="http://www.w3.org/2002/07/owl#Restriction"/>
    <owl:onProperty rdf:resource="http://www.w3.org/ns/sosa/isFeatureOfInterestOf"/>
  </rdf:Description>
  <rdf:Description rdf:nodeID="ub1bL653C19">
    <owl:allValuesFrom rdf:resource="http://www.w3.org/2001/XMLSchema#string"/>
    <owl:onProperty rdf:resource="http://www.w3.org/2000/01/rdf-schema#label"/>
    <rdf:type rdf:resource="http://www.w3.org/2002/07/owl#Restriction"/>
  </rdf:Description>
  <rdf:Description rdf:nodeID="ub1bL1047C25">
    <owl:unionOf rdf:nodeID="fcf4ebf340cd54dc4871b974b242da6f5b12"/>
    <rdf:type rdf:resource="http://www.w3.org/2002/07/owl#Class"/>
  </rdf:Description>
  <rdf:Description rdf:nodeID="fcf4ebf340cd54dc4871b974b242da6f5b7">
    <rdf:rest rdf:nodeID="fcf4ebf340cd54dc4871b974b242da6f5b8"/>
    <rdf:first rdf:resource="http://www.w3.org/2004/02/skos/core#ConceptScheme"/>
  </rdf:Description>
  <rdf:Description rdf:nodeID="ub1bL172C23">
    <rdf:type rdf:resource="http://www.w3.org/ns/prov#Activity"/>
    <rdf:type rdf:resource="http://usefulinc.com/ns/doap#Project"/>
    <doap:repository rdf:resource="https://github.com/ternaustralia/ontology_tern"/>
  </rdf:Description>
  <rdf:Description rdf:nodeID="ub1bL1030C19">
    <owl:allValuesFrom rdf:resource="https://w3id.org/tern/ontologies/tern/Site"/>
    <owl:onProperty rdf:resource="http://purl.org/dc/terms/hasPart"/>
    <rdf:type rdf:resource="http://www.w3.org/2002/07/owl#Restriction"/>
  </rdf:Description>
  <rdf:Description rdf:nodeID="ub1bL868C19">
    <rdf:type rdf:resource="http://www.w3.org/2002/07/owl#Restriction"/>
    <owl:minQualifiedCardinality rdf:datatype="http://www.w3.org/2001/XMLSchema#nonNegativeInteger">1</owl:minQualifiedCardinality>
    <owl:onClass rdf:resource="https://w3id.org/tern/ontologies/tern/Procedure"/>
    <owl:onProperty rdf:resource="http://www.w3.org/ns/ssn/implements"/>
  </rdf:Description>
  <rdf:Description rdf:nodeID="ub1bL658C19">
    <rdf:type rdf:resource="http://www.w3.org/2002/07/owl#Restriction"/>
    <owl:onProperty rdf:resource="http://www.w3.org/ns/sosa/isHostedBy"/>
    <owl:allValuesFrom rdf:resource="https://w3id.org/tern/ontologies/tern/Platform"/>
  </rdf:Description>
  <rdf:Description rdf:nodeID="fcf4ebf340cd54dc4871b974b242da6f5b15">
    <rdf:first rdf:resource="https://w3id.org/tern/ontologies/tern/Sampling"/>
    <rdf:rest rdf:resource="http://www.w3.org/1999/02/22-rdf-syntax-ns#nil"/>
  </rdf:Description>
  <rdf:Description rdf:nodeID="ub1bL1090C19">
    <owl:onClass rdf:resource="http://www.w3.org/2001/XMLSchema#string"/>
    <owl:maxQualifiedCardinality rdf:datatype="http://www.w3.org/2001/XMLSchema#nonNegativeInteger">1</owl:maxQualifiedCardinality>
    <rdf:type rdf:resource="http://www.w3.org/2002/07/owl#Restriction"/>
    <owl:onProperty rdf:resource="https://w3id.org/tern/ontologies/tern/siteDescription"/>
  </rdf:Description>
  <rdf:Description rdf:nodeID="ub1bL1230C19">
    <owl:onProperty rdf:resource="http://www.w3.org/ns/sosa/hasSample"/>
    <rdf:type rdf:resource="http://www.w3.org/2002/07/owl#Restriction"/>
    <owl:allValuesFrom rdf:resource="https://w3id.org/tern/ontologies/tern/PhysicalSpecimen"/>
  </rdf:Description>
  <rdf:Description rdf:nodeID="fcf4ebf340cd54dc4871b974b242da6f5b10">
    <rdf:first rdf:resource="https://w3id.org/tern/ontologies/tern/Observation"/>
    <rdf:rest rdf:nodeID="fcf4ebf340cd54dc4871b974b242da6f5b11"/>
  </rdf:Description>
  <rdf:Description rdf:about="http://linked.data.gov.au/def/datatype/Count">
    <rdfs:subClassOf rdf:resource="https://w3id.org/tern/ontologies/tern/Result"/>
  </rdf:Description>
  <rdf:Description rdf:nodeID="fcf4ebf340cd54dc4871b974b242da6f5b14">
    <rdf:rest rdf:nodeID="fcf4ebf340cd54dc4871b974b242da6f5b15"/>
    <rdf:first rdf:resource="https://w3id.org/tern/ontologies/tern/Observation"/>
  </rdf:Description>
  <rdf:Description rdf:nodeID="fcf4ebf340cd54dc4871b974b242da6f5b12">
    <rdf:rest rdf:nodeID="fcf4ebf340cd54dc4871b974b242da6f5b13"/>
    <rdf:first rdf:resource="https://w3id.org/tern/ontologies/loc/Point"/>
  </rdf:Description>
  <rdf:Description rdf:nodeID="fcf4ebf340cd54dc4871b974b242da6f5b13">
    <rdf:first rdf:resource="https://w3id.org/tern/ontologies/loc/Polygon"/>
    <rdf:rest rdf:resource="http://www.w3.org/1999/02/22-rdf-syntax-ns#nil"/>
  </rdf:Description>
  <rdf:Description rdf:about="http://linked.data.gov.au/def/datatype/Text">
    <rdfs:subClassOf rdf:resource="https://w3id.org/tern/ontologies/tern/Result"/>
  </rdf:Description>
</rdf:RDF>
